# baseURI: http://www.opengis.net/def/ont/specrel

@prefix dc: <http://purl.org/dc/elements/1.1/> .
@prefix dct: <http://purl.org/dc/terms/> .
@prefix owl: <http://www.w3.org/2002/07/owl#> .
@prefix rdf: <http://www.w3.org/1999/02/22-rdf-syntax-ns#> .
@prefix rdfs: <http://www.w3.org/2000/01/rdf-schema#> .
@prefix skos: <http://www.w3.org/2004/02/skos/core#> .
@prefix spec: <http://www.opengis.net/def/ont/modspec/> .
@prefix xsd: <http://www.w3.org/2001/XMLSchema#> .
@prefix specrel: <http://www.opengis.net/def/ont/specrel/> .
@prefix prov: <http://www.w3.org/ns/prov#> .
@prefix prof: <http://www.w3.org/ns/dx/prof/> .
@prefix sh: <http://www.w3.org/ns/shacl#> .
@prefix adms:	<http://www.w3.org/ns/adms#> .

<http://www.opengis.net/def/ont/specrel> a owl:Ontology;
 rdfs:comment "Model of relationships between OGC specifications and related documents and artefacts" ;
  dc:creator "Rob Atkinson" .

specrel:modspec a owl:ObjectProperty ;
rdfs:label "As ModSpec" ;
rdfs:comment "References a model of the document contents modelled using the OGC Modular Specification, where application using the baseURI defined for specification elements in the document."@en;
rdfs:range spec:Specification ;
.


specrel:normativeRef a owl:ObjectProperty ;
rdfs:label "Normatively References" ;
rdfs:comment "Superset of different types of relations that are included in Normative Reference sections"@en ;
rdfs:subPropertyOf specrel:relatesTo ;
.

specrel:implementation a owl:ObjectProperty ;
rdfs:label "Implementation" ;
rdfs:comment "Specification referenced is an implementation of a conceptual model defined in the subject. Note that this may be a self-reference for older specifications before the practice was to separate conceptual models and implementations."@en;
owl:inverseProperty specrel:implements ;
rdfs:subPropertyOf specrel:relatesTo ;
.

specrel:implements a owl:ObjectProperty ;
rdfs:label "Implements" ;
rdfs:comment "This specification implements the referenced conceptual model defined in the subject. Note that this may be a self-reference for older specifications before the practice was to separate conceptual models and implementations."@en;
rdfs:subPropertyOf specrel:normativeRef ;
owl:inverseProperty specrel:conceptualModelOf ;
.

prof:isProfileOf rdfs:subPropertyOf specrel:normativeRef .

specrel:uses a owl:ObjectProperty ;
rdfs:label "Uses" ;
rdfs:comment "The subject specification uses the referenced specification as a normative component"@en;
rdfs:subPropertyOf specrel:normativeRef ;
.

specrel:relatesTo a owl:ObjectProperty ;
rdfs:label "Unspecified relation" ;
rdfs:comment "This specification has some unspecified relation to the referenced document."@en;
rdfs:domain spec:Specification;
rdfs:range spec:Specification;
.


spec:Specification   a sh:NodeShape ;
rdfs:comment "SHACL NodeShape model uses to reference properties from other namespaces that may be used for relations";
sh:property specrel:wasInfluencedBy, specrel:next, specrel:last ;
.

specrel:wasInfluencedBy a sh:PropertyShape ;
  sh:description "Used to relate a specification to documents relating to activities such as Testbeds" ;
  sh:path prov:wasInfluencedBy ;
  sh:class skos:Concept ;
  .

specrel:next a sh:PropertyShape ;
  sh:description "Next version" ;
  sh:path adms:next ;
  sh:class skos:Concept ;
  .

specrel:last a sh:PropertyShape ;
  sh:description "Last version (most recent)" ;
  sh:path adms:last ;
  sh:class skos:Concept ;
  .
  

specrel:prev a sh:PropertyShape ;
  sh:description "Previous version" ;
  sh:path adms:prev ;
  sh:class skos:Concept ;
  .
  
specrel:guidance a owl:ObjectProperty ;
rdfs:label "Guidance" ;
rdfs:comment "The referenced document provides guidance for this specification."@en;
.
