@prefix ft: <http://www.opengis.net/def/metamodel/featuretypes/> .
@prefix owl: <http://www.w3.org/2002/07/owl#> .
@prefix prov: <http://www.w3.org/ns/prov#> .
@prefix rdf: <http://www.w3.org/1999/02/22-rdf-syntax-ns#> .
@prefix rdfs: <http://www.w3.org/2000/01/rdf-schema#> .
@prefix skos: <http://www.w3.org/2004/02/skos/core#> .
@prefix dct: <http://purl.org/dc/terms/> .

<http://www.opengis.net/def/metamodel/featuretypes>
  a owl:Ontology ;
  dct:creator "Rob Atkinson" ;
  dct:title "Feature Type Catalog Display Ontology" ;
  rdfs:comment """Minimal ontology to support display of OWL Ontologies containing ISO 19109 Feature Types.
  This primarily supports direct associations of properties to feature types (classes) and ontology-level collection views of classes, properties and codelists""" ;
.    

ft:FeatureType rdfs:subClassOf owl:Class ;
    rdfs:label "Feature Type" ;
    rdfs:comment "identifies a class specifically as a FeatureType with properties" ;
.
    
ft:hasProperty 
    rdfs:label "has Property" ;
    skos:prefLabel "has Property" ;
    rdfs:comment "A property of a feature as per ISO19109 General Feature Model - provides a direct reference to a specific property, additional details of the property may be encoded in OWL syntax using a rdfs:subClassOf restriction." ;
    a owl:ObjectProperty. 
    
ft:propertyList 
    rdfs:label "List of Properties" ;
    rdfs:comment "Convenience link from a Model or ConceptScheme view to top level collection of contained Properties" ;
    rdfs:range skos:Collection ;
    a owl:ObjectProperty. 
    
ft:ftList 
    rdfs:label "List of Classes" ;
    rdfs:comment "Convenience link from a Model or ConceptScheme view to top level collection of contained Classes or FeatureTypes" ;
    rdfs:range skos:Collection ;
    a owl:ObjectProperty. 
    
ft:codelistList 
    rdfs:label "List of CodeLists" ;
    rdfs:comment "Convenience link from a Model or ConceptScheme view to top level collection of contained codelists" ;
    rdfs:range skos:Collection ;
    a owl:ObjectProperty. 
       