<?xml version="1.0" encoding="UTF-8"?>
<rdf:RDF
   xmlns:dct="http://purl.org/dc/terms/"
   xmlns:ns1="http://www.opengis.net/def/metamodel/ogc-na/"
   xmlns:prof="http://www.w3.org/ns/dx/prof/"
   xmlns:rdf="http://www.w3.org/1999/02/22-rdf-syntax-ns#"
   xmlns:rdfs="http://www.w3.org/2000/01/rdf-schema#"
   xmlns:skos="http://www.w3.org/2004/02/skos/core#"
>
  <rdf:Description rdf:about="http://www.opengis.net/def/metamodel/profiles/skos_conceptscheme_ogc">
    <skos:broader rdf:resource="http://www.opengis.net/def/metamodel/profiles/vocprez_ogc"/>
    <skos:broader rdf:resource="https://w3id.org/profile/vocpub"/>
    <skos:broader rdf:resource="http://www.opengis.net/def/metamodel/profiles/skos_shared"/>
    <prof:hasResource rdf:nodeID="na98dbebffd0844b086c429bec9aaabdab2"/>
    <prof:hasResource rdf:nodeID="na98dbebffd0844b086c429bec9aaabdab3"/>
    <prof:hasResource rdf:nodeID="na98dbebffd0844b086c429bec9aaabdab1"/>
    <prof:hasToken rdf:datatype="http://www.w3.org/2001/XMLSchema#token">skos_ogc</prof:hasToken>
    <rdf:type rdf:resource="http://www.w3.org/ns/dx/prof/Profile"/>
    <rdf:type rdf:resource="http://www.w3.org/2004/02/skos/core#Concept"/>
    <prof:isProfileOf rdf:resource="https://w3id.org/profile/vocpub"/>
    <prof:isProfileOf rdf:resource="http://www.opengis.net/def/metamodel/profiles/skos_shared"/>
    <prof:isProfileOf rdf:resource="http://www.opengis.net/def/metamodel/profiles/vocprez_ogc"/>
    <skos:prefLabel>SKOS (OGC Profile)</skos:prefLabel>
    <rdfs:label>SKOS (OGC Profile)</rdfs:label>
    <skos:inScheme rdf:resource="http://www.opengis.net/def/metamodel/profiles"/>
    <skos:definition>OGC Naming Authority Profile of SKOS. This profile binds basic SKOS patterns to status and governance metadata accordint to OGC procedural requirements.</skos:definition>
    <dct:description>OGC Naming Authority Profile of SKOS. This profile binds basic SKOS patterns to status and governance metadata accordint to OGC procedural requirements.</dct:description>
    <ns1:status rdf:resource="http://www.opengis.net/def/status/valid"/>
    <rdfs:comment>Enforces additional rules, such as presence of a top-level collection for contents, and conformance with the VocPrez tooling requirements.</rdfs:comment>
  </rdf:Description>
  <rdf:Description rdf:nodeID="na98dbebffd0844b086c429bec9aaabdab1">
    <dct:format>text/html</dct:format>
    <rdf:type rdf:resource="http://www.w3.org/ns/dx/prof/ResourceDescriptor"/>
    <prof:hasRole rdf:resource="http://www.w3.org/ns/dx/prof/role/profile"/>
    <prof:hasArtifact rdf:resource="http://www.opengis.net/def/metamodel/profiles/skos_ogc"/>
    <rdfs:comment>Artefact is self reference using canonical URI and content negotiation</rdfs:comment>
    <rdfs:label>Profile description as HTML</rdfs:label>
    <dct:conformsTo rdf:resource="http://www.w3.org/ns/dx/prof/"/>
  </rdf:Description>
  <rdf:Description rdf:nodeID="na98dbebffd0844b086c429bec9aaabdab2">
    <rdfs:label>SHACL Validator</rdfs:label>
    <dct:conformsTo rdf:resource="http://www.w3.org/ns/shacl#"/>
    <prof:hasArtifact rdf:resource="http://defs-dev.opengis.net/ogc-na/scripts/ogc_skos_profile_entailments.ttl"/>
    <dct:format>text/turtle</dct:format>
    <prof:hasRole rdf:resource="http://www.w3.org/ns/dx/prof/role/entailment"/>
    <rdf:type rdf:resource="http://www.w3.org/ns/dx/prof/ResourceDescriptor"/>
    <dct:description>Entailment script to enforce OGC policy requirements.</dct:description>
  </rdf:Description>
  <rdf:Description rdf:nodeID="na98dbebffd0844b086c429bec9aaabdab3">
    <dct:conformsTo rdf:resource="http://www.w3.org/ns/shacl#"/>
    <dct:format>text/turtle</dct:format>
    <dct:description>Validation shapes for SKOS resources against OGC policy requirements.</dct:description>
    <rdf:type rdf:resource="http://www.w3.org/ns/dx/prof/ResourceDescriptor"/>
    <prof:hasRole rdf:resource="http://www.w3.org/ns/dx/prof/role/validation"/>
    <prof:hasArtifact rdf:resource="http://defs-dev.opengis.net/ogc-na/scripts/ogc_skos_profile.shapes.ttl"/>
    <rdfs:label>SHACL Validator</rdfs:label>
  </rdf:Description>
  <rdf:Description rdf:about="http://www.opengis.net/def/metamodel/profiles/skos_shared">
    <skos:narrower rdf:resource="http://www.opengis.net/def/metamodel/profiles/skos_conceptscheme_ogc"/>
  </rdf:Description>
  <rdf:Description rdf:about="http://www.opengis.net/def/metamodel/profiles/vocprez_ogc">
    <skos:narrower rdf:resource="http://www.opengis.net/def/metamodel/profiles/skos_conceptscheme_ogc"/>
  </rdf:Description>
  <rdf:Description rdf:about="https://w3id.org/profile/vocpub">
    <skos:narrower rdf:resource="http://www.opengis.net/def/metamodel/profiles/skos_conceptscheme_ogc"/>
  </rdf:Description>
</rdf:RDF>
