<?xml version="1.0" encoding="UTF-8"?>
<rdf:RDF
   xmlns:dct="http://purl.org/dc/terms/"
   xmlns:ns1="http://www.opengis.net/def/metamodel/ogc-na/"
   xmlns:owl="http://www.w3.org/2002/07/owl#"
   xmlns:prof="http://www.w3.org/ns/dx/prof/"
   xmlns:rdf="http://www.w3.org/1999/02/22-rdf-syntax-ns#"
   xmlns:rdfs="http://www.w3.org/2000/01/rdf-schema#"
   xmlns:skos="http://www.w3.org/2004/02/skos/core#"
>
  <rdf:Description rdf:about="http://www.opengis.net/def/metamodel/profiles/skos">
    <skos:broader rdf:resource="http://www.w3.org/2004/02/skos/core"/>
    <rdf:type rdf:resource="http://www.w3.org/2002/07/owl#Ontology"/>
    <rdf:type rdf:resource="http://www.w3.org/2004/02/skos/core#Concept"/>
    <rdf:type rdf:resource="http://purl.org/dc/terms/Standard"/>
    <rdf:type rdf:resource="http://www.w3.org/ns/dx/prof/Profile"/>
    <ns1:status rdf:resource="http://www.opengis.net/def/status/valid"/>
    <skos:inScheme rdf:resource="http://www.opengis.net/def/metamodel/profiles"/>
    <skos:definition>Defines a proxy for the SKOS standard, allowing discovery and access to implementation resources such as JSON-LD contexts</skos:definition>
    <skos:prefLabel>SKOS Proxy</skos:prefLabel>
    <rdfs:comment>This profile assumes no restrictions beyond the original standard, however implicitly binds JSON-LD prefixes and support use of classes and properties without prefix in JSON documents.</rdfs:comment>
    <owl:imports rdf:resource="http://www.w3.org/ns/dx/prof"/>
    <prof:isProfileOf rdf:resource="http://www.w3.org/2004/02/skos/core"/>
  </rdf:Description>
  <rdf:Description rdf:nodeID="n3d9aeeb6fdb7459d8c11784a5e5cf21bb1">
    <rdf:type rdf:resource="http://www.w3.org/ns/dx/prof/ResourceDescriptor"/>
    <rdfs:comment>Artefact is self reference using canonical URI and content negotiation</rdfs:comment>
    <dct:format>text/html</dct:format>
    <prof:hasArtifact rdf:resource="https://www.w3.org/TR/swbp-skos-core-spec/"/>
    <rdfs:label>SKOS specification</rdfs:label>
    <prof:hasRole rdf:resource="http://www.w3.org/ns/dx/prof/role/specification"/>
  </rdf:Description>
  <rdf:Description rdf:nodeID="n3d9aeeb6fdb7459d8c11784a5e5cf21bb2">
    <rdfs:comment>Proxy resource for JSON-LD context as authoritative resource not yet published</rdfs:comment>
    <dct:format>application/ld+json</dct:format>
    <rdfs:label>JSON-LD Context</rdfs:label>
    <dct:conformsTo rdf:resource="https://www.w3.org/TR/json-ld/"/>
    <dct:conformsTo rdf:resource="http://www.opengis.net/def/metamodel/profiles/json_ld_context"/>
    <prof:hasRole rdf:resource="http://www.w3.org/ns/dx/prof/role/implementation"/>
    <prof:hasArtifact rdf:resource="https://defs-dev.opengis.net/ogc-na/definitions/profiles/resources/skos.jsonld"/>
    <rdf:type rdf:resource="http://www.w3.org/ns/dx/prof/ResourceDescriptor"/>
  </rdf:Description>
  <rdf:Description rdf:about="http://www.w3.org/2004/02/skos/core">
    <rdf:type rdf:resource="http://www.w3.org/2004/02/skos/core#Concept"/>
    <rdf:type rdf:resource="http://purl.org/dc/terms/Standard"/>
    <rdf:type rdf:resource="http://www.w3.org/ns/dx/prof/Profile"/>
    <skos:prefLabel>SKOS Simple Knowledge Organization System</skos:prefLabel>
    <prof:hasResource rdf:nodeID="n3d9aeeb6fdb7459d8c11784a5e5cf21bb1"/>
    <prof:hasResource rdf:nodeID="n3d9aeeb6fdb7459d8c11784a5e5cf21bb2"/>
    <ns1:status rdf:resource="http://www.opengis.net/def/status/valid"/>
    <skos:narrower rdf:resource="http://www.opengis.net/def/metamodel/profiles/skos"/>
    <skos:inScheme rdf:resource="http://www.opengis.net/def/metamodel/profiles"/>
    <prof:hasToken rdf:datatype="http://www.w3.org/2001/XMLSchema#token">skos</prof:hasToken>
    <skos:definition>SKOS Simple Knowledge Organization System</skos:definition>
  </rdf:Description>
</rdf:RDF>
