@prefix dct: <http://purl.org/dc/terms/> .
@prefix ns1: <http://www.opengis.net/def/metamodel/ogc-na/> .
@prefix prof: <http://www.w3.org/ns/dx/prof/> .
@prefix profiles: <http://www.opengis.net/def/metamodel/profiles/> .
@prefix profrole: <http://www.w3.org/ns/dx/prof/role/> .
@prefix rdfs: <http://www.w3.org/2000/01/rdf-schema#> .
@prefix shacl: <http://www.w3.org/ns/shacl#> .
@prefix skos: <http://www.w3.org/2004/02/skos/core#> .
@prefix xsd: <http://www.w3.org/2001/XMLSchema#> .

<http://www.w3.org/2004/02/skos/core> skos:narrower profiles:skos_shared .

profiles:skos_shared a skos:Concept,
        prof:Profile ;
    rdfs:label "Shareable SKOS" ;
    ns1:status <http://www.opengis.net/def/status/valid> ;
    skos:broader <http://www.w3.org/2004/02/skos/core> ;
    skos:definition """Provides a minimal profile for sharing of terms across multiple environments using SKOS. 
  
  The requirement here is that the source of each term can be unambiguosly identified without dereferencing the term successfully in an online environment and successfully navigating to metadata about the scheme that defines the term.
  
  """ ;
    skos:inScheme <http://www.opengis.net/def/metamodel/profiles> ;
    skos:prefLabel "Shareable SKOS" ;
    prof:hasResource [ a prof:ResourceDescriptor ;
            rdfs:label "Profile description as HTML" ;
            dct:conformsTo prof: ;
            dct:format "text/html" ;
            rdfs:comment "Artefact is self reference using canonical URI and content negotiation" ;
            prof:hasArtifact profiles:skos_shared ;
            prof:hasRole profrole:profile ],
        [ a prof:ResourceDescriptor ;
            rdfs:label "Profile constraints as SHACL" ;
            dct:conformsTo shacl: ;
            dct:format "text/turtle" ;
            rdfs:comment "Artefact is self reference using canonical URI and content negotiation" ;
            prof:hasArtifact <http://defs-dev.opengis.net/def/metamodel/profiles/skos_shared?_profile=shacl&_mediatype=text/turtle>,
                profiles:skos_shared,
                <https://defs-dev.opengis.net/ogc-na/definitions/profiles/resources/skos_shared_shacl.ttl> ;
            prof:hasRole profrole:validation ],
        [ a prof:ResourceDescriptor ;
            rdfs:label "Profile Class Diagram" ;
            dct:format "image/png" ;
            rdfs:comment "Crude illustration of profile scope" ;
            prof:hasArtifact <https://defs-dev.opengis.net/ogc-na/definitions/profiles/resources/skos_shared_class_diagram.png> ],
        [ a prof:ResourceDescriptor ;
            rdfs:label "Validation example" ;
            dct:conformsTo shacl: ;
            dct:format "text/turtle" ;
            rdfs:comment "Uses SHACL rules against a sample vocabulary with known issue" ;
            prof:hasArtifact <https://shacl-play.sparna.fr/play/validate?url=http://defs-dev.opengis.net/ogc-na/definitions/conceptschemes/auth.ttl&shapesUrl=http://defs-dev.opengis.net/ogc-na/definitions/profiles/resources/skos_shared_shacl.ttl>,
                <https://shacl-play.sparna.fr/play/validate?url=http://defs-dev.opengis.net/ogc-na/definitions/conceptschemes/entailed/auth.ttl&shapesUrl=http://defs-dev.opengis.net/ogc-na/definitions/profiles/resources/skos_shared_shacl.ttl> ;
            prof:hasRole profrole:example ] ;
    prof:hasToken "skos_shared"^^xsd:token ;
    prof:isProfileOf <http://www.w3.org/2004/02/skos/core> .

