@prefix dct: <http://purl.org/dc/terms/> .
@prefix ns1: <http://www.opengis.net/def/metamodel/ogc-na/> .
@prefix prof: <http://www.w3.org/ns/dx/prof/> .
@prefix profiles: <http://www.opengis.net/def/metamodel/profiles/> .
@prefix profrole: <http://www.w3.org/ns/dx/prof/role/> .
@prefix rdfs: <http://www.w3.org/2000/01/rdf-schema#> .
@prefix shacl: <http://www.w3.org/ns/shacl#> .
@prefix skos: <http://www.w3.org/2004/02/skos/core#> .
@prefix xsd: <http://www.w3.org/2001/XMLSchema#> .

profiles:skos_shared skos:narrower profiles:skos_conceptscheme_ogc .

profiles:vocprez_ogc skos:narrower profiles:skos_conceptscheme_ogc .

<https://w3id.org/profile/vocpub> skos:narrower profiles:skos_conceptscheme_ogc .

profiles:skos_conceptscheme_ogc a skos:Concept,
        prof:Profile ;
    rdfs:label "SKOS (OGC Profile)" ;
    dct:description "OGC Naming Authority Profile of SKOS. This profile binds basic SKOS patterns to status and governance metadata accordint to OGC procedural requirements." ;
    ns1:status <http://www.opengis.net/def/status/valid> ;
    rdfs:comment "Enforces additional rules, such as presence of a top-level collection for contents, and conformance with the VocPrez tooling requirements." ;
    skos:broader profiles:skos_shared,
        profiles:vocprez_ogc,
        <https://w3id.org/profile/vocpub> ;
    skos:definition "OGC Naming Authority Profile of SKOS. This profile binds basic SKOS patterns to status and governance metadata accordint to OGC procedural requirements." ;
    skos:inScheme <http://www.opengis.net/def/metamodel/profiles> ;
    skos:prefLabel "SKOS (OGC Profile)" ;
    prof:hasResource [ a prof:ResourceDescriptor ;
            rdfs:label "Profile description as HTML" ;
            dct:conformsTo prof: ;
            dct:format "text/html" ;
            rdfs:comment "Artefact is self reference using canonical URI and content negotiation" ;
            prof:hasArtifact profiles:skos_ogc ;
            prof:hasRole profrole:profile ],
        [ a prof:ResourceDescriptor ;
            rdfs:label "SHACL Validator" ;
            dct:conformsTo shacl: ;
            dct:description "Entailment script to enforce OGC policy requirements." ;
            dct:format "text/turtle" ;
            prof:hasArtifact <http://defs-dev.opengis.net/ogc-na/scripts/ogc_skos_profile_entailments.ttl> ;
            prof:hasRole profrole:entailment ],
        [ a prof:ResourceDescriptor ;
            rdfs:label "SHACL Validator" ;
            dct:conformsTo shacl: ;
            dct:description "Validation shapes for SKOS resources against OGC policy requirements." ;
            dct:format "text/turtle" ;
            prof:hasArtifact <http://defs-dev.opengis.net/ogc-na/scripts/ogc_skos_profile.shapes.ttl> ;
            prof:hasRole profrole:validation ] ;
    prof:hasToken "skos_ogc"^^xsd:token ;
    prof:isProfileOf profiles:skos_shared,
        profiles:vocprez_ogc,
        <https://w3id.org/profile/vocpub> .

