# baseURI: http://www.opengis.net/def/entities/bodies
# imports: http://www.opengis.net/def/metamodel/ogc-na

@prefix owl: <http://www.w3.org/2002/07/owl#> .
@prefix rdf: <http://www.w3.org/1999/02/22-rdf-syntax-ns#> .
@prefix rdfs: <http://www.w3.org/2000/01/rdf-schema#> .
@prefix xsd: <http://www.w3.org/2001/XMLSchema#> .
@prefix bodies: <http://www.opengis.net/def/entities/bodies/> .
@prefix policy: <http://www.opengis.net/def/metamodel/ogc-na/> .
@prefix prof: <http://www.w3.org/ns/dx/prof/> .
@prefix prov: <http://www.w3.org/ns/prov#> .
@prefix skos: <http://www.w3.org/2004/02/skos/core#> .
@prefix dcat: <http://www.w3.org/ns/dcat#> .
@prefix dct: <http://purl.org/dc/terms/> .
@prefix schema: <http://schema.org/> .
@prefix foaf: <http://xmlns.com/foaf/0.1/> .

<http://www.opengis.net/def/entities/bodies>
  a skos:ConceptScheme ;
  owl:imports <http://www.opengis.net/def/metamodel/ogc-na> ;
  owl:versionInfo "Created with TopBraid Composer" ;
  rdfs:label "Bodies of the OGC" ;
  skos:prefLabel "Bodies of the OGC" ;
  skos:hasTopConcept bodies:swg,bodies:dwg, bodies:auth;
  dct:modified "2022-09-21"^^xsd:date ;
   dct:created "2022-06-03"^^xsd:date ;
  dct:creator  [ 
      schema:affiliation [ foaf:name "OGC" ] ;
      foaf:name "Rob Atkinson" 
    ] ;
.

bodies:swg a skos:Concept;
    skos:prefLabel "Specification Working Group" ;
    skos:narrower bodies:citygmlswg, bodies:ogcapifeatswg, bodies:landinfraswg ;
    skos:definition "Specification Working Group" ;
    skos:topConceptOf <http://www.opengis.net/def/entities/bodies>
.

bodies:dwg a skos:Concept;
    skos:prefLabel "Domain Working Group" ;
    skos:narrower bodies:landinfradwg ;
    skos:definition "Domain Working Group"
.

bodies:ogcna a skos:Concept;
    skos:prefLabel "OGC Naming Authority" ;
    skos:broader bodies:auth ;
    skos:definition "The primary role of the OGC Naming Authority (OGC-NA) is to ensure an orderly process for assigning URIs for OGC resources, such as OGC documents, standards, XML namespaces, ontologies." ;
    rdfs:seeAlso <https://www.ogc.org/standards/na>, <https://www.ogc.org/projects/groups/ogcnasc> ;
.

bodies:oab a skos:Concept;
    skos:prefLabel "OGC Architecture Board" ;
    skos:broader bodies:auth ;
    skos:definition """The OAB is a forum to discuss the OGC-wide standards architecture. The OAB considers architecture consistency and life cycle management of the OGC standards baseline. The OAB evaluates current technology issues and identify gaps in the architecture that need to be responded to by the Membership.   The OAB provides guidance and recommendations to the TC and the PC.""" ;
    rdfs:seeAlso <https://www.ogc.org/projects/groups/oab> ;
.

bodies:auth a skos:Concept;
    skos:prefLabel "Authorities" ;
    skos:narrower bodies:ogcna, bodies:oab ;
    skos:definition "Authorities and delegated Committees" ;
    skos:topConceptOf <http://www.opengis.net/def/entities/bodies>
.

bodies:omswg  a policy:Swg , skos:Concept ;
  skos:inScheme <http://www.opengis.net/def/entities/bodies> ;
  rdfs:label "Observations and Measurements SWG" ;
  skos:prefLabel "Observations and Measurements SWG" ;
  skos:altLabel "O&M SWG", "O&M 3 SWG"
.

bodies:citygmlswg
  a policy:Swg , skos:Concept ;
  skos:inScheme <http://www.opengis.net/def/entities/bodies> ;
  rdfs:label "OGC CityGML Standards Working Group" ;
  skos:prefLabel "OGC CityGML Standards Working Group" ;
  prov:actedOnBehalfOf bodies:wg3dim ;
.

bodies:ogcapifeatswg
  a policy:Swg , skos:Concept ;
  skos:inScheme <http://www.opengis.net/def/entities/bodies> ;
  rdfs:label "Features API Standards Working Group" ;
  skos:prefLabel "Features API Standards Working Group" ;
  skos:altLabel "OGC API Features SWG"
.

bodies:landinfraswg
  a policy:Swg , skos:Concept ;
  skos:inScheme <http://www.opengis.net/def/entities/bodies> ;
  rdfs:label "The Land and Infrastructure Standards Working Group" ;
  skos:prefLabel "The Land and Infrastructure Standards Working Group" ;
  skos:altLabel "OGC LandInfra SWG"
.

bodies:oapitileswg
  a policy:Swg , skos:Concept ;
  skos:inScheme <http://www.opengis.net/def/entities/bodies> ;
  rdfs:label "OGC API - Tiles SWG" ;
  skos:prefLabel "OGC API - Tiles SWG" ;
  skos:altLabel "OGC API – Tiles Standards Working Group"
.
bodies:oapimapswg
  a policy:Swg , skos:Concept ;
  skos:inScheme <http://www.opengis.net/def/entities/bodies> ;
  rdfs:label "OGC API - Maps SWG" ;
  skos:prefLabel "OGC API - Maps SWG" ;
  skos:altLabel "OGC API – Maps Standards Working Group"
.

bodies:landinfradwg
  a policy:Dwg , skos:Concept ;
  skos:inScheme <http://www.opengis.net/def/entities/bodies> ;
  rdfs:label "The Land and Infrastructure Domain Working Group" ;
  skos:prefLabel "The Land and Infrastructure Domain Working Group" ;
  skos:altLabel "OGC LandInfra DWG"
.

bodies:wg3dim
  a policy:Dwg , skos:Concept;
  skos:inScheme <http://www.opengis.net/def/entities/bodies> ;
  rdfs:comment "CityGML also continues to be developed by the members of the Special Interest Group 3D (SIG 3D) of the GDI-DE Geodateninfrastruktur Deutschland (Spatial Data Infrastructure Germany) in joint cooperation with the 3DIM Working Group and the CityGML SWG within OGC." ;
  rdfs:comment "Should http://www.opengeospatial.org/projects/groups/3dimwg  be the canonical URI here? - can it behave as a def? " ;
  skos:prefLabel "OGC 3D Information Management (3DIM) Working Group" ;
  rdfs:seeAlso <http://www.opengeospatial.org/projects/groups/3dimwg> ;
  rdfs:seeAlso <http://www.sig3d.org/> ;
.
