@prefix adms: <http://www.w3.org/ns/adms#> .
@prefix dcat: <http://www.w3.org/ns/dcat#> .
@prefix dct: <http://purl.org/dc/terms/> .
@prefix na: <http://www.opengis.net/def/metamodel/ogc-na/> .
@prefix ns1: <http://purl.org/dc/elements/1.1/> .
@prefix ns2: <https://schema.org/> .
@prefix ogcdt: <http://www.opengis.net/def/doc-type/> .
@prefix owl: <http://www.w3.org/2002/07/owl#> .
@prefix prov: <http://www.w3.org/ns/prov#> .
@prefix rdfs: <http://www.w3.org/2000/01/rdf-schema#> .
@prefix reg: <http://purl.org/linked-data/registry#> .
@prefix skos: <http://www.w3.org/2004/02/skos/core#> .
@prefix spec: <http://www.opengis.net/def/ont/modspec/> .
@prefix specrel: <http://www.opengis.net/def/ont/specrel/> .
@prefix status: <http://www.opengis.net/def/status/> .
@prefix wg: <http://www.opengis.net/def/wg/> .
@prefix xsd: <http://www.w3.org/2001/XMLSchema#> .

dct:hasPart a owl:ObjectProperty ;
    skos:prefLabel "Has Part" .

reg:Register a owl:Class ;
    skos:prefLabel "Governed Artefact" .

spec:Basic a spec:TestType ;
    skos:prefLabel "Basic" .

spec:CM a spec:StandardizationTargetType ;
    skos:prefLabel "Conceptual Model" .

<http://www.opengis.net/def/ont/modspec_validations> a owl:Ontology ;
    ns1:creator "Rob Atkinson" ;
    ns1:description "Minimal validation helpers for instances of the Modspec ontology." ;
    ns1:rights "Copyright © 2021 Open Geospatial Consortium. To obtain additional rights of use, visit http://www.opengeospatial.org/legal/" ;
    ns1:source "The Specification Model — A Standard for Modular specifications. OGC document 08-131r3 https://portal.opengeospatial.org/files/34762" ;
    ns1:title "The Specification Model — A Standard for Modular specifications" ;
    dct:modified "2015-06-10" ;
    rdfs:comment "Needed until pySHACL can be told to use core model without trying to validate it all against a different set of rules" ;
    rdfs:isDefinedBy <http://www.opengis.net/doc/modular-spec> ;
    skos:prefLabel "An RDF/OWL ontology for modular specifications" .

status:iso19135 a skos:Collection ;
    dct:source <https://def.isotc211.org/iso19135/-1/2015/CoreModel.rdf> ;
    skos:definition "Register Item status values according to ISO19135."@en ;
    skos:inScheme <http://www.opengis.net/def/status>,
        <http://www.opengis.net/spec/landinfra/1.0> ;
    skos:member status:invalid,
        status:retired,
        status:submitted,
        status:superseded,
        status:valid ;
    skos:prefLabel "ISO 19135 Register Item status values"@en .

<http://www.opengis.net/spec/docs/15-111r1-anno> a owl:Ontology .

<http://www.opengis.net/spec/landinfra/1.0/> a skos:Collection ;
    dct:source <http://www.opengis.net/def/docs/15-111r1> ;
    skos:definition "LandInfra conceptual model collection of Conformance Classes" ;
    skos:inScheme <http://www.opengis.net/def/status>,
        <http://www.opengis.net/spec/landinfra/1.0> .

status: a skos:Collection ;
    dct:provenance "ISO19135 and subsequent Linked Data Registry extensions"@en ;
    skos:definition "Register Item statuses from ISO19135 and subsequent Linked Data Registry extensions."@en ;
    skos:inScheme <http://www.opengis.net/def/status>,
        <http://www.opengis.net/spec/landinfra/1.0> ;
    skos:member status:accepted,
        status:deprecated,
        status:experimental,
        status:invalid,
        status:notAccepted,
        status:reserved,
        status:retired,
        status:stable,
        status:submitted,
        status:superseded,
        status:valid ;
    skos:prefLabel "Register Item status values"@en .

status:under-development a na:Status,
        skos:Concept ;
    na:status status:experimental ;
    rdfs:isDefinedBy <http://www.opengis.net/def/status> ;
    skos:broader status:notAccepted ;
    skos:definition "An entry that is under development, but is part of a committed roadmap, rather than experimental"@en ;
    skos:inScheme <http://www.opengis.net/def/status> ;
    skos:prefLabel "Under Development"@en .

status:reserved a na:Status,
        skos:Concept ;
    dct:source reg: ;
    na:status status:stable ;
    rdfs:isDefinedBy <http://www.opengis.net/def/status> ;
    owl:sameAs reg:statusReserved ;
    skos:broader status:notAccepted ;
    skos:definition "A reserved entry allocated for some as yet undetermined future use."@en ;
    skos:inScheme <http://www.opengis.net/def/status> ;
    skos:prefLabel "reserved"@en .

<http://www.opengis.net/spec/landinfra/1.0/conf/alignment/CRS> a spec:ConformanceTest,
        skos:Concept ;
    spec:method "Inspect the encoding to verify the above requirement." ;
    spec:purpose "Verify that an encoding requires that all geometry/locations for Alignment2DHorSegments and Alignment2DVertSegments be specified using the Alignment2DHorizontal.crs which shall be a Cartesian local engineering reference system." ;
    spec:requirement <http://www.opengis.net/spec/landinfra/1.0/req/alignment/CRS> ;
    spec:testType spec:Capabilities ;
    skos:broader <http://www.opengis.net/spec/landinfra/1.0/conf/alignment> ;
    skos:definition "Verify that an encoding requires that all geometry/locations for Alignment2DHorSegments and Alignment2DVertSegments be specified using the Alignment2DHorizontal.crs which shall be a Cartesian local engineering reference system." ;
    skos:inScheme <http://www.opengis.net/def/status>,
        <http://www.opengis.net/spec/landinfra/1.0> ;
    skos:prefLabel "Conformance Test http://www.opengis.net/spec/landinfra/1.0/conf/alignment/CRS" .

<http://www.opengis.net/spec/landinfra/1.0/conf/alignment/LR-interfaces> a spec:ConformanceTest,
        skos:Concept ;
    spec:method "Inspect the encoding to verify the above requirement." ;
    spec:purpose "Verify that the encoding implements the OGC Abstract Specification Topic 19 ILinearElement and ISpatial interfaces in a manner consistent with the encoding." ;
    spec:requirement <http://www.opengis.net/spec/landinfra/1.0/req/alignment/LR-interfaces> ;
    spec:testType spec:Capabilities ;
    skos:broader <http://www.opengis.net/spec/landinfra/1.0/conf/alignment> ;
    skos:definition "Verify that the encoding implements the OGC Abstract Specification Topic 19 ILinearElement and ISpatial interfaces in a manner consistent with the encoding." ;
    skos:inScheme <http://www.opengis.net/def/status>,
        <http://www.opengis.net/spec/landinfra/1.0> ;
    skos:prefLabel "Conformance Test http://www.opengis.net/spec/landinfra/1.0/conf/alignment/LR-interfaces" .

<http://www.opengis.net/spec/landinfra/1.0/conf/alignment/classes> a spec:ConformanceTest,
        skos:Concept ;
    spec:method "Inspect the encoding to verify the above requirement." ;
    spec:purpose "If an encoding includes Alignments, then verify that the encoding provides the Alignment Requirements Class Classes shown in blue in Figure 15 in a manner consistent with the encoding." ;
    spec:requirement <http://www.opengis.net/spec/landinfra/1.0/req/alignment/classes> ;
    spec:testType spec:Capabilities ;
    skos:broader <http://www.opengis.net/spec/landinfra/1.0/conf/alignment> ;
    skos:definition "If an encoding includes Alignments, then verify that the encoding provides the Alignment Requirements Class Classes shown in blue in Figure 15 in a manner consistent with the encoding." ;
    skos:inScheme <http://www.opengis.net/def/status>,
        <http://www.opengis.net/spec/landinfra/1.0> ;
    skos:prefLabel "Conformance Test http://www.opengis.net/spec/landinfra/1.0/conf/alignment/classes" .

<http://www.opengis.net/spec/landinfra/1.0/conf/alignment/description> a spec:ConformanceTest,
        skos:Concept ;
    spec:method "Inspect the encoding to verify the above requirement." ;
    spec:purpose "Verify that an encoding which includes Alignments shall specify that all of the included Alignments shall be continuous, non-overlapping, and non-branching (though it may contain intersections with other Alignments) and that if it is used within the context of a Project, the included Alignment shall be for a single alternative, as specified by the ProjectPart." ;
    spec:requirement <http://www.opengis.net/spec/landinfra/1.0/req/alignment/description> ;
    spec:testType spec:Capabilities ;
    skos:broader <http://www.opengis.net/spec/landinfra/1.0/conf/alignment> ;
    skos:definition "Verify that an encoding which includes Alignments shall specify that all of the included Alignments shall be continuous, non-overlapping, and non-branching (though it may contain intersections with other Alignments) and that if it is used within the context of a Project, the included Alignment shall be for a single alternative, as specified by the ProjectPart." ;
    skos:inScheme <http://www.opengis.net/def/status>,
        <http://www.opengis.net/spec/landinfra/1.0> ;
    skos:prefLabel "Conformance Test http://www.opengis.net/spec/landinfra/1.0/conf/alignment/description" .

<http://www.opengis.net/spec/landinfra/1.0/conf/alignment/measures> a spec:ConformanceTest,
        skos:Concept ;
    spec:method "Inspect the encoding to verify the above requirement." ;
    spec:purpose """If an encoding uses Alignment as a linear element, verify that it specifies that:
1) If an Alignment2DHorizontal.2DLinestringRepresentation or an Alignment3D.3DLinestringRepresentation is specified as a linear element, then distanceAlong shall be measured along the LineString and offsetLateralDistance and offsetVerticalDistance values shall be measured normal to the LineString from this DistanceAlong point.
2) If an Alignment2DHorizontal.segment list of Alignment2DHorSegments is used as a linear element, then distanceAlong and offsetLateralDistance values shall be measured in the horizontal plane, ignoring any vertical displacement of the Alignment.  OffsetVerticalDistance values shall be absolute from the horizontal plane unless an Alignment2DVertical is specified as a VerticalOffsetReferent so as to take into consideration vertical displacement of the Alignment, if present.""" ;
    spec:requirement <http://www.opengis.net/spec/landinfra/1.0/req/alignment/measures> ;
    spec:testType spec:Capabilities ;
    skos:broader <http://www.opengis.net/spec/landinfra/1.0/conf/alignment> ;
    skos:definition """If an encoding uses Alignment as a linear element, verify that it specifies that:
1) If an Alignment2DHorizontal.2DLinestringRepresentation or an Alignment3D.3DLinestringRepresentation is specified as a linear element, then distanceAlong shall be measured along the LineString and offsetLateralDistance and offsetVerticalDistance values shall be measured normal to the LineString from this DistanceAlong point.
2) If an Alignment2DHorizontal.segment list of Alignment2DHorSegments is used as a linear element, then distanceAlong and offsetLateralDistance values shall be measured in the horizontal plane, ignoring any vertical displacement of the Alignment.  OffsetVerticalDistance values shall be absolute from the horizontal plane unless an Alignment2DVertical is specified as a VerticalOffsetReferent so as to take into consideration vertical displacement of the Alignment, if present.""" ;
    skos:inScheme <http://www.opengis.net/def/status>,
        <http://www.opengis.net/spec/landinfra/1.0> ;
    skos:prefLabel "Conformance Test http://www.opengis.net/spec/landinfra/1.0/conf/alignment/measures" .

<http://www.opengis.net/spec/landinfra/1.0/conf/condominium/classes> a spec:ConformanceTest,
        skos:Concept ;
    spec:method "Inspect the encoding to verify the above requirement." ;
    spec:purpose "Verify that the encoding provides the Condominium Requirements Class Classes shown in blue in Figure 68 in a manner consistent with the encoding." ;
    spec:requirement <http://www.opengis.net/spec/landinfra/1.0/req/condominium/classes> ;
    spec:testType spec:Capabilities ;
    skos:broader <http://www.opengis.net/spec/landinfra/1.0/conf/condominium> ;
    skos:definition "Verify that the encoding provides the Condominium Requirements Class Classes shown in blue in Figure 68 in a manner consistent with the encoding." ;
    skos:inScheme <http://www.opengis.net/def/status>,
        <http://www.opengis.net/spec/landinfra/1.0> ;
    skos:prefLabel "Conformance Test http://www.opengis.net/spec/landinfra/1.0/conf/condominium/classes" .

<http://www.opengis.net/spec/landinfra/1.0/conf/equipment/classes> a spec:ConformanceTest,
        skos:Concept ;
    spec:method "Inspect the encoding to verify the above requirement." ;
    spec:purpose "Verify that the encoding provides the Equipment Requirements Class Classes shown in blue in Figure 48 in a manner consistent with the encoding.  An encoding shall decide which SurveySensor types it will support and define appropriate requirements classes accordingly." ;
    spec:requirement <http://www.opengis.net/spec/landinfra/1.0/req/equipment/classes> ;
    spec:testType spec:Capabilities ;
    skos:broader <http://www.opengis.net/spec/landinfra/1.0/conf/equipment> ;
    skos:definition "Verify that the encoding provides the Equipment Requirements Class Classes shown in blue in Figure 48 in a manner consistent with the encoding.  An encoding shall decide which SurveySensor types it will support and define appropriate requirements classes accordingly." ;
    skos:inScheme <http://www.opengis.net/def/status>,
        <http://www.opengis.net/spec/landinfra/1.0> ;
    skos:prefLabel "Conformance Test: http://www.opengis.net/spec/landinfra/1.0/conf/equipment/classes" .

<http://www.opengis.net/spec/landinfra/1.0/conf/equipment/observation-correction> a spec:ConformanceTest,
        skos:Concept ;
    spec:method "Inspect the encoding to verify the above requirement." ;
    spec:purpose "Verify that the encoding provides the ObservationCorrection Classes in blue in Figure 51 in a manner consistent with the encoding.  The encoding shall decide which correction types it will support and define appropriate requirements classes accordingly." ;
    spec:requirement <http://www.opengis.net/spec/landinfra/1.0/req/equipment/observation-correction> ;
    spec:testType spec:Capabilities ;
    skos:broader <http://www.opengis.net/spec/landinfra/1.0/conf/equipment> ;
    skos:definition "Verify that the encoding provides the ObservationCorrection Classes in blue in Figure 51 in a manner consistent with the encoding.  The encoding shall decide which correction types it will support and define appropriate requirements classes accordingly." ;
    skos:inScheme <http://www.opengis.net/def/status>,
        <http://www.opengis.net/spec/landinfra/1.0> ;
    skos:prefLabel "Conformance Test: http://www.opengis.net/spec/landinfra/1.0/conf/equipment/observation-correction" .

<http://www.opengis.net/spec/landinfra/1.0/conf/facility/classes> a spec:ConformanceTest,
        skos:Concept ;
    spec:dependency <http://www.opengis.net/spec/landinfra/1.0/conf/land-infra> ;
    spec:method "Inspect the encoding to verify the above requirement." ;
    spec:purpose "Verify that the encoding provides the Facility Requirements class Classes shown in blue in Figure 10 in a manner consistent with the encoding." ;
    spec:requirement <http://www.opengis.net/spec/landinfra/1.0/req/facility/classes> ;
    spec:testType spec:Capabilities ;
    skos:broader <http://www.opengis.net/spec/landinfra/1.0/conf/facility> ;
    skos:definition "Verify that the encoding provides the Facility Requirements class Classes shown in blue in Figure 10 in a manner consistent with the encoding." ;
    skos:inScheme <http://www.opengis.net/def/status>,
        <http://www.opengis.net/spec/landinfra/1.0> ;
    skos:prefLabel "Conformance Test: http://www.opengis.net/spec/landinfra/1.0/conf/facility/classes" .

<http://www.opengis.net/spec/landinfra/1.0/conf/land-division/classes> a spec:ConformanceTest,
        skos:Concept ;
    spec:method "Inspect the encoding to verify the above requirement." ;
    spec:purpose "Verify that the encoding provides the LandDivision Requirements Class Classes shown in blue in Figure 60 in a manner consistent with the encoding." ;
    spec:requirement <http://www.opengis.net/spec/landinfra/1.0/req/land-division/classes> ;
    spec:testType spec:Capabilities ;
    skos:broader <http://www.opengis.net/spec/landinfra/1.0/conf/land-division> ;
    skos:definition "Verify that the encoding provides the LandDivision Requirements Class Classes shown in blue in Figure 60 in a manner consistent with the encoding." ;
    skos:inScheme <http://www.opengis.net/def/status>,
        <http://www.opengis.net/spec/landinfra/1.0> ;
    skos:prefLabel "ConformanceTest: http://www.opengis.net/spec/landinfra/1.0/conf/land-division/classes" .

<http://www.opengis.net/spec/landinfra/1.0/conf/land-feature/classes> a spec:ConformanceTest,
        skos:Concept ;
    spec:method "Inspect the encoding to verify the above requirement." ;
    spec:purpose "Verify that the encoding provides the LandFeature Requirements Class Classes shown in blue in Figure 55 in a manner consistent with the encoding." ;
    spec:requirement <http://www.opengis.net/spec/landinfra/1.0/req/land-feature/classes> ;
    spec:testType spec:Capabilities ;
    skos:broader <http://www.opengis.net/spec/landinfra/1.0/conf/land-feature> ;
    skos:definition "Verify that the encoding provides the LandFeature Requirements Class Classes shown in blue in Figure 55 in a manner consistent with the encoding." ;
    skos:inScheme <http://www.opengis.net/def/status>,
        <http://www.opengis.net/spec/landinfra/1.0> ;
    skos:prefLabel "ConformanceTest: http://www.opengis.net/spec/landinfra/1.0/conf/land-feature/classes" .

<http://www.opengis.net/spec/landinfra/1.0/conf/land-infra/19103> a spec:ConformanceTest,
        skos:Concept ;
    spec:method "Inspect the encoding to verify the above requirement." ;
    spec:purpose "Verify that the encoding provides the core data types specified in ISO 19103 Clause 7 and shown in pink in Figure 5 that are appropriate to the supported subject area(s)." ;
    spec:requirement <http://www.opengis.net/spec/landinfra/1.0/req/land-infra/19103> ;
    spec:testType spec:Capabilities ;
    skos:broader <http://www.opengis.net/spec/landinfra/1.0/conf/land-infra> ;
    skos:definition "Verify that the encoding provides the core data types specified in ISO 19103 Clause 7 and shown in pink in Figure 5 that are appropriate to the supported subject area(s)." ;
    skos:inScheme <http://www.opengis.net/def/status>,
        <http://www.opengis.net/spec/landinfra/1.0> ;
    skos:prefLabel "Conformance Test: http://www.opengis.net/spec/landinfra/1.0/conf/land-infra/19103" .

<http://www.opengis.net/spec/landinfra/1.0/conf/land-infra/19109> a spec:ConformanceTest,
        skos:Concept ;
    spec:method "Inspect the encoding to verify the above requirement." ;
    spec:purpose "Verify that Features shall be supported by a Land and Infrastructure encoding in accordance with the uml:feature requirement in ISO 19109:2015 Clause 8.2.6 and shown in Figure 9, as follows:   Each instance of FeatureType shall be implemented by the encoding’s equivalent of a UML Class having a generalization association with AnyFeature and with a stereotype of <<FeatureType>>." ;
    spec:requirement <http://www.opengis.net/spec/landinfra/1.0/req/land-infra/19109> ;
    spec:testType spec:Capabilities ;
    skos:broader <http://www.opengis.net/spec/landinfra/1.0/conf/land-infra> ;
    skos:definition "Verify that Features shall be supported by a Land and Infrastructure encoding in accordance with the uml:feature requirement in ISO 19109:2015 Clause 8.2.6 and shown in Figure 9, as follows:   Each instance of FeatureType shall be implemented by the encoding’s equivalent of a UML Class having a generalization association with AnyFeature and with a stereotype of <<FeatureType>>." ;
    skos:inScheme <http://www.opengis.net/def/status>,
        <http://www.opengis.net/spec/landinfra/1.0> ;
    skos:prefLabel "Conformance Test: http://www.opengis.net/spec/landinfra/1.0/conf/land-infra/19109" .

<http://www.opengis.net/spec/landinfra/1.0/conf/land-infra/classes> a spec:ConformanceTest,
        skos:Concept ;
    spec:method "Inspect the encoding to verify the above requirement." ;
    spec:purpose "Verify that theencoding provides the LandInfra Requirements Class Classes shown in blue in Figure 2 in a manner consistent with the encoding." ;
    spec:requirement <http://www.opengis.net/spec/landinfra/1.0/req/land-infra/classes> ;
    spec:testType spec:Capabilities ;
    skos:broader <http://www.opengis.net/spec/landinfra/1.0/conf/land-infra> ;
    skos:definition "Verify that theencoding provides the LandInfra Requirements Class Classes shown in blue in Figure 2 in a manner consistent with the encoding." ;
    skos:inScheme <http://www.opengis.net/def/status>,
        <http://www.opengis.net/spec/landinfra/1.0> ;
    skos:prefLabel "Conformance Test: http://www.opengis.net/spec/landinfra/1.0/conf/land-infra/classes" .

<http://www.opengis.net/spec/landinfra/1.0/conf/land-infra/crs> a spec:ConformanceTest,
        skos:Concept ;
    spec:method "Inspect the encoding to verify the above requirement." ;
    spec:purpose "Verify that the encoding requirement for coordinate reference systems is consistent with OGC Abstract Specification Topic 2." ;
    spec:requirement <http://www.opengis.net/spec/landinfra/1.0/req/land-infra/crs> ;
    spec:testType spec:Capabilities ;
    skos:broader <http://www.opengis.net/spec/landinfra/1.0/conf/land-infra> ;
    skos:definition "Verify that the encoding requirement for coordinate reference systems is consistent with OGC Abstract Specification Topic 2." ;
    skos:inScheme <http://www.opengis.net/def/status>,
        <http://www.opengis.net/spec/landinfra/1.0> ;
    skos:prefLabel "Conformance Test: http://www.opengis.net/spec/landinfra/1.0/conf/land-infra/crs" .

<http://www.opengis.net/spec/landinfra/1.0/conf/land-infra/dataset> a spec:ConformanceTest,
        skos:Concept ;
    spec:method "Inspect the encoding to verify the above requirement." ;
    spec:purpose "Verify that the encoding specifies a LandInfra dataset in a format appropriate for that encoding." ;
    spec:requirement <http://www.opengis.net/spec/landinfra/1.0/req/land-infra/dataset> ;
    spec:testType spec:Capabilities ;
    skos:broader <http://www.opengis.net/spec/landinfra/1.0/conf/land-infra> ;
    skos:definition "Verify that the encoding specifies a LandInfra dataset in a format appropriate for that encoding." ;
    skos:inScheme <http://www.opengis.net/def/status>,
        <http://www.opengis.net/spec/landinfra/1.0> ;
    skos:prefLabel "Conformance Test: http://www.opengis.net/spec/landinfra/1.0/conf/land-infra/dataset" .

<http://www.opengis.net/spec/landinfra/1.0/conf/land-infra/featureID> a spec:ConformanceTest,
        skos:Concept ;
    spec:method "Inspect the encoding to verify the above requirement." ;
    spec:purpose "Verify that the encoding specifies whether it supports ID at the feature level, ID at the Feature sub-type level, or both." ;
    spec:requirement <http://www.opengis.net/spec/landinfra/1.0/req/land-infra/featureID> ;
    spec:testType spec:Capabilities ;
    skos:broader <http://www.opengis.net/spec/landinfra/1.0/conf/land-infra> ;
    skos:definition "Verify that the encoding specifies whether it supports ID at the feature level, ID at the Feature sub-type level, or both." ;
    skos:inScheme <http://www.opengis.net/def/status>,
        <http://www.opengis.net/spec/landinfra/1.0> ;
    skos:prefLabel "Conformance Test: http://www.opengis.net/spec/landinfra/1.0/conf/land-infra/featureID" .

<http://www.opengis.net/spec/landinfra/1.0/conf/land-infra/subjects> a spec:ConformanceTest,
        skos:Concept ;
    spec:method "Inspect the encoding to verify the above requirement." ;
    spec:purpose "Verify that the encoding specifies which of the LandInfra subjects it supports." ;
    spec:requirement <http://www.opengis.net/spec/landinfra/1.0/req/land-infra/subjects> ;
    spec:testType spec:Capabilities ;
    skos:broader <http://www.opengis.net/spec/landinfra/1.0/conf/land-infra> ;
    skos:definition "Verify that the encoding specifies which of the LandInfra subjects it supports." ;
    skos:inScheme <http://www.opengis.net/def/status>,
        <http://www.opengis.net/spec/landinfra/1.0> ;
    skos:prefLabel "Conformance Test: http://www.opengis.net/spec/landinfra/1.0/conf/land-infra/subjects" .

<http://www.opengis.net/spec/landinfra/1.0/conf/land-infra/topic-1> a spec:ConformanceTest,
        skos:Concept ;
    spec:method "Inspect the encoding to verify the above requirement." ;
    spec:purpose """Verify that the encoding provides the geometry types specified in the OGC Abstract Specification Topic 1, Feature Geometry as shown in pink and the SimpleTriangle, TIN, and PolyfaceMesh extensions shown in beige in Figure 6, that are appropriate to the supported subject area(s).
  Verify that the encoding provides the additional geometry types not found in Topic 1, but required by a specific supported requirements class, are specified in that requirements class.""" ;
    spec:requirement <http://www.opengis.net/spec/landinfra/1.0/req/land-infra/topic-1> ;
    spec:testType spec:Capabilities ;
    skos:broader <http://www.opengis.net/spec/landinfra/1.0/conf/land-infra> ;
    skos:definition """Verify that the encoding provides the geometry types specified in the OGC Abstract Specification Topic 1, Feature Geometry as shown in pink and the SimpleTriangle, TIN, and PolyfaceMesh extensions shown in beige in Figure 6, that are appropriate to the supported subject area(s).
  Verify that the encoding provides the additional geometry types not found in Topic 1, but required by a specific supported requirements class, are specified in that requirements class.""" ;
    skos:inScheme <http://www.opengis.net/def/status>,
        <http://www.opengis.net/spec/landinfra/1.0> ;
    skos:prefLabel "Conformance Test: http://www.opengis.net/spec/landinfra/1.0/conf/land-infra/topic-1" .

<http://www.opengis.net/spec/landinfra/1.0/conf/land-infra/topic-19-core> a spec:ConformanceTest,
        skos:Concept ;
    spec:method "Inspect the encoding to verify the above requirement." ;
    spec:purpose "Verify that, if the encoding supports linearly referenced locations, then the encoding provides the PositionExpression and related Classes specified in the OGC Abstract Specification Topic 19, core Linear Referencing (LR) Package shown in pink in Figure 7 that are appropriate to the supported subject area(s)." ;
    spec:requirement <http://www.opengis.net/spec/landinfra/1.0/req/land-infra/topic-19-core> ;
    spec:testType spec:Capabilities ;
    skos:broader <http://www.opengis.net/spec/landinfra/1.0/conf/land-infra> ;
    skos:definition "Verify that, if the encoding supports linearly referenced locations, then the encoding provides the PositionExpression and related Classes specified in the OGC Abstract Specification Topic 19, core Linear Referencing (LR) Package shown in pink in Figure 7 that are appropriate to the supported subject area(s)." ;
    skos:inScheme <http://www.opengis.net/def/status>,
        <http://www.opengis.net/spec/landinfra/1.0> ;
    skos:prefLabel "Conformance Test: http://www.opengis.net/spec/landinfra/1.0/conf/land-infra/topic-19-core" .

<http://www.opengis.net/spec/landinfra/1.0/conf/land-infra/topic-19-extensions> a spec:ConformanceTest,
        skos:Concept ;
    spec:method "Inspect the encoding to verify the above requirement." ;
    spec:purpose "Verify that, if the encoding supports linearly referenced locations, then the encoding specifies which of the OGC Abstract Specification Topic 19, Linear Referencing extension packages it supports and therefore supports the appropriate Classes shown in Figure 7 and Figure 8 for those packages that are appropriate to the supported subject area(s)." ;
    spec:requirement <http://www.opengis.net/spec/landinfra/1.0/req/land-infra/topic-19-extensions> ;
    spec:testType spec:Capabilities ;
    skos:broader <http://www.opengis.net/spec/landinfra/1.0/conf/land-infra> ;
    skos:definition "Verify that, if the encoding supports linearly referenced locations, then the encoding specifies which of the OGC Abstract Specification Topic 19, Linear Referencing extension packages it supports and therefore supports the appropriate Classes shown in Figure 7 and Figure 8 for those packages that are appropriate to the supported subject area(s)." ;
    skos:inScheme <http://www.opengis.net/def/status>,
        <http://www.opengis.net/spec/landinfra/1.0> ;
    skos:prefLabel "Conformance Test: Conformance Test: http://www.opengis.net/spec/landinfra/1.0/conf/land-infra/topic-19-extensions" .

<http://www.opengis.net/spec/landinfra/1.0/conf/observations/classes> a spec:ConformanceTest,
        skos:Concept ;
    spec:method "Inspect the encoding to verify the above requirement." ;
    spec:purpose "Verify that the encoding provides the Observation Requirements Class Classes shown in blue in Figure 43 in a manner consistent with the encoding.  An encoding shall decide which SurveyObservation types it will support and define appropriate requirements classes accordingly. This then would include any dependent types (example SatelliteSystemType has only to be supported if the encoding will support GNSS Observations)." ;
    spec:requirement <http://www.opengis.net/spec/landinfra/1.0/req/observations/classes> ;
    spec:testType spec:Capabilities ;
    skos:broader <http://www.opengis.net/spec/landinfra/1.0/conf/observations> ;
    skos:definition "Verify that the encoding provides the Observation Requirements Class Classes shown in blue in Figure 43 in a manner consistent with the encoding.  An encoding shall decide which SurveyObservation types it will support and define appropriate requirements classes accordingly. This then would include any dependent types (example SatelliteSystemType has only to be supported if the encoding will support GNSS Observations)." ;
    skos:inScheme <http://www.opengis.net/def/status>,
        <http://www.opengis.net/spec/landinfra/1.0> ;
    skos:prefLabel "Conformance Test: http://www.opengis.net/spec/landinfra/1.0/conf/observations/classes" .

<http://www.opengis.net/spec/landinfra/1.0/conf/project/classes> a spec:ConformanceTest,
        skos:Concept ;
    spec:dependency <http://www.opengis.net/spec/landinfra/1.0/conf/facility> ;
    spec:method "Inspect the encoding to verify the above requirement." ;
    spec:purpose "Verify that the encoding provides the Project Requirements Class Classes shown in blue in Figure 13 in a manner consistent with the encoding." ;
    spec:requirement <http://www.opengis.net/spec/landinfra/1.0/req/project/classes> ;
    spec:testType spec:Capabilities ;
    skos:broader <http://www.opengis.net/spec/landinfra/1.0/conf/project> ;
    skos:definition "Verify that the encoding provides the Project Requirements Class Classes shown in blue in Figure 13 in a manner consistent with the encoding." ;
    skos:inScheme <http://www.opengis.net/def/status>,
        <http://www.opengis.net/spec/landinfra/1.0> ;
    skos:prefLabel "Conformance Test: http://www.opengis.net/spec/landinfra/1.0/conf/project/classes" .

<http://www.opengis.net/spec/landinfra/1.0/conf/railway/alignment> a spec:ConformanceTest,
        skos:Concept ;
    spec:method "Inspect the encoding to verify the above requirement." ;
    spec:purpose "Verify that if the encoding allows the linear element used for locating RailwayElements or CantEvents to be an Alignment, then that encoding supports the Alignment Requirements Class." ;
    spec:requirement <http://www.opengis.net/spec/landinfra/1.0/req/railway/alignment> ;
    spec:testType spec:Capabilities ;
    skos:broader <http://www.opengis.net/spec/landinfra/1.0/conf/railway> ;
    skos:definition "Verify that if the encoding allows the linear element used for locating RailwayElements or CantEvents to be an Alignment, then that encoding supports the Alignment Requirements Class." ;
    skos:inScheme <http://www.opengis.net/def/status>,
        <http://www.opengis.net/spec/landinfra/1.0> ;
    skos:prefLabel "http://www.opengis.net/spec/landinfra/1.0/conf/railway/alignment" .

<http://www.opengis.net/spec/landinfra/1.0/conf/railway/cant> a spec:ConformanceTest,
        skos:Concept ;
    spec:method "Inspect the encoding to verify the above requirement." ;
    spec:purpose "Verify that the encoding specifies as a requirement that each CantSpecification shall cover the entire linear element the CantSpecification is located along from the linear element’s start to its end, and that the CantSpecification shall include CantEvents at the start and end of the linear element and wherever else there is a cant break along the linear element." ;
    spec:requirement <http://www.opengis.net/spec/landinfra/1.0/req/railway/cant> ;
    spec:testType spec:Capabilities ;
    skos:broader <http://www.opengis.net/spec/landinfra/1.0/conf/railway> ;
    skos:definition "Verify that the encoding specifies as a requirement that each CantSpecification shall cover the entire linear element the CantSpecification is located along from the linear element’s start to its end, and that the CantSpecification shall include CantEvents at the start and end of the linear element and wherever else there is a cant break along the linear element." ;
    skos:inScheme <http://www.opengis.net/def/status>,
        <http://www.opengis.net/spec/landinfra/1.0> ;
    skos:prefLabel "http://www.opengis.net/spec/landinfra/1.0/conf/railway/cant" .

<http://www.opengis.net/spec/landinfra/1.0/conf/railway/classes> a spec:ConformanceTest,
        skos:Concept ;
    spec:method "Inspect the encoding to verify the above requirement." ;
    spec:purpose "Verify that the encoding provides the Railway Requirements Class Classes shown in blue in Figure 36 in a manner consistent with the encoding." ;
    spec:requirement <http://www.opengis.net/spec/landinfra/1.0/req/railway/classes> ;
    spec:testType spec:Capabilities ;
    skos:broader <http://www.opengis.net/spec/landinfra/1.0/conf/railway> ;
    skos:definition "Verify that the encoding provides the Railway Requirements Class Classes shown in blue in Figure 36 in a manner consistent with the encoding." ;
    skos:inScheme <http://www.opengis.net/def/status>,
        <http://www.opengis.net/spec/landinfra/1.0> ;
    skos:prefLabel "http://www.opengis.net/spec/landinfra/1.0/conf/railway/classes" .

<http://www.opengis.net/spec/landinfra/1.0/conf/road-cross-section/alignment> a spec:ConformanceTest,
        skos:Concept ;
    spec:method "Inspect the encoding to verify the above requirement." ;
    spec:purpose "Verify that if the encoding allows the linear element used for locating CrossSections to be an Alignment, then that encoding supports the Alignment Requirements Class." ;
    spec:requirement <http://www.opengis.net/spec/landinfra/1.0/req/road-cross-section/alignment> ;
    spec:testType spec:Capabilities ;
    skos:broader <http://www.opengis.net/spec/landinfra/1.0/conf/road-cross-section> ;
    skos:definition "Verify that if the encoding allows the linear element used for locating CrossSections to be an Alignment, then that encoding supports the Alignment Requirements Class." ;
    skos:inScheme <http://www.opengis.net/def/status>,
        <http://www.opengis.net/spec/landinfra/1.0> ;
    skos:prefLabel "http://www.opengis.net/spec/landinfra/1.0/conf/road-cross-section/alignment" .

<http://www.opengis.net/spec/landinfra/1.0/conf/road-cross-section/classes> a spec:ConformanceTest,
        skos:Concept ;
    spec:method "Inspect the encoding to verify the above requirement." ;
    spec:purpose "Verify that the encoding provides the RoadCrossSection Requirements Class Classes shown in blue in Figure 25 in a manner consistent with the encoding." ;
    spec:requirement <http://www.opengis.net/spec/landinfra/1.0/req/road-cross-section/classes> ;
    spec:testType spec:Capabilities ;
    skos:broader <http://www.opengis.net/spec/landinfra/1.0/conf/road-cross-section> ;
    skos:definition "Verify that the encoding provides the RoadCrossSection Requirements Class Classes shown in blue in Figure 25 in a manner consistent with the encoding." ;
    skos:inScheme <http://www.opengis.net/def/status>,
        <http://www.opengis.net/spec/landinfra/1.0> ;
    skos:prefLabel "http://www.opengis.net/spec/landinfra/1.0/conf/road-cross-section/classes" .

<http://www.opengis.net/spec/landinfra/1.0/conf/road/alignment> a spec:ConformanceTest,
        skos:Concept ;
    spec:method "Inspect the encoding to verify the above requirement." ;
    spec:purpose "Verify that if the encoding allows the linear element used for locating RoadElements to be an Alignment, then that encoding supports the Alignment Requirements Class." ;
    spec:requirement <http://www.opengis.net/spec/landinfra/1.0/req/road/alignment> ;
    spec:testType spec:Capabilities ;
    skos:broader <http://www.opengis.net/spec/landinfra/1.0/conf/road> ;
    skos:definition "Verify that if the encoding allows the linear element used for locating RoadElements to be an Alignment, then that encoding supports the Alignment Requirements Class." ;
    skos:inScheme <http://www.opengis.net/def/status>,
        <http://www.opengis.net/spec/landinfra/1.0> ;
    skos:prefLabel "http://www.opengis.net/spec/landinfra/1.0/conf/road/alignment" .

<http://www.opengis.net/spec/landinfra/1.0/conf/road/classes> a spec:ConformanceTest,
        skos:Concept ;
    spec:method "Inspect the encoding to verify the above requirement." ;
    spec:purpose "Verify that the encoding provides the Road Requirements Class Classes shown in blue in Figure 21 in a manner consistent with the encoding." ;
    spec:requirement <http://www.opengis.net/spec/landinfra/1.0/req/road/classes> ;
    spec:testType spec:Capabilities ;
    skos:broader <http://www.opengis.net/spec/landinfra/1.0/conf/road> ;
    skos:definition "Verify that the encoding provides the Road Requirements Class Classes shown in blue in Figure 21 in a manner consistent with the encoding." ;
    skos:inScheme <http://www.opengis.net/def/status>,
        <http://www.opengis.net/spec/landinfra/1.0> ;
    skos:prefLabel "http://www.opengis.net/spec/landinfra/1.0/conf/road/classes" .

<http://www.opengis.net/spec/landinfra/1.0/conf/survey-results/classes> a spec:ConformanceTest,
        skos:Concept ;
    spec:method "Inspect the encoding to verify the above requirement." ;
    spec:purpose "Verify that the encoding provides the SurveyResults Requirements Class Classes shown in blue in Figure 52 in a manner consistent with the encoding.  An encoding shall decide which SurveyResult types it will support and define appropriate requirements classes accordingly." ;
    spec:requirement <http://www.opengis.net/spec/landinfra/1.0/req/survey-results/classes> ;
    spec:testType spec:Capabilities ;
    skos:broader <http://www.opengis.net/spec/landinfra/1.0/conf/survey-results> ;
    skos:definition "Verify that the encoding provides the SurveyResults Requirements Class Classes shown in blue in Figure 52 in a manner consistent with the encoding.  An encoding shall decide which SurveyResult types it will support and define appropriate requirements classes accordingly." ;
    skos:inScheme <http://www.opengis.net/def/status>,
        <http://www.opengis.net/spec/landinfra/1.0> ;
    skos:prefLabel "http://www.opengis.net/spec/landinfra/1.0/conf/survey-results/classes" .

<http://www.opengis.net/spec/landinfra/1.0/conf/survey-results/topic-20> a spec:ConformanceTest,
        skos:Concept ;
    spec:method "Inspect the encoding to verify the above requirement." ;
    spec:purpose "Verify that, if the encoding supports survey results subjects, then the encoding shall support the SF_SamplingFeature and related Classes specified in the OGC Abstract Specification Topic 20, Observation and Measurements shown in Figure 54 that are appropriate to the supported subject area(s)." ;
    spec:requirement <http://www.opengis.net/spec/landinfra/1.0/req/survey-results/topic-20> ;
    spec:testType spec:Capabilities ;
    skos:broader <http://www.opengis.net/spec/landinfra/1.0/conf/survey-results> ;
    skos:definition "Verify that, if the encoding supports survey results subjects, then the encoding shall support the SF_SamplingFeature and related Classes specified in the OGC Abstract Specification Topic 20, Observation and Measurements shown in Figure 54 that are appropriate to the supported subject area(s)." ;
    skos:inScheme <http://www.opengis.net/def/status>,
        <http://www.opengis.net/spec/landinfra/1.0> ;
    skos:prefLabel "http://www.opengis.net/spec/landinfra/1.0/conf/survey-results/topic-20" .

<http://www.opengis.net/spec/landinfra/1.0/conf/survey/classes> a spec:ConformanceTest,
        skos:Concept ;
    spec:method "Inspect the encoding to verify the above requirement." ;
    spec:purpose "Verify that the encoding provides the Survey Requirements Class Classes shown in blue in Figure 41 in a manner consistent with the encoding." ;
    spec:requirement <http://www.opengis.net/spec/landinfra/1.0/req/survey/classes> ;
    spec:testType spec:Capabilities ;
    skos:broader <http://www.opengis.net/spec/landinfra/1.0/conf/survey> ;
    skos:definition "Verify that the encoding provides the Survey Requirements Class Classes shown in blue in Figure 41 in a manner consistent with the encoding." ;
    skos:inScheme <http://www.opengis.net/def/status>,
        <http://www.opengis.net/spec/landinfra/1.0> ;
    skos:prefLabel "http://www.opengis.net/spec/landinfra/1.0/conf/survey/classes" .

<https://www.ogc.org> a ns2:Organization ;
    ns2:name "Open Geospatial Consortium" ;
    ns2:url "https://www.ogc.org"^^xsd:anyURI .

<http://www.opengis.net/def/docs/15-111r1> a spec:Specification,
        skos:Concept ;
    dct:creator "Paul Scarponcini" ;
    dct:dateAccepted "2016-08-02"^^xsd:date ;
    dct:dateSubmitted "2016-05-16"^^xsd:date ;
    dct:identifier "http://www.opengis.net/doc/is/landinfra/1.0" ;
    reg:status reg:statusValid ;
    na:doctype ogcdt:ip ;
    na:status status:valid ;
    spec:authority "Open Geospatial Consortium" ;
    spec:class <http://www.opengis.net/spec/landinfra/1.0/conf/alignment>,
        <http://www.opengis.net/spec/landinfra/1.0/conf/condominium>,
        <http://www.opengis.net/spec/landinfra/1.0/conf/equipment>,
        <http://www.opengis.net/spec/landinfra/1.0/conf/facility>,
        <http://www.opengis.net/spec/landinfra/1.0/conf/land-division>,
        <http://www.opengis.net/spec/landinfra/1.0/conf/land-feature>,
        <http://www.opengis.net/spec/landinfra/1.0/conf/land-infra>,
        <http://www.opengis.net/spec/landinfra/1.0/conf/observations>,
        <http://www.opengis.net/spec/landinfra/1.0/conf/project>,
        <http://www.opengis.net/spec/landinfra/1.0/conf/railway>,
        <http://www.opengis.net/spec/landinfra/1.0/conf/road>,
        <http://www.opengis.net/spec/landinfra/1.0/conf/road-cross-section>,
        <http://www.opengis.net/spec/landinfra/1.0/conf/survey>,
        <http://www.opengis.net/spec/landinfra/1.0/conf/survey-results> ;
    spec:date "2016-12-20"^^xsd:date ;
    spec:status status:valid ;
    specrel:implementation <http://www.opengis.net/def/docs/16-000r1>,
        <http://www.opengis.net/def/docs/16-100r2>,
        <http://www.opengis.net/def/docs/16-101r2>,
        <http://www.opengis.net/def/docs/16-102r2>,
        <http://www.opengis.net/def/docs/16-103r2>,
        <http://www.opengis.net/def/docs/16-104r2>,
        <http://www.opengis.net/def/docs/16-105r2>,
        <http://www.opengis.net/def/docs/16-106r2>,
        <http://www.opengis.net/def/docs/16-107r2> ;
    skos:definition "OGC® Land and Infrastructure Conceptual Model Standard (LandInfra)" ;
    skos:inScheme <http://www.opengis.net/def/docs> ;
    skos:notation "15-111r1"^^na:doc_no ;
    skos:prefLabel "OGC® Land and Infrastructure Conceptual Model Standard (LandInfra)" ;
    adms:last <http://www.opengis.net/def/docs/15-111r1> ;
    adms:version "1.0" ;
    dcat:landingPage <http://docs.opengeospatial.org/is/15-111r1/15-111r1.html> ;
    prov:wasAttributedTo wg:landinfraswg .

status:invalid a na:Status,
        skos:Concept ;
    dct:source <https://def.isotc211.org/iso19135/-1/2015/catalog-v001.xml> ;
    na:status status:stable ;
    rdfs:isDefinedBy <http://www.opengis.net/def/status> ;
    owl:sameAs reg:statusInvalid ;
    skos:broader status:notAccepted ;
    skos:definition "An entry which has been invalidated due to serious flaws, distinct from retirement. Corresponds to ISO 19135(redraft) 'invalid'."@en ;
    skos:inScheme <http://www.opengis.net/def/status> ;
    skos:prefLabel "invalid"@en .

status:retired a na:Status,
        skos:Concept ;
    dct:source <https://def.isotc211.org/iso19135/-1/2015/catalog-v001.xml> ;
    na:status status:stable ;
    rdfs:isDefinedBy <http://www.opengis.net/def/status> ;
    owl:sameAs reg:statusRetired ;
    skos:altlabel "withdrawn"@en ;
    skos:broader status:deprecated ;
    skos:definition "An entry that has been withdrawn from use.  Corresponds to ISO 19135:2005 'retired'."@en ;
    skos:inScheme <http://www.opengis.net/def/status> ;
    skos:prefLabel "retired"@en .

status:submitted a na:Status,
        skos:Concept ;
    dct:source <https://def.isotc211.org/iso19135/-1/2015/catalog-v001.xml> ;
    na:status status:stable ;
    rdfs:isDefinedBy <http://www.opengis.net/def/status> ;
    owl:sameAs reg:statusSubmitted ;
    skos:broader status:notAccepted ;
    skos:definition "A proposed entry which is not yet approved for use for use. Corresponds to ISO 19135:(redraft) 'submitted'."@en ;
    skos:inScheme <http://www.opengis.net/def/status> ;
    skos:prefLabel "submitted"@en .

status:superseded a na:Status,
        skos:Concept ;
    dct:source <https://def.isotc211.org/iso19135/-1/2015/catalog-v001.xml> ;
    na:status status:stable ;
    rdfs:isDefinedBy <http://www.opengis.net/def/status> ;
    owl:sameAs reg:statusSuperceded ;
    skos:altlabel "replaced"@en ;
    skos:broader status:deprecated ;
    skos:definition "An entry that has been replaced by a new alternative which should be used instead.  Corresponds to ISO 19135:2005 'superseded'."@en ;
    skos:inScheme <http://www.opengis.net/def/status> ;
    skos:prefLabel "superseded"@en .

<http://www.opengis.net/spec/landinfra/1.0/conf/facility/subtypes> a spec:ConformanceTest,
        skos:Concept ;
    spec:dependency <http://www.opengis.net/spec/landinfra/1.0/conf/land-infra> ;
    spec:method "Inspect the encoding to verify the above requirement." ;
    spec:purpose "Verify that the encoding specifies which of the FacilityPart subtypes shown in Figure 10 it supports." ;
    spec:requirement <http://www.opengis.net/spec/landinfra/1.0/req/facility/subtypes> ;
    spec:testType spec:Capabilities ;
    skos:broader <http://www.opengis.net/spec/landinfra/1.0/conf/facility/subtypes> ;
    skos:definition "Verify that the encoding specifies which of the FacilityPart subtypes shown in Figure 10 it supports." ;
    skos:inScheme <http://www.opengis.net/def/status>,
        <http://www.opengis.net/spec/landinfra/1.0> ;
    skos:narrower <http://www.opengis.net/spec/landinfra/1.0/conf/facility/subtypes> ;
    skos:prefLabel "ConformanceTest: http://www.opengis.net/spec/landinfra/1.0/conf/facility/subtypes" .

<http://www.opengis.net/spec/landinfra/1.0/conf/land-feature/alignment> a spec:ConformanceTest,
        skos:Concept ;
    spec:method "Inspect the encoding to verify the above requirement." ;
    spec:purpose "If an encoding allows the linear element used for a LandLayer to be an Alignment, then verify that the encoding supports the Alignment Requirements class." ;
    spec:requirement <http://www.opengis.net/spec/landinfra/1.0/req/land-feature/alignment> ;
    spec:testType spec:Capabilities ;
    skos:broader <http://www.opengis.net/spec/landinfra/1.0/conf/land-feature/alignment> ;
    skos:definition "If an encoding allows the linear element used for a LandLayer to be an Alignment, then verify that the encoding supports the Alignment Requirements class." ;
    skos:inScheme <http://www.opengis.net/def/status>,
        <http://www.opengis.net/spec/landinfra/1.0> ;
    skos:narrower <http://www.opengis.net/spec/landinfra/1.0/conf/land-feature/alignment> ;
    skos:prefLabel "Conformance Test: http://www.opengis.net/spec/landinfra/1.0/conf/land-feature/alignment" .

<http://www.opengis.net/spec/landinfra/1.0/req/alignment/CRS> a spec:Requirement,
        skos:Concept ;
    dct:description "All geometry/locations for Alignment2DHorSegments and Alignment2DVertSegments shall be specified using the Alignment2DHorizontal.crs which shall be a Cartesian local engineering reference system." ;
    skos:broader <http://www.opengis.net/spec/landinfra/1.0/req/alignment> ;
    skos:definition "All geometry/locations for Alignment2DHorSegments and Alignment2DVertSegments shall be specified using the Alignment2DHorizontal.crs which shall be a Cartesian local engineering reference system." ;
    skos:inScheme <http://www.opengis.net/def/status>,
        <http://www.opengis.net/spec/landinfra/1.0> ;
    skos:prefLabel "Requirement: /req/alignment/CRS" .

<http://www.opengis.net/spec/landinfra/1.0/req/alignment/LR-interfaces> a spec:Requirement,
        skos:Concept ;
    dct:description "An encoding shall implement the OGC Abstract Specification Topic 19 ILinearElement and ISpatial interfaces in a manner consistent with the encoding." ;
    skos:broader <http://www.opengis.net/spec/landinfra/1.0/req/alignment> ;
    skos:definition "An encoding shall implement the OGC Abstract Specification Topic 19 ILinearElement and ISpatial interfaces in a manner consistent with the encoding." ;
    skos:inScheme <http://www.opengis.net/def/status>,
        <http://www.opengis.net/spec/landinfra/1.0> ;
    skos:prefLabel "Requirement: /req/alignment/LR-interfaces" .

<http://www.opengis.net/spec/landinfra/1.0/req/alignment/classes> a spec:Requirement,
        skos:Concept ;
    dct:description """The Alignment Requirements class Classes shown in blue in Figure 15 shall be
provided for by any encoding which includes Alignments and then in such a
manner as is consistent with the encoding.""" ;
    skos:broader <http://www.opengis.net/spec/landinfra/1.0/req/alignment> ;
    skos:definition "An encoding shall implement the OGC Abstract Specification Topic 19 ILinearElement and ISpatial interfaces in a manner consistent with the encoding." ;
    skos:inScheme <http://www.opengis.net/def/status>,
        <http://www.opengis.net/spec/landinfra/1.0> ;
    skos:prefLabel "Requirement: /req/alignment/classes" .

<http://www.opengis.net/spec/landinfra/1.0/req/alignment/description> a spec:Requirement,
        skos:Concept ;
    dct:description "An encoding which includes Alignments shall specify that all of the included Alignments shall be continuous, non-overlapping, and non-branching (though it may contain intersections with other Alignments) and that if it is used within the context of a Project, the included Alignment shall be for a single alternative, as specified by the ProjectPart." ;
    skos:broader <http://www.opengis.net/spec/landinfra/1.0/req/alignment> ;
    skos:definition "An encoding which includes Alignments shall specify that all of the included Alignments shall be continuous, non-overlapping, and non-branching (though it may contain intersections with other Alignments) and that if it is used within the context of a Project, the included Alignment shall be for a single alternative, as specified by the ProjectPart." ;
    skos:inScheme <http://www.opengis.net/def/status>,
        <http://www.opengis.net/spec/landinfra/1.0> ;
    skos:prefLabel "Requirement: /req/alignment/description" .

<http://www.opengis.net/spec/landinfra/1.0/req/alignment/measures> a spec:Requirement,
        skos:Concept ;
    dct:description "If an Alignment2DHorizontal.2DLinestringRepresentation or an Alignment3D.3DLinestringRepresentation is specified as a linear element, then distanceAlong shall be measured along the LineString and offsetLateralDistance and offsetVerticalDistance values shall be measured normal to the LineString from this DistanceAlong point. If an Alignment2DHorizontal.segment list of Alignment2DHorSegments is used as a linear element, then distanceAlong and offsetLateralDistance values shall be measured in the horizontal plane, ignoring any vertical displacement of the Alignment. OffsetVerticalDistance values shall be absolute from the horizontal plane unless an Alignment2DVertical is specified as a VerticalOffsetReferent so as to take into consideration vertical displacement of the Alignment, if present." ;
    skos:broader <http://www.opengis.net/spec/landinfra/1.0/req/alignment> ;
    skos:definition "If an Alignment2DHorizontal.2DLinestringRepresentation or an Alignment3D.3DLinestringRepresentation is specified as a linear element, then distanceAlong shall be measured along the LineString and offsetLateralDistance and offsetVerticalDistance values shall be measured normal to the LineString from this DistanceAlong point. If an Alignment2DHorizontal.segment list of Alignment2DHorSegments is used as a linear element, then distanceAlong and offsetLateralDistance values shall be measured in the horizontal plane, ignoring any vertical displacement of the Alignment. OffsetVerticalDistance values shall be absolute from the horizontal plane unless an Alignment2DVertical is specified as a VerticalOffsetReferent so as to take into consideration vertical displacement of the Alignment, if present." ;
    skos:inScheme <http://www.opengis.net/def/status>,
        <http://www.opengis.net/spec/landinfra/1.0> ;
    skos:prefLabel "Requirement: /req/alignment/measures" .

<http://www.opengis.net/spec/landinfra/1.0/req/condominium> a spec:RequirementClass,
        skos:Concept ;
    spec:normativeStatement <http://www.opengis.net/spec/landinfra/1.0/req/condominium/classes> ;
    skos:broader <http://www.opengis.net/spec/landinfra/1.0/conf/condominium> ;
    skos:definition "Requirement Class: Condominium" ;
    skos:inScheme <http://www.opengis.net/def/status>,
        <http://www.opengis.net/spec/landinfra/1.0> ;
    skos:narrower <http://www.opengis.net/spec/landinfra/1.0/req/condominium/classes> ;
    skos:prefLabel "Requirement Class: Condominium" .

<http://www.opengis.net/spec/landinfra/1.0/req/condominium/classes> a spec:Requirement,
        skos:Concept ;
    dct:description "The Condominium Requirements Class Classes shown in blue in Figure 68 shall be provided for by the encoding in a manner consistent with the encoding." ;
    skos:broader <http://www.opengis.net/spec/landinfra/1.0/req/condominium> ;
    skos:definition "The Condominium Requirements Class Classes shown in blue in Figure 68 shall be provided for by the encoding in a manner consistent with the encoding." ;
    skos:inScheme <http://www.opengis.net/def/status>,
        <http://www.opengis.net/spec/landinfra/1.0> ;
    skos:prefLabel "Requirement: /req/condominium/classes" .

<http://www.opengis.net/spec/landinfra/1.0/req/equipment/classes> a spec:Requirement,
        skos:Concept ;
    dct:description "The Equipment Requirements Class Classes shown in blue in Figure 48 shall be provided for by the encoding in a manner consistent with the encoding. An encoding shall decide which SurveySensor types it will support and define appropriate requirements classes accordingly." ;
    skos:broader <http://www.opengis.net/spec/landinfra/1.0/req/equipment> ;
    skos:definition "The Equipment Requirements Class Classes shown in blue in Figure 48 shall be provided for by the encoding in a manner consistent with the encoding. An encoding shall decide which SurveySensor types it will support and define appropriate requirements classes accordingly." ;
    skos:inScheme <http://www.opengis.net/def/status>,
        <http://www.opengis.net/spec/landinfra/1.0> ;
    skos:prefLabel "Requirement: /req/equipment/classes" .

<http://www.opengis.net/spec/landinfra/1.0/req/equipment/observation-correction> a spec:Requirement,
        skos:Concept ;
    dct:description "The ObservationCorrection Classes in blue in Figure 51 shall be provided for by the encoding in a manner consistent with the encoding. The encoding shall decide which correction types it will support and define appropriate requirements classes accordingly." ;
    skos:broader <http://www.opengis.net/spec/landinfra/1.0/req/equipment> ;
    skos:definition "The ObservationCorrection Classes in blue in Figure 51 shall be provided for by the encoding in a manner consistent with the encoding. The encoding shall decide which correction types it will support and define appropriate requirements classes accordingly." ;
    skos:inScheme <http://www.opengis.net/def/status>,
        <http://www.opengis.net/spec/landinfra/1.0> ;
    skos:prefLabel "Requirement: /req/equipment/observation-correction" .

<http://www.opengis.net/spec/landinfra/1.0/req/facility/classes> a spec:Requirement,
        skos:Concept ;
    dct:description "The Facility Requirements Class Classes shown in blue in Figure 10 shall be provided for by the encoding in a manner consistent with the encoding." ;
    skos:broader <http://www.opengis.net/spec/landinfra/1.0/req/facility> ;
    skos:definition "The Facility Requirements Class Classes shown in blue in Figure 10 shall be provided for by the encoding in a manner consistent with the encoding." ;
    skos:inScheme <http://www.opengis.net/def/status>,
        <http://www.opengis.net/spec/landinfra/1.0> ;
    skos:prefLabel "Requirement: /req/facility/classes" .

<http://www.opengis.net/spec/landinfra/1.0/req/facility/subtypes> a spec:Requirement,
        skos:Concept ;
    dct:description "A Land and Infrastructure encoding shall specify which of the FacilityPart subtypes shown in Figure 10 it supports." ;
    skos:broader <http://www.opengis.net/spec/landinfra/1.0/req/facility> ;
    skos:definition "A Land and Infrastructure encoding shall specify which of the FacilityPart subtypes shown in Figure 10 it supports." ;
    skos:inScheme <http://www.opengis.net/def/status>,
        <http://www.opengis.net/spec/landinfra/1.0> ;
    skos:prefLabel "Requirement: /req/facility/subtypes" .

<http://www.opengis.net/spec/landinfra/1.0/req/land-division> a spec:RequirementClass,
        skos:Concept ;
    spec:normativeStatement <http://www.opengis.net/spec/landinfra/1.0/req/land-division/classes> ;
    skos:broader <http://www.opengis.net/spec/landinfra/1.0/conf/land-division> ;
    skos:definition "Requirement Class: LandVision" ;
    skos:inScheme <http://www.opengis.net/def/status>,
        <http://www.opengis.net/spec/landinfra/1.0> ;
    skos:narrower <http://www.opengis.net/spec/landinfra/1.0/req/land-division/classes> ;
    skos:prefLabel "Requirement Class: LandVision" .

<http://www.opengis.net/spec/landinfra/1.0/req/land-division/classes> a spec:Requirement,
        skos:Concept ;
    dct:description "The LandDivision Requirements Class Classes shown in blue in Figure 60 shall be provided for by the encoding in a manner consistent with the encoding." ;
    skos:broader <http://www.opengis.net/spec/landinfra/1.0/req/land-division> ;
    skos:definition "The LandDivision Requirements Class Classes shown in blue in Figure 60 shall be provided for by the encoding in a manner consistent with the encoding." ;
    skos:inScheme <http://www.opengis.net/def/status>,
        <http://www.opengis.net/spec/landinfra/1.0> ;
    skos:prefLabel "Requirement: /req/land-division/classes" .

<http://www.opengis.net/spec/landinfra/1.0/req/land-feature/alignment> a spec:Requirement,
        skos:Concept ;
    dct:description "If an encoding allows the linear element used for a LandLayer to be an Alignment, then that encoding shall support the Alignment Requirements Class." ;
    skos:broader <http://www.opengis.net/spec/landinfra/1.0/req/land-feature> ;
    skos:definition "If an encoding allows the linear element used for a LandLayer to be an Alignment, then that encoding shall support the Alignment Requirements Class." ;
    skos:inScheme <http://www.opengis.net/def/status>,
        <http://www.opengis.net/spec/landinfra/1.0> ;
    skos:prefLabel "Requirement: /req/land-feature/alignment" .

<http://www.opengis.net/spec/landinfra/1.0/req/land-feature/classes> a spec:Requirement,
        skos:Concept ;
    dct:description "The LandFeature Requirements Class Classes shown in blue in Figure 55 shall be provided for by the encoding in a manner consistent with the encoding." ;
    skos:broader <http://www.opengis.net/spec/landinfra/1.0/req/land-feature> ;
    skos:definition "The LandFeature Requirements Class Classes shown in blue in Figure 55 shall be provided for by the encoding in a manner consistent with the encoding." ;
    skos:inScheme <http://www.opengis.net/def/status>,
        <http://www.opengis.net/spec/landinfra/1.0> ;
    skos:prefLabel "Requirement: /req/land-feature/classes" .

<http://www.opengis.net/spec/landinfra/1.0/req/land-infra/19103> a spec:Requirement,
        skos:Concept ;
    dct:description "A Land and Infrastructure encoding shall support the core data types specified in ISO 19103 Clause 7 and shown in pink in Figure 5 that are appropriate to the supported subject area(s)." ;
    skos:broader <http://www.opengis.net/spec/landinfra/1.0/req/land-infra> ;
    skos:definition "A Land and Infrastructure encoding shall support the core data types specified in ISO 19103 Clause 7 and shown in pink in Figure 5 that are appropriate to the supported subject area(s)." ;
    skos:inScheme <http://www.opengis.net/def/status>,
        <http://www.opengis.net/spec/landinfra/1.0> ;
    skos:prefLabel "Requirement: /req/land-infra/19103" .

<http://www.opengis.net/spec/landinfra/1.0/req/land-infra/19109> a spec:Requirement,
        skos:Concept ;
    dct:description "Features shall be supported by a Land and Infrastructure encoding in accordance with the uml:feature requirement in ISO 19109:2015 Clause 8.2.6 and shown in Figure 9, as follows: Each instance of FeatureType shall be implemented by the encoding’s equivalent of a UML Class having a generalization association with AnyFeature and with a stereotype of <>." ;
    skos:broader <http://www.opengis.net/spec/landinfra/1.0/req/land-infra> ;
    skos:definition "Features shall be supported by a Land and Infrastructure encoding in accordance with the uml:feature requirement in ISO 19109:2015 Clause 8.2.6 and shown in Figure 9, as follows: Each instance of FeatureType shall be implemented by the encoding’s equivalent of a UML Class having a generalization association with AnyFeature and with a stereotype of <>." ;
    skos:inScheme <http://www.opengis.net/def/status>,
        <http://www.opengis.net/spec/landinfra/1.0> ;
    skos:prefLabel "Requirement: /req/land-infra/19109" .

<http://www.opengis.net/spec/landinfra/1.0/req/land-infra/classes> a spec:Requirement,
        skos:Concept ;
    dct:description "The LandInfra Requirements Class Classes shown in blue in Figure 2 shall be provided by the encoding in a manner consistent with the encoding." ;
    skos:broader <http://www.opengis.net/spec/landinfra/1.0/req/land-infra> ;
    skos:definition "The LandInfra Requirements Class Classes shown in blue in Figure 2 shall be provided by the encoding in a manner consistent with the encoding." ;
    skos:inScheme <http://www.opengis.net/def/status>,
        <http://www.opengis.net/spec/landinfra/1.0> ;
    skos:prefLabel "Requirement: /req/land-infra/classes" .

<http://www.opengis.net/spec/landinfra/1.0/req/land-infra/crs> a spec:Requirement,
        skos:Concept ;
    dct:description "An encoding shall support coordinate reference systems in accordance with OGC Abstract Specification Topic 2, Spatial Referencing by Coordinates." ;
    skos:broader <http://www.opengis.net/spec/landinfra/1.0/req/land-infra> ;
    skos:definition "An encoding shall support coordinate reference systems in accordance with OGC Abstract Specification Topic 2, Spatial Referencing by Coordinates." ;
    skos:inScheme <http://www.opengis.net/def/status>,
        <http://www.opengis.net/spec/landinfra/1.0> ;
    skos:prefLabel "Requirement: /req/land-infra/crs" .

<http://www.opengis.net/spec/landinfra/1.0/req/land-infra/dataset> a spec:Requirement,
        skos:Concept ;
    dct:description "A Land and Infrastructure encoding shall specify a LandInfra dataset in whatever format that is appropriate to that encoding (e.g., an XML document for a GML encoding)." ;
    skos:broader <http://www.opengis.net/spec/landinfra/1.0/req/land-infra> ;
    skos:definition "A Land and Infrastructure encoding shall specify a LandInfra dataset in whatever format that is appropriate to that encoding (e.g., an XML document for a GML encoding)." ;
    skos:inScheme <http://www.opengis.net/def/status>,
        <http://www.opengis.net/spec/landinfra/1.0> ;
    skos:prefLabel "Requirement: /req/land-infra/dataset" .

<http://www.opengis.net/spec/landinfra/1.0/req/land-infra/featureID> a spec:Requirement,
        skos:Concept ;
    dct:description "An encoding shall specify if it supports ID at the feature level, ID at the Feature sub-type level, or both." ;
    skos:broader <http://www.opengis.net/spec/landinfra/1.0/req/land-infra> ;
    skos:definition "An encoding shall specify if it supports ID at the feature level, ID at the Feature sub-type level, or both." ;
    skos:inScheme <http://www.opengis.net/def/status>,
        <http://www.opengis.net/spec/landinfra/1.0> ;
    skos:prefLabel "Requirement: /req/land-infra/featureID" .

<http://www.opengis.net/spec/landinfra/1.0/req/land-infra/subjects> a spec:Requirement,
        skos:Concept ;
    dct:description "A Land and Infrastructure encoding shall specify which of the LandInfra subjects it supports: Facility, LandFeature, LandDivision, and Survey." ;
    skos:broader <http://www.opengis.net/spec/landinfra/1.0/req/land-infra> ;
    skos:definition "A Land and Infrastructure encoding shall specify which of the LandInfra subjects it supports: Facility, LandFeature, LandDivision, and Survey." ;
    skos:inScheme <http://www.opengis.net/def/status>,
        <http://www.opengis.net/spec/landinfra/1.0> ;
    skos:prefLabel "Requirement: /req/land-infra/subjects" .

<http://www.opengis.net/spec/landinfra/1.0/req/land-infra/topic-1> a spec:Requirement,
        skos:Concept ;
    dct:description "A Land and Infrastructure encoding shall support the geometry types specified in the OGC Abstract Specification Topic 1, Feature Geometry as shown in pink and the SimpleTriangle, TIN, and PolyfaceMesh extensions shown in beige in Figure 6, that are appropriate to the supported subject area(s). Additional geometry types, not found in Topic 1, but required by a specific requirements class, are specified in that requirements class. If a Land and Infrastructure encoding supports linearly referenced locations, then the encoding shall support the PositionExpression and related Classes specified in the OGC Abstract Specification Topic 19, core Linear Referencing (LR) Package shown in pink in Figure 7 that are appropriate to the supported subject area(s). If a Land and Infrastructure encoding supports linearly referenced locations, then the encoding shall specify which of the OGC Abstract Specification Topic 19, Linear Referencing extension packages it supports and shall therefore support the appropriate Classes shown in Figure 7 and Figure 8 for those packages that are appropriate to the supported subject area(s)." ;
    skos:broader <http://www.opengis.net/spec/landinfra/1.0/req/land-infra> ;
    skos:definition "A Land and Infrastructure encoding shall support the geometry types specified in the OGC Abstract Specification Topic 1, Feature Geometry as shown in pink and the SimpleTriangle, TIN, and PolyfaceMesh extensions shown in beige in Figure 6, that are appropriate to the supported subject area(s). Additional geometry types, not found in Topic 1, but required by a specific requirements class, are specified in that requirements class. If a Land and Infrastructure encoding supports linearly referenced locations, then the encoding shall support the PositionExpression and related Classes specified in the OGC Abstract Specification Topic 19, core Linear Referencing (LR) Package shown in pink in Figure 7 that are appropriate to the supported subject area(s). If a Land and Infrastructure encoding supports linearly referenced locations, then the encoding shall specify which of the OGC Abstract Specification Topic 19, Linear Referencing extension packages it supports and shall therefore support the appropriate Classes shown in Figure 7 and Figure 8 for those packages that are appropriate to the supported subject area(s)." ;
    skos:inScheme <http://www.opengis.net/def/status>,
        <http://www.opengis.net/spec/landinfra/1.0> ;
    skos:prefLabel "Requirement: /req/land-infra/topic-1" .

<http://www.opengis.net/spec/landinfra/1.0/req/land-infra/topic-19-core> a spec:Requirement,
        skos:Concept ;
    dct:description "If a Land and Infrastructure encoding supports linearly referenced locations, then the encoding shall support the PositionExpression and related Classes specified in the OGC Abstract Specification Topic 19, core Linear Referencing (LR) Package shown in pink in Figure 7 that are appropriate to the supported subject area(s)." ;
    skos:broader <http://www.opengis.net/spec/landinfra/1.0/req/land-infra> ;
    skos:definition "If a Land and Infrastructure encoding supports linearly referenced locations, then the encoding shall support the PositionExpression and related Classes specified in the OGC Abstract Specification Topic 19, core Linear Referencing (LR) Package shown in pink in Figure 7 that are appropriate to the supported subject area(s)." ;
    skos:inScheme <http://www.opengis.net/def/status>,
        <http://www.opengis.net/spec/landinfra/1.0> ;
    skos:prefLabel "Requirement: /req/land-infra/topic-19-core" .

<http://www.opengis.net/spec/landinfra/1.0/req/land-infra/topic-19-extensions> a spec:Requirement,
        skos:Concept ;
    dct:description "If a Land and Infrastructure encoding supports linearly referenced locations, then the encoding shall specify which of the OGC Abstract Specification Topic 19, Linear Referencing extension packages it supports and shall therefore support the appropriate Classes shown in Figure 7 and Figure 8 for those packages that are appropriate to the supported subject area(s)." ;
    skos:broader <http://www.opengis.net/spec/landinfra/1.0/req/land-infra> ;
    skos:definition "If a Land and Infrastructure encoding supports linearly referenced locations, then the encoding shall specify which of the OGC Abstract Specification Topic 19, Linear Referencing extension packages it supports and shall therefore support the appropriate Classes shown in Figure 7 and Figure 8 for those packages that are appropriate to the supported subject area(s)." ;
    skos:inScheme <http://www.opengis.net/def/status>,
        <http://www.opengis.net/spec/landinfra/1.0> ;
    skos:prefLabel "Requirement: /req/land-infra/topic-19-extensions" .

<http://www.opengis.net/spec/landinfra/1.0/req/observations> a spec:RequirementClass,
        skos:Concept ;
    spec:normativeStatement <http://www.opengis.net/spec/landinfra/1.0/req/observations/classes> ;
    skos:broader <http://www.opengis.net/spec/landinfra/1.0/conf/observations> ;
    skos:definition "Requirement Class: Observations" ;
    skos:inScheme <http://www.opengis.net/def/status>,
        <http://www.opengis.net/spec/landinfra/1.0> ;
    skos:narrower <http://www.opengis.net/spec/landinfra/1.0/req/observations/classes> ;
    skos:prefLabel "Requirement Class: Observations" .

<http://www.opengis.net/spec/landinfra/1.0/req/observations/classes> a spec:Requirement,
        skos:Concept ;
    dct:description """The Observations Requirements Class Classes shown in blue in Figure 41Figure
43 shall be provided for by the encoding in a manner consistent with the
encoding. An encoding shall decide which SurveyObservation types it will
support and define appropriate requirements classes accordingly. This then
would include any dependent types (example SatelliteSystemType has only to be
supported if the encoding will support GNSS Observations).""" ;
    skos:broader <http://www.opengis.net/spec/landinfra/1.0/req/observations> ;
    skos:definition """The Observations Requirements Class Classes shown in blue in Figure 41Figure
43 shall be provided for by the encoding in a manner consistent with the
encoding. An encoding shall decide which SurveyObservation types it will
support and define appropriate requirements classes accordingly. This then
would include any dependent types (example SatelliteSystemType has only to be
supported if the encoding will support GNSS Observations).""" ;
    skos:inScheme <http://www.opengis.net/def/status>,
        <http://www.opengis.net/spec/landinfra/1.0> ;
    skos:prefLabel "Requirement: /req/observations/classes" .

<http://www.opengis.net/spec/landinfra/1.0/req/project> a spec:RequirementClass,
        skos:Concept ;
    spec:normativeStatement <http://www.opengis.net/spec/landinfra/1.0/req/project/classes> ;
    skos:broader <http://www.opengis.net/spec/landinfra/1.0/conf/project> ;
    skos:definition "Requirement Class: Project" ;
    skos:inScheme <http://www.opengis.net/def/status>,
        <http://www.opengis.net/spec/landinfra/1.0> ;
    skos:narrower <http://www.opengis.net/spec/landinfra/1.0/req/project/classes> ;
    skos:prefLabel "Requirement Class: Project" .

<http://www.opengis.net/spec/landinfra/1.0/req/project/classes> a spec:Requirement,
        skos:Concept ;
    dct:description "The Project Requirements Class Classes shown in blue in Figure 13 shall be provided for by the encoding in a manner consistent with the encoding." ;
    skos:broader <http://www.opengis.net/spec/landinfra/1.0/req/project> ;
    skos:definition "The Project Requirements Class Classes shown in blue in Figure 13 shall be provided for by the encoding in a manner consistent with the encoding." ;
    skos:inScheme <http://www.opengis.net/def/status>,
        <http://www.opengis.net/spec/landinfra/1.0> ;
    skos:prefLabel "Requirement: /req/project/classes" .

<http://www.opengis.net/spec/landinfra/1.0/req/railway/alignment> a spec:Requirement,
        skos:Concept ;
    dct:description """If an encoding allows the linear element used for locating RailwayElements or
CantEvents to be an Alignment, then that encoding shall support the Alignment
Requirements Class.""" ;
    skos:broader <http://www.opengis.net/spec/landinfra/1.0/req/railway> ;
    skos:definition """If an encoding allows the linear element used for locating RailwayElements or
CantEvents to be an Alignment, then that encoding shall support the Alignment
Requirements Class.""" ;
    skos:inScheme <http://www.opengis.net/def/status>,
        <http://www.opengis.net/spec/landinfra/1.0> ;
    skos:prefLabel "Requirement: /req/railway/alignment" .

<http://www.opengis.net/spec/landinfra/1.0/req/railway/cant> a spec:Requirement,
        skos:Concept ;
    dct:description """An encoding shall specify as a requirement that each CantSpecification shall
cover the entire linear element the CantSpecification is located along from
the linear element’s start to its end, and that the CantSpecification shall
include CantEvents at the start and end of the linear element and wherever
else there is a cant break along the linear element.""" ;
    skos:broader <http://www.opengis.net/spec/landinfra/1.0/req/railway> ;
    skos:definition """An encoding shall specify as a requirement that each CantSpecification shall
cover the entire linear element the CantSpecification is located along from
the linear element’s start to its end, and that the CantSpecification shall
include CantEvents at the start and end of the linear element and wherever
else there is a cant break along the linear element.""" ;
    skos:inScheme <http://www.opengis.net/def/status>,
        <http://www.opengis.net/spec/landinfra/1.0> ;
    skos:prefLabel "Requirement: /req/railway/cant" .

<http://www.opengis.net/spec/landinfra/1.0/req/railway/classes> a spec:Requirement,
        skos:Concept ;
    dct:description """The Railway Requirements Class Classes shown in blue in Figure 36 shall be
provided for by the encoding in a manner consistent with the encoding.""" ;
    skos:broader <http://www.opengis.net/spec/landinfra/1.0/req/railway> ;
    skos:definition """The Railway Requirements Class Classes shown in blue in Figure 36 shall be
provided for by the encoding in a manner consistent with the encoding.""" ;
    skos:inScheme <http://www.opengis.net/def/status>,
        <http://www.opengis.net/spec/landinfra/1.0> ;
    skos:prefLabel "Requirement: /req/railway/classes" .

<http://www.opengis.net/spec/landinfra/1.0/req/road/alignment> a spec:Requirement,
        skos:Concept ;
    dct:description """If an encoding allows the linear element used for locating RoadElements to be
an Alignment, then that encoding shall support the Alignment Requirements
Class.""" ;
    skos:broader <http://www.opengis.net/spec/landinfra/1.0/req/road> ;
    skos:definition """If an encoding allows the linear element used for locating RoadElements to be
an Alignment, then that encoding shall support the Alignment Requirements
Class.""" ;
    skos:inScheme <http://www.opengis.net/def/status>,
        <http://www.opengis.net/spec/landinfra/1.0> ;
    skos:prefLabel "Requirement: /req/road/alignment" .

<http://www.opengis.net/spec/landinfra/1.0/req/road/classes> a spec:Requirement,
        skos:Concept ;
    dct:description """The Road Requirements Class Classes shown in blue in Figure 21 shall be
provided for by the encoding in a manner consistent with the encoding.""" ;
    skos:broader <http://www.opengis.net/spec/landinfra/1.0/req/road> ;
    skos:definition """The Road Requirements Class Classes shown in blue in Figure 21 shall be
provided for by the encoding in a manner consistent with the encoding.""" ;
    skos:inScheme <http://www.opengis.net/def/status>,
        <http://www.opengis.net/spec/landinfra/1.0> ;
    skos:prefLabel "Requirement: /req/road/classes" .

<http://www.opengis.net/spec/landinfra/1.0/req/survey/classes> a spec:Requirement,
        skos:Concept ;
    dct:description """The Survey Requirements Class Classes shown in blue in Figure 41 shall be
provided for by the encoding in a manner consistent with the encoding.""" ;
    skos:broader <http://www.opengis.net/spec/landinfra/1.0/req/survey> ;
    skos:definition """The Survey Requirements Class Classes shown in blue in Figure 41 shall be
provided for by the encoding in a manner consistent with the encoding.""" ;
    skos:inScheme <http://www.opengis.net/def/status>,
        <http://www.opengis.net/spec/landinfra/1.0> ;
    skos:prefLabel "Requirement: /req/survey/classes" .

status:accepted a na:Status,
        skos:Concept ;
    dct:source reg: ;
    na:status status:stable ;
    rdfs:isDefinedBy <http://www.opengis.net/def/status> ;
    owl:sameAs reg:statusAccepted ;
    skos:definition "An entry that has been accepted for use and is visible in the default register listing. Includes entries that have seen been retired or superseded."@en ;
    skos:inScheme <http://www.opengis.net/def/status> ;
    skos:narrower status:deprecated,
        status:valid ;
    skos:prefLabel "accepted"@en ;
    skos:topConceptOf <http://www.opengis.net/def/status> .

status:deprecated a na:Status,
        skos:Concept ;
    dct:source reg: ;
    na:status status:stable ;
    rdfs:isDefinedBy <http://www.opengis.net/def/status> ;
    owl:sameAs reg:statusDeprecated ;
    skos:broader status:accepted ;
    skos:definition "An entry that has been retired or replaced and is no longer to be used."@en ;
    skos:inScheme <http://www.opengis.net/def/status> ;
    skos:narrower status:retired,
        status:superseded ;
    skos:prefLabel "deprecated"@en .

<http://www.opengis.net/spec/landinfra/1.0/conf/condominium> a spec:ConformanceClass,
        skos:Concept ;
    spec:conformanceTest <http://www.opengis.net/spec/landinfra/1.0/conf/condominium/classes> ;
    skos:definition "Conformance Class: Condominium" ;
    skos:inScheme <http://www.opengis.net/def/status>,
        <http://www.opengis.net/spec/landinfra/1.0> ;
    skos:narrower <http://www.opengis.net/spec/landinfra/1.0/conf/condominium/classes>,
        <http://www.opengis.net/spec/landinfra/1.0/req/condominium> ;
    skos:prefLabel "Conformance Class: Condominium" ;
    skos:requirementsTested <http://www.opengis.net/spec/landinfra/1.0/req/condominium> ;
    skos:topConceptOf <http://www.opengis.net/spec/landinfra/1.0> .

<http://www.opengis.net/spec/landinfra/1.0/conf/land-division> a spec:ConformanceClass,
        skos:Concept ;
    spec:conformanceTest <http://www.opengis.net/spec/landinfra/1.0/conf/land-division/classes> ;
    skos:definition "Conformance Class: LandDivision" ;
    skos:inScheme <http://www.opengis.net/def/status>,
        <http://www.opengis.net/spec/landinfra/1.0> ;
    skos:narrower <http://www.opengis.net/spec/landinfra/1.0/conf/land-division/classes>,
        <http://www.opengis.net/spec/landinfra/1.0/req/land-division> ;
    skos:prefLabel "Conformance Class: LandDivision" ;
    skos:requirementsTested <http://www.opengis.net/spec/landinfra/1.0/req/land-division> ;
    skos:topConceptOf <http://www.opengis.net/spec/landinfra/1.0> .

<http://www.opengis.net/spec/landinfra/1.0/conf/land-feature> a spec:ConformanceClass,
        skos:Concept ;
    spec:conformanceTest <http://www.opengis.net/spec/landinfra/1.0/conf/land-feature/alignment>,
        <http://www.opengis.net/spec/landinfra/1.0/conf/land-feature/classes> ;
    skos:definition "Conformance Class: LandFeature" ;
    skos:inScheme <http://www.opengis.net/def/status>,
        <http://www.opengis.net/spec/landinfra/1.0> ;
    skos:narrower <http://www.opengis.net/spec/landinfra/1.0/conf/land-feature/classes>,
        <http://www.opengis.net/spec/landinfra/1.0/req/land-feature> ;
    skos:prefLabel "Conformance Class: LandFeature" ;
    skos:requirementsTested <http://www.opengis.net/spec/landinfra/1.0/req/land-feature> ;
    skos:topConceptOf <http://www.opengis.net/spec/landinfra/1.0> .

<http://www.opengis.net/spec/landinfra/1.0/conf/observations> a spec:ConformanceClass,
        skos:Concept ;
    spec:conformanceTest <http://www.opengis.net/spec/landinfra/1.0/conf/observations/classes> ;
    skos:definition "Conformance Class: Observations" ;
    skos:inScheme <http://www.opengis.net/def/status>,
        <http://www.opengis.net/spec/landinfra/1.0> ;
    skos:narrower <http://www.opengis.net/spec/landinfra/1.0/conf/observations/classes>,
        <http://www.opengis.net/spec/landinfra/1.0/req/observations> ;
    skos:prefLabel "Conformance Class: Observations" ;
    skos:requirementsTested <http://www.opengis.net/spec/landinfra/1.0/req/observations> ;
    skos:topConceptOf <http://www.opengis.net/spec/landinfra/1.0> .

<http://www.opengis.net/spec/landinfra/1.0/conf/project> a spec:ConformanceClass,
        skos:Concept ;
    spec:conformanceTest <http://www.opengis.net/spec/landinfra/1.0/conf/project/classes> ;
    skos:definition "Conformance Class: Project" ;
    skos:inScheme <http://www.opengis.net/def/status>,
        <http://www.opengis.net/spec/landinfra/1.0> ;
    skos:narrower <http://www.opengis.net/spec/landinfra/1.0/conf/project/classes>,
        <http://www.opengis.net/spec/landinfra/1.0/req/project> ;
    skos:prefLabel "Conformance Class: Project" ;
    skos:requirementsTested <http://www.opengis.net/spec/landinfra/1.0/req/project> ;
    skos:topConceptOf <http://www.opengis.net/spec/landinfra/1.0> .

<http://www.opengis.net/spec/landinfra/1.0/conf/survey> a spec:ConformanceClass,
        skos:Concept ;
    spec:conformanceTest <http://www.opengis.net/spec/landinfra/1.0/conf/survey/classes> ;
    skos:definition "Conformance Class: Survey" ;
    skos:inScheme <http://www.opengis.net/def/status>,
        <http://www.opengis.net/spec/landinfra/1.0> ;
    skos:narrower <http://www.opengis.net/spec/landinfra/1.0/conf/survey/classes>,
        <http://www.opengis.net/spec/landinfra/1.0/req/survey> ;
    skos:prefLabel "Conformance Class: Survey" ;
    skos:requirementsTested <http://www.opengis.net/spec/landinfra/1.0/req/survey> ;
    skos:topConceptOf <http://www.opengis.net/spec/landinfra/1.0> .

<http://www.opengis.net/spec/landinfra/1.0/req/equipment> a spec:RequirementClass,
        skos:Concept ;
    spec:normativeStatement <http://www.opengis.net/spec/landinfra/1.0/req/equipment/classes>,
        <http://www.opengis.net/spec/landinfra/1.0/req/equipment/observation-correction> ;
    skos:broader <http://www.opengis.net/spec/landinfra/1.0/conf/equipment> ;
    skos:definition "Requirement Class: Equipment" ;
    skos:inScheme <http://www.opengis.net/def/status>,
        <http://www.opengis.net/spec/landinfra/1.0> ;
    skos:narrower <http://www.opengis.net/spec/landinfra/1.0/req/equipment/classes>,
        <http://www.opengis.net/spec/landinfra/1.0/req/equipment/observation-correction> ;
    skos:prefLabel "Requirement Class: Equipment" .

<http://www.opengis.net/spec/landinfra/1.0/req/facility> a spec:RequirementClass,
        skos:Concept ;
    spec:normativeStatement <http://www.opengis.net/spec/landinfra/1.0/req/facility/classes>,
        <http://www.opengis.net/spec/landinfra/1.0/req/facility/subtypes> ;
    skos:broader <http://www.opengis.net/spec/landinfra/1.0/conf/facility> ;
    skos:definition "Requirement Class: Facility" ;
    skos:inScheme <http://www.opengis.net/def/status>,
        <http://www.opengis.net/spec/landinfra/1.0> ;
    skos:narrower <http://www.opengis.net/spec/landinfra/1.0/req/facility/classes>,
        <http://www.opengis.net/spec/landinfra/1.0/req/facility/subtypes> ;
    skos:prefLabel "Requirement Class: Facility" .

<http://www.opengis.net/spec/landinfra/1.0/req/land-feature> a spec:RequirementClass,
        skos:Concept ;
    spec:normativeStatement <http://www.opengis.net/spec/landinfra/1.0/req/land-feature/alignment>,
        <http://www.opengis.net/spec/landinfra/1.0/req/land-feature/classes> ;
    skos:broader <http://www.opengis.net/spec/landinfra/1.0/conf/land-feature> ;
    skos:definition "Requirement Class: LandFeature" ;
    skos:inScheme <http://www.opengis.net/def/status>,
        <http://www.opengis.net/spec/landinfra/1.0> ;
    skos:narrower <http://www.opengis.net/spec/landinfra/1.0/req/land-feature/alignment>,
        <http://www.opengis.net/spec/landinfra/1.0/req/land-feature/classes> ;
    skos:prefLabel "Requirement Class: LandFeature" .

<http://www.opengis.net/spec/landinfra/1.0/req/road-cross-section> a spec:RequirementClass,
        skos:Concept ;
    spec:normativeStatement <http://www.opengis.net/spec/landinfra/1.0/req/road-cross-section/alignment>,
        <http://www.opengis.net/spec/landinfra/1.0/req/road-cross-section/classes> ;
    skos:broader <http://www.opengis.net/spec/landinfra/1.0/conf/road-cross-section> ;
    skos:definition "Requirement Class: RoadCrossSection" ;
    skos:inScheme <http://www.opengis.net/def/status>,
        <http://www.opengis.net/spec/landinfra/1.0> ;
    skos:narrower <http://www.opengis.net/spec/landinfra/1.0/req/road-cross-section/alignment>,
        <http://www.opengis.net/spec/landinfra/1.0/req/road-cross-section/classes> ;
    skos:prefLabel "Requirement Class: RoadCrossSection" .

<http://www.opengis.net/spec/landinfra/1.0/req/survey-results> a spec:RequirementClass,
        skos:Concept ;
    spec:normativeStatement <http://www.opengis.net/spec/landinfra/1.0/req/survey-results/classes>,
        <http://www.opengis.net/spec/landinfra/1.0/req/survey-results/topic-20> ;
    skos:broader <http://www.opengis.net/spec/landinfra/1.0/conf/survey-results> ;
    skos:definition "Requirement Class: SurveyResult" ;
    skos:inScheme <http://www.opengis.net/def/status>,
        <http://www.opengis.net/spec/landinfra/1.0> ;
    skos:narrower <http://www.opengis.net/spec/landinfra/1.0/req/survey-results/classes>,
        <http://www.opengis.net/spec/landinfra/1.0/req/survey-results/topic-20> ;
    skos:prefLabel "Requirement Class: SurveyResult" .

<http://www.opengis.net/spec/landinfra/1.0/conf/equipment> a spec:ConformanceClass,
        skos:Concept ;
    spec:conformanceTest <http://www.opengis.net/spec/landinfra/1.0/conf/equipment/classes>,
        <http://www.opengis.net/spec/landinfra/1.0/conf/equipment/observation-correction> ;
    skos:definition "Conformance Class: Equipment" ;
    skos:inScheme <http://www.opengis.net/def/status>,
        <http://www.opengis.net/spec/landinfra/1.0> ;
    skos:narrower <http://www.opengis.net/spec/landinfra/1.0/conf/equipment/classes>,
        <http://www.opengis.net/spec/landinfra/1.0/conf/equipment/observation-correction>,
        <http://www.opengis.net/spec/landinfra/1.0/req/equipment> ;
    skos:prefLabel "Conformance Class: Equipment" ;
    skos:requirementsTested <http://www.opengis.net/spec/landinfra/1.0/req/equipment> ;
    skos:topConceptOf <http://www.opengis.net/spec/landinfra/1.0> .

<http://www.opengis.net/spec/landinfra/1.0/conf/facility> a spec:ConformanceClass,
        skos:Concept ;
    spec:conformanceTest <http://www.opengis.net/spec/landinfra/1.0/conf/facility/classes>,
        <http://www.opengis.net/spec/landinfra/1.0/conf/facility/subtypes> ;
    skos:definition "Conformance Class: Facility" ;
    skos:inScheme <http://www.opengis.net/def/status>,
        <http://www.opengis.net/spec/landinfra/1.0> ;
    skos:narrower <http://www.opengis.net/spec/landinfra/1.0/conf/facility/classes>,
        <http://www.opengis.net/spec/landinfra/1.0/req/facility> ;
    skos:prefLabel "Conformance Class: Facility" ;
    skos:requirementsTested <http://www.opengis.net/spec/landinfra/1.0/req/facility> ;
    skos:topConceptOf <http://www.opengis.net/spec/landinfra/1.0> .

<http://www.opengis.net/spec/landinfra/1.0/conf/road> a spec:ConformanceClass,
        skos:Concept ;
    spec:conformanceTest <http://www.opengis.net/spec/landinfra/1.0/conf/road/alignment>,
        <http://www.opengis.net/spec/landinfra/1.0/conf/road/classes> ;
    skos:definition "Conformance Class: Road" ;
    skos:inScheme <http://www.opengis.net/def/status>,
        <http://www.opengis.net/spec/landinfra/1.0> ;
    skos:narrower <http://www.opengis.net/spec/landinfra/1.0/conf/road/alignment>,
        <http://www.opengis.net/spec/landinfra/1.0/conf/road/classes>,
        <http://www.opengis.net/spec/landinfra/1.0/req/road> ;
    skos:prefLabel "Conformance Class: Road" ;
    skos:requirementsTested <http://www.opengis.net/spec/landinfra/1.0/req/road> ;
    skos:topConceptOf <http://www.opengis.net/spec/landinfra/1.0> .

<http://www.opengis.net/spec/landinfra/1.0/conf/road-cross-section> a spec:ConformanceClass,
        skos:Concept ;
    spec:conformanceTest <http://www.opengis.net/spec/landinfra/1.0/conf/road-cross-section/alignment>,
        <http://www.opengis.net/spec/landinfra/1.0/conf/road-cross-section/classes> ;
    skos:definition "Conformance Class: RoadCrossSection" ;
    skos:inScheme <http://www.opengis.net/def/status>,
        <http://www.opengis.net/spec/landinfra/1.0> ;
    skos:narrower <http://www.opengis.net/spec/landinfra/1.0/conf/road-cross-section/alignment>,
        <http://www.opengis.net/spec/landinfra/1.0/conf/road-cross-section/classes>,
        <http://www.opengis.net/spec/landinfra/1.0/req/road-cross-section> ;
    skos:prefLabel "Conformance Class: RoadCrossSection" ;
    skos:requirementsTested <http://www.opengis.net/spec/landinfra/1.0/req/road-cross-section> ;
    skos:topConceptOf <http://www.opengis.net/spec/landinfra/1.0> .

<http://www.opengis.net/spec/landinfra/1.0/conf/survey-results> a spec:ConformanceClass,
        skos:Concept ;
    spec:conformanceTest <http://www.opengis.net/spec/landinfra/1.0/conf/survey-results/classes>,
        <http://www.opengis.net/spec/landinfra/1.0/conf/survey-results/topic-20> ;
    skos:definition "Conformance Class: SurveyResults" ;
    skos:inScheme <http://www.opengis.net/def/status>,
        <http://www.opengis.net/spec/landinfra/1.0> ;
    skos:narrower <http://www.opengis.net/spec/landinfra/1.0/conf/survey-results/classes>,
        <http://www.opengis.net/spec/landinfra/1.0/conf/survey-results/topic-20>,
        <http://www.opengis.net/spec/landinfra/1.0/req/survey-results> ;
    skos:prefLabel "Conformance Class: SurveyResults" ;
    skos:requirementsTested <http://www.opengis.net/spec/landinfra/1.0/req/survey-results> ;
    skos:topConceptOf <http://www.opengis.net/spec/landinfra/1.0> .

<http://www.opengis.net/spec/landinfra/1.0/req/railway> a spec:RequirementClass,
        skos:Concept ;
    spec:normativeStatement <http://www.opengis.net/spec/landinfra/1.0/req/railway/alignment>,
        <http://www.opengis.net/spec/landinfra/1.0/req/railway/cant>,
        <http://www.opengis.net/spec/landinfra/1.0/req/railway/classes> ;
    skos:broader <http://www.opengis.net/spec/landinfra/1.0/conf/railway> ;
    skos:definition "Requirement Class: Railway" ;
    skos:inScheme <http://www.opengis.net/def/status>,
        <http://www.opengis.net/spec/landinfra/1.0> ;
    skos:narrower <http://www.opengis.net/spec/landinfra/1.0/req/railway/alignment>,
        <http://www.opengis.net/spec/landinfra/1.0/req/railway/cant>,
        <http://www.opengis.net/spec/landinfra/1.0/req/railway/classes> ;
    skos:prefLabel "Requirement Class: Railway" .

<http://www.opengis.net/spec/landinfra/1.0/req/road-cross-section/alignment> a spec:Requirement,
        skos:Concept ;
    dct:description """If an encoding allows the linear element used for locating CrossSections to be
an Alignment, then that encoding shall support the Alignment Requirements
Class.""" ;
    skos:broader <http://www.opengis.net/spec/landinfra/1.0/req/road>,
        <http://www.opengis.net/spec/landinfra/1.0/req/road-cross-section> ;
    skos:definition """If an encoding allows the linear element used for locating CrossSections to be
an Alignment, then that encoding shall support the Alignment Requirements
Class.""" ;
    skos:inScheme <http://www.opengis.net/def/status>,
        <http://www.opengis.net/spec/landinfra/1.0> ;
    skos:prefLabel "Requirement: /req/road-cross-section/alignment" .

<http://www.opengis.net/spec/landinfra/1.0/req/road-cross-section/classes> a spec:Requirement,
        skos:Concept ;
    dct:description """The RoadCrossSection Requirements Class Classes shown in blue in Figure 25
shall be provided for by the encoding in a manner consistent with the
encoding.""" ;
    skos:broader <http://www.opengis.net/spec/landinfra/1.0/req/road>,
        <http://www.opengis.net/spec/landinfra/1.0/req/road-cross-section> ;
    skos:definition """The RoadCrossSection Requirements Class Classes shown in blue in Figure 25
shall be provided for by the encoding in a manner consistent with the
encoding.""" ;
    skos:inScheme <http://www.opengis.net/def/status>,
        <http://www.opengis.net/spec/landinfra/1.0> ;
    skos:prefLabel "Requirement: /req/road-cross-section/classes" .

<http://www.opengis.net/spec/landinfra/1.0/req/survey> a spec:RequirementClass,
        skos:Concept ;
    spec:normativeStatement <http://www.opengis.net/spec/landinfra/1.0/req/survey-results/classes>,
        <http://www.opengis.net/spec/landinfra/1.0/req/survey-results/topic-20>,
        <http://www.opengis.net/spec/landinfra/1.0/req/survey/classes> ;
    skos:broader <http://www.opengis.net/spec/landinfra/1.0/conf/survey> ;
    skos:definition "Requirement Class: Survey" ;
    skos:inScheme <http://www.opengis.net/def/status>,
        <http://www.opengis.net/spec/landinfra/1.0> ;
    skos:narrower <http://www.opengis.net/spec/landinfra/1.0/req/survey-results/classes>,
        <http://www.opengis.net/spec/landinfra/1.0/req/survey-results/topic-20>,
        <http://www.opengis.net/spec/landinfra/1.0/req/survey/classes> ;
    skos:prefLabel "Requirement Class: Survey" .

<http://www.opengis.net/spec/landinfra/1.0/req/survey-results/classes> a spec:Requirement,
        skos:Concept ;
    dct:description """The SurveyResults Requirements Class Classes shown in blue in Figure 52 shall
be provided for by the encoding in a manner consistent with the encoding. An
encoding shall decide which SurveyResult types it will support and define
appropriate requirements classes accordingly.""" ;
    skos:broader <http://www.opengis.net/spec/landinfra/1.0/req/survey>,
        <http://www.opengis.net/spec/landinfra/1.0/req/survey-results> ;
    skos:definition """The SurveyResults Requirements Class Classes shown in blue in Figure 52 shall
be provided for by the encoding in a manner consistent with the encoding. An
encoding shall decide which SurveyResult types it will support and define
appropriate requirements classes accordingly.""" ;
    skos:inScheme <http://www.opengis.net/def/status>,
        <http://www.opengis.net/spec/landinfra/1.0> ;
    skos:prefLabel "Requirement: /req/survey-results/classes" .

<http://www.opengis.net/spec/landinfra/1.0/req/survey-results/topic-20> a spec:Requirement,
        skos:Concept ;
    dct:description "If a Land and Infrastructure encoding supports survey results subjects, then the encoding shall support the SF_SamplingFeature and related Classes specified in the OGC Abstract Specification Topic 20, Observation and Measurements shown in Figure 54 that are appropriate to the supported subject area(s)." ;
    skos:broader <http://www.opengis.net/spec/landinfra/1.0/req/survey>,
        <http://www.opengis.net/spec/landinfra/1.0/req/survey-results> ;
    skos:definition "If a Land and Infrastructure encoding supports survey results subjects, then the encoding shall support the SF_SamplingFeature and related Classes specified in the OGC Abstract Specification Topic 20, Observation and Measurements shown in Figure 54 that are appropriate to the supported subject area(s)." ;
    skos:inScheme <http://www.opengis.net/def/status>,
        <http://www.opengis.net/spec/landinfra/1.0> ;
    skos:prefLabel "Requirement: /req/survey-results/topic-20" .

status:notAccepted a na:Status,
        skos:Concept ;
    dct:source reg: ;
    na:status status:stable ;
    rdfs:isDefinedBy <http://www.opengis.net/def/status> ;
    owl:sameAs reg:statusNotAccepted ;
    skos:definition "An entry that should not be visible in the default register listing. Corresponds to ISO 19135:2005 'notValid'."@en ;
    skos:inScheme <http://www.opengis.net/def/status> ;
    skos:narrower status:invalid,
        status:reserved,
        status:submitted,
        status:under-development ;
    skos:prefLabel "not accepted"@en ;
    skos:topConceptOf <http://www.opengis.net/def/status> .

<http://www.opengis.net/spec/landinfra/1.0/conf/railway> a spec:ConformanceClass,
        skos:Concept ;
    spec:conformanceTest <http://www.opengis.net/spec/landinfra/1.0/conf/railway/alignment>,
        <http://www.opengis.net/spec/landinfra/1.0/conf/railway/cant>,
        <http://www.opengis.net/spec/landinfra/1.0/conf/railway/classes> ;
    skos:definition "Conformance Class: Railway" ;
    skos:inScheme <http://www.opengis.net/def/status>,
        <http://www.opengis.net/spec/landinfra/1.0> ;
    skos:narrower <http://www.opengis.net/spec/landinfra/1.0/conf/railway/alignment>,
        <http://www.opengis.net/spec/landinfra/1.0/conf/railway/cant>,
        <http://www.opengis.net/spec/landinfra/1.0/conf/railway/classes>,
        <http://www.opengis.net/spec/landinfra/1.0/req/railway> ;
    skos:prefLabel "Conformance Class: Railway" ;
    skos:requirementsTested <http://www.opengis.net/spec/landinfra/1.0/req/railway> ;
    skos:topConceptOf <http://www.opengis.net/spec/landinfra/1.0> .

<http://www.opengis.net/spec/landinfra/1.0/req/road> a spec:RequirementClass,
        skos:Concept ;
    spec:normativeStatement <http://www.opengis.net/spec/landinfra/1.0/req/road-cross-section/alignment>,
        <http://www.opengis.net/spec/landinfra/1.0/req/road-cross-section/classes>,
        <http://www.opengis.net/spec/landinfra/1.0/req/road/alignment>,
        <http://www.opengis.net/spec/landinfra/1.0/req/road/classes> ;
    skos:broader <http://www.opengis.net/spec/landinfra/1.0/conf/road> ;
    skos:definition "Requirement Class: Road" ;
    skos:inScheme <http://www.opengis.net/def/status>,
        <http://www.opengis.net/spec/landinfra/1.0> ;
    skos:narrower <http://www.opengis.net/spec/landinfra/1.0/req/road-cross-section/alignment>,
        <http://www.opengis.net/spec/landinfra/1.0/req/road-cross-section/classes>,
        <http://www.opengis.net/spec/landinfra/1.0/req/road/alignment>,
        <http://www.opengis.net/spec/landinfra/1.0/req/road/classes> ;
    skos:prefLabel "Requirement Class: Road" .

status:experimental a na:Status,
        skos:Concept ;
    dct:source reg: ;
    na:status status:stable ;
    rdfs:isDefinedBy <http://www.opengis.net/def/status> ;
    owl:sameAs reg:statusExperimental ;
    skos:altlabel "provisional"@en ;
    skos:broader status:valid ;
    skos:definition "An entry that has been accepted into the register temporarily and may be subject to change or withdrawal."@en ;
    skos:inScheme <http://www.opengis.net/def/status> ;
    skos:prefLabel "experimental"@en .

status:valid a na:Status,
        skos:Concept ;
    dct:source <https://def.isotc211.org/iso19135/-1/2015/catalog-v001.xml> ;
    na:status status:stable ;
    rdfs:isDefinedBy <http://www.opengis.net/def/status> ;
    owl:sameAs reg:statusValid ;
    skos:broader status:accepted ;
    skos:definition "An entry that has been accepted into the register and is deemed fit for use. Corresponds to ISO 19135:2005 'valid'."@en ;
    skos:inScheme <http://www.opengis.net/def/status> ;
    skos:narrower status:experimental,
        status:stable ;
    skos:prefLabel "valid"@en .

<http://www.opengis.net/spec/landinfra/1.0/req/alignment> a spec:RequirementClass,
        skos:Concept ;
    spec:normativeStatement <http://www.opengis.net/spec/landinfra/1.0/req/alignment/CRS>,
        <http://www.opengis.net/spec/landinfra/1.0/req/alignment/LR-interfaces>,
        <http://www.opengis.net/spec/landinfra/1.0/req/alignment/classes>,
        <http://www.opengis.net/spec/landinfra/1.0/req/alignment/description>,
        <http://www.opengis.net/spec/landinfra/1.0/req/alignment/measures> ;
    skos:broader <http://www.opengis.net/spec/landinfra/1.0/conf/alignment> ;
    skos:definition "Requirement Class: Alignment" ;
    skos:inScheme <http://www.opengis.net/def/status>,
        <http://www.opengis.net/spec/landinfra/1.0> ;
    skos:narrower <http://www.opengis.net/spec/landinfra/1.0/req/alignment/CRS>,
        <http://www.opengis.net/spec/landinfra/1.0/req/alignment/LR-interfaces>,
        <http://www.opengis.net/spec/landinfra/1.0/req/alignment/classes>,
        <http://www.opengis.net/spec/landinfra/1.0/req/alignment/description>,
        <http://www.opengis.net/spec/landinfra/1.0/req/alignment/measures> ;
    skos:prefLabel "Requirement Class: Alignment" .

<http://www.opengis.net/spec/landinfra/1.0/conf/alignment> a spec:ConformanceClass,
        skos:Concept ;
    spec:conformanceTest <http://www.opengis.net/spec/landinfra/1.0/conf/alignment/CRS>,
        <http://www.opengis.net/spec/landinfra/1.0/conf/alignment/LR-interfaces>,
        <http://www.opengis.net/spec/landinfra/1.0/conf/alignment/classes>,
        <http://www.opengis.net/spec/landinfra/1.0/conf/alignment/description>,
        <http://www.opengis.net/spec/landinfra/1.0/conf/alignment/measures> ;
    skos:definition "Conformance Class: Alignment" ;
    skos:inScheme <http://www.opengis.net/def/status>,
        <http://www.opengis.net/spec/landinfra/1.0> ;
    skos:narrower <http://www.opengis.net/spec/landinfra/1.0/conf/alignment/CRS>,
        <http://www.opengis.net/spec/landinfra/1.0/conf/alignment/LR-interfaces>,
        <http://www.opengis.net/spec/landinfra/1.0/conf/alignment/classes>,
        <http://www.opengis.net/spec/landinfra/1.0/conf/alignment/description>,
        <http://www.opengis.net/spec/landinfra/1.0/conf/alignment/measures>,
        <http://www.opengis.net/spec/landinfra/1.0/req/alignment> ;
    skos:prefLabel "Conformance Class: Alignment" ;
    skos:requirementsTested <http://www.opengis.net/spec/landinfra/1.0/req/alignment> ;
    skos:topConceptOf <http://www.opengis.net/spec/landinfra/1.0> .

<http://www.opengis.net/spec/landinfra/1.0/req/land-infra> a spec:RequirementClass,
        skos:Concept ;
    spec:normativeStatement <http://www.opengis.net/spec/landinfra/1.0/req/land-infra/19103>,
        <http://www.opengis.net/spec/landinfra/1.0/req/land-infra/19109>,
        <http://www.opengis.net/spec/landinfra/1.0/req/land-infra/classes>,
        <http://www.opengis.net/spec/landinfra/1.0/req/land-infra/crs>,
        <http://www.opengis.net/spec/landinfra/1.0/req/land-infra/dataset>,
        <http://www.opengis.net/spec/landinfra/1.0/req/land-infra/featureID>,
        <http://www.opengis.net/spec/landinfra/1.0/req/land-infra/subjects>,
        <http://www.opengis.net/spec/landinfra/1.0/req/land-infra/topic-1>,
        <http://www.opengis.net/spec/landinfra/1.0/req/land-infra/topic-19-core>,
        <http://www.opengis.net/spec/landinfra/1.0/req/land-infra/topic-19-extensions> ;
    skos:broader <http://www.opengis.net/spec/landinfra/1.0/conf/land-infra> ;
    skos:definition "Requirement Class: LandInfra" ;
    skos:inScheme <http://www.opengis.net/def/status>,
        <http://www.opengis.net/spec/landinfra/1.0> ;
    skos:narrower <http://www.opengis.net/spec/landinfra/1.0/req/land-infra/19103>,
        <http://www.opengis.net/spec/landinfra/1.0/req/land-infra/19109>,
        <http://www.opengis.net/spec/landinfra/1.0/req/land-infra/classes>,
        <http://www.opengis.net/spec/landinfra/1.0/req/land-infra/crs>,
        <http://www.opengis.net/spec/landinfra/1.0/req/land-infra/dataset>,
        <http://www.opengis.net/spec/landinfra/1.0/req/land-infra/featureID>,
        <http://www.opengis.net/spec/landinfra/1.0/req/land-infra/subjects>,
        <http://www.opengis.net/spec/landinfra/1.0/req/land-infra/topic-1>,
        <http://www.opengis.net/spec/landinfra/1.0/req/land-infra/topic-19-core>,
        <http://www.opengis.net/spec/landinfra/1.0/req/land-infra/topic-19-extensions> ;
    skos:prefLabel "Requirement Class: LandInfra" .

status:stable a na:Status,
        skos:Concept ;
    dct:source reg: ;
    na:status status:stable ;
    rdfs:isDefinedBy <http://www.opengis.net/def/status> ;
    owl:sameAs reg:statusStable ;
    skos:broader status:valid ;
    skos:definition "An entry that is seen as having a reasonable measure of stability, may be used to mark the full adoption of a previously 'experimental' entry."@en ;
    skos:inScheme <http://www.opengis.net/def/status> ;
    skos:prefLabel "stable"@en .

<http://www.opengis.net/spec/landinfra/1.0/conf/land-infra> a spec:ConformanceClass,
        skos:Concept ;
    spec:conformanceTest <http://www.opengis.net/spec/landinfra/1.0/conf/land-infra/19103>,
        <http://www.opengis.net/spec/landinfra/1.0/conf/land-infra/19109>,
        <http://www.opengis.net/spec/landinfra/1.0/conf/land-infra/classes>,
        <http://www.opengis.net/spec/landinfra/1.0/conf/land-infra/crs>,
        <http://www.opengis.net/spec/landinfra/1.0/conf/land-infra/dataset>,
        <http://www.opengis.net/spec/landinfra/1.0/conf/land-infra/featureID>,
        <http://www.opengis.net/spec/landinfra/1.0/conf/land-infra/subjects>,
        <http://www.opengis.net/spec/landinfra/1.0/conf/land-infra/topic-1>,
        <http://www.opengis.net/spec/landinfra/1.0/conf/land-infra/topic-19-core>,
        <http://www.opengis.net/spec/landinfra/1.0/conf/land-infra/topic-19-extensions> ;
    skos:definition "Core Conformance Class: LandInfra" ;
    skos:inScheme <http://www.opengis.net/def/status>,
        <http://www.opengis.net/spec/landinfra/1.0> ;
    skos:narrower <http://www.opengis.net/spec/landinfra/1.0/conf/land-infra/19103>,
        <http://www.opengis.net/spec/landinfra/1.0/conf/land-infra/19109>,
        <http://www.opengis.net/spec/landinfra/1.0/conf/land-infra/classes>,
        <http://www.opengis.net/spec/landinfra/1.0/conf/land-infra/crs>,
        <http://www.opengis.net/spec/landinfra/1.0/conf/land-infra/dataset>,
        <http://www.opengis.net/spec/landinfra/1.0/conf/land-infra/featureID>,
        <http://www.opengis.net/spec/landinfra/1.0/conf/land-infra/subjects>,
        <http://www.opengis.net/spec/landinfra/1.0/conf/land-infra/topic-1>,
        <http://www.opengis.net/spec/landinfra/1.0/conf/land-infra/topic-19-core>,
        <http://www.opengis.net/spec/landinfra/1.0/conf/land-infra/topic-19-extensions>,
        <http://www.opengis.net/spec/landinfra/1.0/req/land-infra> ;
    skos:prefLabel "Core Conformance Class: LandInfra" ;
    skos:requirementsTested <http://www.opengis.net/spec/landinfra/1.0/req/land-infra> ;
    skos:topConceptOf <http://www.opengis.net/spec/landinfra/1.0> .

spec:Capabilities a spec:TestType ;
    skos:prefLabel "Capabilities" .

<http://www.opengis.net/spec/landinfra/1.0> a skos:ConceptScheme ;
    dct:created "2016-12-20"^^xsd:date ;
    dct:modified "2016-12-20"^^xsd:date ;
    dct:source <http://www.opengis.net/def/docs/15-111r1> ;
    na:status status:experimental ;
    spec:status status:experimental ;
    skos:definition "A convenience hierarchy for navigating the elements of a specification using the SKOS model" ;
    skos:hasTopConcept <http://www.opengis.net/spec/landinfra/1.0/conf/alignment>,
        <http://www.opengis.net/spec/landinfra/1.0/conf/condominium>,
        <http://www.opengis.net/spec/landinfra/1.0/conf/equipment>,
        <http://www.opengis.net/spec/landinfra/1.0/conf/facility>,
        <http://www.opengis.net/spec/landinfra/1.0/conf/land-division>,
        <http://www.opengis.net/spec/landinfra/1.0/conf/land-feature>,
        <http://www.opengis.net/spec/landinfra/1.0/conf/land-infra>,
        <http://www.opengis.net/spec/landinfra/1.0/conf/observations>,
        <http://www.opengis.net/spec/landinfra/1.0/conf/project>,
        <http://www.opengis.net/spec/landinfra/1.0/conf/railway>,
        <http://www.opengis.net/spec/landinfra/1.0/conf/road>,
        <http://www.opengis.net/spec/landinfra/1.0/conf/road-cross-section>,
        <http://www.opengis.net/spec/landinfra/1.0/conf/survey>,
        <http://www.opengis.net/spec/landinfra/1.0/conf/survey-results> ;
    skos:prefLabel "Specification elements for OGC 15-111r LandInfra" .

<http://www.opengis.net/def/status> a skos:ConceptScheme ;
    dct:contributor <https://orcid.org/0000-0002-8742-7730> ;
    dct:created "2020-07-05"^^xsd:date ;
    dct:creator <https://www.ogc.org> ;
    dct:modified "2020-07-05"^^xsd:date ;
    dct:provenance """This vocabulary was originally pulbished by the OGC containing ISO 19135 terms. 19135 + additional terms were published by the British Government in 2012 as part of their work on Linked Data registry service. It was then adopted by the Australian Government Linked Data Working Group for Linked Data items in 2018. The extension of this vocabulary to include these additional terms, and term hierarchy, occured in July, 2020.
  
  The source of each Concept is indicated per-Concept as well as with a Collection for all ISO 19135 terms."""@en ;
    dct:publisher <https://www.ogc.org> ;
    dct:source reg:,
        <https://def.isotc211.org/iso19135/-1/2015/catalog-v001.xml> ;
    na:collectionView status: ;
    na:status status:experimental ;
    spec:status status:experimental ;
    rdfs:seeAlso <http://www.opengis.net/ogc-na-policy#Status> ;
    skos:definition """Statuses of items within a controlled register.
  
This vocabulary is a SKOS Concept Hierarchy of the RE_ItemStatus enumeration of ISO 19135: Geographic Information -- Procedures for item registration's Register with additional Concepts from the Core Ontology for Linked Data Registry Services."""@en ;
    skos:hasTopConcept status:accepted,
        status:notAccepted ;
    skos:prefLabel "Register Item status values"@en .

