<http://www.opengis.net/def/media-type/ogc/1.0/3dtiles>
        a       <http://www.w3.org/2004/02/skos/core#Concept> ;
        <http://www.w3.org/2000/01/rdf-schema#label>
                "Media type for 3D Tiles" ;
        <http://purl.org/dc/terms/created>
                "2020-06-01"^^<http://www.w3.org/2001/XMLSchema#date> ;
        <http://purl.org/dc/terms/modified>
                "2020-06-08"^^<http://www.w3.org/2001/XMLSchema#date> ;
        <http://www.w3.org/2004/02/skos/core#definition>
                "Composite tiles use the .cmpt extension and application/octet-stream MIME type.\n\nAn explicit file extension is optional. Valid implementations may ignore it and identify a content‚Äôs format by the magic field in its header."@en ;
        <http://www.w3.org/2004/02/skos/core#notation>
                "application/octet-stream"^^<https://www.iana.org/assignments/media-types> ;
        <http://www.w3.org/2004/02/skos/core#prefLabel>
                "Media type for 3D Tiles"@en ;
        <http://www.w3.org/2004/02/skos/core#related>
                <http://www.opengis.net/def/encoding/ogc/3dtiles> .

<http://www.opengis.net/def/media-type/ogc/1.0/gml>
        a       <http://www.w3.org/2004/02/skos/core#Concept> ;
        <http://www.w3.org/2000/01/rdf-schema#label>
                "Media type for Geography Markup Language (GML)" ;
        <http://www.w3.org/2000/01/rdf-schema#seeAlso>
                <https://www.iana.org/assignments/media-types/application/gml+xml> ;
        <http://purl.org/dc/terms/created>
                "2020-06-01"^^<http://www.w3.org/2001/XMLSchema#date> ;
        <http://purl.org/dc/terms/modified>
                "2020-06-08"^^<http://www.w3.org/2001/XMLSchema#date> ;
        <http://www.w3.org/2004/02/skos/core#definition>
                "Media type for Geography Markup Language (GML)"@en ;
        <http://www.w3.org/2004/02/skos/core#notation>
                "application/gml+xml"^^<https://www.iana.org/assignments/media-types> ;
        <http://www.w3.org/2004/02/skos/core#prefLabel>
                "Media type for Geography Markup Language (GML)"@en ;
        <http://www.w3.org/2004/02/skos/core#related>
                <http://www.opengis.net/def/encoding/ogc/gml> .

<http://www.opengis.net/def/media-type/ogc/1.0/cis-json>
        a       <http://www.w3.org/2004/02/skos/core#Concept> ;
        <http://www.w3.org/2000/01/rdf-schema#label>
                "Media type for CIS - JSON encoding" ;
        <http://www.w3.org/2000/01/rdf-schema#seeAlso>
                <https://www.iana.org/assignments/media-types/application/json> ;
        <http://purl.org/dc/terms/created>
                "2020-06-01"^^<http://www.w3.org/2001/XMLSchema#date> ;
        <http://purl.org/dc/terms/modified>
                "2020-06-08"^^<http://www.w3.org/2001/XMLSchema#date> ;
        <http://www.w3.org/2004/02/skos/core#definition>
                "Media type for the JavaScript Object Notation (JSON) encoding of the Coverage Implementation Schema (CIS)"@en ;
        <http://www.w3.org/2004/02/skos/core#notation>
                "application/json"^^<https://www.iana.org/assignments/media-types> ;
        <http://www.w3.org/2004/02/skos/core#prefLabel>
                "Media type for CIS - JSON encoding"@en .

<http://www.opengis.net/def/media-type/ogc/1.0/cdb>
        a       <http://www.w3.org/2004/02/skos/core#Concept> ;
        <http://www.w3.org/2000/01/rdf-schema#comment>
                "Not yet registered with IANA"@en ;
        <http://www.w3.org/2000/01/rdf-schema#label>
                "Media type for CDB" ;
        <http://purl.org/dc/terms/created>
                "2020-06-01"^^<http://www.w3.org/2001/XMLSchema#date> ;
        <http://purl.org/dc/terms/modified>
                "2020-06-08"^^<http://www.w3.org/2001/XMLSchema#date> ;
        <http://www.w3.org/2004/02/skos/core#definition>
                "Media type for CDB"@en ;
        <http://www.w3.org/2004/02/skos/core#prefLabel>
                "Media type for CDB"@en ;
        <http://www.w3.org/2004/02/skos/core#related>
                <http://www.opengis.net/def/encoding/ogc/cdb> .

<http://www.opengis.net/def/media-type/ogc/1.0/netcdf>
        a       <http://www.w3.org/2004/02/skos/core#Concept> ;
        <http://www.w3.org/2000/01/rdf-schema#comment>
                "Not yet registered with IANA"@en ;
        <http://www.w3.org/2000/01/rdf-schema#label>
                "Media type for NetCDF" ;
        <http://purl.org/dc/terms/created>
                "2020-06-01"^^<http://www.w3.org/2001/XMLSchema#date> ;
        <http://purl.org/dc/terms/modified>
                "2020-06-08"^^<http://www.w3.org/2001/XMLSchema#date> ;
        <http://www.w3.org/2004/02/skos/core#definition>
                "Media type for NetCDF"@en ;
        <http://www.w3.org/2004/02/skos/core#prefLabel>
                "Media type for NetCDF"@en ;
        <http://www.w3.org/2004/02/skos/core#related>
                <http://www.opengis.net/def/encoding/ogc/netcdf> .

<http://www.opengis.net/def/media-type/ogc/1.0/wktcrs>
        a       <http://www.w3.org/2004/02/skos/core#Concept> ;
        <http://www.w3.org/2000/01/rdf-schema#comment>
                "Not yet registered with IANA"@en ;
        <http://www.w3.org/2000/01/rdf-schema#label>
                "Media type for WKT CRS" ;
        <http://purl.org/dc/terms/created>
                "2020-06-01"^^<http://www.w3.org/2001/XMLSchema#date> ;
        <http://purl.org/dc/terms/modified>
                "2020-06-08"^^<http://www.w3.org/2001/XMLSchema#date> ;
        <http://www.w3.org/2004/02/skos/core#definition>
                "Media type for WKT CRS"@en ;
        <http://www.w3.org/2004/02/skos/core#prefLabel>
                "Media type for WKT CRS"@en ;
        <http://www.w3.org/2004/02/skos/core#related>
                <http://www.opengis.net/def/encoding/ogc/wktcrs> .

<http://www.opengis.net/def/media-type/ogc/1.0/landinfragml>
        a       <http://www.w3.org/2004/02/skos/core#Concept> ;
        <http://www.w3.org/2000/01/rdf-schema#comment>
                "Not yet registered with IANA"@en ;
        <http://www.w3.org/2000/01/rdf-schema#label>
                "Media type for LandInfra/InfraGML" ;
        <http://purl.org/dc/terms/created>
                "2020-06-01"^^<http://www.w3.org/2001/XMLSchema#date> ;
        <http://purl.org/dc/terms/modified>
                "2020-06-08"^^<http://www.w3.org/2001/XMLSchema#date> ;
        <http://www.w3.org/2004/02/skos/core#definition>
                "Media type for LandInfra/InfraGML"@en ;
        <http://www.w3.org/2004/02/skos/core#prefLabel>
                "Media type for LandInfra/InfraGML"@en ;
        <http://www.w3.org/2004/02/skos/core#related>
                <http://www.opengis.net/def/encoding/ogc/infragml> .

<http://www.opengis.net/def/media-type/ogc/1.0/guf>
        a       <http://www.w3.org/2004/02/skos/core#Concept> ;
        <http://www.w3.org/2000/01/rdf-schema#comment>
                "Not yet registered with IANA"@en ;
        <http://www.w3.org/2000/01/rdf-schema#label>
                "Media type for Geospatial User Feedback (GUF)" ;
        <http://purl.org/dc/terms/created>
                "2020-06-01"^^<http://www.w3.org/2001/XMLSchema#date> ;
        <http://purl.org/dc/terms/modified>
                "2020-06-08"^^<http://www.w3.org/2001/XMLSchema#date> ;
        <http://www.w3.org/2004/02/skos/core#definition>
                "Media type for Geospatial User Feedback (GUF)"@en ;
        <http://www.w3.org/2004/02/skos/core#prefLabel>
                "Media type for Geospatial User Feedback (GUF)"@en ;
        <http://www.w3.org/2004/02/skos/core#related>
                <http://www.opengis.net/def/encoding/ogc/guf> .

<http://www.opengis.net/def/media-type/ogc/1.0/georss>
        a       <http://www.w3.org/2004/02/skos/core#Concept> ;
        <http://www.w3.org/2000/01/rdf-schema#comment>
                "Not yet registered with IANA"@en ;
        <http://www.w3.org/2000/01/rdf-schema#label>
                "Media type for GeoRSS" ;
        <http://purl.org/dc/terms/created>
                "2020-06-01"^^<http://www.w3.org/2001/XMLSchema#date> ;
        <http://purl.org/dc/terms/modified>
                "2020-06-08"^^<http://www.w3.org/2001/XMLSchema#date> ;
        <http://www.w3.org/2004/02/skos/core#definition>
                "Media type for GeoRSS"@en ;
        <http://www.w3.org/2004/02/skos/core#prefLabel>
                "Media type for GeoRSS"@en ;
        <http://www.w3.org/2004/02/skos/core#related>
                <http://www.opengis.net/def/encoding/ogc/georss> .

<http://www.opengis.net/def/media-type/ogc/1.0/mf>
        a       <http://www.w3.org/2004/02/skos/core#Concept> ;
        <http://www.w3.org/2000/01/rdf-schema#comment>
                "Not yet registered with IANA"@en ;
        <http://www.w3.org/2000/01/rdf-schema#label>
                "Media type for Moving Features" ;
        <http://purl.org/dc/terms/created>
                "2020-06-01"^^<http://www.w3.org/2001/XMLSchema#date> ;
        <http://purl.org/dc/terms/modified>
                "2020-06-08"^^<http://www.w3.org/2001/XMLSchema#date> ;
        <http://www.w3.org/2004/02/skos/core#definition>
                "Media type for Moving Features"@en ;
        <http://www.w3.org/2004/02/skos/core#prefLabel>
                "Media type for Moving Features"@en ;
        <http://www.w3.org/2004/02/skos/core#related>
                <http://www.opengis.net/def/encoding/ogc/mf> .

<http://www.opengis.net/def/media-type/ogc/1.0/owc>
        a       <http://www.w3.org/2004/02/skos/core#Concept> ;
        <http://www.w3.org/2000/01/rdf-schema#comment>
                "Not yet registered with IANA"@en ;
        <http://www.w3.org/2000/01/rdf-schema#label>
                "Media type for OWS Context" ;
        <http://purl.org/dc/terms/created>
                "2020-06-01"^^<http://www.w3.org/2001/XMLSchema#date> ;
        <http://purl.org/dc/terms/modified>
                "2020-06-08"^^<http://www.w3.org/2001/XMLSchema#date> ;
        <http://www.w3.org/2004/02/skos/core#definition>
                "Media type for OWS Context"@en ;
        <http://www.w3.org/2004/02/skos/core#prefLabel>
                "Media type for OWS Context"@en ;
        <http://www.w3.org/2004/02/skos/core#related>
                <http://www.opengis.net/def/encoding/ogc/owc> .

<http://www.opengis.net/def/media-type/ogc/1.0/las>
        a       <http://www.w3.org/2004/02/skos/core#Concept> ;
        <http://www.w3.org/2000/01/rdf-schema#comment>
                "Not yet registered with IANA"@en ;
        <http://www.w3.org/2000/01/rdf-schema#label>
                "Media type for LAS" ;
        <http://purl.org/dc/terms/created>
                "2020-06-01"^^<http://www.w3.org/2001/XMLSchema#date> ;
        <http://purl.org/dc/terms/modified>
                "2020-06-08"^^<http://www.w3.org/2001/XMLSchema#date> ;
        <http://www.w3.org/2004/02/skos/core#definition>
                "Media type for LAS"@en ;
        <http://www.w3.org/2004/02/skos/core#prefLabel>
                "Media type for LAS"@en ;
        <http://www.w3.org/2004/02/skos/core#related>
                <http://www.opengis.net/def/encoding/ogc/las> .

<http://www.opengis.net/def/media-type/ogc/1.0/tsml>
        a       <http://www.w3.org/2004/02/skos/core#Concept> ;
        <http://www.w3.org/2000/01/rdf-schema#comment>
                "Not yet registered with IANA"@en ;
        <http://www.w3.org/2000/01/rdf-schema#label>
                "Media type for TimeseriesML (tsml)" ;
        <http://purl.org/dc/terms/created>
                "2020-06-01"^^<http://www.w3.org/2001/XMLSchema#date> ;
        <http://purl.org/dc/terms/modified>
                "2020-06-08"^^<http://www.w3.org/2001/XMLSchema#date> ;
        <http://www.w3.org/2004/02/skos/core#definition>
                "Media type for TimeseriesML (tsml)"@en ;
        <http://www.w3.org/2004/02/skos/core#prefLabel>
                "Media type for TimeseriesML (tsml)"@en ;
        <http://www.w3.org/2004/02/skos/core#related>
                <http://www.opengis.net/def/encoding/ogc/tsml> .

<http://www.opengis.net/def/media-type/ogc/1.0/indoorgml>
        a       <http://www.w3.org/2004/02/skos/core#Concept> ;
        <http://www.w3.org/2000/01/rdf-schema#comment>
                "Not yet registered with IANA"@en ;
        <http://www.w3.org/2000/01/rdf-schema#label>
                "Media type for IndoorGML" ;
        <http://purl.org/dc/terms/created>
                "2020-06-01"^^<http://www.w3.org/2001/XMLSchema#date> ;
        <http://purl.org/dc/terms/modified>
                "2020-06-08"^^<http://www.w3.org/2001/XMLSchema#date> ;
        <http://www.w3.org/2004/02/skos/core#definition>
                "Media type for IndoorGML"@en ;
        <http://www.w3.org/2004/02/skos/core#prefLabel>
                "Media type for IndoorGML"@en ;
        <http://www.w3.org/2004/02/skos/core#related>
                <http://www.opengis.net/def/encoding/ogc/indoorgml> .

<http://www.opengis.net/def/media-type/ogc/1.0/kml>
        a       <http://www.w3.org/2004/02/skos/core#Concept> ;
        <http://www.w3.org/2000/01/rdf-schema#label>
                "Media type for  the XML encoding of KML" ;
        <http://www.w3.org/2000/01/rdf-schema#seeAlso>
                <https://www.iana.org/assignments/media-types/application/vnd.google-earth.kml+xml> ;
        <http://purl.org/dc/terms/created>
                "2020-06-01"^^<http://www.w3.org/2001/XMLSchema#date> ;
        <http://purl.org/dc/terms/modified>
                "2020-06-08"^^<http://www.w3.org/2001/XMLSchema#date> ;
        <http://www.w3.org/2004/02/skos/core#definition>
                "KML documents can be distributed as uncompressed KML or compressed KMZ files.\n\nKML files are plain-text based XML files with a ‘.kml’ file extension. The internet media type: application/vnd.google-earth.kml+xml has been registered with the Internet Assigned Numbers Authority (IANA) for KML files.\n\nKMZ files are ZIP archives with a ‘.kmz’ file extension. The internet media type: application/vnd.google-earth.kmz has been registered with the Internet Assigned Numbers Authority (IANA) for KMZ archives, but application/zip can also be used to identify the entity as a KMZ archive. See Annex C for details regarding the structure and content of a KMZ archive."@en ;
        <http://www.w3.org/2004/02/skos/core#notation>
                "application/vnd.google-earth.kml+xml"^^<https://www.iana.org/assignments/media-types> ;
        <http://www.w3.org/2004/02/skos/core#prefLabel>
                "Media type for  the XML encoding of KML"@en ;
        <http://www.w3.org/2004/02/skos/core#related>
                <http://www.opengis.net/def/encoding/ogc/kml> .

<http://www.opengis.net/def/media-type/ogc/1.0/i3s>
        a       <http://www.w3.org/2004/02/skos/core#Concept> ;
        <http://www.w3.org/2000/01/rdf-schema#comment>
                "Not yet registered with IANA"@en ;
        <http://www.w3.org/2000/01/rdf-schema#label>
                "Media type for i3s" ;
        <http://purl.org/dc/terms/created>
                "2020-06-01"^^<http://www.w3.org/2001/XMLSchema#date> ;
        <http://purl.org/dc/terms/modified>
                "2020-06-08"^^<http://www.w3.org/2001/XMLSchema#date> ;
        <http://www.w3.org/2004/02/skos/core#definition>
                "Media type for i3s"@en ;
        <http://www.w3.org/2004/02/skos/core#prefLabel>
                "Media type for i3s"@en ;
        <http://www.w3.org/2004/02/skos/core#related>
                <http://www.opengis.net/def/encoding/ogc/i3s> .

<http://www.opengis.net/def/register/>
        <http://www.w3.org/2004/02/skos/core#member>
                <http://www.opengis.net/def/media-type/> .

<http://www.opengis.net/def/media-type/ogc/1.0/geoxacml>
        a       <http://www.w3.org/2004/02/skos/core#Concept> ;
        <http://www.w3.org/2000/01/rdf-schema#label>
                "Media type for Geospatial eXtensible Access Control Markup Language (GeoXACML)" ;
        <http://www.w3.org/2000/01/rdf-schema#seeAlso>
                <https://www.iana.org/assignments/media-types/application/geoxacml+xml> ;
        <http://purl.org/dc/terms/created>
                "2020-06-01"^^<http://www.w3.org/2001/XMLSchema#date> ;
        <http://purl.org/dc/terms/modified>
                "2020-06-08"^^<http://www.w3.org/2001/XMLSchema#date> ;
        <http://www.w3.org/2004/02/skos/core#definition>
                "Media type for Geospatial eXtensible Access Control Markup Language (GeoXACML)"@en ;
        <http://www.w3.org/2004/02/skos/core#notation>
                "application/geoxacml+xml"^^<https://www.iana.org/assignments/media-types> ;
        <http://www.w3.org/2004/02/skos/core#prefLabel>
                "Media type for Geospatial eXtensible Access Control Markup Language (GeoXACML)"@en ;
        <http://www.w3.org/2004/02/skos/core#related>
                <http://www.opengis.net/def/encoding/ogc/geoxacml> .

<http://www.opengis.net/def/media-type/ogc/1.0/cis-gml>
        a       <http://www.w3.org/2004/02/skos/core#Concept> ;
        <http://www.w3.org/2000/01/rdf-schema#label>
                "Media type for CIS - GML encoding" ;
        <http://www.w3.org/2000/01/rdf-schema#seeAlso>
                <https://www.iana.org/assignments/media-types/application/gml+xml> ;
        <http://purl.org/dc/terms/created>
                "2020-06-01"^^<http://www.w3.org/2001/XMLSchema#date> ;
        <http://purl.org/dc/terms/modified>
                "2020-06-08"^^<http://www.w3.org/2001/XMLSchema#date> ;
        <http://www.w3.org/2004/02/skos/core#definition>
                "Media type for the GML encoding of the Coverage Implementation Schema (CIS)"@en ;
        <http://www.w3.org/2004/02/skos/core#notation>
                "application/gml+xml"^^<https://www.iana.org/assignments/media-types> ;
        <http://www.w3.org/2004/02/skos/core#prefLabel>
                "Media type for CIS - GML encoding"@en .

<http://www.opengis.net/def/media-type/ogc/1.0/geosciml>
        a       <http://www.w3.org/2004/02/skos/core#Concept> ;
        <http://www.w3.org/2000/01/rdf-schema#comment>
                "Not yet registered with IANA"@en ;
        <http://www.w3.org/2000/01/rdf-schema#label>
                "Media type for GeoSciML" ;
        <http://purl.org/dc/terms/created>
                "2020-06-01"^^<http://www.w3.org/2001/XMLSchema#date> ;
        <http://purl.org/dc/terms/modified>
                "2020-06-08"^^<http://www.w3.org/2001/XMLSchema#date> ;
        <http://www.w3.org/2004/02/skos/core#definition>
                "Media type for GeoSciML"@en ;
        <http://www.w3.org/2004/02/skos/core#prefLabel>
                "Media type for GeoSciML"@en ;
        <http://www.w3.org/2004/02/skos/core#related>
                <http://www.opengis.net/def/encoding/ogc/geosciml> .

<http://www.opengis.net/def/media-type/ogc/1.0/geotiff>
        a       <http://www.w3.org/2004/02/skos/core#Concept> ;
        <http://www.w3.org/2000/01/rdf-schema#label>
                "Media type for OGC GeoTIFF" ;
        <http://purl.org/dc/terms/created>
                "2020-06-01"^^<http://www.w3.org/2001/XMLSchema#date> ;
        <http://purl.org/dc/terms/modified>
                "2020-06-08"^^<http://www.w3.org/2001/XMLSchema#date> ;
        <http://www.w3.org/2004/02/skos/core#definition>
                "A GeoTIFF file is a TIFF file. It is common to use the tiff MIME type,\timage/tiff\taccording to [RFC3302] (see also http://www.iana.org/assignments/media-types/media-types.xhtml#image).\n\nOGC GMLCOV GeoTIFF extension (OGC 12-100r1) specifies image/tiff as the MIME identifier (cf. Requirement #5 in OGC 12-100r1).\n\nThe recommendation for the MIME type is to use the image/tiff application parameter, with the geotiff value, therefore as follows: image/tiff; application=geotiff."@en ;
        <http://www.w3.org/2004/02/skos/core#notation>
                "image/tiff; application=geotiff"^^<https://www.iana.org/assignments/media-types> ;
        <http://www.w3.org/2004/02/skos/core#prefLabel>
                "Media type for OGC GeoTIFF"@en ;
        <http://www.w3.org/2004/02/skos/core#related>
                <http://www.opengis.net/def/encoding/ogc/geotiff> .

<http://www.opengis.net/def/media-type/ogc/1.0/geopackage>
        a       <http://www.w3.org/2004/02/skos/core#Concept> ;
        <http://www.w3.org/2000/01/rdf-schema#label>
                "Media type for GeoPackage" ;
        <http://www.w3.org/2000/01/rdf-schema#seeAlso>
                <https://www.iana.org/assignments/media-types/application/geopackage+sqlite3> ;
        <http://purl.org/dc/terms/created>
                "2020-06-01"^^<http://www.w3.org/2001/XMLSchema#date> ;
        <http://purl.org/dc/terms/modified>
                "2020-06-08"^^<http://www.w3.org/2001/XMLSchema#date> ;
        <http://www.w3.org/2004/02/skos/core#definition>
                "Media type for GeoPackage"@en ;
        <http://www.w3.org/2004/02/skos/core#notation>
                "application/geopackage+sqlite3"^^<https://www.iana.org/assignments/media-types> ;
        <http://www.w3.org/2004/02/skos/core#prefLabel>
                "Media type for GeoPackage"@en ;
        <http://www.w3.org/2004/02/skos/core#related>
                <http://www.opengis.net/def/encoding/ogc/geopackage> .

<http://www.opengis.net/def/media-type/ogc/1.0/kml-kmz>
        a       <http://www.w3.org/2004/02/skos/core#Concept> ;
        <http://www.w3.org/2000/01/rdf-schema#label>
                "Media type for  the Zip archive encoding of KML" ;
        <http://www.w3.org/2000/01/rdf-schema#seeAlso>
                <https://www.iana.org/assignments/media-types/application/vnd.google-earth.kmz> ;
        <http://purl.org/dc/terms/created>
                "2020-06-01"^^<http://www.w3.org/2001/XMLSchema#date> ;
        <http://purl.org/dc/terms/modified>
                "2020-06-08"^^<http://www.w3.org/2001/XMLSchema#date> ;
        <http://www.w3.org/2004/02/skos/core#definition>
                "KML documents can be distributed as uncompressed KML or compressed KMZ files.\n\nKML files are plain-text based XML files with a ‘.kml’ file extension. The internet media type: application/vnd.google-earth.kml+xml has been registered with the Internet Assigned Numbers Authority (IANA) for KML files.\n\nKMZ files are ZIP archives with a ‘.kmz’ file extension. The internet media type: application/vnd.google-earth.kmz has been registered with the Internet Assigned Numbers Authority (IANA) for KMZ archives, but application/zip can also be used to identify the entity as a KMZ archive. See Annex C for details regarding the structure and content of a KMZ archive."@en ;
        <http://www.w3.org/2004/02/skos/core#notation>
                "application/vnd.google-earth.kmz"^^<https://www.iana.org/assignments/media-types> ;
        <http://www.w3.org/2004/02/skos/core#prefLabel>
                "Media type for  the Zip archive encoding of KML"@en ;
        <http://www.w3.org/2004/02/skos/core#related>
                <http://www.opengis.net/def/encoding/ogc/kml> .

<http://www.opengis.net/def/media-type/ogc/1.0/gmljp2>
        a       <http://www.w3.org/2004/02/skos/core#Concept> ;
        <http://www.w3.org/2000/01/rdf-schema#comment>
                "Not yet registered with IANA"@en ;
        <http://www.w3.org/2000/01/rdf-schema#label>
                "Media type for GML in JPEG 2000" ;
        <http://purl.org/dc/terms/created>
                "2020-06-01"^^<http://www.w3.org/2001/XMLSchema#date> ;
        <http://purl.org/dc/terms/modified>
                "2020-06-08"^^<http://www.w3.org/2001/XMLSchema#date> ;
        <http://www.w3.org/2004/02/skos/core#definition>
                "Media type for GML in JPEG 2000"@en ;
        <http://www.w3.org/2004/02/skos/core#prefLabel>
                "Media type for GML in JPEG 2000"@en ;
        <http://www.w3.org/2004/02/skos/core#related>
                <http://www.opengis.net/def/encoding/ogc/gmljp2> .

<http://www.opengis.net/def/media-type/ogc/1.0/sld>
        a       <http://www.w3.org/2004/02/skos/core#Concept> ;
        <http://www.w3.org/2000/01/rdf-schema#comment>
                "Not yet registered with IANA"@en ;
        <http://www.w3.org/2000/01/rdf-schema#label>
                "Media type for Styled Layer Descriptor" ;
        <http://purl.org/dc/terms/created>
                "2020-06-01"^^<http://www.w3.org/2001/XMLSchema#date> ;
        <http://purl.org/dc/terms/modified>
                "2020-06-08"^^<http://www.w3.org/2001/XMLSchema#date> ;
        <http://www.w3.org/2004/02/skos/core#definition>
                "Media type for Styled Layer Descriptor"@en ;
        <http://www.w3.org/2004/02/skos/core#prefLabel>
                "Media type for Styled Layer Descriptor"@en ;
        <http://www.w3.org/2004/02/skos/core#related>
                <http://www.opengis.net/def/encoding/ogc/sld> .

<http://www.opengis.net/def/media-type/ogc/1.0/hdf>
        a       <http://www.w3.org/2004/02/skos/core#Concept> ;
        <http://www.w3.org/2000/01/rdf-schema#comment>
                "Not yet registered with IANA"@en ;
        <http://www.w3.org/2000/01/rdf-schema#label>
                "Media type for the OGC Hierarchical Data Format Version 5 (HDF5) Standard" ;
        <http://purl.org/dc/terms/created>
                "2020-06-01"^^<http://www.w3.org/2001/XMLSchema#date> ;
        <http://purl.org/dc/terms/modified>
                "2020-06-08"^^<http://www.w3.org/2001/XMLSchema#date> ;
        <http://www.w3.org/2004/02/skos/core#definition>
                "The MIME type application/x-hdf5 is unregistered and it doesn’t appear in the list at http://www.iana.org/assignments/media-types/index.html. "@en ;
        <http://www.w3.org/2004/02/skos/core#notation>
                "application/x-hdf5"^^<https://www.iana.org/assignments/media-types> ;
        <http://www.w3.org/2004/02/skos/core#prefLabel>
                "Media type for the OGC Hierarchical Data Format Version 5 (HDF5) Standard"@en ;
        <http://www.w3.org/2004/02/skos/core#related>
                <http://www.opengis.net/def/encoding/ogc/hdf> .

<http://www.opengis.net/def/media-type/ogc/1.0/citygml>
        a       <http://www.w3.org/2004/02/skos/core#Concept> ;
        <http://www.w3.org/2000/01/rdf-schema#comment>
                "Not yet registered with IANA"@en ;
        <http://www.w3.org/2000/01/rdf-schema#label>
                "Media type for CityGML" ;
        <http://purl.org/dc/terms/created>
                "2020-06-01"^^<http://www.w3.org/2001/XMLSchema#date> ;
        <http://purl.org/dc/terms/modified>
                "2020-06-08"^^<http://www.w3.org/2001/XMLSchema#date> ;
        <http://www.w3.org/2004/02/skos/core#definition>
                "Media type for CityGML"@en ;
        <http://www.w3.org/2004/02/skos/core#prefLabel>
                "Media type for CityGML"@en ;
        <http://www.w3.org/2004/02/skos/core#related>
                <http://www.opengis.net/def/encoding/ogc/citygml> .

<https://www.opengis.net/def/media-type>
        a       <http://www.w3.org/2004/02/skos/core#ConceptScheme> ;
        <http://www.w3.org/2000/01/rdf-schema#label>
                "OGC Media Type Register" ;
        <http://www.opengis.net/def/metamodel/ogc-na/collectionView>
                <http://www.opengis.net/def/media-type/> ;
        <http://www.w3.org/2004/02/skos/core#definition>
                "This is a register of media types used by OGC standards. The register also identifies OGC media types that have been registered with IANA."@en ;
        <http://www.w3.org/2004/02/skos/core#prefLabel>
                "OGC Media Type Register"@en .

<http://www.opengis.net/def/media-type/ogc/1.0/cis-rdf>
        a       <http://www.w3.org/2004/02/skos/core#Concept> ;
        <http://www.w3.org/2000/01/rdf-schema#label>
                "Media type for CIS - RDF encoding" ;
        <http://www.w3.org/2000/01/rdf-schema#seeAlso>
                <https://www.iana.org/assignments/media-types/application/ld+json> ;
        <http://purl.org/dc/terms/created>
                "2020-06-01"^^<http://www.w3.org/2001/XMLSchema#date> ;
        <http://purl.org/dc/terms/modified>
                "2020-06-08"^^<http://www.w3.org/2001/XMLSchema#date> ;
        <http://www.w3.org/2004/02/skos/core#definition>
                "Media type for the encoding of the Coverage Implementation Schema (CIS) in Resource Description Framework (RDF) JavaScript Object Notation for Linked Data (JSON-LD)"@en ;
        <http://www.w3.org/2004/02/skos/core#notation>
                "application/ld+json"^^<https://www.iana.org/assignments/media-types> ;
        <http://www.w3.org/2004/02/skos/core#prefLabel>
                "Media type for CIS - RDF encoding"@en .

<http://www.opengis.net/def/media-type/ogc/1.0/arml>
        a       <http://www.w3.org/2004/02/skos/core#Concept> ;
        <http://www.w3.org/2000/01/rdf-schema#comment>
                "Not yet registered with IANA"@en ;
        <http://www.w3.org/2000/01/rdf-schema#label>
                "Media type for ARML2.0" ;
        <http://purl.org/dc/terms/created>
                "2020-06-01"^^<http://www.w3.org/2001/XMLSchema#date> ;
        <http://purl.org/dc/terms/modified>
                "2020-06-08"^^<http://www.w3.org/2001/XMLSchema#date> ;
        <http://www.w3.org/2004/02/skos/core#definition>
                "Media type for ARML2.0"@en ;
        <http://www.w3.org/2004/02/skos/core#prefLabel>
                "Media type for ARML2.0"@en ;
        <http://www.w3.org/2004/02/skos/core#related>
                <http://www.opengis.net/def/encoding/ogc/arml2> .


<http://www.opengis.net/def/media-type/ogc/1.0/se>
        a       <http://www.w3.org/2004/02/skos/core#Concept> ;
        <http://www.w3.org/2000/01/rdf-schema#comment>
                "Not yet registered with IANA"@en ;
        <http://www.w3.org/2000/01/rdf-schema#label>
                "Media type for Symbology Encoding" ;
        <http://purl.org/dc/terms/created>
                "2020-06-01"^^<http://www.w3.org/2001/XMLSchema#date> ;
        <http://purl.org/dc/terms/modified>
                "2020-06-08"^^<http://www.w3.org/2001/XMLSchema#date> ;
        <http://www.w3.org/2004/02/skos/core#definition>
                "Media type for Symbology Encoding"@en ;
        <http://www.w3.org/2004/02/skos/core#prefLabel>
                "Media type for Symbology Encoding"@en ;
        <http://www.w3.org/2004/02/skos/core#related>
                <http://www.opengis.net/def/encoding/ogc/se> .

<http://www.opengis.net/def/media-type/ogc/1.0/filter>
        a       <http://www.w3.org/2004/02/skos/core#Concept> ;
        <http://www.w3.org/2000/01/rdf-schema#comment>
                "Not yet registered with IANA"@en ;
        <http://www.w3.org/2000/01/rdf-schema#label>
                "Media type for Filter Encoding" ;
        <http://purl.org/dc/terms/created>
                "2020-06-01"^^<http://www.w3.org/2001/XMLSchema#date> ;
        <http://purl.org/dc/terms/modified>
                "2020-06-08"^^<http://www.w3.org/2001/XMLSchema#date> ;
        <http://www.w3.org/2004/02/skos/core#definition>
                "Media type for Filter Encoding"@en ;
        <http://www.w3.org/2004/02/skos/core#prefLabel>
                "Media type for Filter Encoding"@en ;
        <http://www.w3.org/2004/02/skos/core#related>
                <http://www.opengis.net/def/encoding/ogc/filter> .

<http://www.opengis.net/def/media-type/>
        a       <http://www.w3.org/2004/02/skos/core#Collection> ;
        <http://www.w3.org/2000/01/rdf-schema#label>
                "OGC Media Type Register" ;
        <http://www.w3.org/2004/02/skos/core#definition>
                "This is a register of media types used by OGC standards. The register also identifies OGC media types that have been registered with IANA."@en ;
        <http://www.w3.org/2004/02/skos/core#inScheme>
                <https://www.opengis.net/def/media-type> ;
        <http://www.w3.org/2004/02/skos/core#member>
                <http://www.opengis.net/def/media-type/ogc/1.0/cis-rdf> , <http://www.opengis.net/def/media-type/ogc/1.0/geosciml> , <http://www.opengis.net/def/media-type/ogc/1.0/hdf> ,  <http://www.opengis.net/def/media-type/ogc/1.0/tsml> , <http://www.opengis.net/def/media-type/ogc/1.0/netcdf> , <http://www.opengis.net/def/media-type/ogc/1.0/owc> , <http://www.opengis.net/def/media-type/ogc/1.0/georss> , <http://www.opengis.net/def/media-type/ogc/1.0/gmljp2> , <http://www.opengis.net/def/media-type/ogc/1.0/cdb> , <http://www.opengis.net/def/media-type/ogc/1.0/citygml> , <http://www.opengis.net/def/media-type/ogc/1.0/geopackage> , <http://www.opengis.net/def/media-type/ogc/1.0/om> , <http://www.opengis.net/def/media-type/ogc/1.0/cis-json> , <http://www.opengis.net/def/media-type/ogc/1.0/landinfragml> , <http://www.opengis.net/def/media-type/ogc/1.0/waterml> , <http://www.opengis.net/def/media-type/ogc/1.0/indoorgml> , <http://www.opengis.net/def/media-type/ogc/1.0/gml> , <http://www.opengis.net/def/media-type/ogc/1.0/filter> , <http://www.opengis.net/def/media-type/ogc/1.0/arml> , <http://www.opengis.net/def/media-type/ogc/1.0/sld> , <http://www.opengis.net/def/media-type/ogc/1.0/i3s> , <http://www.opengis.net/def/media-type/ogc/1.0/mf> , <http://www.opengis.net/def/media-type/ogc/1.0/kml> , <http://www.opengis.net/def/media-type/ogc/1.0/guf> , <http://www.opengis.net/def/media-type/ogc/1.0/se> , <http://www.opengis.net/def/media-type/ogc/1.0/las> , <http://www.opengis.net/def/media-type/ogc/1.0/kml-kmz> , <http://www.opengis.net/def/media-type/ogc/1.0/geoxacml> , <http://www.opengis.net/def/media-type/ogc/1.0/wktcrs> , <http://www.opengis.net/def/media-type/ogc/1.0/cis-gml> , <http://www.opengis.net/def/media-type/ogc/1.0/gwml> , <http://www.opengis.net/def/media-type/ogc/1.0/3dtiles> , <http://www.opengis.net/def/media-type/ogc/1.0/geotiff> ;
        <http://www.w3.org/2004/02/skos/core#prefLabel>
                "OGC Media Type Register"@en .

<http://www.opengis.net/def/media-type/ogc/1.0/gwml>
        a       <http://www.w3.org/2004/02/skos/core#Concept> ;
        <http://www.w3.org/2000/01/rdf-schema#label>
                "Media type for GroundwaterML" ;
        <http://purl.org/dc/terms/created>
                "2020-06-01"^^<http://www.w3.org/2001/XMLSchema#date> ;
        <http://purl.org/dc/terms/modified>
                "2020-06-08"^^<http://www.w3.org/2001/XMLSchema#date> ;
        <http://www.w3.org/2004/02/skos/core#definition>
                "The standard MIME-type and sub-type for GML data should be used to indicate the encoding choice as specified in MIME Media Types for GML, namely: application/gml+xml."@en ;
        <http://www.w3.org/2004/02/skos/core#notation>
                "application/gml+xml"^^<https://www.iana.org/assignments/media-types> ;
        <http://www.w3.org/2004/02/skos/core#prefLabel>
                "Media type for GroundwaterML"@en ;
        <http://www.w3.org/2004/02/skos/core#related>
                <http://www.opengis.net/def/encoding/ogc/groundwaterml> .

<http://www.opengis.net/def/media-type/ogc/1.0/waterml>
        a       <http://www.w3.org/2004/02/skos/core#Concept> ;
        <http://www.w3.org/2000/01/rdf-schema#comment>
                "Not yet registered with IANA"@en ;
        <http://www.w3.org/2000/01/rdf-schema#label>
                "Media type for WaterML" ;
        <http://purl.org/dc/terms/created>
                "2020-06-01"^^<http://www.w3.org/2001/XMLSchema#date> ;
        <http://purl.org/dc/terms/modified>
                "2020-06-08"^^<http://www.w3.org/2001/XMLSchema#date> ;
        <http://www.w3.org/2004/02/skos/core#definition>
                "Media type for WaterML"@en ;
        <http://www.w3.org/2004/02/skos/core#prefLabel>
                "Media type for WaterML"@en ;
        <http://www.w3.org/2004/02/skos/core#related>
                <http://www.opengis.net/def/encoding/ogc/waterml> .

<http://www.opengis.net/def/media-type/ogc/1.0/om>
        a       <http://www.w3.org/2004/02/skos/core#Concept> ;
        <http://www.w3.org/2000/01/rdf-schema#comment>
                "Not yet registered with IANA"@en ;
        <http://www.w3.org/2000/01/rdf-schema#label>
                "Media type for Observations and Measurements" ;
        <http://purl.org/dc/terms/created>
                "2020-06-01"^^<http://www.w3.org/2001/XMLSchema#date> ;
        <http://purl.org/dc/terms/modified>
                "2020-06-08"^^<http://www.w3.org/2001/XMLSchema#date> ;
        <http://www.w3.org/2004/02/skos/core#definition>
                "Media type for Observations and Measurements"@en ;
        <http://www.w3.org/2004/02/skos/core#prefLabel>
                "Media type for Observations and Measurements"@en ;
        <http://www.w3.org/2004/02/skos/core#related>
                <http://www.opengis.net/def/ogc-om> .
