<http://www.opengis.net/def/wkss/OGC/1.0/GlobalCRS84Scale>
        a       <http://www.w3.org/2004/02/skos/core#Concept> ;
        <http://www.w3.org/2000/01/rdf-schema#label>
                "GlobalCRS84Scale" ;
        <http://www.w3.org/2000/01/rdf-schema#seeAlso>
                <http://docs.opengeospatial.org/is/17-083r2/17-083r2.html#57> ;
        <http://purl.org/dc/terms/created>
                "2020-10-04"^^<http://www.w3.org/2001/XMLSchema#date> ;
        <http://www.w3.org/2004/02/skos/core#definition>
                "GlobalCRS84Scale well-known scale set definition"@en ;
        <http://www.w3.org/2004/02/skos/core#inScheme>
                <http://www.opengis.net/def/wkss/OGC> ;
        <http://www.w3.org/2004/02/skos/core#prefLabel>
                "GlobalCRS84Scale"@en .

<http://www.opengis.net/def/wkss/OGC/1.0/GoogleCRS84Quad>
        a       <http://www.w3.org/2004/02/skos/core#Concept> ;
        <http://www.w3.org/2000/01/rdf-schema#label>
                "GoogleCRS84Quad" ;
        <http://www.w3.org/2000/01/rdf-schema#seeAlso>
                <http://docs.opengeospatial.org/is/17-083r2/17-083r2.html#59> ;
        <http://purl.org/dc/terms/created>
                "2020-10-04"^^<http://www.w3.org/2001/XMLSchema#date> ;
        <http://www.w3.org/2004/02/skos/core#definition>
                "GoogleCRS84Quad well-known scale set definition"@en ;
        <http://www.w3.org/2004/02/skos/core#inScheme>
                <http://www.opengis.net/def/wkss/OGC> ;
        <http://www.w3.org/2004/02/skos/core#prefLabel>
                "GoogleCRS84Quad"@en .

<http://www.opengis.net/def/wkss/OGC/1.0/GoogleMapsCompatible>
        a       <http://www.w3.org/2004/02/skos/core#Concept> ;
        <http://www.w3.org/2000/01/rdf-schema#label>
                "GoogleMapsCompatible" ;
        <http://www.w3.org/2000/01/rdf-schema#seeAlso>
                <http://docs.opengeospatial.org/is/17-083r2/17-083r2.html> ;
        <http://purl.org/dc/terms/created>
                "2021-11-30"^^<http://www.w3.org/2001/XMLSchema#date> ;
        <http://www.w3.org/2004/02/skos/core#definition>
                "GoogleMapsCompatible well-known scale set definition"@en ;
        <http://www.w3.org/2004/02/skos/core#inScheme>
                <http://www.opengis.net/def/wkss/OGC> ;
        <http://www.w3.org/2004/02/skos/core#prefLabel>
                "GoogleMapsCompatible"@en .

<http://www.opengis.net/def/wkss/OGC/1.0/WorldMercatorWGS84>
        a       <http://www.w3.org/2004/02/skos/core#Concept> ;
        <http://www.w3.org/2000/01/rdf-schema#label>
                "WorldMercatorWGS84" ;
        <http://www.w3.org/2000/01/rdf-schema#seeAlso>
                <http://docs.opengeospatial.org/is/17-083r2/17-083r2.html#60> ;
        <http://purl.org/dc/terms/created>
                "2020-10-04"^^<http://www.w3.org/2001/XMLSchema#date> ;
        <http://www.w3.org/2004/02/skos/core#definition>
                "WorldMercatorWGS84 well-known scale set definition"@en ;
        <http://www.w3.org/2004/02/skos/core#inScheme>
                <http://www.opengis.net/def/wkss/OGC> ;
        <http://www.w3.org/2004/02/skos/core#prefLabel>
                "WorldMercatorWGS84"@en .

<http://www.opengis.net/def/wkss/OGC/>
        a       <http://www.w3.org/2004/02/skos/core#Collection> ;
        <http://www.w3.org/2000/01/rdf-schema#label>
                "OGC Well-Known Scale Sets (WKSS)" ;
        <http://purl.org/dc/terms/created>
                "2020-10-04"^^<http://www.w3.org/2001/XMLSchema#date> ;
        <http://www.w3.org/2004/02/skos/core#definition>
                "The Well-Known Scale Sets(WKSS) concept was introduced in the Web Map Tile Service (WMTS) standard (OGC 07-057r7) to improve interoperability and further described in the 2D Tile Matrix Set standard (OGC 17-083r2)."@en ;
        <http://www.w3.org/2004/02/skos/core#inScheme>
                <http://www.opengis.net/def/wkss/OGC> ;
        <http://www.w3.org/2004/02/skos/core#member>
                <http://www.opengis.net/def/wkss/OGC/1.0/WorldMercatorWGS84> , <http://www.opengis.net/def/wkss/OGC/1.0/GoogleCRS84Quad>, <http://www.opengis.net/def/wkss/OGC/1.0/GoogleMapsCompatible> , <http://www.opengis.net/def/wkss/OGC/1.0/GlobalCRS84Pixel> , <http://www.opengis.net/def/wkss/OGC/1.0/GlobalCRS84Scale> ;
        <http://www.w3.org/2004/02/skos/core#prefLabel>
                "OGC Well-Known Scale Sets (WKSS)"@en .

<http://www.opengis.net/def/wkss/OGC>
        a       <http://www.w3.org/2004/02/skos/core#ConceptScheme> ;
        <http://www.w3.org/2000/01/rdf-schema#label>
                "OGC Well-Known Scale Sets (WKSS)" ;
        <http://purl.org/dc/terms/created>
                "2020-10-04"^^<http://www.w3.org/2001/XMLSchema#date> ;
        <http://www.opengis.net/def/metamodel/ogc-na/collectionView>
                <http://www.opengis.net/def/wkss/OGC/> ;
        <http://www.w3.org/2004/02/skos/core#definition>
                "The Well-Known Scale Sets(WKSS) concept was introduced in the Web Map Tile Service (WMTS) standard (OGC 07-057r7) to improve interoperability and further described in the 2D Tile Matrix Set standard (OGC 17-083r2)."@en ;
        <http://www.w3.org/2004/02/skos/core#prefLabel>
                "OGC Well-Known Scale Sets (WKSS)"@en .

<http://www.opengis.net/def/wkss/OGC/1.0/GlobalCRS84Pixel>
        a       <http://www.w3.org/2004/02/skos/core#Concept> ;
        <http://www.w3.org/2000/01/rdf-schema#label>
                "GlobalCRS84Pixel" ;
        <http://www.w3.org/2000/01/rdf-schema#seeAlso>
                <http://docs.opengeospatial.org/is/17-083r2/17-083r2.html#58> ;
        <http://purl.org/dc/terms/created>
                "2020-10-04"^^<http://www.w3.org/2001/XMLSchema#date> ;
        <http://www.w3.org/2004/02/skos/core#definition>
                "GlobalCRS84Pixel well-known scale set definition"@en ;
        <http://www.w3.org/2004/02/skos/core#inScheme>
                <http://www.opengis.net/def/wkss/OGC> ;
        <http://www.w3.org/2004/02/skos/core#prefLabel>
                "GlobalCRS84Pixel"@en .

<http://www.opengis.net/def/register/>
        <http://www.w3.org/2004/02/skos/core#member>
                <http://www.opengis.net/def/wkss/> .

<http://www.opengis.net/def/wkss/>
        a       <http://www.w3.org/2004/02/skos/core#Collection> ;
        <http://www.w3.org/2000/01/rdf-schema#label>
                "Well-Known Scale Sets (WKSS) Register" ;
        <http://purl.org/dc/terms/created>
                "2020-10-04"^^<http://www.w3.org/2001/XMLSchema#date> ;
        <http://www.w3.org/2004/02/skos/core#definition>
                "The Well-Known Scale Sets(WKSS) concept was introduced in the Web Map Tile Service (WMTS) standard (OGC 07-057r7) to improve interoperability and further described in the 2D Tile Matrix Set standard (OGC 17-083r2)."@en ;
        <http://www.w3.org/2004/02/skos/core#inScheme>
                <http://www.opengis.net/def/wkss> ;
        <http://www.w3.org/2004/02/skos/core#member>
                <http://www.opengis.net/def/wkss/OGC/> ;
        <http://www.w3.org/2004/02/skos/core#prefLabel>
                "Well-Known Scale Sets (WKSS)"@en .

<http://www.opengis.net/def/wkss>
        a       <http://www.w3.org/2004/02/skos/core#ConceptScheme> ;
        <http://www.w3.org/2000/01/rdf-schema#label>
                "Well-Known Scale Sets (WKSS) Register" ;
        <http://purl.org/dc/terms/created>
                "2020-10-04"^^<http://www.w3.org/2001/XMLSchema#date> ;
        <http://www.opengis.net/def/metamodel/ogc-na/collectionView>
                <http://www.opengis.net/def/wkss/> ;
        <http://www.w3.org/2004/02/skos/core#definition>
                "The Well-Known Scale Sets(WKSS) concept was introduced in the Web Map Tile Service (WMTS) standard (OGC 07-057r7) to improve interoperability and further described in the 2D Tile Matrix Set standard (OGC 17-083r2)."@en ;
        <http://www.w3.org/2004/02/skos/core#prefLabel>
                "Well-Known Scale Sets (WKSS) Register"@en .
