@prefix adms: <http://www.w3.org/ns/adms#> .
@prefix dcat: <http://www.w3.org/ns/dcat#> .
@prefix dct: <http://purl.org/dc/terms/> .
@prefix na: <http://www.opengis.net/def/metamodel/ogc-na/> .
@prefix ogcdt: <http://www.opengis.net/def/doc-type/> .
@prefix owl: <http://www.w3.org/2002/07/owl#> .
@prefix reg: <http://purl.org/linked-data/registry#> .
@prefix skos: <http://www.w3.org/2004/02/skos/core#> .
@prefix spec: <http://www.opengis.net/def/ont/modspec/> .
@prefix specrel: <http://www.opengis.net/def/ont/specrel/> .
@prefix xsd: <http://www.w3.org/2001/XMLSchema#> .
@prefix prov: <http://www.w3.org/ns/prov#> .
@prefix wg: <http://www.opengis.net/def/wg/> .
@prefix status: <http://www.opengis.net/def/status/> .

<http://www.opengis.net/spec/docs/16-100r2-anno> a owl:Ontology .

<http://www.opengis.net/spec/infragml/part0/1.0> a skos:ConceptScheme ;
  dct:source <http://www.opengis.net/def/docs/16-100r2> ;
  skos:prefLabel "Specification elements for OGC 16-100r2 LandInfra" ;
  skos:definition "A convenience hierarchy for navigating the elements of a specification using the SKOS model" ;
  dct:modified "2017-06-02"^^xsd:date ;
  dct:created "2017-03-24"^^xsd:date ;
  skos:hasTopConcept <http://www.opengis.net/spec/landinfra/part0/1.0/conf/core> ;
.

<http://www.opengis.net/def/docs/16-100r2> a spec:Specification ;
    dct:creator "Paul Scarponcini" ;
    dct:dateAccepted "2017-06-02"^^xsd:date ;
    dct:dateSubmitted "2017-03-24"^^xsd:date ;
    dct:identifier "http://www.opengis.net/doc/is/landinfra/part0/1.0" ;
    reg:status reg:statusValid ;
    spec:status status:valid ;
    na:doctype ogcdt:ip ;
    spec:authority "Open Geospatial Consortium" ;
    spec:class <http://www.opengis.net/spec/landinfra/part0/1.0/conf/core>;
    spec:date "2017-06-02"^^xsd:date ;
    skos:notation "16-100r2"^^na:doc_no ;
    skos:prefLabel "OGC InfraGML 1.0: Part 0 – LandInfra Core - Encoding Standard" ;
    skos:definition "OGC® Encoding Standard; Core one required by any other encoding parts" ;
    adms:version "1.0" ;
    dcat:landingPage <https://docs.opengeospatial.org/is/16-100r2/16-100r2.html> ;
    skos:topConceptOf <http://www.opengis.net/spec/landinfra> ;
    adms:last <http://www.opengis.net/def/docs/16-100r2> ;
    prov:wasAttributedTo wg:landinfraswg ;
    specrel:implements <http://www.opengis.net/def/docs/15-111r1> ;
    skos:inScheme <http://www.opengis.net/def/docs> .


<http://www.opengis.net/spec/landinfra/part0/1.0/req/core> a spec:RequirementsClass,
    skos:Concept ;
    spec:normativeStatement <http://www.opengis.net/spec/landinfra/part0/1.0/req/core/valid> ,
        <http://www.opengis.net/spec/landinfra/part0/1.0/req/core/header> ,
        <http://www.opengis.net/spec/landinfra/part0/1.0/req/core/gml3.2> ,
        <http://www.opengis.net/spec/landinfra/part0/1.0/req/core/gml3.3lr> ,
        <http://www.opengis.net/spec/landinfra/part0/1.0/req/core/gml3.3lro> ,
        <http://www.opengis.net/spec/landinfra/part0/1.0/req/core/elements> ;
    # spec:dependency  ; #several, but to the specifications in a whole like 3.2 or parts like 3.3 linearRef that does not exist yet in the defserver
    skos:definition "LandInfra Core is the core Requirements Class and is the only mandatory Requirements Class. This class contains information about the Land and Infrastructure dataset that can contain information about facilities, land features, land division, documents, survey marks, surveys, sets, and feature associations. LandInfra Core also contains the definition of types common across other Requirements Classes, such as the Status CodeList." ;
    skos:prefLabel "Requirement Class: Core" .

<http://www.opengis.net/spec/landinfra/part0/1.0/conf/core> a spec:ConformanceClass,
        skos:Concept ;
    spec:conformanceTest <http://www.opengis.net/spec/landinfra/part0/1.0/conf/core/valid> ,
        <http://www.opengis.net/spec/landinfra/part0/1.0/conf/core/header> ,
        <http://www.opengis.net/spec/landinfra/part0/1.0/conf/core/gml3.2> ,
        <http://www.opengis.net/spec/landinfra/part0/1.0/conf/core/gml3.3lr> ,
        <http://www.opengis.net/spec/landinfra/part0/1.0/conf/core/gml3.3lro> ,
        <http://www.opengis.net/spec/landinfra/part0/1.0/conf/core/elements> ;
    spec:requirementsTested <http://www.opengis.net/spec/landinfra/part0/1.0/req/core> ;
    # spec:dependency ? ; # shall it have dependencies like RequirementsClass or traversal dependency is enought?
    skos:topConceptOf <http://www.opengis.net/spec/landinfra/part0/1.0> ;
    skos:inScheme <http://www.opengis.net/spec/landinfra/part0/1.0> ;
    dcat:landingPage <https://docs.opengeospatial.org/is/16-100r2/16-100r2.html#_conformance_class_core> ;
    skos:definition "Conformance Class: Core" ;
    skos:prefLabel "Conformance Class: Core" .

<http://www.opengis.net/spec/landinfra/part0/1.0/conf/core/valid> a spec:ConformanceTest,
        skos:Concept ;
    spec:method "Verify that XML instance documents of any Part of InfraGML is valid according to the XML grammar specified in that Part for each Requirements Class contained in that Part and available at http://schemas.opengis.net/infragml/part<n>/1.0/<schema name>.xsd where <n> is the Part number and <schema name> is the name of the schema equal to the name of the respective Requirements Class." ;
    spec:purpose "Validate the XML document using the XML schema document(s) for the applicable Part(s). Pass if no errors reported. Fail otherwise." ;
    skos:definition "Validate the XML document using the XML schema document(s) for the applicable Part(s). Pass if no errors reported. Fail otherwise." ;# it could be extracted from purpose?
    spec:requirement <http://www.opengis.net/spec/landinfra/part0/1.0/req/core/valid> ;
    spec:testType spec:Basic ;
    skos:prefLabel "Conformance Test: http://www.opengis.net/spec/landinfra/part0/1.0/conf/core/valid" .

<http://www.opengis.net/spec/landinfra/part0/1.0/conf/core/header> a spec:ConformanceTest,
        skos:Concept ;
    spec:method "Inspect the schema definition file used by the application." ;
    spec:purpose "Verify that the conforming application uses a schema definition file which contains a properly formed schema header appropriate to the InfraGML Requirements Classes it claims to support." ;
    skos:definition "Verify that the encoding specifies whether it supports ID at the feature level, ID at the Feature sub-type level, or both." ;
    spec:requirement <http://www.opengis.net/spec/landinfra/part0/1.0/req/core/header> ;
    spec:testType spec:Basic ;
    skos:prefLabel "Conformance Test: http://www.opengis.net/spec/landinfra/part0/1.0/conf/core/header" .

<http://www.opengis.net/spec/landinfra/part0/1.0/conf/core/gml3.2> a spec:ConformanceTest,
        skos:Concept ;
    spec:method "Inspect the GML output to verify that all appropriate elements have a 'gml:' prefix." ;
    spec:purpose "Verify that the conforming application utilizes and depends upon the OGC GML 3.2 standard schema within the http://www.opengis.net/gml/3.2 namespace identified by 'gml'." ;
    skos:definition "Verify that the conforming application utilizes and depends upon the OGC GML 3.2 standard schema within the http://www.opengis.net/gml/3.2 namespace identified by 'gml'." ;
    spec:requirement <http://www.opengis.net/spec/landinfra/part0/1.0/req/core/gml3.2> ;
    spec:testType spec:Capability ;
    skos:prefLabel "Conformance Test: http://www.opengis.net/spec/landinfra/part0/1.0/conf/core/gml3.2" .

<http://www.opengis.net/spec/landinfra/part0/1.0/conf/core/gml3.3lr> a spec:ConformanceTest,
        skos:Concept ;
    spec:method "Inspect the GML output to verify that all appropriate elements have a 'gmllr:' prefix." ;
    spec:purpose "Verify that the conforming application utilizes and depends upon the OGC GML 3.3 linearRef standard schema within the http://www.opengis.net/gml/3.3/lr namespace identified by 'gmllr'." ;
    skos:definition "Verify that the conforming application utilizes and depends upon the OGC GML 3.3 linearRef standard schema within the http://www.opengis.net/gml/3.3/lr namespace identified by 'gmllr'." ;
    spec:requirement <http://www.opengis.net/spec/landinfra/part0/1.0/req/core/gml3.3lr> ;
    spec:testType spec:Capabilities ;
    skos:prefLabel "Conformance Test: http://www.opengis.net/spec/landinfra/part0/1.0/conf/core/gml3.3lr" .

<http://www.opengis.net/spec/landinfra/part0/1.0/conf/core/gml3.3lro> a spec:ConformanceTest,
        skos:Concept ;
    spec:method "Inspect the GML output to verify that all appropriate elements have a 'gmllro:' prefix." ;
    spec:purpose "Verify that the conforming application utilizes and depends upon the OGC GML 3.3 linearRefOffset standard schema within the http://www.opengis.net/gml/3.3/lro namespace identified by 'gmllro'." ;
    skos:definition "Verify that the conforming application utilizes and depends upon the OGC GML 3.3 linearRefOffset standard schema within the http://www.opengis.net/gml/3.3/lro namespace identified by 'gmllro'." ;
    spec:requirement <http://www.opengis.net/spec/landinfra/part0/1.0/req/core/gml3.3lro> ;
    spec:testType spec:Capabilities ;
    skos:prefLabel "Conformance Test: http://www.opengis.net/spec/landinfra/part0/1.0/conf/core/gml3.3lro" .

<http://www.opengis.net/spec/landinfra/part0/1.0/conf/core/elements> a spec:ConformanceTest,
        skos:Concept ;
    spec:method "Inspect the GML output to verify the above requirement." ;
    spec:purpose "Verify that the conforming application supports the Core XML elements listed in Table 1 in accordance with the GML XSD specified in http://schemas.opengis.net/infragml/part0/1.0/core.xsd." ;
    skos:definition "Verify that the conforming application supports the Core XML elements listed in Table 1 in accordance with the GML XSD specified in http://schemas.opengis.net/infragml/part0/1.0/core.xsd." ;
    spec:requirement <http://www.opengis.net/spec/landinfra/part0/1.0/req/core/elements> ;
    spec:testType spec:Capabilities ;
    skos:prefLabel "Conformance Test: http://www.opengis.net/spec/landinfra/part0/1.0/conf/core/elements" .

<http://www.opengis.net/spec/landinfra/part0/1.0/req/core/valid> a spec:Requirement ,
skos:Concept ;
skos:definition """Every XML instance document of any Part of InfraGML shall be valid according to the XML grammar specified in that Part for each Requirements Class contained in that Part and available at http://schemas.opengis.net/infragml/part<n>/1.0/<schema name>.xsd where <n> is the Part number and <schema name> is the name of the schema equal to the name of the respective Requirements Class.""" ;
skos:prefLabel "Requirement: /req/core/valid" .

<http://www.opengis.net/spec/landinfra/part0/1.0/req/core/header> a spec:Requirement ,
skos:Concept ;
skos:definition """An InfraGML conforming application shall use a schema definition file which shall contain a properly formed schema header appropriate to the InfraGML Requirements Classes it claims to support.""" ;
skos:prefLabel "Requirement: /req/core/header" .

<http://www.opengis.net/spec/landinfra/part0/1.0/req/core/gml3.2> a spec:Requirement ,
skos:Concept ;
skos:definition """This LandGML standard shall utilize and depend upon the OGC GML 3.2 standard schema within the http://www.opengis.net/gml/3.2 namespace identified by “gml”.""" ;
skos:prefLabel "Requirement: /req/core/gml3.2" .

<http://www.opengis.net/spec/landinfra/part0/1.0/req/core/gml3.3lr> a spec:Requirement ,
skos:Concept ;
skos:definition """This LandGML standard shall utilize and depend upon the OGC GML 3.3 linearRef standard schema within the http://www.opengis.net/gml/3.3/lr namespace identified by “gmllr”.""" ;
skos:prefLabel "Requirement: /req/core/gml3.3lr" .

<http://www.opengis.net/spec/landinfra/part0/1.0/req/core/gml3.3lro> a spec:Requirement ,
skos:Concept ;
skos:definition """This LandGML standard shall utilize and depend upon the OGC GML 3.3 linearRefOffset standard schema within the http://www.opengis.net/gml/3.3/lro namespace identified by “gmllro”.""" ;
skos:prefLabel "Requirement: /req/core/gml3.3lro" .

<http://www.opengis.net/spec/landinfra/part0/1.0/req/core/elements> a spec:Requirement ,
skos:Concept ;
skos:definition """A conforming application shall support the Core XML elements listed in Table 1 in accordance with the GML XSD specified in http://schemas.opengis.net/infragml/part0/1.0/core.xsd.""" ;
skos:prefLabel "Requirement: /req/core/elements" .
