@prefix owl:   <http://www.w3.org/2002/07/owl#> .
@prefix rdf:   <http://www.w3.org/1999/02/22-rdf-syntax-ns#> .
@prefix skos:  <http://www.w3.org/2004/02/skos/core#> .
@prefix dcterms: <http://purl.org/dc/terms/> .
@prefix rdfs:  <http://www.w3.org/2000/01/rdf-schema#> .
@prefix dc:    <http://purl.org/dc/elements/1.1/> .
@prefix prov:  <http://www.w3.org/ns/prov#> .
@prefix status: <http://www.opengis.net/def/status/> .
@prefix policy: <http://www.opengis.net/def/metamodel/ogc-na/> .
@prefix xsd:   <http://www.w3.org/2001/XMLSchema#> .



<http://www.opengis.net/def/sensor-model-param/csmwg>
        a                      skos:ConceptScheme ;
        rdfs:seeAlso           <https://xdomes.org/> ;
        dc:creator              "Community Sensor Model Working Group" ;
        dc:source              "Botts Innovative Research" ;
        dcterms:created        "2019-01-26"^^xsd:date ;

        skos:prefLabel         "Community Sensor Model (CSM) - Parameters" ;
        rdfs:label             "Community Sensor Model (CSM) - Parameters" ;
        policy:collectionView <http://www.opengis.net/def/sensor-model-param/csmwg/>.





<http://www.opengis.net/def/sensor-model-param/csmwg/>
        skos:inScheme             <http://www.opengis.net/def/sensor-model-param/csmwg>;
        rdfs:label "collection view of Community Sensor Model (CSM) - Parameters";
        <http://www.w3.org/2004/02/skos/core#member>  <http://www.opengis.net/def/sensor-model-param/csmwg/DISTOR_A1> , <http://www.opengis.net/def/sensor-model-param/csmwg/PLATFORM_STATE> , <http://www.opengis.net/def/sensor-model-param/csmwg/PLATFORM_ROLL> , <http://www.opengis.net/def/sensor-model-param/csmwg/DISTOR_RAD2> , <http://www.opengis.net/def/sensor-model-param/csmwg/SENSOR_ARRAY_DIMENSIONS> , <http://www.opengis.net/def/sensor-model-param/csmwg/SENSOR_ROTATION> , <http://www.opengis.net/def/sensor-model-param/csmwg/FOCAL_LENGTH_CAL> , <http://www.opengis.net/def/sensor-model-param/csmwg/DISTOR_B2> , <http://www.opengis.net/def/sensor-model-param/csmwg/SENSOR_ROTATION_Y> , <http://www.opengis.net/def/sensor-model-param/csmwg/DISTOR_C2> , <http://www.opengis.net/def/sensor-model-param/csmwg/NCOLS> , <http://www.opengis.net/def/sensor-model-param/csmwg/ROW_AXIS_OFFSET> , <http://www.opengis.net/def/sensor-model-param/csmwg/PLATFORM_TIME> , <http://www.opengis.net/def/sensor-model-param/csmwg/ROW_SPACING> , <http://www.opengis.net/def/sensor-model-param/csmwg/SENSOR_ROTATION_X> , <http://www.opengis.net/def/sensor-model-param/csmwg/FOCAL_LENGTH> , <http://www.opengis.net/def/sensor-model-param/csmwg/PIXELSPACING> , <http://www.opengis.net/def/sensor-model-param/csmwg/SENSOR_TYPE> , <http://www.opengis.net/def/sensor-model-param/csmwg/SENSOR_ROTATION_Z> , <http://www.opengis.net/def/sensor-model-param/csmwg/DISTOR_RAD1> , <http://www.opengis.net/def/sensor-model-param/csmwg/PRIN_OFFSETY> , <http://www.opengis.net/def/sensor-model-param/csmwg/Z_VECTOR_COMPONENT> , <http://www.opengis.net/def/sensor-model-param/csmwg/PLATFORM_TRUEHDG> , <http://www.opengis.net/def/sensor-model-param/csmwg/SENSOR_POSITION> , <http://www.opengis.net/def/sensor-model-param/csmwg/DISTOR_C1> , <http://www.opengis.net/def/sensor-model-param/csmwg/PLATFORM_PITCH> , <http://www.opengis.net/def/sensor-model-param/csmwg/DECEN_LENS> , <http://www.opengis.net/def/sensor-model-param/csmwg/DECEN_LENS2> , <http://www.opengis.net/def/sensor-model-param/csmwg/DISTOR_RAD> , <http://www.opengis.net/def/sensor-model-param/csmwg/DISTOR_A2> , <http://www.opengis.net/def/sensor-model-param/csmwg/PLATFORM_GEOLOC> , <http://www.opengis.net/def/sensor-model-param/csmwg/DISTOR_RAD3> , <http://www.opengis.net/def/sensor-model-param/csmwg/PRIN_OFFSET> , <http://www.opengis.net/def/sensor-model-param/csmwg/COLLECTION_START_TIME> , <http://www.opengis.net/def/sensor-model-param/csmwg/X_VECTOR_COMPONENT> , <http://www.opengis.net/def/sensor-model-param/csmwg/Y_VECTOR_COMPONENT> , <http://www.opengis.net/def/sensor-model-param/csmwg/PRIN_OFFSETX> , <http://www.opengis.net/def/sensor-model-param/csmwg/COL_SPACING> , <http://www.opengis.net/def/sensor-model-param/csmwg/FRAME_PARAMS> , <http://www.opengis.net/def/sensor-model-param/csmwg/DISTOR_B1> , <http://www.opengis.net/def/sensor-model-param/csmwg/PLATFORM_ALTITUDE> , <http://www.opengis.net/def/sensor-model-param/csmwg/AXIS_OFFSET> , <http://www.opengis.net/def/sensor-model-param/csmwg/COL_AXIS_OFFSET> , <http://www.opengis.net/def/sensor-model-param/csmwg/DECEN_LENS1> , <http://www.opengis.net/def/sensor-model-param/csmwg/DISTOR_AFFINE> , <http://www.opengis.net/def/sensor-model-param/csmwg/NROWS> .

<http://www.opengis.net/def/sensor-model-param/csmwg/SENSOR_TYPE> a skos:Concept,prov:Entity;
rdfs:label "Sensor Type" ;
skos:prefLabel "Sensor Type" ;
skos:definition "Classification indicative of the characteristics of the collection device." ;
skos:exactMatch <http://sensorml.com/ont/csm/property/SENSOR_TYPE>;
dcterms:created   "2019-01-15"^^<http://www.w3.org/2001/XMLSchema#date> ;
dcterms:modified  "2019-01-15"^^<http://www.w3.org/2001/XMLSchema#date> ;
prov:hadPrimarySource <http://www.gwg.nga.mil/csmwg.php>;
skos:inScheme     <http://www.opengis.net/def/sensor-model/csmwg/> ;
policy:status     status:valid .

<http://www.opengis.net/def/sensor-model-param/csmwg/SENSOR_ARRAY_DIMENSIONS> a skos:Concept,prov:Entity;
rdfs:label "Sensor Array Dimensions" ;
skos:prefLabel "Sensor Array Dimensions" ;
skos:definition "The number of row and column detection elements in the sensor array." ;
skos:exactMatch <http://sensorml.com/ont/csm/property/SENSOR_ARRAY_DIMENSIONS>;
dcterms:created   "2019-01-15"^^<http://www.w3.org/2001/XMLSchema#date> ;
dcterms:modified  "2019-01-15"^^<http://www.w3.org/2001/XMLSchema#date> ;
prov:hadPrimarySource <http://www.gwg.nga.mil/csmwg.php>;
skos:inScheme     <http://www.opengis.net/def/sensor-model/csmwg/> ;
policy:status     status:valid .

<http://www.opengis.net/def/sensor-model-param/csmwg/NCOLS> a skos:Concept,prov:Entity;
rdfs:label "Number of  Columns in sensor array." ;
skos:prefLabel "Number of  Columns in sensor array." ;
skos:definition "The number of columns in the sensor array. (unitless) " ;
skos:exactMatch <http://sensorml.com/ont/csm/property/NCOLS>;
dcterms:created   "2019-01-15"^^<http://www.w3.org/2001/XMLSchema#date> ;
dcterms:modified  "2019-01-15"^^<http://www.w3.org/2001/XMLSchema#date> ;
prov:hadPrimarySource <http://www.gwg.nga.mil/csmwg.php>;
skos:inScheme     <http://www.opengis.net/def/sensor-model/csmwg/> ;
policy:status     status:valid .

<http://www.opengis.net/def/sensor-model-param/csmwg/NROWS> a skos:Concept,prov:Entity;
rdfs:label "Number of Rows in sensor array." ;
skos:prefLabel "Number of Rows in sensor array." ;
skos:definition "The number of rows in the sensor array. (unitless) " ;
skos:exactMatch <http://sensorml.com/ont/csm/property/NROWS>;
dcterms:created   "2019-01-15"^^<http://www.w3.org/2001/XMLSchema#date> ;
dcterms:modified  "2019-01-15"^^<http://www.w3.org/2001/XMLSchema#date> ;
prov:hadPrimarySource <http://www.gwg.nga.mil/csmwg.php>;
skos:inScheme     <http://www.opengis.net/def/sensor-model/csmwg/> ;
policy:status     status:valid .

<http://www.opengis.net/def/sensor-model-param/csmwg/COLLECTION_START_TIME> a skos:Concept,prov:Entity;
rdfs:label "Collection Start Time" ;
skos:prefLabel "Collection Start Time" ;
skos:definition "The date and time at the start of the sensor activation. " ;
skos:exactMatch <http://sensorml.com/ont/csm/property/COLLECTION_START_TIME>;
dcterms:created   "2019-01-15"^^<http://www.w3.org/2001/XMLSchema#date> ;
dcterms:modified  "2019-01-15"^^<http://www.w3.org/2001/XMLSchema#date> ;
prov:hadPrimarySource <http://www.gwg.nga.mil/csmwg.php>;
skos:inScheme     <http://www.opengis.net/def/sensor-model/csmwg/> ;
policy:status     status:valid .

<http://www.opengis.net/def/sensor-model-param/csmwg/SENSOR_POSITION> a skos:Concept,prov:Entity;
rdfs:label "Sensor Position" ;
skos:prefLabel "Sensor Position" ;
skos:definition "The measurement (in mm) of the vector offset from the origin of the sensor mounting frame, which must be stated (e.g. gimbal, platform, or ECEF coordinate system), to the origin of the sensor perspective center, L. Offset vector describes the position of the sensor perspective center relative to a gimbal position (if any) which, in turn may be referenced to the platform coordinate system; or the offset may be given directly to the platform coordinate system, if known.  Conditional in the case where a sensor may provide position information directly referenced to, say, an ECEF system. " ;
skos:exactMatch <http://sensorml.com/ont/csm/property/SENSOR_POSITION>;
dcterms:created   "2019-01-15"^^<http://www.w3.org/2001/XMLSchema#date> ;
dcterms:modified  "2019-01-15"^^<http://www.w3.org/2001/XMLSchema#date> ;
prov:hadPrimarySource <http://www.gwg.nga.mil/csmwg.php>;
skos:inScheme     <http://www.opengis.net/def/sensor-model/csmwg/> ;
policy:status     status:valid .

<http://www.opengis.net/def/sensor-model-param/csmwg/X_VECTOR_COMPONENT> a skos:Concept,prov:Entity;
rdfs:label "Sensor Position, X Vector Component" ;
skos:prefLabel "Sensor Position, X Vector Component" ;
skos:definition "The x-axis measurement (in mm) of the vector offset from the origin of the sensor mounting frame, which must be stated, e.g. gimbal, platform, or ECEF coordinate system, to the origin of the sensor perspective center, L. " ;
skos:exactMatch <http://sensorml.com/ont/csm/property/X_VECTOR_COMPONENT>;
dcterms:created   "2019-01-15"^^<http://www.w3.org/2001/XMLSchema#date> ;
dcterms:modified  "2019-01-15"^^<http://www.w3.org/2001/XMLSchema#date> ;
prov:hadPrimarySource <http://www.gwg.nga.mil/csmwg.php>;
skos:inScheme     <http://www.opengis.net/def/sensor-model/csmwg/> ;
policy:status     status:valid .

<http://www.opengis.net/def/sensor-model-param/csmwg/Y_VECTOR_COMPONENT> a skos:Concept,prov:Entity;
rdfs:label "Sensor Position, Y Vector Component" ;
skos:prefLabel "Sensor Position, Y Vector Component" ;
skos:definition "The y-axis measurement (in mm) of the vector offset from the origin of the sensor mounting frame, which must be stated (e.g. gimbal, platform, or ECEF coordinate system), to the origin of the sensor perspective center, L. " ;
skos:exactMatch <http://sensorml.com/ont/csm/property/Y_VECTOR_COMPONENT>;
dcterms:created   "2019-01-15"^^<http://www.w3.org/2001/XMLSchema#date> ;
dcterms:modified  "2019-01-15"^^<http://www.w3.org/2001/XMLSchema#date> ;
prov:hadPrimarySource <http://www.gwg.nga.mil/csmwg.php>;
skos:inScheme     <http://www.opengis.net/def/sensor-model/csmwg/> ;
policy:status     status:valid .

<http://www.opengis.net/def/sensor-model-param/csmwg/Z_VECTOR_COMPONENT> a skos:Concept,prov:Entity;
rdfs:label "Sensor Position, Z Vector Component" ;
skos:prefLabel "Sensor Position, Z Vector Component" ;
skos:definition "The z-axis measurement (in mm) of the vector offset from the origin of the sensor mounting frame, which must be stated (e.g. gimbal, platform, or ECEF coordinate system), to the origin of the sensor perspective center, L. " ;
skos:exactMatch <http://sensorml.com/ont/csm/property/Z_VECTOR_COMPONENT>;
dcterms:created   "2019-01-15"^^<http://www.w3.org/2001/XMLSchema#date> ;
dcterms:modified  "2019-01-15"^^<http://www.w3.org/2001/XMLSchema#date> ;
prov:hadPrimarySource <http://www.gwg.nga.mil/csmwg.php>;
skos:inScheme     <http://www.opengis.net/def/sensor-model/csmwg/> ;
policy:status     status:valid .

<http://www.opengis.net/def/sensor-model-param/csmwg/SENSOR_ROTATION> a skos:Concept,prov:Entity;
rdfs:label "Sensor Rotation" ;
skos:prefLabel "Sensor Rotation" ;
skos:definition "Rotation of the sensor relative to a specified reference system.  If these rotation angles are gimbal mounting angles, this development transforms them into the required sequential Euler angles. Reference may be made to gimbal mounting or to platform reference system; but must be specified.  If these rotation angles are gimbal mounting angles, this development transforms them into the required sequential Euler angles. " ;
skos:exactMatch <http://sensorml.com/ont/csm/property/SENSOR_ROTATION>;
dcterms:created   "2019-01-15"^^<http://www.w3.org/2001/XMLSchema#date> ;
dcterms:modified  "2019-01-15"^^<http://www.w3.org/2001/XMLSchema#date> ;
prov:hadPrimarySource <http://www.gwg.nga.mil/csmwg.php>;
skos:inScheme     <http://www.opengis.net/def/sensor-model/csmwg/> ;
policy:status     status:valid .

<http://www.opengis.net/def/sensor-model-param/csmwg/SENSOR_ROTATION_X> a skos:Concept,prov:Entity;
rdfs:label "Sensor Rotation about X-axis" ;
skos:prefLabel "Sensor Rotation about X-axis" ;
skos:definition "Rotation of the sensor in the yz-plane of the sensor reference frame; positive when positive +z-axis rotates directly towards +y-axis. (radians) " ;
skos:exactMatch <http://sensorml.com/ont/csm/property/SENSOR_ROTATION_X>;
dcterms:created   "2019-01-15"^^<http://www.w3.org/2001/XMLSchema#date> ;
dcterms:modified  "2019-01-15"^^<http://www.w3.org/2001/XMLSchema#date> ;
prov:hadPrimarySource <http://www.gwg.nga.mil/csmwg.php>;
skos:inScheme     <http://www.opengis.net/def/sensor-model/csmwg/> ;
policy:status     status:valid .

<http://www.opengis.net/def/sensor-model-param/csmwg/SENSOR_ROTATION_Y> a skos:Concept,prov:Entity;
rdfs:label "Sensor Rotation about X-axis" ;
skos:prefLabel "Sensor Rotation about X-axis" ;
skos:definition "Rotation of the sensor in the xz-plane of the sensor reference frame; positive when positive +z-axis rotates directly towards +x-axis. (radians) " ;
skos:exactMatch <http://sensorml.com/ont/csm/property/SENSOR_ROTATION_Y>;
dcterms:created   "2019-01-15"^^<http://www.w3.org/2001/XMLSchema#date> ;
dcterms:modified  "2019-01-15"^^<http://www.w3.org/2001/XMLSchema#date> ;
prov:hadPrimarySource <http://www.gwg.nga.mil/csmwg.php>;
skos:inScheme     <http://www.opengis.net/def/sensor-model/csmwg/> ;
policy:status     status:valid .

<http://www.opengis.net/def/sensor-model-param/csmwg/SENSOR_ROTATION_Z> a skos:Concept,prov:Entity;
rdfs:label "Sensor Rotation about X-axis" ;
skos:prefLabel "Sensor Rotation about X-axis" ;
skos:definition "Rotation of the sensor in the xy-plane of the sensor reference frame; positive when positive +x-axis rotates directly towards +y-axis. (radians) " ;
skos:exactMatch <http://sensorml.com/ont/csm/property/SENSOR_ROTATION_Z>;
dcterms:created   "2019-01-15"^^<http://www.w3.org/2001/XMLSchema#date> ;
dcterms:modified  "2019-01-15"^^<http://www.w3.org/2001/XMLSchema#date> ;
prov:hadPrimarySource <http://www.gwg.nga.mil/csmwg.php>;
skos:inScheme     <http://www.opengis.net/def/sensor-model/csmwg/> ;
policy:status     status:valid .

<http://www.opengis.net/def/sensor-model-param/csmwg/FOCAL_LENGTH> a skos:Concept,prov:Entity;
rdfs:label "Sensor Focal Length" ;
skos:prefLabel "Sensor Focal Length" ;
skos:definition "f, lens focal length; effective distance from optical lens to sensor array. " ;
skos:exactMatch <http://sensorml.com/ont/csm/property/FOCAL_LENGTH>;
dcterms:created   "2019-01-15"^^<http://www.w3.org/2001/XMLSchema#date> ;
dcterms:modified  "2019-01-15"^^<http://www.w3.org/2001/XMLSchema#date> ;
prov:hadPrimarySource <http://www.gwg.nga.mil/csmwg.php>;
skos:inScheme     <http://www.opengis.net/def/sensor-model/csmwg/> ;
policy:status     status:valid .

<http://www.opengis.net/def/sensor-model-param/csmwg/FOCAL_LENGTH_CAL> a skos:Concept,prov:Entity;
rdfs:label "Sensor Calibrated Focal Length (mm); corrected effective distance from optical lens to sensor array. " ;
skos:prefLabel "Sensor Calibrated Focal Length (mm); corrected effective distance from optical lens to sensor array. " ;
skos:definition "Lens calibrated focal length, f, " ;
skos:exactMatch <http://sensorml.com/ont/csm/property/FOCAL_LENGTH_CAL>;
dcterms:created   "2019-01-15"^^<http://www.w3.org/2001/XMLSchema#date> ;
dcterms:modified  "2019-01-15"^^<http://www.w3.org/2001/XMLSchema#date> ;
prov:hadPrimarySource <http://www.gwg.nga.mil/csmwg.php>;
skos:inScheme     <http://www.opengis.net/def/sensor-model/csmwg/> ;
policy:status     status:valid .

<http://www.opengis.net/def/sensor-model-param/csmwg/PRIN_OFFSET> a skos:Concept,prov:Entity;
rdfs:label "Principal Point Offset" ;
skos:prefLabel "Principal Point Offset" ;
skos:definition "Principal point coordinate offset within the sensor array  coordinate system of the foot of the perpendicular dropped from sensor perspective center of the camera lens onto the collection array. (mm). " ;
skos:exactMatch <http://sensorml.com/ont/csm/property/PRIN_OFFSET>;
dcterms:created   "2019-01-15"^^<http://www.w3.org/2001/XMLSchema#date> ;
dcterms:modified  "2019-01-15"^^<http://www.w3.org/2001/XMLSchema#date> ;
prov:hadPrimarySource <http://www.gwg.nga.mil/csmwg.php>;
skos:inScheme     <http://www.opengis.net/def/sensor-model/csmwg/> ;
policy:status     status:valid .

<http://www.opengis.net/def/sensor-model-param/csmwg/PRIN_OFFSETX> a skos:Concept,prov:Entity;
rdfs:label "Principal Point Offset, x-axis" ;
skos:prefLabel "Principal Point Offset, x-axis" ;
skos:definition "x0: x-coordinate within the sensor array  coordinate system of the foot of the perpendicular dropped from sensor perspective center of the camera lens onto the collection array. (mm). " ;
skos:exactMatch <http://sensorml.com/ont/csm/property/PRIN_OFFSETX>;
dcterms:created   "2019-01-15"^^<http://www.w3.org/2001/XMLSchema#date> ;
dcterms:modified  "2019-01-15"^^<http://www.w3.org/2001/XMLSchema#date> ;
prov:hadPrimarySource <http://www.gwg.nga.mil/csmwg.php>;
skos:inScheme     <http://www.opengis.net/def/sensor-model/csmwg/> ;
policy:status     status:valid .

<http://www.opengis.net/def/sensor-model-param/csmwg/PRIN_OFFSETY> a skos:Concept,prov:Entity;
rdfs:label "Principal Point Offset, y-axis" ;
skos:prefLabel "Principal Point Offset, y-axis" ;
skos:definition "y0: y-coordinate within the sensor array  coordinate system of the foot of the perpendicular dropped from sensor perspective center of the camera lens onto the collection array. (mm). " ;
skos:exactMatch <http://sensorml.com/ont/csm/property/PRIN_OFFSETY>;
dcterms:created   "2019-01-15"^^<http://www.w3.org/2001/XMLSchema#date> ;
dcterms:modified  "2019-01-15"^^<http://www.w3.org/2001/XMLSchema#date> ;
prov:hadPrimarySource <http://www.gwg.nga.mil/csmwg.php>;
skos:inScheme     <http://www.opengis.net/def/sensor-model/csmwg/> ;
policy:status     status:valid .

<http://www.opengis.net/def/sensor-model-param/csmwg/PIXELSPACING> a skos:Concept,prov:Entity;
rdfs:label "Pixel Spacing" ;
skos:prefLabel "Pixel Spacing" ;
skos:definition "Distance between pixels at the center of the image. Can use angular or linear measurement methods" ;
skos:exactMatch <http://sensorml.com/ont/csm/property/PIXELSPACING>;
dcterms:created   "2019-01-15"^^<http://www.w3.org/2001/XMLSchema#date> ;
dcterms:modified  "2019-01-15"^^<http://www.w3.org/2001/XMLSchema#date> ;
prov:hadPrimarySource <http://www.gwg.nga.mil/csmwg.php>;
skos:inScheme     <http://www.opengis.net/def/sensor-model/csmwg/> ;
policy:status     status:valid .

<http://www.opengis.net/def/sensor-model-param/csmwg/COL_SPACING> a skos:Concept,prov:Entity;
rdfs:label "Column Spacing" ;
skos:prefLabel "Column Spacing" ;
skos:definition "Column spacing, dy, measured at the center of the image; distance in the image plane between adjacent pixels within a row. " ;
skos:exactMatch <http://sensorml.com/ont/csm/property/COL_SPACING>;
dcterms:created   "2019-01-15"^^<http://www.w3.org/2001/XMLSchema#date> ;
dcterms:modified  "2019-01-15"^^<http://www.w3.org/2001/XMLSchema#date> ;
prov:hadPrimarySource <http://www.gwg.nga.mil/csmwg.php>;
skos:inScheme     <http://www.opengis.net/def/sensor-model/csmwg/> ;
policy:status     status:valid .

<http://www.opengis.net/def/sensor-model-param/csmwg/ROW_SPACING> a skos:Concept,prov:Entity;
rdfs:label "Row Spacing" ;
skos:prefLabel "Row Spacing" ;
skos:definition "Row spacing, dx, measured at the center of the image; distance in the image plane between corresponding pixels of adjacent columns. " ;
skos:exactMatch <http://sensorml.com/ont/csm/property/ROW_SPACING>;
dcterms:created   "2019-01-15"^^<http://www.w3.org/2001/XMLSchema#date> ;
dcterms:modified  "2019-01-15"^^<http://www.w3.org/2001/XMLSchema#date> ;
prov:hadPrimarySource <http://www.gwg.nga.mil/csmwg.php>;
skos:inScheme     <http://www.opengis.net/def/sensor-model/csmwg/> ;
policy:status     status:valid .

<http://www.opengis.net/def/sensor-model-param/csmwg/AXIS_OFFSET> a skos:Concept,prov:Entity;
rdfs:label "Axis Offset" ;
skos:prefLabel "Axis Offset" ;
skos:definition "Linear translation from the image upper-left corner pixel to the collection array origin (mm)." ;
skos:exactMatch <http://sensorml.com/ont/csm/property/AXIS_OFFSET>;
dcterms:created   "2019-01-15"^^<http://www.w3.org/2001/XMLSchema#date> ;
dcterms:modified  "2019-01-15"^^<http://www.w3.org/2001/XMLSchema#date> ;
prov:hadPrimarySource <http://www.gwg.nga.mil/csmwg.php>;
skos:inScheme     <http://www.opengis.net/def/sensor-model/csmwg/> ;
policy:status     status:valid .

<http://www.opengis.net/def/sensor-model-param/csmwg/COL_AXIS_OFFSET> a skos:Concept,prov:Entity;
rdfs:label "Column Axis Offset" ;
skos:prefLabel "Column Axis Offset" ;
skos:definition "Cl, linear translation from the image upper-left corner pixel to the collection array origin (mm), s-axis " ;
skos:exactMatch <http://sensorml.com/ont/csm/property/COL_AXIS_OFFSET>;
dcterms:created   "2019-01-15"^^<http://www.w3.org/2001/XMLSchema#date> ;
dcterms:modified  "2019-01-15"^^<http://www.w3.org/2001/XMLSchema#date> ;
prov:hadPrimarySource <http://www.gwg.nga.mil/csmwg.php>;
skos:inScheme     <http://www.opengis.net/def/sensor-model/csmwg/> ;
policy:status     status:valid .

<http://www.opengis.net/def/sensor-model-param/csmwg/ROW_AXIS_OFFSET> a skos:Concept,prov:Entity;
rdfs:label "Row Axis Offset" ;
skos:prefLabel "Row Axis Offset" ;
skos:definition "Cs,  linear translation from the image upper-left corner pixel to the to collection array origin (mm), l-axis " ;
skos:exactMatch <http://sensorml.com/ont/csm/property/ROW_AXIS_OFFSET>;
dcterms:created   "2019-01-15"^^<http://www.w3.org/2001/XMLSchema#date> ;
dcterms:modified  "2019-01-15"^^<http://www.w3.org/2001/XMLSchema#date> ;
prov:hadPrimarySource <http://www.gwg.nga.mil/csmwg.php>;
skos:inScheme     <http://www.opengis.net/def/sensor-model/csmwg/> ;
policy:status     status:valid .

<http://www.opengis.net/def/sensor-model-param/csmwg/DISTOR_RAD> a skos:Concept,prov:Entity;
rdfs:label "Lens Radial Distortion Coefficients" ;
skos:prefLabel "Lens Radial Distortion Coefficients" ;
skos:definition "Coefficients for describing radial distortion of lenses. Coefficients are typically applied to the third, fifth, and seventh order products of the radial distance from lens center. Include k1 (mm^-2), k2 (mm^-4), and k3 (mm^-6)." ;
skos:exactMatch <http://sensorml.com/ont/csm/property/DISTOR_RAD>;
dcterms:created   "2019-01-15"^^<http://www.w3.org/2001/XMLSchema#date> ;
dcterms:modified  "2019-01-15"^^<http://www.w3.org/2001/XMLSchema#date> ;
prov:hadPrimarySource <http://www.gwg.nga.mil/csmwg.php>;
skos:inScheme     <http://www.opengis.net/def/sensor-model/csmwg/> ;
policy:status     status:valid .

<http://www.opengis.net/def/sensor-model-param/csmwg/DISTOR_RAD1> a skos:Concept,prov:Entity;
rdfs:label "Third-order Lens Radial Distortion Coefficient, k1" ;
skos:prefLabel "Third-order Lens Radial Distortion Coefficient, k1" ;
skos:definition "k1 (mm^-2) coefficient for describing radial distortion of lenses. Applied to the third order product of the radial distance from lens center. " ;
skos:exactMatch <http://sensorml.com/ont/csm/property/DISTOR_RAD1>;
dcterms:created   "2019-01-15"^^<http://www.w3.org/2001/XMLSchema#date> ;
dcterms:modified  "2019-01-15"^^<http://www.w3.org/2001/XMLSchema#date> ;
prov:hadPrimarySource <http://www.gwg.nga.mil/csmwg.php>;
skos:inScheme     <http://www.opengis.net/def/sensor-model/csmwg/> ;
policy:status     status:valid .

<http://www.opengis.net/def/sensor-model-param/csmwg/DISTOR_RAD2> a skos:Concept,prov:Entity;
rdfs:label "Fifth-order Lens Radial Distortion Coefficient, k2" ;
skos:prefLabel "Fifth-order Lens Radial Distortion Coefficient, k2" ;
skos:definition "k2 (mm^-4) coefficient for describing radial distortion of lenses. Applied to the fifth order product of the radial distance from lens center. " ;
skos:exactMatch <http://sensorml.com/ont/csm/property/DISTOR_RAD2>;
dcterms:created   "2019-01-15"^^<http://www.w3.org/2001/XMLSchema#date> ;
dcterms:modified  "2019-01-15"^^<http://www.w3.org/2001/XMLSchema#date> ;
prov:hadPrimarySource <http://www.gwg.nga.mil/csmwg.php>;
skos:inScheme     <http://www.opengis.net/def/sensor-model/csmwg/> ;
policy:status     status:valid .

<http://www.opengis.net/def/sensor-model-param/csmwg/DISTOR_RAD3> a skos:Concept,prov:Entity;
rdfs:label "Seventh-order Lens Radial Distortion Coefficient, k3" ;
skos:prefLabel "Seventh-order Lens Radial Distortion Coefficient, k3" ;
skos:definition "k3 (mm^-6) coefficient for describing radial distortion of lenses. Applied to the seventh order product of the radial distance from lens center. " ;
skos:exactMatch <http://sensorml.com/ont/csm/property/DISTOR_RAD3>;
dcterms:created   "2019-01-15"^^<http://www.w3.org/2001/XMLSchema#date> ;
dcterms:modified  "2019-01-15"^^<http://www.w3.org/2001/XMLSchema#date> ;
prov:hadPrimarySource <http://www.gwg.nga.mil/csmwg.php>;
skos:inScheme     <http://www.opengis.net/def/sensor-model/csmwg/> ;
policy:status     status:valid .

<http://www.opengis.net/def/sensor-model-param/csmwg/DECEN_LENS> a skos:Concept,prov:Entity;
rdfs:label "Decentering Lens Correction Coefficient" ;
skos:prefLabel "Decentering Lens Correction Coefficient" ;
skos:definition "Coefficients for describing rotational asymmetry within a lens system; Include p1 and p2" ;
skos:exactMatch <http://sensorml.com/ont/csm/property/DECEN_LENS>;
dcterms:created   "2019-01-15"^^<http://www.w3.org/2001/XMLSchema#date> ;
dcterms:modified  "2019-01-15"^^<http://www.w3.org/2001/XMLSchema#date> ;
prov:hadPrimarySource <http://www.gwg.nga.mil/csmwg.php>;
skos:inScheme     <http://www.opengis.net/def/sensor-model/csmwg/> ;
policy:status     status:valid .

<http://www.opengis.net/def/sensor-model-param/csmwg/DECEN_LENS1> a skos:Concept,prov:Entity;
rdfs:label "First Decentering Lens Correction Coefficient, p1" ;
skos:prefLabel "First Decentering Lens Correction Coefficient, p1" ;
skos:definition "First coefficient for describing rotational asymmetry within a lens system; (mm^-1). p1" ;
skos:exactMatch <http://sensorml.com/ont/csm/property/DECEN_LENS1>;
dcterms:created   "2019-01-15"^^<http://www.w3.org/2001/XMLSchema#date> ;
dcterms:modified  "2019-01-15"^^<http://www.w3.org/2001/XMLSchema#date> ;
prov:hadPrimarySource <http://www.gwg.nga.mil/csmwg.php>;
skos:inScheme     <http://www.opengis.net/def/sensor-model/csmwg/> ;
policy:status     status:valid .

<http://www.opengis.net/def/sensor-model-param/csmwg/DECEN_LENS2> a skos:Concept,prov:Entity;
rdfs:label "Second Decentering Lens Correction Coefficient, p2" ;
skos:prefLabel "Second Decentering Lens Correction Coefficient, p2" ;
skos:definition "Second coefficient for describing rotational asymmetry within a lens system; (mm^-1). p2" ;
skos:exactMatch <http://sensorml.com/ont/csm/property/DECEN_LENS2>;
dcterms:created   "2019-01-15"^^<http://www.w3.org/2001/XMLSchema#date> ;
dcterms:modified  "2019-01-15"^^<http://www.w3.org/2001/XMLSchema#date> ;
prov:hadPrimarySource <http://www.gwg.nga.mil/csmwg.php>;
skos:inScheme     <http://www.opengis.net/def/sensor-model/csmwg/> ;
policy:status     status:valid .

<http://www.opengis.net/def/sensor-model-param/csmwg/DISTOR_AFFINE> a skos:Concept,prov:Entity;
rdfs:label "Affine Distortion Coefficients" ;
skos:prefLabel "Affine Distortion Coefficients" ;
skos:definition "Affine distortion coefficients used to define scaling, rotation, skew, and shift distortions in lenses." ;
skos:exactMatch <http://sensorml.com/ont/csm/property/DISTOR_AFFINE>;
dcterms:created   "2019-01-15"^^<http://www.w3.org/2001/XMLSchema#date> ;
dcterms:modified  "2019-01-15"^^<http://www.w3.org/2001/XMLSchema#date> ;
prov:hadPrimarySource <http://www.gwg.nga.mil/csmwg.php>;
skos:inScheme     <http://www.opengis.net/def/sensor-model/csmwg/> ;
policy:status     status:valid .

<http://www.opengis.net/def/sensor-model-param/csmwg/DISTOR_A1> a skos:Concept,prov:Entity;
rdfs:label "Affine Distortion Coefficients, A1" ;
skos:prefLabel "Affine Distortion Coefficients, A1" ;
skos:definition "Affine distortion coefficient, A1, used to define scaling, rotation, skew, and shift distortions in lenses." ;
skos:exactMatch <http://sensorml.com/ont/csm/property/DISTOR_A1>;
dcterms:created   "2019-01-15"^^<http://www.w3.org/2001/XMLSchema#date> ;
dcterms:modified  "2019-01-15"^^<http://www.w3.org/2001/XMLSchema#date> ;
prov:hadPrimarySource <http://www.gwg.nga.mil/csmwg.php>;
skos:inScheme     <http://www.opengis.net/def/sensor-model/csmwg/> ;
policy:status     status:valid .

<http://www.opengis.net/def/sensor-model-param/csmwg/DISTOR_A2> a skos:Concept,prov:Entity;
rdfs:label "Affine Distortion Coefficients, A2" ;
skos:prefLabel "Affine Distortion Coefficients, A2" ;
skos:definition "Affine distortion coefficient, A2, used to define scaling, rotation, skew, and shift distortions in lenses." ;
skos:exactMatch <http://sensorml.com/ont/csm/property/DISTOR_A2>;
dcterms:created   "2019-01-15"^^<http://www.w3.org/2001/XMLSchema#date> ;
dcterms:modified  "2019-01-15"^^<http://www.w3.org/2001/XMLSchema#date> ;
prov:hadPrimarySource <http://www.gwg.nga.mil/csmwg.php>;
skos:inScheme     <http://www.opengis.net/def/sensor-model/csmwg/> ;
policy:status     status:valid .

<http://www.opengis.net/def/sensor-model-param/csmwg/DISTOR_B1> a skos:Concept,prov:Entity;
rdfs:label "Affine Distortion Coefficients, B1" ;
skos:prefLabel "Affine Distortion Coefficients, B1" ;
skos:definition "Affine distortion coefficient, B1, used to define scaling, rotation, skew, and shift distortions in lenses." ;
skos:exactMatch <http://sensorml.com/ont/csm/property/DISTOR_B1>;
dcterms:created   "2019-01-15"^^<http://www.w3.org/2001/XMLSchema#date> ;
dcterms:modified  "2019-01-15"^^<http://www.w3.org/2001/XMLSchema#date> ;
prov:hadPrimarySource <http://www.gwg.nga.mil/csmwg.php>;
skos:inScheme     <http://www.opengis.net/def/sensor-model/csmwg/> ;
policy:status     status:valid .

<http://www.opengis.net/def/sensor-model-param/csmwg/DISTOR_B2> a skos:Concept,prov:Entity;
rdfs:label "Affine Distortion Coefficients, B2" ;
skos:prefLabel "Affine Distortion Coefficients, B2" ;
skos:definition "Affine distortion coefficient, B2, used to define scaling, rotation, skew, and shift distortions in lenses." ;
skos:exactMatch <http://sensorml.com/ont/csm/property/DISTOR_B2>;
dcterms:created   "2019-01-15"^^<http://www.w3.org/2001/XMLSchema#date> ;
dcterms:modified  "2019-01-15"^^<http://www.w3.org/2001/XMLSchema#date> ;
prov:hadPrimarySource <http://www.gwg.nga.mil/csmwg.php>;
skos:inScheme     <http://www.opengis.net/def/sensor-model/csmwg/> ;
policy:status     status:valid .

<http://www.opengis.net/def/sensor-model-param/csmwg/DISTOR_C1> a skos:Concept,prov:Entity;
rdfs:label "Affine Distortion Coefficients, C1" ;
skos:prefLabel "Affine Distortion Coefficients, C1" ;
skos:definition "Affine distortion coefficient, C1, used to define scaling, rotation, skew, and shift distortions in lenses." ;
skos:exactMatch <http://sensorml.com/ont/csm/property/DISTOR_C1>;
dcterms:created   "2019-01-15"^^<http://www.w3.org/2001/XMLSchema#date> ;
dcterms:modified  "2019-01-15"^^<http://www.w3.org/2001/XMLSchema#date> ;
prov:hadPrimarySource <http://www.gwg.nga.mil/csmwg.php>;
skos:inScheme     <http://www.opengis.net/def/sensor-model/csmwg/> ;
policy:status     status:valid .

<http://www.opengis.net/def/sensor-model-param/csmwg/DISTOR_C2> a skos:Concept,prov:Entity;
rdfs:label "Affine Distortion Coefficients, C2" ;
skos:prefLabel "Affine Distortion Coefficients, C2" ;
skos:definition "Affine distortion coefficient, C2, used to define scaling, rotation, skew, and shift distortions in lenses." ;
skos:exactMatch <http://sensorml.com/ont/csm/property/DISTOR_C2>;
dcterms:created   "2019-01-15"^^<http://www.w3.org/2001/XMLSchema#date> ;
dcterms:modified  "2019-01-15"^^<http://www.w3.org/2001/XMLSchema#date> ;
prov:hadPrimarySource <http://www.gwg.nga.mil/csmwg.php>;
skos:inScheme     <http://www.opengis.net/def/sensor-model/csmwg/> ;
policy:status     status:valid .

<http://www.opengis.net/def/sensor-model-param/csmwg/PLATFORM_STATE> a skos:Concept,prov:Entity;
rdfs:label "Platform State" ;
skos:prefLabel "Platform State" ;
skos:definition "The position, orientation, and velocity state of a platform at any particulr time." ;
skos:exactMatch <http://sensorml.com/ont/csm/property/PLATFORM_STATE>;
dcterms:created   "2019-01-15"^^<http://www.w3.org/2001/XMLSchema#date> ;
dcterms:modified  "2019-01-15"^^<http://www.w3.org/2001/XMLSchema#date> ;
prov:hadPrimarySource <http://www.gwg.nga.mil/csmwg.php>;
skos:inScheme     <http://www.opengis.net/def/sensor-model/csmwg/> ;
policy:status     status:valid .

<http://www.opengis.net/def/sensor-model-param/csmwg/PLATFORM_TIME> a skos:Concept,prov:Entity;
rdfs:label "Platform Time" ;
skos:prefLabel "Platform Time" ;
skos:definition "Time at which data about the platform state was collected." ;
skos:exactMatch <http://sensorml.com/ont/csm/property/PLATFORM_TIME>;
dcterms:created   "2019-01-15"^^<http://www.w3.org/2001/XMLSchema#date> ;
dcterms:modified  "2019-01-15"^^<http://www.w3.org/2001/XMLSchema#date> ;
prov:hadPrimarySource <http://www.gwg.nga.mil/csmwg.php>;
skos:inScheme     <http://www.opengis.net/def/sensor-model/csmwg/> ;
policy:status     status:valid .

<http://www.opengis.net/def/sensor-model-param/csmwg/PLATFORM_GEOLOC> a skos:Concept,prov:Entity;
rdfs:label "Platform Geolocation" ;
skos:prefLabel "Platform Geolocation" ;
skos:definition "The position of the platform given as latitude and longitude (radians)." ;
skos:exactMatch <http://sensorml.com/ont/csm/property/PLATFORM_GEOLOC>;
dcterms:created   "2019-01-15"^^<http://www.w3.org/2001/XMLSchema#date> ;
dcterms:modified  "2019-01-15"^^<http://www.w3.org/2001/XMLSchema#date> ;
prov:hadPrimarySource <http://www.gwg.nga.mil/csmwg.php>;
skos:inScheme     <http://www.opengis.net/def/sensor-model/csmwg/> ;
policy:status     status:valid .

<http://www.opengis.net/def/sensor-model-param/csmwg/PLATFORM_ALTITUDE> a skos:Concept,prov:Entity;
rdfs:label "Platform Altitude" ;
skos:prefLabel "Platform Altitude" ;
skos:definition "Platform altitude (ft or m) specified above a specified reference at image acquisition time." ;
skos:exactMatch <http://sensorml.com/ont/csm/property/PLATFORM_ALTITUDE>;
dcterms:created   "2019-01-15"^^<http://www.w3.org/2001/XMLSchema#date> ;
dcterms:modified  "2019-01-15"^^<http://www.w3.org/2001/XMLSchema#date> ;
prov:hadPrimarySource <http://www.gwg.nga.mil/csmwg.php>;
skos:inScheme     <http://www.opengis.net/def/sensor-model/csmwg/> ;
policy:status     status:valid .

<http://www.opengis.net/def/sensor-model-param/csmwg/PLATFORM_TRUEHDG> a skos:Concept,prov:Entity;
rdfs:label "Platform True-Heading at Scan Line Time" ;
skos:prefLabel "Platform True-Heading at Scan Line Time" ;
skos:definition "Platform heading relative to true north (positive from north to east)." ;
skos:exactMatch <http://sensorml.com/ont/csm/property/PLATFORM_TRUEHDG>;
dcterms:created   "2019-01-15"^^<http://www.w3.org/2001/XMLSchema#date> ;
dcterms:modified  "2019-01-15"^^<http://www.w3.org/2001/XMLSchema#date> ;
prov:hadPrimarySource <http://www.gwg.nga.mil/csmwg.php>;
skos:inScheme     <http://www.opengis.net/def/sensor-model/csmwg/> ;
policy:status     status:valid .

<http://www.opengis.net/def/sensor-model-param/csmwg/PLATFORM_PITCH> a skos:Concept,prov:Entity;
rdfs:label "Platform Pitch" ;
skos:prefLabel "Platform Pitch" ;
skos:definition "Rotation about platform local y-axis (Ya), positive nose-up; 0.0 = platform z-axis (Za) aligned to Nadir, limited to values between +/-90degrees. " ;
skos:exactMatch <http://sensorml.com/ont/csm/property/PLATFORM_PITCH>;
dcterms:created   "2019-01-15"^^<http://www.w3.org/2001/XMLSchema#date> ;
dcterms:modified  "2019-01-15"^^<http://www.w3.org/2001/XMLSchema#date> ;
prov:hadPrimarySource <http://www.gwg.nga.mil/csmwg.php>;
skos:inScheme     <http://www.opengis.net/def/sensor-model/csmwg/> ;
policy:status     status:valid .

<http://www.opengis.net/def/sensor-model-param/csmwg/PLATFORM_ROLL> a skos:Concept,prov:Entity;
rdfs:label "Platform Roll" ;
skos:prefLabel "Platform Roll" ;
skos:definition "Rotation about platform local x-axis (Xa). Positive port wing up (degrees)." ;
skos:exactMatch <http://sensorml.com/ont/csm/property/PLATFORM_ROLL>;
dcterms:created   "2019-01-15"^^<http://www.w3.org/2001/XMLSchema#date> ;
dcterms:modified  "2019-01-15"^^<http://www.w3.org/2001/XMLSchema#date> ;
prov:hadPrimarySource <http://www.gwg.nga.mil/csmwg.php>;
skos:inScheme     <http://www.opengis.net/def/sensor-model/csmwg/> ;
policy:status     status:valid .

<http://www.opengis.net/def/sensor-model-param/csmwg/FRAME_PARAMS> a skos:Concept,prov:Entity;
rdfs:label "Frame Camera Parameters" ;
skos:prefLabel "Frame Camera Parameters" ;
skos:definition "Parameters used to define the properties of a frame camera, including distortions and imperfections, required to provide precise geolocation of imagery from that sensor." ;
skos:exactMatch <http://sensorml.com/ont/csm/property/FRAME_PARAMS>;
dcterms:created   "2019-01-15"^^<http://www.w3.org/2001/XMLSchema#date> ;
dcterms:modified  "2019-01-15"^^<http://www.w3.org/2001/XMLSchema#date> ;
prov:hadPrimarySource <http://www.gwg.nga.mil/csmwg.php>;
skos:inScheme     <http://www.opengis.net/def/sensor-model/csmwg/> ;
policy:status     status:valid .
