<?xml version="1.0" encoding="UTF-8"?>
<rdf:RDF
   xmlns:adms="http://www.w3.org/ns/adms#"
   xmlns:dcat="http://www.w3.org/ns/dcat#"
   xmlns:dct="http://purl.org/dc/terms/"
   xmlns:na="http://www.opengis.net/def/metamodel/ogc-na/"
   xmlns:prov="http://www.w3.org/ns/prov#"
   xmlns:rdf="http://www.w3.org/1999/02/22-rdf-syntax-ns#"
   xmlns:reg="http://purl.org/linked-data/registry#"
   xmlns:skos="http://www.w3.org/2004/02/skos/core#"
   xmlns:spec="http://www.opengis.net/def/ont/modspec/"
   xmlns:specrel="http://www.opengis.net/def/ont/specrel/"
>
  <rdf:Description rdf:about="http://www.opengis.net/spec/landinfra/part0/1.0/req/core/gml3.3lr">
    <rdf:type rdf:resource="http://www.opengis.net/def/ont/modspec/Requirement"/>
    <rdf:type rdf:resource="http://www.w3.org/2004/02/skos/core#Concept"/>
    <skos:broader rdf:resource="http://www.opengis.net/spec/landinfra/part0/1.0/conf/core/gml3.3lr"/>
    <skos:broader rdf:resource="http://www.opengis.net/spec/landinfra/part0/1.0/req/core"/>
    <skos:prefLabel>Requirement: /req/core/gml3.3lr</skos:prefLabel>
    <skos:definition>This LandGML standard shall utilize and depend upon the OGC GML 3.3 linearRef standard schema within the http://www.opengis.net/gml/3.3/lr namespace identified by “gmllr”.</skos:definition>
  </rdf:Description>
  <rdf:Description rdf:about="http://www.opengis.net/spec/landinfra/part0/1.0/conf/core/gml3.3lro">
    <skos:definition>Verify that the conforming application utilizes and depends upon the OGC GML 3.3 linearRefOffset standard schema within the http://www.opengis.net/gml/3.3/lro namespace identified by 'gmllro'.</skos:definition>
    <spec:requirement rdf:resource="http://www.opengis.net/spec/landinfra/part0/1.0/req/core/gml3.3lro"/>
    <rdf:type rdf:resource="http://www.opengis.net/def/ont/modspec/ConformanceTest"/>
    <rdf:type rdf:resource="http://www.w3.org/2004/02/skos/core#Concept"/>
    <spec:testType rdf:resource="http://www.opengis.net/def/ont/modspec/Capabilities"/>
    <skos:prefLabel>Conformance Test: http://www.opengis.net/spec/landinfra/part0/1.0/conf/core/gml3.3lro</skos:prefLabel>
    <skos:narrower rdf:resource="http://www.opengis.net/spec/landinfra/part0/1.0/req/core/gml3.3lro"/>
    <spec:purpose>Verify that the conforming application utilizes and depends upon the OGC GML 3.3 linearRefOffset standard schema within the http://www.opengis.net/gml/3.3/lro namespace identified by 'gmllro'.</spec:purpose>
    <skos:broader rdf:resource="http://www.opengis.net/spec/landinfra/part0/1.0/conf/core"/>
    <spec:method>Inspect the GML output to verify that all appropriate elements have a 'gmllro:' prefix.</spec:method>
  </rdf:Description>
  <rdf:Description rdf:about="http://www.opengis.net/spec/landinfra/part0/1.0/conf/core/elements">
    <spec:testType rdf:resource="http://www.opengis.net/def/ont/modspec/Capabilities"/>
    <skos:narrower rdf:resource="http://www.opengis.net/spec/landinfra/part0/1.0/req/core/elements"/>
    <spec:purpose>Verify that the conforming application supports the Core XML elements listed in Table 1 in accordance with the GML XSD specified in http://schemas.opengis.net/infragml/part0/1.0/core.xsd.</spec:purpose>
    <spec:method>Inspect the GML output to verify the above requirement.</spec:method>
    <skos:broader rdf:resource="http://www.opengis.net/spec/landinfra/part0/1.0/conf/core"/>
    <rdf:type rdf:resource="http://www.w3.org/2004/02/skos/core#Concept"/>
    <rdf:type rdf:resource="http://www.opengis.net/def/ont/modspec/ConformanceTest"/>
    <skos:prefLabel>Conformance Test: http://www.opengis.net/spec/landinfra/part0/1.0/conf/core/elements</skos:prefLabel>
    <spec:requirement rdf:resource="http://www.opengis.net/spec/landinfra/part0/1.0/req/core/elements"/>
    <skos:definition>Verify that the conforming application supports the Core XML elements listed in Table 1 in accordance with the GML XSD specified in http://schemas.opengis.net/infragml/part0/1.0/core.xsd.</skos:definition>
  </rdf:Description>
  <rdf:Description rdf:about="http://www.opengis.net/def/docs/16-100r2">
    <prov:wasAttributedTo rdf:resource="http://www.opengis.net/def/wg/landinfraswg"/>
    <reg:status rdf:resource="http://purl.org/linked-data/registry#statusValid"/>
    <skos:topConceptOf rdf:resource="http://www.opengis.net/spec/landinfra"/>
    <dct:creator>Paul Scarponcini</dct:creator>
    <spec:authority>Open Geospatial Consortium</spec:authority>
    <dct:dateSubmitted rdf:datatype="http://www.w3.org/2001/XMLSchema#date">2017-03-24</dct:dateSubmitted>
    <specrel:implements rdf:resource="http://www.opengis.net/def/docs/15-111r1"/>
    <dct:dateAccepted rdf:datatype="http://www.w3.org/2001/XMLSchema#date">2017-06-02</dct:dateAccepted>
    <skos:notation rdf:datatype="http://www.opengis.net/def/metamodel/ogc-na/doc_no">16-100r2</skos:notation>
    <spec:date rdf:datatype="http://www.w3.org/2001/XMLSchema#date">2017-06-02</spec:date>
    <na:doctype rdf:resource="http://www.opengis.net/def/doc-type/ip"/>
    <adms:last rdf:resource="http://www.opengis.net/def/docs/16-100r2"/>
    <rdf:type rdf:resource="http://www.opengis.net/def/ont/modspec/Specification"/>
    <rdf:type rdf:resource="http://www.w3.org/2004/02/skos/core#Concept"/>
    <skos:prefLabel>OGC InfraGML 1.0: Part 0 – LandInfra Core - Encoding Standard</skos:prefLabel>
    <spec:class rdf:resource="http://www.opengis.net/spec/landinfra/part0/1.0/conf/core"/>
    <dcat:landingPage rdf:resource="https://docs.opengeospatial.org/is/16-100r2/16-100r2.html"/>
    <skos:inScheme rdf:resource="http://www.opengis.net/def/docs"/>
    <na:status rdf:resource="http://www.opengis.net/def/status/valid"/>
    <dct:identifier>http://www.opengis.net/doc/is/landinfra/part0/1.0</dct:identifier>
    <skos:definition>OGC® Encoding Standard; Core one required by any other encoding parts</skos:definition>
    <adms:version>1.0</adms:version>
    <spec:status rdf:resource="http://www.opengis.net/def/status/valid"/>
  </rdf:Description>
  <rdf:Description rdf:about="http://www.opengis.net/spec/landinfra/part0/1.0/conf/core/valid">
    <spec:requirement rdf:resource="http://www.opengis.net/spec/landinfra/part0/1.0/req/core/valid"/>
    <spec:purpose>Validate the XML document using the XML schema document(s) for the applicable Part(s). Pass if no errors reported. Fail otherwise.</spec:purpose>
    <skos:broader rdf:resource="http://www.opengis.net/spec/landinfra/part0/1.0/conf/core"/>
    <spec:testType rdf:resource="http://www.opengis.net/def/ont/modspec/Basic"/>
    <spec:method>Verify that XML instance documents of any Part of InfraGML is valid according to the XML grammar specified in that Part for each Requirements Class contained in that Part and available at http://schemas.opengis.net/infragml/part&lt;n&gt;/1.0/&lt;schema name&gt;.xsd where &lt;n&gt; is the Part number and &lt;schema name&gt; is the name of the schema equal to the name of the respective Requirements Class.</spec:method>
    <rdf:type rdf:resource="http://www.opengis.net/def/ont/modspec/ConformanceTest"/>
    <rdf:type rdf:resource="http://www.w3.org/2004/02/skos/core#Concept"/>
    <skos:prefLabel>Conformance Test: http://www.opengis.net/spec/landinfra/part0/1.0/conf/core/valid</skos:prefLabel>
    <skos:definition>Validate the XML document using the XML schema document(s) for the applicable Part(s). Pass if no errors reported. Fail otherwise.</skos:definition>
    <skos:narrower rdf:resource="http://www.opengis.net/spec/landinfra/part0/1.0/req/core/valid"/>
  </rdf:Description>
  <rdf:Description rdf:about="http://www.opengis.net/spec/landinfra/part0/1.0/conf/core">
    <spec:conformanceTest rdf:resource="http://www.opengis.net/spec/landinfra/part0/1.0/conf/core/gml3.3lr"/>
    <spec:conformanceTest rdf:resource="http://www.opengis.net/spec/landinfra/part0/1.0/conf/core/gml3.2"/>
    <spec:conformanceTest rdf:resource="http://www.opengis.net/spec/landinfra/part0/1.0/conf/core/gml3.3lro"/>
    <spec:conformanceTest rdf:resource="http://www.opengis.net/spec/landinfra/part0/1.0/conf/core/valid"/>
    <spec:conformanceTest rdf:resource="http://www.opengis.net/spec/landinfra/part0/1.0/conf/core/header"/>
    <spec:conformanceTest rdf:resource="http://www.opengis.net/spec/landinfra/part0/1.0/conf/core/elements"/>
    <skos:narrower rdf:resource="http://www.opengis.net/spec/landinfra/part0/1.0/conf/core/gml3.3lro"/>
    <skos:narrower rdf:resource="http://www.opengis.net/spec/landinfra/part0/1.0/req/core"/>
    <skos:narrower rdf:resource="http://www.opengis.net/spec/landinfra/part0/1.0/conf/core/valid"/>
    <skos:narrower rdf:resource="http://www.opengis.net/spec/landinfra/part0/1.0/conf/core/header"/>
    <skos:narrower rdf:resource="http://www.opengis.net/spec/landinfra/part0/1.0/conf/core/elements"/>
    <skos:narrower rdf:resource="http://www.opengis.net/spec/landinfra/part0/1.0/conf/core/gml3.3lr"/>
    <skos:narrower rdf:resource="http://www.opengis.net/spec/landinfra/part0/1.0/conf/core/gml3.2"/>
    <spec:requirementsTested rdf:resource="http://www.opengis.net/spec/landinfra/part0/1.0/req/core"/>
    <skos:definition>Conformance Class: Core</skos:definition>
    <skos:prefLabel>Conformance Class: Core</skos:prefLabel>
    <skos:inScheme rdf:resource="http://www.opengis.net/spec/landinfra/part0/1.0"/>
    <rdf:type rdf:resource="http://www.w3.org/2004/02/skos/core#Concept"/>
    <rdf:type rdf:resource="http://www.opengis.net/def/ont/modspec/ConformanceClass"/>
    <dcat:landingPage rdf:resource="https://docs.opengeospatial.org/is/16-100r2/16-100r2.html#_conformance_class_core"/>
    <na:status rdf:resource="http://www.opengis.net/def/status/valid"/>
    <skos:topConceptOf rdf:resource="http://www.opengis.net/spec/landinfra/part0/1.0"/>
  </rdf:Description>
  <rdf:Description rdf:about="http://www.opengis.net/spec/infragml/part0/1.0">
    <na:status rdf:resource="http://www.opengis.net/def/status/experimental"/>
    <skos:hasTopConcept rdf:resource="http://www.opengis.net/spec/landinfra/part0/1.0/conf/core"/>
    <spec:status rdf:resource="http://www.opengis.net/def/status/experimental"/>
    <skos:prefLabel>Specification elements for OGC 16-100r2 LandInfra</skos:prefLabel>
    <dct:created rdf:datatype="http://www.w3.org/2001/XMLSchema#date">2017-03-24</dct:created>
    <dct:source rdf:resource="http://www.opengis.net/def/docs/16-100r2"/>
    <skos:definition>A convenience hierarchy for navigating the elements of a specification using the SKOS model</skos:definition>
    <dct:modified rdf:datatype="http://www.w3.org/2001/XMLSchema#date">2017-06-02</dct:modified>
    <na:collectionView rdf:resource="http://www.opengis.net/spec/infragml/part0/1.0/"/>
    <rdf:type rdf:resource="http://www.w3.org/2004/02/skos/core#ConceptScheme"/>
  </rdf:Description>
  <rdf:Description rdf:about="http://www.opengis.net/spec/landinfra/part0/1.0/req/core/valid">
    <skos:broader rdf:resource="http://www.opengis.net/spec/landinfra/part0/1.0/req/core"/>
    <skos:broader rdf:resource="http://www.opengis.net/spec/landinfra/part0/1.0/conf/core/valid"/>
    <skos:prefLabel>Requirement: /req/core/valid</skos:prefLabel>
    <rdf:type rdf:resource="http://www.w3.org/2004/02/skos/core#Concept"/>
    <rdf:type rdf:resource="http://www.opengis.net/def/ont/modspec/Requirement"/>
    <skos:definition>Every XML instance document of any Part of InfraGML shall be valid according to the XML grammar specified in that Part for each Requirements Class contained in that Part and available at http://schemas.opengis.net/infragml/part&lt;n&gt;/1.0/&lt;schema name&gt;.xsd where &lt;n&gt; is the Part number and &lt;schema name&gt; is the name of the schema equal to the name of the respective Requirements Class.</skos:definition>
  </rdf:Description>
  <rdf:Description rdf:about="http://www.opengis.net/spec/landinfra/part0/1.0/req/core/header">
    <skos:broader rdf:resource="http://www.opengis.net/spec/landinfra/part0/1.0/conf/core/header"/>
    <skos:broader rdf:resource="http://www.opengis.net/spec/landinfra/part0/1.0/req/core"/>
    <skos:prefLabel>Requirement: /req/core/header</skos:prefLabel>
    <rdf:type rdf:resource="http://www.w3.org/2004/02/skos/core#Concept"/>
    <rdf:type rdf:resource="http://www.opengis.net/def/ont/modspec/Requirement"/>
    <skos:definition>An InfraGML conforming application shall use a schema definition file which shall contain a properly formed schema header appropriate to the InfraGML Requirements Classes it claims to support.</skos:definition>
  </rdf:Description>
  <rdf:Description rdf:about="http://www.opengis.net/spec/landinfra/part0/1.0/req/core">
    <rdf:type rdf:resource="http://www.opengis.net/def/ont/modspec/RequirementsClass"/>
    <rdf:type rdf:resource="http://www.w3.org/2004/02/skos/core#Concept"/>
    <spec:normativeStatement rdf:resource="http://www.opengis.net/spec/landinfra/part0/1.0/req/core/gml3.3lro"/>
    <spec:normativeStatement rdf:resource="http://www.opengis.net/spec/landinfra/part0/1.0/req/core/header"/>
    <spec:normativeStatement rdf:resource="http://www.opengis.net/spec/landinfra/part0/1.0/req/core/valid"/>
    <spec:normativeStatement rdf:resource="http://www.opengis.net/spec/landinfra/part0/1.0/req/core/gml3.2"/>
    <spec:normativeStatement rdf:resource="http://www.opengis.net/spec/landinfra/part0/1.0/req/core/gml3.3lr"/>
    <spec:normativeStatement rdf:resource="http://www.opengis.net/spec/landinfra/part0/1.0/req/core/elements"/>
    <skos:definition>LandInfra Core is the core Requirements Class and is the only mandatory Requirements Class. This class contains information about the Land and Infrastructure dataset that can contain information about facilities, land features, land division, documents, survey marks, surveys, sets, and feature associations. LandInfra Core also contains the definition of types common across other Requirements Classes, such as the Status CodeList.</skos:definition>
    <skos:broader rdf:resource="http://www.opengis.net/spec/landinfra/part0/1.0/conf/core"/>
    <skos:narrower rdf:resource="http://www.opengis.net/spec/landinfra/part0/1.0/req/core/gml3.3lr"/>
    <skos:narrower rdf:resource="http://www.opengis.net/spec/landinfra/part0/1.0/req/core/elements"/>
    <skos:narrower rdf:resource="http://www.opengis.net/spec/landinfra/part0/1.0/req/core/gml3.2"/>
    <skos:narrower rdf:resource="http://www.opengis.net/spec/landinfra/part0/1.0/req/core/gml3.3lro"/>
    <skos:narrower rdf:resource="http://www.opengis.net/spec/landinfra/part0/1.0/req/core/header"/>
    <skos:narrower rdf:resource="http://www.opengis.net/spec/landinfra/part0/1.0/req/core/valid"/>
    <skos:prefLabel>Requirement Class: Core</skos:prefLabel>
  </rdf:Description>
  <rdf:Description rdf:about="http://www.opengis.net/spec/infragml/part0/1.0/">
    <skos:member rdf:resource="http://www.opengis.net/def/status/"/>
    <skos:member rdf:resource="http://www.opengis.net/def/status/iso19135"/>
    <rdf:type rdf:resource="http://www.w3.org/2004/02/skos/core#Collection"/>
    <dct:provenance>Generated by the OGC Definitions Server to support integration of the elements of this ConceptScheme into bigger collections. ogc_skos_profile_entailements.ttl</dct:provenance>
    <skos:prefLabel>Concepts in Specification elements for OGC 16-100r2 LandInfra</skos:prefLabel>
    <skos:inScheme rdf:resource="http://www.opengis.net/spec/infragml/part0/1.0"/>
    <skos:definition>Collection hierarchy for this ConceptScheme</skos:definition>
  </rdf:Description>
  <rdf:Description rdf:about="http://www.opengis.net/spec/landinfra/part0/1.0/req/core/elements">
    <skos:prefLabel>Requirement: /req/core/elements</skos:prefLabel>
    <rdf:type rdf:resource="http://www.w3.org/2004/02/skos/core#Concept"/>
    <rdf:type rdf:resource="http://www.opengis.net/def/ont/modspec/Requirement"/>
    <skos:definition>A conforming application shall support the Core XML elements listed in Table 1 in accordance with the GML XSD specified in http://schemas.opengis.net/infragml/part0/1.0/core.xsd.</skos:definition>
    <skos:broader rdf:resource="http://www.opengis.net/spec/landinfra/part0/1.0/req/core"/>
    <skos:broader rdf:resource="http://www.opengis.net/spec/landinfra/part0/1.0/conf/core/elements"/>
  </rdf:Description>
  <rdf:Description rdf:about="http://www.opengis.net/spec/landinfra/part0/1.0/conf/core/header">
    <skos:narrower rdf:resource="http://www.opengis.net/spec/landinfra/part0/1.0/req/core/header"/>
    <rdf:type rdf:resource="http://www.w3.org/2004/02/skos/core#Concept"/>
    <rdf:type rdf:resource="http://www.opengis.net/def/ont/modspec/ConformanceTest"/>
    <skos:broader rdf:resource="http://www.opengis.net/spec/landinfra/part0/1.0/conf/core"/>
    <skos:definition>Verify that the encoding specifies whether it supports ID at the feature level, ID at the Feature sub-type level, or both.</skos:definition>
    <spec:purpose>Verify that the conforming application uses a schema definition file which contains a properly formed schema header appropriate to the InfraGML Requirements Classes it claims to support.</spec:purpose>
    <spec:testType rdf:resource="http://www.opengis.net/def/ont/modspec/Basic"/>
    <skos:prefLabel>Conformance Test: http://www.opengis.net/spec/landinfra/part0/1.0/conf/core/header</skos:prefLabel>
    <spec:method>Inspect the schema definition file used by the application.</spec:method>
    <spec:requirement rdf:resource="http://www.opengis.net/spec/landinfra/part0/1.0/req/core/header"/>
  </rdf:Description>
  <rdf:Description rdf:about="http://www.opengis.net/spec/landinfra/part0/1.0/conf/core/gml3.2">
    <spec:method>Inspect the GML output to verify that all appropriate elements have a 'gml:' prefix.</spec:method>
    <skos:prefLabel>Conformance Test: http://www.opengis.net/spec/landinfra/part0/1.0/conf/core/gml3.2</skos:prefLabel>
    <rdf:type rdf:resource="http://www.w3.org/2004/02/skos/core#Concept"/>
    <rdf:type rdf:resource="http://www.opengis.net/def/ont/modspec/ConformanceTest"/>
    <skos:broader rdf:resource="http://www.opengis.net/spec/landinfra/part0/1.0/conf/core"/>
    <skos:definition>Verify that the conforming application utilizes and depends upon the OGC GML 3.2 standard schema within the http://www.opengis.net/gml/3.2 namespace identified by 'gml'.</skos:definition>
    <spec:purpose>Verify that the conforming application utilizes and depends upon the OGC GML 3.2 standard schema within the http://www.opengis.net/gml/3.2 namespace identified by 'gml'.</spec:purpose>
    <spec:requirement rdf:resource="http://www.opengis.net/spec/landinfra/part0/1.0/req/core/gml3.2"/>
    <skos:narrower rdf:resource="http://www.opengis.net/spec/landinfra/part0/1.0/req/core/gml3.2"/>
    <spec:testType rdf:resource="http://www.opengis.net/def/ont/modspec/Capability"/>
  </rdf:Description>
  <rdf:Description rdf:about="http://www.opengis.net/spec/landinfra/part0/1.0/req/core/gml3.3lro">
    <skos:prefLabel>Requirement: /req/core/gml3.3lro</skos:prefLabel>
    <skos:definition>This LandGML standard shall utilize and depend upon the OGC GML 3.3 linearRefOffset standard schema within the http://www.opengis.net/gml/3.3/lro namespace identified by “gmllro”.</skos:definition>
    <rdf:type rdf:resource="http://www.opengis.net/def/ont/modspec/Requirement"/>
    <rdf:type rdf:resource="http://www.w3.org/2004/02/skos/core#Concept"/>
    <skos:broader rdf:resource="http://www.opengis.net/spec/landinfra/part0/1.0/conf/core/gml3.3lro"/>
    <skos:broader rdf:resource="http://www.opengis.net/spec/landinfra/part0/1.0/req/core"/>
  </rdf:Description>
  <rdf:Description rdf:about="http://www.opengis.net/spec/landinfra/part0/1.0/req/core/gml3.2">
    <skos:broader rdf:resource="http://www.opengis.net/spec/landinfra/part0/1.0/req/core"/>
    <skos:broader rdf:resource="http://www.opengis.net/spec/landinfra/part0/1.0/conf/core/gml3.2"/>
    <skos:definition>This LandGML standard shall utilize and depend upon the OGC GML 3.2 standard schema within the http://www.opengis.net/gml/3.2 namespace identified by “gml”.</skos:definition>
    <skos:prefLabel>Requirement: /req/core/gml3.2</skos:prefLabel>
    <rdf:type rdf:resource="http://www.w3.org/2004/02/skos/core#Concept"/>
    <rdf:type rdf:resource="http://www.opengis.net/def/ont/modspec/Requirement"/>
  </rdf:Description>
  <rdf:Description rdf:about="http://www.opengis.net/spec/landinfra/part0/1.0/conf/core/gml3.3lr">
    <spec:testType rdf:resource="http://www.opengis.net/def/ont/modspec/Capabilities"/>
    <skos:definition>Verify that the conforming application utilizes and depends upon the OGC GML 3.3 linearRef standard schema within the http://www.opengis.net/gml/3.3/lr namespace identified by 'gmllr'.</skos:definition>
    <skos:prefLabel>Conformance Test: http://www.opengis.net/spec/landinfra/part0/1.0/conf/core/gml3.3lr</skos:prefLabel>
    <rdf:type rdf:resource="http://www.opengis.net/def/ont/modspec/ConformanceTest"/>
    <rdf:type rdf:resource="http://www.w3.org/2004/02/skos/core#Concept"/>
    <skos:narrower rdf:resource="http://www.opengis.net/spec/landinfra/part0/1.0/req/core/gml3.3lr"/>
    <spec:purpose>Verify that the conforming application utilizes and depends upon the OGC GML 3.3 linearRef standard schema within the http://www.opengis.net/gml/3.3/lr namespace identified by 'gmllr'.</spec:purpose>
    <spec:method>Inspect the GML output to verify that all appropriate elements have a 'gmllr:' prefix.</spec:method>
    <skos:broader rdf:resource="http://www.opengis.net/spec/landinfra/part0/1.0/conf/core"/>
    <spec:requirement rdf:resource="http://www.opengis.net/spec/landinfra/part0/1.0/req/core/gml3.3lr"/>
  </rdf:Description>
  <rdf:Description rdf:about="http://www.opengis.net/spec/docs/16-100r2-anno">
    <rdf:type rdf:resource="http://www.w3.org/2002/07/owl#Ontology"/>
  </rdf:Description>
</rdf:RDF>
