<?xml version="1.0" encoding="UTF-8"?>
<rdf:RDF
   xmlns:adms="http://www.w3.org/ns/adms#"
   xmlns:dcat="http://www.w3.org/ns/dcat#"
   xmlns:dct="http://purl.org/dc/terms/"
   xmlns:na="http://www.opengis.net/def/metamodel/ogc-na/"
   xmlns:rdf="http://www.w3.org/1999/02/22-rdf-syntax-ns#"
   xmlns:reg="http://purl.org/linked-data/registry#"
   xmlns:skos="http://www.w3.org/2004/02/skos/core#"
   xmlns:spec="http://www.opengis.net/def/ont/modspec/"
>
  <rdf:Description rdf:about="http://www.opengis.net/def/docs/19-008r4">
    <skos:narrower rdf:resource="http://www.opengis.net/spec/GeoTIFF/1.1/req/PrimeMeridianGeoKey"/>
    <skos:narrower rdf:resource="http://www.opengis.net/spec/GeoTIFF/1.1/req/ProjMethodGeoKey"/>
    <skos:narrower rdf:resource="http://www.opengis.net/spec/GeoTIFF/1.1/req/Core"/>
    <skos:narrower rdf:resource="http://www.opengis.net/spec/GeoTIFF/1.1/req/PrimeMeridianLongitudeGeoKey"/>
    <skos:narrower rdf:resource="http://www.opengis.net/spec/GeoTIFF/1.1/req/GeoKeyCode"/>
    <skos:narrower rdf:resource="http://www.opengis.net/spec/GeoTIFF/1.1/req/EllipsoidSemiMajorAxisGeoKey"/>
    <skos:narrower rdf:resource="http://www.opengis.net/spec/GeoTIFF/1.1/req/ModelPixelScaleTag"/>
    <skos:narrower rdf:resource="http://www.opengis.net/spec/GeoTIFF/1.1/req/GeoAsciiParamsTag"/>
    <skos:narrower rdf:resource="http://www.opengis.net/spec/GeoTIFF/1.1/req/ProjectedCRSGeoKey"/>
    <skos:narrower rdf:resource="http://www.opengis.net/spec/GeoTIFF/1.1/req/GeoShortParamsTag"/>
    <skos:narrower rdf:resource="http://www.opengis.net/spec/GeoTIFF/1.1/req/GTModelTypeGeoKey"/>
    <skos:narrower rdf:resource="http://www.opengis.net/spec/GeoTIFF/1.1/req/UnitsGeoKey"/>
    <skos:narrower rdf:resource="http://www.opengis.net/spec/GeoTIFF/1.1/req/GTRasterTypeGeoKey"/>
    <skos:narrower rdf:resource="http://www.opengis.net/spec/GeoTIFF/1.1/req/GeoKeyDirectoryTag"/>
    <skos:narrower rdf:resource="http://www.opengis.net/spec/GeoTIFF/1.1/req/EllipsoidGeoKey"/>
    <skos:narrower rdf:resource="http://www.opengis.net/spec/GeoTIFF/1.1/req/GeodeticCRSGeoKey"/>
    <skos:narrower rdf:resource="http://www.opengis.net/spec/GeoTIFF/1.1/req/ProjectionGeoKey"/>
    <skos:narrower rdf:resource="http://www.opengis.net/spec/GeoTIFF/1.1/req/VerticalDatumGeoKey"/>
    <skos:narrower rdf:resource="http://www.opengis.net/spec/GeoTIFF/1.1/req/GeodeticDatumGeoKey"/>
    <skos:narrower rdf:resource="http://www.opengis.net/spec/GeoTIFF/1.1/req/ModelTransformationTag"/>
    <skos:narrower rdf:resource="http://www.opengis.net/spec/GeoTIFF/1.1/req/GeoDoubleParamsTag"/>
    <skos:narrower rdf:resource="http://www.opengis.net/spec/GeoTIFF/1.1/req/ModelTiepointTag"/>
    <skos:narrower rdf:resource="http://www.opengis.net/spec/GeoTIFF/1.1/req/UnitSizeGeoKey"/>
    <skos:narrower rdf:resource="http://www.opengis.net/spec/GeoTIFF/1.1/req/CitationGeoKeys"/>
    <skos:narrower rdf:resource="http://www.opengis.net/spec/GeoTIFF/1.1/req/VerticalGeoKey"/>
    <spec:class rdf:resource="http://www.opengis.net/spec/GeoTIFF/1.1/req/GeodeticCRSGeoKey"/>
    <spec:class rdf:resource="http://www.opengis.net/spec/GeoTIFF/1.1/req/ProjectionGeoKey"/>
    <spec:class rdf:resource="http://www.opengis.net/spec/GeoTIFF/1.1/req/ProjectedCRSGeoKey"/>
    <spec:class rdf:resource="http://www.opengis.net/spec/GeoTIFF/1.1/req/VerticalDatumGeoKey"/>
    <spec:class rdf:resource="http://www.opengis.net/spec/GeoTIFF/1.1/req/GeodeticDatumGeoKey"/>
    <spec:class rdf:resource="http://www.opengis.net/spec/GeoTIFF/1.1/req/ModelTransformationTag"/>
    <spec:class rdf:resource="http://www.opengis.net/spec/GeoTIFF/1.1/req/GeoDoubleParamsTag"/>
    <spec:class rdf:resource="http://www.opengis.net/spec/GeoTIFF/1.1/req/ModelTiepointTag"/>
    <spec:class rdf:resource="http://www.opengis.net/spec/GeoTIFF/1.1/req/UnitSizeGeoKey"/>
    <spec:class rdf:resource="http://www.opengis.net/spec/GeoTIFF/1.1/req/VerticalGeoKey"/>
    <spec:class rdf:resource="http://www.opengis.net/spec/GeoTIFF/1.1/req/PrimeMeridianGeoKey"/>
    <spec:class rdf:resource="http://www.opengis.net/spec/GeoTIFF/1.1/req/ProjMethodGeoKey"/>
    <spec:class rdf:resource="http://www.opengis.net/spec/GeoTIFF/1.1/req/PrimeMeridianLongitudeGeoKey"/>
    <spec:class rdf:resource="http://www.opengis.net/spec/GeoTIFF/1.1/req/GeoKeyCode"/>
    <spec:class rdf:resource="http://www.opengis.net/spec/GeoTIFF/1.1/req/ModelPixelScaleTag"/>
    <spec:class rdf:resource="http://www.opengis.net/spec/GeoTIFF/1.1/req/GeoAsciiParamsTag"/>
    <spec:class rdf:resource="http://www.opengis.net/spec/GeoTIFF/1.1/req/CitationGeoKeys"/>
    <spec:class rdf:resource="http://www.opengis.net/spec/GeoTIFF/1.1/req/GeoShortParamsTag"/>
    <spec:class rdf:resource="http://www.opengis.net/spec/GeoTIFF/1.1/req/GTModelTypeGeoKey"/>
    <spec:class rdf:resource="http://www.opengis.net/spec/GeoTIFF/1.1/req/Core"/>
    <spec:class rdf:resource="http://www.opengis.net/spec/GeoTIFF/1.1/req/UnitsGeoKey"/>
    <spec:class rdf:resource="http://www.opengis.net/spec/GeoTIFF/1.1/req/GTRasterTypeGeoKey"/>
    <spec:class rdf:resource="http://www.opengis.net/spec/GeoTIFF/1.1/req/GeoKeyDirectoryTag"/>
    <spec:class rdf:resource="http://www.opengis.net/spec/GeoTIFF/1.1/req/EllipsoidGeoKey"/>
    <spec:class rdf:resource="http://www.opengis.net/spec/GeoTIFF/1.1/req/EllipsoidSemiMajorAxisGeoKey"/>
    <adms:version>1.1</adms:version>
    <skos:notation rdf:datatype="http://www.opengis.net/def/metamodel/ogc-na/doc_no">19-008r4</skos:notation>
    <skos:note>Approved</skos:note>
    <reg:status rdf:resource="http://purl.org/linked-data/registry#statusValid"/>
    <dct:creator>Emmanuel Devys, Ted Habermann, Chuck Heazel, Roger Lott, Even Rouault</dct:creator>
    <skos:inScheme rdf:resource="http://www.opengis.net/def/docs"/>
    <na:status rdf:resource="http://www.opengis.net/def/status/under-development"/>
    <spec:authority>Open Geospatial Consortium</spec:authority>
    <dcat:landingPage rdf:resource="http://docs.opengeospatial.org/is/19-008r4/19-008r4.html"/>
    <rdf:type rdf:resource="http://www.opengis.net/def/ont/modspec/Specification"/>
    <rdf:type rdf:resource="http://www.w3.org/2004/02/skos/core#Concept"/>
    <dct:identifier>http://www.opengis.net/doc/IS/GeoTIFF/1.1</dct:identifier>
    <skos:definition>OGC GeoTIFF standard</skos:definition>
    <na:doctype rdf:resource="http://www.opengis.net/def/doc-type/is"/>
    <spec:testSuite rdf:resource="http://www.opengis.net/spec/GeoTIFF/1.1/csuite"/>
    <skos:prefLabel>OGC GeoTIFF standard</skos:prefLabel>
    <dct:dateSubmitted rdf:datatype="http://www.w3.org/2001/XMLSchema#date">2019-06-05</dct:dateSubmitted>
  </rdf:Description>
  <rdf:Description rdf:about="http://www.opengis.net/spec/GeoTIFF/1.1/conf/TIFF.Tags">
    <skos:broader rdf:resource="http://www.opengis.net/spec/GeoTIFF/1.1/conf/Core"/>
    <spec:requirement rdf:resource="http://www.opengis.net/spec/GeoTIFF/1.1/req/ByteOrder"/>
    <spec:requirement rdf:resource="http://www.opengis.net/spec/GeoTIFF/1.1/req/TagSort"/>
    <spec:requirement rdf:resource="http://www.opengis.net/spec/GeoTIFF/1.1/req/GeoAsciiParamsTag.ID"/>
    <spec:requirement rdf:resource="http://www.opengis.net/spec/GeoTIFF/1.1/req/ModelTiepointTag.type"/>
    <spec:requirement rdf:resource="http://www.opengis.net/spec/GeoTIFF/1.1/req/GeoKeyDirectoryTag.count"/>
    <spec:requirement rdf:resource="http://www.opengis.net/spec/GeoTIFF/1.1/req/ModelTransformationTag.ID"/>
    <spec:requirement rdf:resource="http://www.opengis.net/spec/GeoTIFF/1.1/req/ModelPixelScaleTag.ID"/>
    <spec:requirement rdf:resource="http://www.opengis.net/spec/GeoTIFF/1.1/req/GeoAsciiParamsTag.type"/>
    <spec:requirement rdf:resource="http://www.opengis.net/spec/GeoTIFF/1.1/req/GeoDoubleParamsTag.count"/>
    <spec:requirement rdf:resource="http://www.opengis.net/spec/GeoTIFF/1.1/req/ModelTransformationTag.type"/>
    <spec:requirement rdf:resource="http://www.opengis.net/spec/GeoTIFF/1.1/req/GeoDoubleParamsTag.ID"/>
    <spec:requirement rdf:resource="http://www.opengis.net/spec/GeoTIFF/1.1/req/GeoKeyDirectoryTag.ID"/>
    <spec:requirement rdf:resource="http://www.opengis.net/spec/GeoTIFF/1.1/req/GeoKeyDirectoryTag.type"/>
    <spec:requirement rdf:resource="http://www.opengis.net/spec/GeoTIFF/1.1/req/TIFF"/>
    <spec:requirement rdf:resource="http://www.opengis.net/spec/GeoTIFF/1.1/req/ModelTiepointTag.ID"/>
    <spec:requirement rdf:resource="http://www.opengis.net/spec/GeoTIFF/1.1/req/DataGeoTags"/>
    <spec:requirement rdf:resource="http://www.opengis.net/spec/GeoTIFF/1.1/req/ModelPixelScaleTag.type"/>
    <skos:narrower rdf:resource="http://www.opengis.net/spec/GeoTIFF/1.1/req/ByteOrder"/>
    <skos:narrower rdf:resource="http://www.opengis.net/spec/GeoTIFF/1.1/req/TagSort"/>
    <skos:narrower rdf:resource="http://www.opengis.net/spec/GeoTIFF/1.1/req/ModelPixelScaleTag.ID"/>
    <skos:narrower rdf:resource="http://www.opengis.net/spec/GeoTIFF/1.1/req/GeoKeyDirectoryTag.count"/>
    <skos:narrower rdf:resource="http://www.opengis.net/spec/GeoTIFF/1.1/req/ModelTransformationTag.ID"/>
    <skos:narrower rdf:resource="http://www.opengis.net/spec/GeoTIFF/1.1/req/GeoAsciiParamsTag.type"/>
    <skos:narrower rdf:resource="http://www.opengis.net/spec/GeoTIFF/1.1/req/GeoDoubleParamsTag.count"/>
    <skos:narrower rdf:resource="http://www.opengis.net/spec/GeoTIFF/1.1/req/ModelTransformationTag.type"/>
    <skos:narrower rdf:resource="http://www.opengis.net/spec/GeoTIFF/1.1/req/GeoDoubleParamsTag.ID"/>
    <skos:narrower rdf:resource="http://www.opengis.net/spec/GeoTIFF/1.1/req/GeoAsciiParamsTag.ID"/>
    <skos:narrower rdf:resource="http://www.opengis.net/spec/GeoTIFF/1.1/req/GeoKeyDirectoryTag.ID"/>
    <skos:narrower rdf:resource="http://www.opengis.net/spec/GeoTIFF/1.1/req/ModelTiepointTag.type"/>
    <skos:narrower rdf:resource="http://www.opengis.net/spec/GeoTIFF/1.1/req/GeoKeyDirectoryTag.type"/>
    <skos:narrower rdf:resource="http://www.opengis.net/spec/GeoTIFF/1.1/req/TIFF"/>
    <skos:narrower rdf:resource="http://www.opengis.net/spec/GeoTIFF/1.1/req/ModelTiepointTag.ID"/>
    <skos:narrower rdf:resource="http://www.opengis.net/spec/GeoTIFF/1.1/req/DataGeoTags"/>
    <skos:narrower rdf:resource="http://www.opengis.net/spec/GeoTIFF/1.1/req/ModelPixelScaleTag.type"/>
    <spec:purpose>Verify the TIFF header and prepare for processing the GeoTIFF tags.</spec:purpose>
    <rdf:type rdf:resource="http://www.w3.org/2004/02/skos/core#Concept"/>
    <rdf:type rdf:resource="http://www.opengis.net/def/ont/modspec/ConformanceTest"/>
    <skos:definition>TIFF Tags Test</skos:definition>
    <spec:testType rdf:resource="http://www.opengis.net/def/ont/modspec/Basic"/>
    <skos:prefLabel>TIFF Tags Test</skos:prefLabel>
    <spec:method rdf:datatype="http://www.w3.org/1999/02/22-rdf-syntax-ns#HTML">%3Cdiv%20class%3D%22paragraph%22%3E%0A%3Cp%3EValidate%20and%20process%20the%20TIFF%20header%3C/p%3E%0A%3C/div%3E%3Cdiv%20class%3D%22ulist%22%3E%0A%3Cul%3E%0A%3Cli%3E%0A%3Cp%3EVerify%20that%20Bytes%200-1%20%3D%200X4949%20%28%22II%22%20%3D%20little%20endian%29%20or%200X4D4D%20%28%22MM%22%20%3D%20big%20endian%29.%3C/p%3E%0A%3C/li%3E%0A%3Cli%3E%0A%3Cp%3EVerify%20that%20Bytes%202-3%20%3D%20the%20short%20integer%20value%2042%20interpreted%20using%20the%20byte%20order%20specified%20in%20bytes%200-1.%3C/p%3E%0A%3C/li%3E%0A%3Cli%3E%0A%3Cp%3EBytes%204-7%20are%20the%20offset%20to%20the%20first%20Image%20File%20Directory.%20Save%20this%20value%20as%20IFD_Offset.%3C/p%3E%0A%3C/li%3E%0A%3C/ul%3E%0A%3C/div%3E%3Cdiv%20class%3D%22paragraph%22%3E%0A%3Cp%3EProcess%20each%20IFD%20using%20the%20following%20pseudocode%3A%3C/p%3E%0A%3C/div%3E%3Cdiv%20class%3D%22literalblock%22%3E%0A%3Cdiv%20class%3D%22content%22%3E%0A%3Cpre%3EWHILE%20IFD_Offset%20is%20not%200%2C%20process%20this%20IFD%0A%20%20%20%7B%0A%20%20%20Bytes%200-1%20contain%20the%20number%20of%20IFD%20entries%20in%20this%20IFD.%0A%20%20%20DO%20FOR%20each%20IFD%20entry%20%28processed%20in%20sequence%29%0A%20%20%20%20%20%20%7B%0A%20%20%20%20%20%20Bytes%200-1%20contain%20the%20TIFF%20tag%20value.%0A%20%20%20%20%20%20Verify%20that%20the%20new%20tag%20value%20is%20greater%20than%20the%20previous%20tag%20value.%0A%20%20%20%20%20%20IF%20value%20%3D%2034735%20THEN%0A%20%20%20%20%20%20%20%20%20%20%7B%0A%20%20%20%20%20%20%20%20%20%20Validate%20that%20Bytes%202-3%20%3D%203%20%28Short%20Integer%29%0A%20%20%20%20%20%20%20%20%20%20Validate%20that%20Bytes%204-7%20represent%20an%20Integer%20value%20greater%20than%20or%20equal%20to%204%0A%20%20%20%20%20%20%20%20%20%20Set%20GeoKeyDirectory%20to%20the%20value%20in%20Bytes%208-11%0A%20%20%20%20%20%20%20%20%20%20%7D%0A%20%20%20%20%20%20IF%20value%20%3D%2034736%20THEN%0A%20%20%20%20%20%20%20%20%20%20%7B%0A%20%20%20%20%20%20%20%20%20%20Validate%20that%20Bytes%202-3%20%3D%2012%20%28Double%29%0A%20%20%20%20%20%20%20%20%20%20Set%20DoubleValues%20to%20the%20value%20in%20Bytes%208-11%0A%20%20%20%20%20%20%20%20%20%20%7D%0A%20%20%20%20%20%20IF%20value%20%3D%2034737%20THEN%0A%20%20%20%20%20%20%20%20%20%20%7B%0A%20%20%20%20%20%20%20%20%20%20Validate%20that%20Bytes%202-3%20%3D%202%20%28ASCII%29%0A%20%20%20%20%20%20%20%20%20%20Set%20ASCIIValues%20to%20the%20value%20in%20Bytes%208-11%0A%20%20%20%20%20%20%20%20%20%20%7D%0A%20%20%20%20%20%20IF%20value%20%3D%2033550%20%28ModelPixelScaleTag%29%20THEN%0A%20%20%20%20%20%20%20%20%20%20%7B%0A%20%20%20%20%20%20%20%20%20%20Set%20PixelScaleTag%20to%20the%20location%20of%20this%20IFD%20entry%20in%20the%20GeoTIFF%20file%0A%20%20%20%20%20%20%20%20%20%20%7D%0A%20%20%20%20%20%20IF%20value%20%3D%2033922%20%28ModelTiepointTag%29%20THEN%0A%20%20%20%20%20%20%20%20%20%20%7B%0A%20%20%20%20%20%20%20%20%20%20Set%20TiepointTag%20to%20the%20location%20of%20this%20IFD%20entry%20in%20the%20GeoTIFF%20file%0A%20%20%20%20%20%20%20%20%20%20%7D%0A%20%20%20%20%20%20IF%20value%20%3D%2034264%20%28ModelTransformationTag%29%20THEN%0A%20%20%20%20%20%20%20%20%20%20%7B%0A%20%20%20%20%20%20%20%20%20%20Set%20TransformTag%20to%20the%20location%20of%20this%20IFD%20entry%20in%20the%20GeoTIFF%20file%0A%20%20%20%20%20%20%20%20%20%20%7D%0A%20%20%20%20%20%20%7D%0A%20%20IF%20GeoKeyDirectory%20has%20been%20set%20THEN%0A%20%20%20%20%20%20%7B%0A%20%20%20%20%20%20execute%20test%20http%3A//www.opengis.net/spec/GeoTIFF/1.1/conf/GeoKeyDirectory%0A%20%20%20%20%20%20Validate%20that%20there%20is%20a%20GTModelType%20GeoKey%20in%20the%20GeoKey%20Directory%0A%20%20%20%20%20%20%7D%0A%20%20%20%20%20%20ELSE%20Throw%20an%20error.%0A%20%20IF%20PixelScaleTag%20has%20been%20set%20THEN%0A%20%20%20%20%20%20%7B%0A%20%20%20%20%20%20Validate%20that%20Bytes%202-3%20%3D%2012%20%28Double%29%0A%20%20%20%20%20%20Set%20TagLength%20to%20the%20value%20in%20Bytes%204-7%0A%20%20%20%20%20%20Set%20TagValue%20to%20the%20value%20in%20Bytes%208-11%0A%20%20%20%20%20%20Validate%20that%20this%20IFD%20contains%20a%20ModelTiepointTag%0A%20%20%20%20%20%20Execute%20test%20http%3A//www.opengis.net/spec/GeoTIFF/1.1/conf/Raster2Model_CoordinateTransformation_GeoKey/ModelPixelScaleTag%0A%20%20%20%20%20%20%7D%0A%20%20IF%20TiepointTag%20has%20been%20set%20THEN%0A%20%20%20%20%20%20%7B%0A%20%20%20%20%20%20Validate%20that%20Bytes%202-3%20%3D%2012%20%28Double%29%0A%20%20%20%20%20%20Set%20TagLength%20to%20the%20value%20in%20Bytes%204-7%0A%20%20%20%20%20%20Set%20TagValue%20to%20the%20value%20in%20Bytes%208-11%0A%20%20%20%20%20%20Execute%20test%20http%3A//www.opengis.net/spec/GeoTIFF/1.1/conf/Raster2Model_CoordinateTransformation_GeoKey/ModelTiepointTag%0A%20%20%20%20%20%20%7D%0A%20%20IF%20TransformTag%20has%20been%20set%20THEN%0A%20%20%20%20%20%20%7B%0A%20%20%20%20%20%20Validate%20that%20Bytes%202-3%20%3D%2012%20%28Double%29%0A%20%20%20%20%20%20Set%20TagLength%20to%20the%20value%20in%20Bytes%204-7%0A%20%20%20%20%20%20Set%20TagValue%20to%20the%20value%20in%20Bytes%208-1%0A%20%20%20%20%20%20Validate%20that%20this%20IFD%20does%20not%20contain%20a%20ModelPixelScaleTag%0A%20%20%20%20%20%20Execute%20test%20http%3A//www.opengis.net/spec/GeoTIFF/1.1/conf/Raster2Model_CoordinateTransformation_GeoKey/ModelTransformationTag%0A%20%20%20%20%20%20%7D%0A%20%20Validate%20that%20this%20IFD%20contains%20either%20a%20ModelTransformationTag%20or%20a%20ModelTiepointTag.%0A%20%20IFD_Offset%20%3D%20the%20last%20four%20bytes%20of%20the%20current%20IFD%0A%20%20%7D%3C/pre%3E%0A%3C/div%3E%0A%3C/div%3E</spec:method>
    <spec:method>Text Variables

**Variable**

|

**Scope**

|

**Description**

---|---|---

IFD_Offset

|

Local

|

Location within the TIFF file of an IFD

GeoKeyDirectory

|

Global

|

Location of the GeoTIFF GeoKey directory

ASCIIValues

|

Global

|

Location of the ASCII values for GeoTIFF ASCII GeoKeys

DoubleValues

|

Global

|

Location of the Double values for GeoTIFF Double GeoKeys

TransformTag

|

Local

|

Location of the Model Transform Tag

PixelScaleTag

|

Local

|

Location of the ModelPixelScale Tag

TiepointTag

|

Local

|

Location of the ModelTiepoint Tag

TagLength

|

Parameter

|

Length of the value of a TIFF Tag

TagValue

|

Parameter

|

Location of the value of a TIFF tag in the GeoTIFF file

Validate and process the TIFF header

  * Verify that Bytes 0-1 = 0X4949 (II = little endian) or 0X4D4D (MM = big endian).

  * Verify that Bytes 2-3 = the short integer value 42 interpreted using the byte order specified in bytes 0-1.

  * Bytes 4-7 are the offset to the first Image File Directory. Save this value as IFD_Offset.

Process each IFD using the following pseudocode:



    WHILE IFD_Offset is not 0, process this IFD
       {
       Bytes 0-1 contain the number of IFD entries in this IFD.
       DO FOR each IFD entry (processed in sequence)
          {
          Bytes 0-1 contain the TIFF tag value.
          Verify that the new tag value is greater than the previous tag value.
          IF value = 34735 THEN
              {
              Validate that Bytes 2-3 = 3 (Short Integer)
              Validate that Bytes 4-7 represent an Integer value greater than or equal to 4
              Set GeoKeyDirectory to the value in Bytes 8-11
              }
          IF value = 34736 THEN
              {
              Validate that Bytes 2-3 = 12 (Double)
              Set DoubleValues to the value in Bytes 8-11
              }
          IF value = 34737 THEN
              {
              Validate that Bytes 2-3 = 2 (ASCII)
              Set ASCIIValues to the value in Bytes 8-11
              }
          IF value = 33550 (ModelPixelScaleTag) THEN
              {
              Set PixelScaleTag to the location of this IFD entry in the GeoTIFF file
              }
          IF value = 33922 (ModelTiepointTag) THEN
              {
              Set TiepointTag to the location of this IFD entry in the GeoTIFF file
              }
          IF value = 34264 (ModelTransformationTag) THEN
              {
              Set TransformTag to the location of this IFD entry in the GeoTIFF file
              }
          }
      IF GeoKeyDirectory has been set THEN
          {
          execute test http://www.opengis.net/spec/GeoTIFF/1.1/conf/GeoKeyDirectory
          Validate that there is a GTModelType GeoKey in the GeoKey Directory
          }
          ELSE Throw an error.
      IF PixelScaleTag has been set THEN
          {
          Validate that Bytes 2-3 = 12 (Double)
          Set TagLength to the value in Bytes 4-7
          Set TagValue to the value in Bytes 8-11
          Validate that this IFD contains a ModelTiepointTag
          Execute test http://www.opengis.net/spec/GeoTIFF/1.1/conf/Raster2Model_CoordinateTransformation_GeoKey/ModelPixelScaleTag
          }
      IF TiepointTag has been set THEN
          {
          Validate that Bytes 2-3 = 12 (Double)
          Set TagLength to the value in Bytes 4-7
          Set TagValue to the value in Bytes 8-11
          Execute test http://www.opengis.net/spec/GeoTIFF/1.1/conf/Raster2Model_CoordinateTransformation_GeoKey/ModelTiepointTag
          }
      IF TransformTag has been set THEN
          {
          Validate that Bytes 2-3 = 12 (Double)
          Set TagLength to the value in Bytes 4-7
          Set TagValue to the value in Bytes 8-1
          Validate that this IFD does not contain a ModelPixelScaleTag
          Execute test http://www.opengis.net/spec/GeoTIFF/1.1/conf/Raster2Model_CoordinateTransformation_GeoKey/ModelTransformationTag
          }
      Validate that this IFD contains either a ModelTransformationTag or a ModelTiepointTag.
      IFD_Offset = the last four bytes of the current IFD
      }</spec:method>
  </rdf:Description>
  <rdf:Description rdf:about="http://www.opengis.net/spec/GeoTIFF/1.1/req/VerticalGeoKey">
    <skos:broader rdf:resource="http://www.opengis.net/spec/GeoTIFF/1.1/conf/ShortParameters"/>
    <skos:broader rdf:resource="http://www.opengis.net/def/docs/19-008r4"/>
    <spec:normativeStatement rdf:resource="http://www.opengis.net/spec/GeoTIFF/1.1/req/VerticalGeoKey.EPSG"/>
    <spec:normativeStatement rdf:resource="http://www.opengis.net/spec/GeoTIFF/1.1/reqVerticalGeoKey.private"/>
    <spec:normativeStatement rdf:resource="http://www.opengis.net/spec/GeoTIFF/1.1/req/VerticalGeoKey.ID"/>
    <spec:normativeStatement rdf:resource="http://www.opengis.net/spec/GeoTIFF/1.1/req/VerticalGeoKey.type"/>
    <spec:normativeStatement rdf:resource="http://www.opengis.net/spec/GeoTIFF/1.1/req/VerticalGeoKey.userdefined"/>
    <spec:normativeStatement rdf:resource="http://www.opengis.net/spec/GeoTIFF/1.1/req/VerticalGeoKey.reserved"/>
    <skos:narrower rdf:resource="http://www.opengis.net/spec/GeoTIFF/1.1/req/VerticalGeoKey.EPSG"/>
    <skos:narrower rdf:resource="http://www.opengis.net/spec/GeoTIFF/1.1/req/VerticalGeoKey.ID"/>
    <skos:narrower rdf:resource="http://www.opengis.net/spec/GeoTIFF/1.1/req/VerticalGeoKey.userdefined"/>
    <skos:narrower rdf:resource="http://www.opengis.net/spec/GeoTIFF/1.1/req/VerticalGeoKey.reserved"/>
    <skos:narrower rdf:resource="http://www.opengis.net/spec/GeoTIFF/1.1/reqVerticalGeoKey.private"/>
    <skos:narrower rdf:resource="http://www.opengis.net/spec/GeoTIFF/1.1/req/VerticalGeoKey.type"/>
    <rdf:type rdf:resource="http://www.opengis.net/def/ont/modspec/RequirementClass"/>
    <rdf:type rdf:resource="http://www.w3.org/2004/02/skos/core#Concept"/>
    <skos:prefLabel>Requirements Class VerticalGeoKey</skos:prefLabel>
    <skos:definition>This key is provided to specify the vertical coordinate reference system from the GeoTIFF CRS register or to indicate that the CRS is a user-defined vertical coordinate reference system. The value for VerticalGeoKey should follow the recommendations for including height in model CRS definitions as provided in Annex D.




Note


In GeoTIFF 1.0 this key was called VerticalCSTypeGeoKey. In GeoTIFF v1.0 vertical coordinate reference systems were described in draft form, with the statement Vertical coordinate systems are not yet implemented. These sections are provided for future development, and any vertical coordinate systems in the current revision must be defined using the VerticalCitationGeoKey.</skos:definition>
  </rdf:Description>
  <rdf:Description rdf:about="http://www.opengis.net/spec/GeoTIFF/1.1/req/UnitsGeoKey">
    <skos:definition>These keys are used to specify Units of Measure (UoM) through the identification of a unit from the GeoTIFF CRS register or to indicate that the unit is user-defined.

The GeogAngularUnitsGeoKey key is used to specify the angular unit for:



the axes in user-defined geographic 2D CRSs;


the horizontal axes in user-defined geographic 3D CRSs;


the longitude from the reference meridian in user-defined prime meridians; and


user-defined map projection parameters that are angles.



The GeogAzimuthUnitsGeoKey key is used to specify the angular unit for user-defined map projection parameters when these differ from the angular unit described through the GeogAngularUnitsGeoKey.

The GeogLinearUnitsGeoKey key is used to specify the linear unit for:



the axes in user-defined geocentric Cartesian CRSs;


the height axis of a user-defined geographic 3D CRS; and


for user-defined ellipsoid axes.



The ProjLinearUnitsGeoKey key is used to specify the linear units for:



the axes of  a user-defined projected CRS; and


map projection parameters that are lengths.



The VerticalUnitsGeoKey key is used to specify the linear unit for:



the axis of a user-defined vertical CRS.</skos:definition>
    <spec:normativeStatement rdf:resource="http://www.opengis.net/spec/GeoTIFF/1.1/req/UnitsGeoKey.userdefinedVertical"/>
    <spec:normativeStatement rdf:resource="http://www.opengis.net/spec/GeoTIFF/1.1/req/UnitsGeoKey.reserved"/>
    <spec:normativeStatement rdf:resource="http://www.opengis.net/spec/GeoTIFF/1.1/req/UnitsGeoKey.userdefinedProjLinear"/>
    <spec:normativeStatement rdf:resource="http://www.opengis.net/spec/GeoTIFF/1.1/req/UnitsGeoKey.userdefinedAngular"/>
    <spec:normativeStatement rdf:resource="http://www.opengis.net/spec/GeoTIFF/1.1/req/UnitsGeoKey.angular"/>
    <spec:normativeStatement rdf:resource="http://www.opengis.net/spec/GeoTIFF/1.1/req/UnitsGeoKey.type"/>
    <spec:normativeStatement rdf:resource="http://www.opengis.net/spec/GeoTIFF/1.1/req/UnitsGeoKey.userdefinedGeogLinear"/>
    <spec:normativeStatement rdf:resource="http://www.opengis.net/spec/GeoTIFF/1.1/req/UnitsGeoKey.linear"/>
    <spec:normativeStatement rdf:resource="http://www.opengis.net/spec/GeoTIFF/1.1/req/UnitsGeoKey.ID"/>
    <spec:normativeStatement rdf:resource="http://www.opengis.net/spec/GeoTIFF/1.1/req/UnitsGeoKey.private"/>
    <skos:narrower rdf:resource="http://www.opengis.net/spec/GeoTIFF/1.1/req/UnitsGeoKey.userdefinedVertical"/>
    <skos:narrower rdf:resource="http://www.opengis.net/spec/GeoTIFF/1.1/req/UnitsGeoKey.reserved"/>
    <skos:narrower rdf:resource="http://www.opengis.net/spec/GeoTIFF/1.1/req/UnitsGeoKey.angular"/>
    <skos:narrower rdf:resource="http://www.opengis.net/spec/GeoTIFF/1.1/req/UnitsGeoKey.userdefinedProjLinear"/>
    <skos:narrower rdf:resource="http://www.opengis.net/spec/GeoTIFF/1.1/req/UnitsGeoKey.userdefinedGeogLinear"/>
    <skos:narrower rdf:resource="http://www.opengis.net/spec/GeoTIFF/1.1/req/UnitsGeoKey.userdefinedAngular"/>
    <skos:narrower rdf:resource="http://www.opengis.net/spec/GeoTIFF/1.1/req/UnitsGeoKey.type"/>
    <skos:narrower rdf:resource="http://www.opengis.net/spec/GeoTIFF/1.1/req/UnitsGeoKey.linear"/>
    <skos:narrower rdf:resource="http://www.opengis.net/spec/GeoTIFF/1.1/req/UnitsGeoKey.ID"/>
    <skos:narrower rdf:resource="http://www.opengis.net/spec/GeoTIFF/1.1/req/UnitsGeoKey.private"/>
    <skos:broader rdf:resource="http://www.opengis.net/spec/GeoTIFF/1.1/conf/ShortParameters"/>
    <skos:broader rdf:resource="http://www.opengis.net/def/docs/19-008r4"/>
    <rdf:type rdf:resource="http://www.opengis.net/def/ont/modspec/RequirementClass"/>
    <rdf:type rdf:resource="http://www.w3.org/2004/02/skos/core#Concept"/>
    <skos:prefLabel>Requirements Class Units GeoKeys</skos:prefLabel>
  </rdf:Description>
  <rdf:Description rdf:about="http://www.opengis.net/spec/GeoTIFF/1.1/req/VerticalGeoKey.userdefined">
    <dct:description>If the VerticalGeoKey value is 32767 (User-Defined) then the
VerticalCitationGeoKey, the VerticalUnitsGeoKey and VerticalDatumGeoKey SHALL
be populated.</dct:description>
    <skos:prefLabel>Requirement 14.5</skos:prefLabel>
    <rdf:type rdf:resource="http://www.opengis.net/def/ont/modspec/Requirement"/>
    <rdf:type rdf:resource="http://www.w3.org/2004/02/skos/core#Concept"/>
    <skos:definition>If the VerticalGeoKey value is 32767 (User-Defined) then the
VerticalCitationGeoKey, the VerticalUnitsGeoKey and VerticalDatumGeoKey SHALL
be populated.</skos:definition>
    <skos:broader rdf:resource="http://www.opengis.net/spec/GeoTIFF/1.1/req/VerticalGeoKey"/>
  </rdf:Description>
  <rdf:Description rdf:about="http://www.opengis.net/spec/GeoTIFF/1.1/req/ProjAngularParameterGeoKey">
    <skos:broader rdf:resource="http://www.opengis.net/spec/GeoTIFF/1.1/conf/DoubleParameters"/>
  </rdf:Description>
  <rdf:Description rdf:about="http://www.opengis.net/spec/GeoTIFF/1.1/req/EllipsoidSemiMajorAxisGeoKey">
    <skos:narrower rdf:resource="http://www.opengis.net/spec/GeoTIFF/1.1/req/EllipsoidSemiMinorAxisGeoKey.ID"/>
    <skos:narrower rdf:resource="http://www.opengis.net/spec/GeoTIFF/1.1/req/EllipsoidSemiMinorAxisGeoKey.type"/>
    <skos:narrower rdf:resource="http://www.opengis.net/spec/GeoTIFF/1.1/req/EllipsoidSemiMajorAxisGeoKey.ID"/>
    <skos:narrower rdf:resource="http://www.opengis.net/spec/GeoTIFF/1.1/req/EllipsoidSemiMinorAxisGeoKey.units"/>
    <skos:narrower rdf:resource="http://www.opengis.net/spec/GeoTIFF/1.1/req/EllipsoidSemiMajorAxisGeoKey.type"/>
    <skos:narrower rdf:resource="http://www.opengis.net/spec/GeoTIFF/1.1/req/EllipsoidSemiMajorAxisGeoKey.units"/>
    <skos:narrower rdf:resource="http://www.opengis.net/spec/GeoTIFF/1.1/req/EllipsoidInvFlatteningGeoKey.type"/>
    <skos:narrower rdf:resource="http://www.opengis.net/spec/GeoTIFF/1.1/req/EllipsoidInvFlatteningGeoKey.ID"/>
    <skos:broader rdf:resource="http://www.opengis.net/spec/GeoTIFF/1.1/conf/DoubleParameters"/>
    <skos:broader rdf:resource="http://www.opengis.net/def/docs/19-008r4"/>
    <spec:normativeStatement rdf:resource="http://www.opengis.net/spec/GeoTIFF/1.1/req/EllipsoidSemiMajorAxisGeoKey.units"/>
    <spec:normativeStatement rdf:resource="http://www.opengis.net/spec/GeoTIFF/1.1/req/EllipsoidInvFlatteningGeoKey.ID"/>
    <spec:normativeStatement rdf:resource="http://www.opengis.net/spec/GeoTIFF/1.1/req/EllipsoidSemiMinorAxisGeoKey.units"/>
    <spec:normativeStatement rdf:resource="http://www.opengis.net/spec/GeoTIFF/1.1/req/EllipsoidSemiMinorAxisGeoKey.ID"/>
    <spec:normativeStatement rdf:resource="http://www.opengis.net/spec/GeoTIFF/1.1/req/EllipsoidSemiMajorAxisGeoKey.type"/>
    <spec:normativeStatement rdf:resource="http://www.opengis.net/spec/GeoTIFF/1.1/req/EllipsoidSemiMajorAxisGeoKey.ID"/>
    <spec:normativeStatement rdf:resource="http://www.opengis.net/spec/GeoTIFF/1.1/req/EllipsoidInvFlatteningGeoKey.type"/>
    <spec:normativeStatement rdf:resource="http://www.opengis.net/spec/GeoTIFF/1.1/req/EllipsoidSemiMinorAxisGeoKey.type"/>
    <skos:definition>These keys are used to specify the size and shape of a user-defined ellipsoid or sphere used as the model of the earth. Only bi-axial ellipsoids and spheres are catered for. An ellipsoid is defined through two parameters,

its semi-major axis (a)

and either its semi-minor axis (b) or its inverse flattening (1/f) where 1/f = a/(a - b).

If the model is a sphere, 1/f is infinite so a and b must be used, with the value of b set to that of a.

Requirements Class EllipsoidSemiMajorAxisGeoKey

This key is provided to specify the first defining parameter of a user-defined bi-axial ellipsoid  or a user-defined sphere. It allows the specification of the ellipsoid semi-major axis (a) or the sphere’s radius.




Note


In GeoTIFF 1.0 this key was called GeogSemiMajorAxisGeoKey.




Requirements Class EllipsoidSemiMinorAxisGeoKey

This key is provided to specify the second defining parameter of a user-defined bi-axial ellipsoid or of a user-defined sphere. It allows the specification of the ellipsoid semi-minor axis (b) or the sphere’s radius.




Note


In GeoTIFF 1.0 this key was called GeogSemiMinorAxisGeoKey.




EllipsoidInvFlatteningGeoKey

This key is provided to specify the second defining parameter of a user-defined bi-axial ellipsoid. It allows the specification of the ellipsoid inverse flattening (1/f). It is a ratio and does not require a unit.




Note


In GeoTIFF 1.0 this key was called GeogInvFlatteningGeoKey.</skos:definition>
    <rdf:type rdf:resource="http://www.opengis.net/def/ont/modspec/RequirementClass"/>
    <rdf:type rdf:resource="http://www.w3.org/2004/02/skos/core#Concept"/>
    <skos:prefLabel>Requirements Class Ellipsoid parameter GeoKeys</skos:prefLabel>
  </rdf:Description>
  <rdf:Description rdf:about="http://www.opengis.net/spec/GeoTIFF/1.1/req/VerticalGeoKey.type">
    <dct:description>The VerticalGeoKey SHALL have type = SHORT</dct:description>
    <rdf:type rdf:resource="http://www.w3.org/2004/02/skos/core#Concept"/>
    <rdf:type rdf:resource="http://www.opengis.net/def/ont/modspec/Requirement"/>
    <skos:prefLabel>Requirement 14.2</skos:prefLabel>
    <skos:definition>The VerticalGeoKey SHALL have type = SHORT</skos:definition>
    <skos:broader rdf:resource="http://www.opengis.net/spec/GeoTIFF/1.1/req/VerticalGeoKey"/>
  </rdf:Description>
  <rdf:Description rdf:about="http://www.opengis.net/spec/GeoTIFF/1.1/req/GeoDoubleParamsTag.ID">
    <skos:broader rdf:resource="http://www.opengis.net/spec/GeoTIFF/1.1/conf/DoubleParameters"/>
    <skos:broader rdf:resource="http://www.opengis.net/spec/GeoTIFF/1.1/req/GeoDoubleParamsTag"/>
    <skos:broader rdf:resource="http://www.opengis.net/spec/GeoTIFF/1.1/conf/TIFF.Tags"/>
    <rdf:type rdf:resource="http://www.opengis.net/def/ont/modspec/Requirement"/>
    <rdf:type rdf:resource="http://www.w3.org/2004/02/skos/core#Concept"/>
    <skos:definition>The GeoDoubleParamsTag SHALL have ID = 34736</skos:definition>
    <dct:description>The GeoDoubleParamsTag SHALL have ID = 34736</dct:description>
    <skos:prefLabel>Requirement 5.1</skos:prefLabel>
  </rdf:Description>
  <rdf:Description rdf:about="http://www.opengis.net/spec/GeoTIFF/1.1/req/PrimeMeridianLongitudeGeoKey">
    <skos:narrower rdf:resource="http://www.opengis.net/spec/GeoTIFF/1.1/req/PrimeMeridianLongitudeGeoKey.ID"/>
    <skos:narrower rdf:resource="http://www.opengis.net/spec/GeoTIFF/1.1/req/PrimeMeridianLongitudeGeoKey.units"/>
    <skos:narrower rdf:resource="http://www.opengis.net/spec/GeoTIFF/1.1/req/PrimeMeridianLongitudeGeoKey.type"/>
    <skos:definition>This key allows definition of a user-defined Prime Meridian, the location of which is defined by its longitude relative to the international reference meridian (for the earth this is Greenwich).




Note


In GeoTIFF 1.0 this key was called GeogPrimeMeridianLongGeoKey.</skos:definition>
    <skos:broader rdf:resource="http://www.opengis.net/def/docs/19-008r4"/>
    <skos:broader rdf:resource="http://www.opengis.net/spec/GeoTIFF/1.1/conf/DoubleParameters"/>
    <rdf:type rdf:resource="http://www.w3.org/2004/02/skos/core#Concept"/>
    <rdf:type rdf:resource="http://www.opengis.net/def/ont/modspec/RequirementClass"/>
    <spec:normativeStatement rdf:resource="http://www.opengis.net/spec/GeoTIFF/1.1/req/PrimeMeridianLongitudeGeoKey.ID"/>
    <spec:normativeStatement rdf:resource="http://www.opengis.net/spec/GeoTIFF/1.1/req/PrimeMeridianLongitudeGeoKey.units"/>
    <spec:normativeStatement rdf:resource="http://www.opengis.net/spec/GeoTIFF/1.1/req/PrimeMeridianLongitudeGeoKey.type"/>
    <skos:prefLabel>Requirements Class PrimeMeridianLongitudeGeoKey</skos:prefLabel>
  </rdf:Description>
  <rdf:Description rdf:about="http://www.opengis.net/spec/GeoTIFF/1.1/req/EllipsoidInvFlatteningGeoKey.type">
    <dct:description>The EllipsoidInvFlatteningGeoKey SHALL have type = DOUBLE</dct:description>
    <rdf:type rdf:resource="http://www.opengis.net/def/ont/modspec/Requirement"/>
    <rdf:type rdf:resource="http://www.w3.org/2004/02/skos/core#Concept"/>
    <skos:definition>The EllipsoidInvFlatteningGeoKey SHALL have type = DOUBLE</skos:definition>
    <skos:prefLabel>Requirement 24.2</skos:prefLabel>
    <skos:broader rdf:resource="http://www.opengis.net/spec/GeoTIFF/1.1/req/EllipsoidSemiMajorAxisGeoKey"/>
  </rdf:Description>
  <rdf:Description rdf:about="http://www.opengis.net/spec/GeoTIFF/1.1/req/PrimeMeridianGeoKey.userdefined">
    <dct:description>If the PrimeMeridianGeoKey value is 32767 (User-Defined) then the
GeodeticCitationGeoKey, and PrimeMeridianLongGeoKey SHALL be populated</dct:description>
    <rdf:type rdf:resource="http://www.opengis.net/def/ont/modspec/Requirement"/>
    <rdf:type rdf:resource="http://www.w3.org/2004/02/skos/core#Concept"/>
    <skos:broader rdf:resource="http://www.opengis.net/spec/GeoTIFF/1.1/req/PrimeMeridianGeoKey"/>
    <skos:definition>If the PrimeMeridianGeoKey value is 32767 (User-Defined) then the
GeodeticCitationGeoKey, and PrimeMeridianLongGeoKey SHALL be populated</skos:definition>
    <skos:prefLabel>Requirement 19.5</skos:prefLabel>
  </rdf:Description>
  <rdf:Description rdf:about="http://www.opengis.net/spec/GeoTIFF/1.1/req/UnitsGeoKey.reserved">
    <skos:broader rdf:resource="http://www.opengis.net/spec/GeoTIFF/1.1/req/UnitsGeoKey"/>
    <rdf:type rdf:resource="http://www.opengis.net/def/ont/modspec/Requirement"/>
    <rdf:type rdf:resource="http://www.w3.org/2004/02/skos/core#Concept"/>
    <skos:definition>GeogAngularUnitsGeoKey, GeogAzimuthUnitsGeoKey, GeogLinearUnitsGeoKey,
ProjLinearUnitsGeoKey and VerticalUnitsGeoKey values in the range 1-1023 SHALL
be reserved.NOTE: In GeoTIFF v1.0 the range 0001-2000 was used for obsolete
GeoTIFF codes.</skos:definition>
    <dct:description>GeogAngularUnitsGeoKey, GeogAzimuthUnitsGeoKey, GeogLinearUnitsGeoKey,
ProjLinearUnitsGeoKey and VerticalUnitsGeoKey values in the range 1-1023 SHALL
be reserved.NOTE: In GeoTIFF v1.0 the range 0001-2000 was used for obsolete
GeoTIFF codes.</dct:description>
    <skos:prefLabel>Requirement 16.3</skos:prefLabel>
  </rdf:Description>
  <rdf:Description rdf:about="http://www.opengis.net/spec/GeoTIFF/1.1/conf/DoubleParameters">
    <spec:requirement rdf:resource="http://www.opengis.net/spec/GeoTIFF/1.1/req/ProjLinearParameterGeoKey"/>
    <spec:requirement rdf:resource="http://www.opengis.net/spec/GeoTIFF/1.1/req/GeoKeyDirectoryTag.keyEntryValueOffset"/>
    <spec:requirement rdf:resource="http://www.opengis.net/spec/GeoTIFF/1.1/req/ProjAngularParameterGeoKey"/>
    <spec:requirement rdf:resource="http://www.opengis.net/spec/GeoTIFF/1.1/req/GeoDoubleParamsTag.count"/>
    <spec:requirement rdf:resource="http://www.opengis.net/spec/GeoTIFF/1.1/req/ProjAzimuthAngleGeoKey"/>
    <spec:requirement rdf:resource="http://www.opengis.net/spec/GeoTIFF/1.1/req/GeoKeyDirectoryTag.keyEntryTIFFTagLocation"/>
    <spec:requirement rdf:resource="http://www.opengis.net/spec/GeoTIFF/1.1/req/UnitSizeGeoKey"/>
    <spec:requirement rdf:resource="http://www.opengis.net/spec/GeoTIFF/1.1/req/GeoDoubleParamsTag.ID"/>
    <spec:requirement rdf:resource="http://www.opengis.net/spec/GeoTIFF/1.1/req/PrimeMeridianLongitudeGeoKey"/>
    <spec:requirement rdf:resource="http://www.opengis.net/spec/GeoTIFF/1.1/req/EllipsoidSemiMajorAxisGeoKey"/>
    <spec:requirement rdf:resource="http://www.opengis.net/spec/GeoTIFF/1.1/req/EllipsoidInvFlatteningGeoKey"/>
    <spec:requirement rdf:resource="http://www.opengis.net/spec/GeoTIFF/1.1/req/GeoKeyDirectoryTag.keyEntryKeyCount"/>
    <spec:requirement rdf:resource="http://www.opengis.net/spec/GeoTIFF/1.1/req/ProjScalarParameterGeoKey"/>
    <spec:requirement rdf:resource="http://www.opengis.net/spec/GeoTIFF/1.1/req/GeoKeyDirectoryTag.KeyEntry.ID"/>
    <spec:requirement rdf:resource="http://www.opengis.net/spec/GeoTIFF/1.1/req/EllipsoidSemiMinorAxisGeoKey"/>
    <spec:purpose>Verify Double parameters</spec:purpose>
    <rdf:type rdf:resource="http://www.w3.org/2004/02/skos/core#Concept"/>
    <rdf:type rdf:resource="http://www.opengis.net/def/ont/modspec/ConformanceTest"/>
    <skos:narrower rdf:resource="http://www.opengis.net/spec/GeoTIFF/1.1/req/ProjLinearParameterGeoKey"/>
    <skos:narrower rdf:resource="http://www.opengis.net/spec/GeoTIFF/1.1/req/GeoKeyDirectoryTag.keyEntryValueOffset"/>
    <skos:narrower rdf:resource="http://www.opengis.net/spec/GeoTIFF/1.1/req/ProjAngularParameterGeoKey"/>
    <skos:narrower rdf:resource="http://www.opengis.net/spec/GeoTIFF/1.1/req/GeoDoubleParamsTag.count"/>
    <skos:narrower rdf:resource="http://www.opengis.net/spec/GeoTIFF/1.1/req/ProjAzimuthAngleGeoKey"/>
    <skos:narrower rdf:resource="http://www.opengis.net/spec/GeoTIFF/1.1/req/GeoKeyDirectoryTag.keyEntryTIFFTagLocation"/>
    <skos:narrower rdf:resource="http://www.opengis.net/spec/GeoTIFF/1.1/req/EllipsoidInvFlatteningGeoKey"/>
    <skos:narrower rdf:resource="http://www.opengis.net/spec/GeoTIFF/1.1/req/UnitSizeGeoKey"/>
    <skos:narrower rdf:resource="http://www.opengis.net/spec/GeoTIFF/1.1/req/GeoKeyDirectoryTag.keyEntryKeyCount"/>
    <skos:narrower rdf:resource="http://www.opengis.net/spec/GeoTIFF/1.1/req/GeoDoubleParamsTag.ID"/>
    <skos:narrower rdf:resource="http://www.opengis.net/spec/GeoTIFF/1.1/req/PrimeMeridianLongitudeGeoKey"/>
    <skos:narrower rdf:resource="http://www.opengis.net/spec/GeoTIFF/1.1/req/EllipsoidSemiMajorAxisGeoKey"/>
    <skos:narrower rdf:resource="http://www.opengis.net/spec/GeoTIFF/1.1/req/EllipsoidSemiMinorAxisGeoKey"/>
    <skos:narrower rdf:resource="http://www.opengis.net/spec/GeoTIFF/1.1/req/ProjScalarParameterGeoKey"/>
    <skos:narrower rdf:resource="http://www.opengis.net/spec/GeoTIFF/1.1/req/GeoKeyDirectoryTag.KeyEntry.ID"/>
    <spec:testType rdf:resource="http://www.opengis.net/def/ont/modspec/Basic"/>
    <spec:method>Pre-conditions

The GeoKeyDirectory, DoubleValues and GeoKeyOffset values have been set.

Text Variables

**Variable**

|

**Scope**

|

**Description**

---|---|---

GeoKeyDirectory

|

Global

|

Location of the GeoTIFF GeoKey directory

DoubleValues

|

Global

|

Location of the Double values for GeoTIFF Double GeoKeys

GeoKeyOffset

|

Parameter

|

Location of this Key Entry Set in the GeoKey directory

GeoKey

|

Local

|

Temporary value of the GeoKey

KeyLength

|

Local

|

Temporary value for the length of the value for the GeoKey

KeyValueOffset

|

Local

|

The location of the GeoKey value in the file


    Locate the Key Entry Set using the GeoKeyDirectory and GeoKeyOffset values.


    Process the second Short integer in the Key Entry Set
        {
        IF value != 34736 THEN error out
        }
    Process the first Short integer in the Key Entry Set
        {
        Set GeoKey to the value
        }
    Process the third Short integer in the Key Entry Set
        {
        Set KeyLength to the value
        }
    Process the fourth Short integer in the Key Entry Set
        {
        SET KeyValueOffset to the value
        }
    SET KeyValueOffset = DoubleValues + (KeyValueOffset * 8)


    Read a KeyLength Double values from the GeoTIFF file starting at KeyValueOffset.
    Validate the value
        Locate the GeoKey in the following table
        Verify that the values read satisfy the constraints defined in the associated Requirements Class.
        Verify that any GeoKeys required by the associated Requirements Class are present in the GeoKey Directory.

Double GeoKey Tests</spec:method>
    <spec:method rdf:datatype="http://www.w3.org/1999/02/22-rdf-syntax-ns#HTML">%3Cdiv%3E%3Cdiv%3EPre-conditions%3Cdiv%3E%3Cdiv%3EThe%20GeoKeyDirectory%2C%20DoubleValues%20and%20GeoKeyOffset%20values%20have%20been%20set.%3C/div%3E%3C/div%3E%3Cdiv%20class%3D%22literalblock%22%3E%0A%3Cdiv%20class%3D%22content%22%3E%0A%3Cpre%3ELocate%20the%20Key%20Entry%20Set%20using%20the%20GeoKeyDirectory%20and%20GeoKeyOffset%20values.%3C/pre%3E%0A%3C/div%3E%0A%3C/div%3E%3Cdiv%20class%3D%22literalblock%22%3E%0A%3Cdiv%20class%3D%22content%22%3E%0A%3Cpre%3EProcess%20the%20second%20Short%20integer%20in%20the%20Key%20Entry%20Set%0A%20%20%20%20%7B%0A%20%20%20%20IF%20value%20%21%3D%2034736%20THEN%20error%20out%0A%20%20%20%20%7D%0AProcess%20the%20first%20Short%20integer%20in%20the%20Key%20Entry%20Set%0A%20%20%20%20%7B%0A%20%20%20%20Set%20GeoKey%20to%20the%20value%0A%20%20%20%20%7D%0AProcess%20the%20third%20Short%20integer%20in%20the%20Key%20Entry%20Set%0A%20%20%20%20%7B%0A%20%20%20%20Set%20KeyLength%20to%20the%20value%0A%20%20%20%20%7D%0AProcess%20the%20fourth%20Short%20integer%20in%20the%20Key%20Entry%20Set%0A%20%20%20%20%7B%0A%20%20%20%20SET%20KeyValueOffset%20to%20the%20value%0A%20%20%20%20%7D%0ASET%20KeyValueOffset%20%3D%20DoubleValues%20%2B%20%28KeyValueOffset%20%2A%208%29%3C/pre%3E%0A%3C/div%3E%0A%3C/div%3E%3Cdiv%20class%3D%22literalblock%22%3E%0A%3Cdiv%20class%3D%22content%22%3E%0A%3Cpre%3ERead%20a%20KeyLength%20Double%20values%20from%20the%20GeoTIFF%20file%20starting%20at%20KeyValueOffset.%0AValidate%20the%20value%0A%20%20%20%20Locate%20the%20GeoKey%20in%20the%20following%20table%0A%20%20%20%20Verify%20that%20the%20values%20read%20satisfy%20the%20constraints%20defined%20in%20the%20associated%20Requirements%20Class.%0A%20%20%20%20Verify%20that%20any%20GeoKeys%20required%20by%20the%20associated%20Requirements%20Class%20are%20present%20in%20the%20GeoKey%20Directory.%3C/pre%3E%0A%3C/div%3E%0A%3C/div%3E%3Cdiv%20class%3D%22paragraph%22%3E%0A%3Cp%3EDouble%20GeoKey%20Tests%3C/p%3E%0A%3C/div%3E</spec:method>
    <skos:broader rdf:resource="http://www.opengis.net/spec/GeoTIFF/1.1/conf/Core"/>
    <skos:definition>Double Parameters Test</skos:definition>
    <skos:prefLabel>Double Parameters Test</skos:prefLabel>
  </rdf:Description>
  <rdf:Description rdf:about="http://www.opengis.net/spec/GeoTIFF/1.1/req/GeoDoubleParamsTag">
    <skos:narrower rdf:resource="http://www.opengis.net/spec/GeoTIFF/1.1/req/GeoDoubleParamsTag.ID"/>
    <skos:narrower rdf:resource="http://www.opengis.net/spec/GeoTIFF/1.1/req/GeoDoubleParamsTag.count"/>
    <rdf:type rdf:resource="http://www.w3.org/2004/02/skos/core#Concept"/>
    <rdf:type rdf:resource="http://www.opengis.net/def/ont/modspec/RequirementClass"/>
    <spec:normativeStatement rdf:resource="http://www.opengis.net/spec/GeoTIFF/1.1/req/GeoDoubleParamsTag.count"/>
    <spec:normativeStatement rdf:resource="http://www.opengis.net/spec/GeoTIFF/1.1/req/GeoDoubleParamsTag.ID"/>
    <skos:prefLabel>Requirements Class GeoDoubleParamsTag</skos:prefLabel>
    <skos:definition>The following requirements govern the storage of parameter values when the values are of type Double.</skos:definition>
    <skos:broader rdf:resource="http://www.opengis.net/def/docs/19-008r4"/>
  </rdf:Description>
  <rdf:Description rdf:about="http://www.opengis.net/spec/GeoTIFF/1.1/req/ProjMethodGeoKey.ID">
    <rdf:type rdf:resource="http://www.opengis.net/def/ont/modspec/Requirement"/>
    <rdf:type rdf:resource="http://www.w3.org/2004/02/skos/core#Concept"/>
    <skos:broader rdf:resource="http://www.opengis.net/spec/GeoTIFF/1.1/req/ProjMethodGeoKey"/>
    <skos:prefLabel>Requirement 27.1</skos:prefLabel>
    <dct:description>The ProjMethodGeoKey SHALL have ID = 3075</dct:description>
    <skos:definition>The ProjMethodGeoKey SHALL have ID = 3075</skos:definition>
  </rdf:Description>
  <rdf:Description rdf:about="http://www.opengis.net/spec/GeoTIFF/1.1/req/GTModelTypeGeoKey.userdefined">
    <skos:prefLabel>Requirement 8.10</skos:prefLabel>
    <skos:definition>If the GTModelTypeGeoKey value is 32767 (user-defined) then the
GTCitationGeoKey SHALL be populated.</skos:definition>
    <skos:broader rdf:resource="http://www.opengis.net/spec/GeoTIFF/1.1/req/GTModelTypeGeoKey"/>
    <rdf:type rdf:resource="http://www.w3.org/2004/02/skos/core#Concept"/>
    <rdf:type rdf:resource="http://www.opengis.net/def/ont/modspec/Requirement"/>
    <dct:description>If the GTModelTypeGeoKey value is 32767 (user-defined) then the
GTCitationGeoKey SHALL be populated.</dct:description>
  </rdf:Description>
  <rdf:Description rdf:about="http://www.opengis.net/spec/GeoTIFF/1.1/req/GeoKeyDirectoryTag.keyEntryKeyID">
    <dct:description>The first unsigned short integer in the Key Entry SHALL hold the key
identifier.</dct:description>
    <rdf:type rdf:resource="http://www.w3.org/2004/02/skos/core#Concept"/>
    <rdf:type rdf:resource="http://www.opengis.net/def/ont/modspec/Requirement"/>
    <skos:broader rdf:resource="http://www.opengis.net/spec/GeoTIFF/1.1/req/GeoKeyDirectoryTag"/>
    <skos:broader rdf:resource="http://www.opengis.net/spec/GeoTIFF/1.1/conf/GeoKeyDirectory"/>
    <skos:definition>The first unsigned short integer in the Key Entry SHALL hold the key
identifier.</skos:definition>
    <skos:prefLabel>Requirement 2.13</skos:prefLabel>
  </rdf:Description>
  <rdf:Description rdf:about="http://www.opengis.net/spec/GeoTIFF/1.1/req/ModelPixelScaleTag">
    <skos:broader rdf:resource="http://www.opengis.net/def/docs/19-008r4"/>
    <skos:narrower rdf:resource="http://www.opengis.net/spec/GeoTIFF/1.1/req/ModelPixelScaleTag.axisReversal"/>
    <skos:narrower rdf:resource="http://www.opengis.net/spec/GeoTIFF/1.1/req/ModelPixelScaleTag.count"/>
    <skos:narrower rdf:resource="http://www.opengis.net/spec/GeoTIFF/1.1/req/ModelPixelScaleTag.type"/>
    <skos:narrower rdf:resource="http://www.opengis.net/spec/GeoTIFF/1.1/req/ModelPixelScaleTag.ID"/>
    <skos:narrower rdf:resource="http://www.opengis.net/spec/GeoTIFF/1.1/req/ModelPixelScaleTag.standardConvention"/>
    <rdf:type rdf:resource="http://www.w3.org/2004/02/skos/core#Concept"/>
    <rdf:type rdf:resource="http://www.opengis.net/def/ont/modspec/RequirementClass"/>
    <spec:normativeStatement rdf:resource="http://www.opengis.net/spec/GeoTIFF/1.1/req/ModelPixelScaleTag.type"/>
    <spec:normativeStatement rdf:resource="http://www.opengis.net/spec/GeoTIFF/1.1/req/ModelPixelScaleTag.axisReversal"/>
    <spec:normativeStatement rdf:resource="http://www.opengis.net/spec/GeoTIFF/1.1/req/ModelPixelScaleTag.count"/>
    <spec:normativeStatement rdf:resource="http://www.opengis.net/spec/GeoTIFF/1.1/req/ModelPixelScaleTag.standardConvention"/>
    <spec:normativeStatement rdf:resource="http://www.opengis.net/spec/GeoTIFF/1.1/req/ModelPixelScaleTag.ID"/>
    <skos:prefLabel>Requirements Class ModelPixelScaleTag</skos:prefLabel>
    <skos:definition></skos:definition>
  </rdf:Description>
  <rdf:Description rdf:about="http://www.opengis.net/spec/GeoTIFF/1.1/req/PrimeMeridianGeoKey.reserved">
    <skos:definition>PrimeMeridianGeoKey values in the range 1-1023 SHALL be reservedNOTE: In
GeoTIFF v1.0 the range was 101-7999 and 9000-32766</skos:definition>
    <skos:prefLabel>Requirement 19.3</skos:prefLabel>
    <rdf:type rdf:resource="http://www.opengis.net/def/ont/modspec/Requirement"/>
    <rdf:type rdf:resource="http://www.w3.org/2004/02/skos/core#Concept"/>
    <skos:broader rdf:resource="http://www.opengis.net/spec/GeoTIFF/1.1/req/PrimeMeridianGeoKey"/>
    <dct:description>PrimeMeridianGeoKey values in the range 1-1023 SHALL be reservedNOTE: In
GeoTIFF v1.0 the range was 101-7999 and 9000-32766</dct:description>
  </rdf:Description>
  <rdf:Description rdf:about="http://www.opengis.net/spec/GeoTIFF/1.1/req/EllipsoidGeoKey">
    <skos:narrower rdf:resource="http://www.opengis.net/spec/GeoTIFF/1.1/req/EllipsoidGeoKey.ID"/>
    <skos:narrower rdf:resource="http://www.opengis.net/spec/GeoTIFF/1.1/req/EllipsoidGeoKey.user-defined"/>
    <skos:narrower rdf:resource="http://www.opengis.net/spec/GeoTIFF/1.1/req/EllipsoidGeoKey.type"/>
    <skos:narrower rdf:resource="http://www.opengis.net/spec/GeoTIFF/1.1/req/EllipsoidGeoKey.EPSG"/>
    <skos:narrower rdf:resource="http://www.opengis.net/spec/GeoTIFF/1.1/req/EllipsoidGeoKey.reserved"/>
    <skos:narrower rdf:resource="http://www.opengis.net/spec/GeoTIFF/1.1/req/EllipsoidGeoKey.private"/>
    <skos:broader rdf:resource="http://www.opengis.net/def/docs/19-008r4"/>
    <skos:broader rdf:resource="http://www.opengis.net/spec/GeoTIFF/1.1/conf/ShortParameters"/>
    <spec:normativeStatement rdf:resource="http://www.opengis.net/spec/GeoTIFF/1.1/req/EllipsoidGeoKey.private"/>
    <spec:normativeStatement rdf:resource="http://www.opengis.net/spec/GeoTIFF/1.1/req/EllipsoidGeoKey.ID"/>
    <spec:normativeStatement rdf:resource="http://www.opengis.net/spec/GeoTIFF/1.1/req/EllipsoidGeoKey.reserved"/>
    <spec:normativeStatement rdf:resource="http://www.opengis.net/spec/GeoTIFF/1.1/req/EllipsoidGeoKey.type"/>
    <spec:normativeStatement rdf:resource="http://www.opengis.net/spec/GeoTIFF/1.1/req/EllipsoidGeoKey.EPSG"/>
    <spec:normativeStatement rdf:resource="http://www.opengis.net/spec/GeoTIFF/1.1/req/EllipsoidGeoKey.user-defined"/>
    <rdf:type rdf:resource="http://www.w3.org/2004/02/skos/core#Concept"/>
    <rdf:type rdf:resource="http://www.opengis.net/def/ont/modspec/RequirementClass"/>
    <skos:definition>This key is provided to specify an ellipsoid (or sphere) from the GeoTIFF CRS register or to indicate that the ellipsoid (or sphere) is user-defined.




Note


In GeoTIFF 1.0 this key was called GeogEllipsoidGeoKey.</skos:definition>
    <skos:prefLabel>Requirements Class EllipsoidGeoKey</skos:prefLabel>
  </rdf:Description>
  <rdf:Description rdf:about="http://www.opengis.net/spec/GeoTIFF/1.1/req/GeodeticCRSGeoKey">
    <spec:normativeStatement rdf:resource="http://www.opengis.net/spec/GeoTIFF/1.1/req/GeodeticCRSGeoKey.user-defined"/>
    <spec:normativeStatement rdf:resource="http://www.opengis.net/spec/GeoTIFF/1.1/req/GeodeticCRSGeoKey.EPSG"/>
    <spec:normativeStatement rdf:resource="http://www.opengis.net/spec/GeoTIFF/1.1/req/GeodeticCRSGeoKey.ID"/>
    <spec:normativeStatement rdf:resource="http://www.opengis.net/spec/GeoTIFF/1.1/req/GeodeticCRSGeoKey.reserved"/>
    <spec:normativeStatement rdf:resource="http://www.opengis.net/spec/GeoTIFF/1.1/req/GeodeticCRSGeoKey.private"/>
    <spec:normativeStatement rdf:resource="http://www.opengis.net/spec/GeoTIFF/1.1/req/GeodeticCRSGeoKey.type"/>
    <skos:broader rdf:resource="http://www.opengis.net/def/docs/19-008r4"/>
    <skos:broader rdf:resource="http://www.opengis.net/spec/GeoTIFF/1.1/conf/ShortParameters"/>
    <skos:narrower rdf:resource="http://www.opengis.net/spec/GeoTIFF/1.1/req/GeodeticCRSGeoKey.EPSG"/>
    <skos:narrower rdf:resource="http://www.opengis.net/spec/GeoTIFF/1.1/req/GeodeticCRSGeoKey.type"/>
    <skos:narrower rdf:resource="http://www.opengis.net/spec/GeoTIFF/1.1/req/GeodeticCRSGeoKey.user-defined"/>
    <skos:narrower rdf:resource="http://www.opengis.net/spec/GeoTIFF/1.1/req/GeodeticCRSGeoKey.private"/>
    <skos:narrower rdf:resource="http://www.opengis.net/spec/GeoTIFF/1.1/req/GeodeticCRSGeoKey.ID"/>
    <skos:narrower rdf:resource="http://www.opengis.net/spec/GeoTIFF/1.1/req/GeodeticCRSGeoKey.reserved"/>
    <rdf:type rdf:resource="http://www.w3.org/2004/02/skos/core#Concept"/>
    <rdf:type rdf:resource="http://www.opengis.net/def/ont/modspec/RequirementClass"/>
    <skos:prefLabel>Requirements Class GeodeticCRSGeoKey</skos:prefLabel>
    <skos:definition>This key is provided to specify the geodetic (geographic or geocentric) coordinate reference system from the GeoTIFF CRS register or to indicate that the Model CRS is a user-defined geodetic coordinate reference system.




Note


In GeoTIFF 1.0 this key was called GeographicTypeGeoKey. Geodetic CRS is a superset of geographic 2D CRS, geographic 3D CRS and geocentric (earth-centred 3D Cartesian) CRS.</skos:definition>
  </rdf:Description>
  <rdf:Description rdf:about="http://www.opengis.net/spec/GeoTIFF/1.1/req/GeodeticDatumGeoKey.ID">
    <dct:description>The GeodeticDatumGeoKey SHALL have ID = 2050</dct:description>
    <skos:prefLabel>Requirement 18.1</skos:prefLabel>
    <rdf:type rdf:resource="http://www.w3.org/2004/02/skos/core#Concept"/>
    <rdf:type rdf:resource="http://www.opengis.net/def/ont/modspec/Requirement"/>
    <skos:definition>The GeodeticDatumGeoKey SHALL have ID = 2050</skos:definition>
    <skos:broader rdf:resource="http://www.opengis.net/spec/GeoTIFF/1.1/req/GeodeticDatumGeoKey"/>
  </rdf:Description>
  <rdf:Description rdf:about="http://www.opengis.net/spec/GeoTIFF/1.1/req/GTRasterTypeGeoKey">
    <rdf:type rdf:resource="http://www.w3.org/2004/02/skos/core#Concept"/>
    <rdf:type rdf:resource="http://www.opengis.net/def/ont/modspec/RequirementClass"/>
    <spec:normativeStatement rdf:resource="http://www.opengis.net/spec/GeoTIFF/1.1/req/GTRasterTypeGeoKey.ID"/>
    <spec:normativeStatement rdf:resource="http://www.opengis.net/spec/GeoTIFF/1.1/req/GTRasterTypeGeoKey.reserved"/>
    <spec:normativeStatement rdf:resource="http://www.opengis.net/spec/GeoTIFF/1.1/req/GTRasterTypeGeoKey.type"/>
    <spec:normativeStatement rdf:resource="http://www.opengis.net/spec/GeoTIFF/1.1/req/GTRasterTypeGeoKey.value"/>
    <spec:normativeStatement rdf:resource="http://www.opengis.net/spec/GeoTIFF/1.1/req/GTRasterTypeGeoKey.private"/>
    <skos:narrower rdf:resource="http://www.opengis.net/spec/GeoTIFF/1.1/req/GTRasterTypeGeoKey.ID"/>
    <skos:narrower rdf:resource="http://www.opengis.net/spec/GeoTIFF/1.1/req/GTRasterTypeGeoKey.reserved"/>
    <skos:narrower rdf:resource="http://www.opengis.net/spec/GeoTIFF/1.1/req/GTRasterTypeGeoKey.value"/>
    <skos:narrower rdf:resource="http://www.opengis.net/spec/GeoTIFF/1.1/req/GTRasterTypeGeoKey.type"/>
    <skos:narrower rdf:resource="http://www.opengis.net/spec/GeoTIFF/1.1/req/GTRasterTypeGeoKey.private"/>
    <skos:broader rdf:resource="http://www.opengis.net/spec/GeoTIFF/1.1/conf/ShortParameters"/>
    <skos:broader rdf:resource="http://www.opengis.net/def/docs/19-008r4"/>
    <skos:prefLabel>Requirements Class GTRasterTypeGeoKey</skos:prefLabel>
    <skos:definition>This requirements class establishes the Raster Space used. There are currently only two options: RasterPixelIsPoint and RasterPixelIsArea. No user-defined raster spaces are currently supported. For variance in imaging display parameters, such as pixel aspect-ratios, use the standard TIFF 6.0 device-space tags.

The use of this geokey is highly recommended for accurate georeferencing of raster.</skos:definition>
  </rdf:Description>
  <rdf:Description rdf:about="http://www.opengis.net/spec/GeoTIFF/1.1/req/ModelTransformationTag.type">
    <rdf:type rdf:resource="http://www.opengis.net/def/ont/modspec/Requirement"/>
    <rdf:type rdf:resource="http://www.w3.org/2004/02/skos/core#Concept"/>
    <skos:definition>The ModelTransformationTag SHALL have type = DOUBLE</skos:definition>
    <skos:broader rdf:resource="http://www.opengis.net/spec/GeoTIFF/1.1/conf/TIFF.Tags"/>
    <skos:broader rdf:resource="http://www.opengis.net/spec/GeoTIFF/1.1/req/ModelTransformationTag"/>
    <skos:prefLabel>Requirement 11.2</skos:prefLabel>
    <dct:description>The ModelTransformationTag SHALL have type = DOUBLE</dct:description>
  </rdf:Description>
  <rdf:Description rdf:about="http://www.opengis.net/spec/GeoTIFF/1.1/req/ProjMethodGeoKey.reserved">
    <skos:prefLabel>Requirement 27.4</skos:prefLabel>
    <rdf:type rdf:resource="http://www.opengis.net/def/ont/modspec/Requirement"/>
    <rdf:type rdf:resource="http://www.w3.org/2004/02/skos/core#Concept"/>
    <skos:broader rdf:resource="http://www.opengis.net/spec/GeoTIFF/1.1/req/ProjMethodGeoKey"/>
    <dct:description>ProjMethodGeoKey values in the range 28-32766 SHALL be reserved</dct:description>
    <skos:definition>ProjMethodGeoKey values in the range 28-32766 SHALL be reserved</skos:definition>
  </rdf:Description>
  <rdf:Description rdf:about="http://www.opengis.net/spec/GeoTIFF/1.1/req/Core">
    <spec:normativeStatement rdf:resource="http://www.opengis.net/spec/GeoTIFF/1.1/req/DataTypes"/>
    <spec:normativeStatement rdf:resource="http://www.opengis.net/spec/GeoTIFF/1.1/req/TIFF"/>
    <spec:normativeStatement rdf:resource="http://www.opengis.net/spec/GeoTIFF/1.1/req/ByteOrder"/>
    <spec:normativeStatement rdf:resource="http://www.opengis.net/spec/GeoTIFF/1.1/req/DataGeoTags"/>
    <spec:normativeStatement rdf:resource="http://www.opengis.net/spec/GeoTIFF/1.1/req/TagSort"/>
    <spec:normativeStatement rdf:resource="http://www.opengis.net/spec/GeoTIFF/1.1/req/GeoKeySort"/>
    <skos:narrower rdf:resource="http://www.opengis.net/spec/GeoTIFF/1.1/req/GeoKeySort"/>
    <skos:narrower rdf:resource="http://www.opengis.net/spec/GeoTIFF/1.1/req/DataTypes"/>
    <skos:narrower rdf:resource="http://www.opengis.net/spec/GeoTIFF/1.1/req/TIFF"/>
    <skos:narrower rdf:resource="http://www.opengis.net/spec/GeoTIFF/1.1/req/DataGeoTags"/>
    <skos:narrower rdf:resource="http://www.opengis.net/spec/GeoTIFF/1.1/req/ByteOrder"/>
    <skos:narrower rdf:resource="http://www.opengis.net/spec/GeoTIFF/1.1/req/TagSort"/>
    <skos:broader rdf:resource="http://www.opengis.net/def/docs/19-008r4"/>
    <rdf:type rdf:resource="http://www.w3.org/2004/02/skos/core#Concept"/>
    <rdf:type rdf:resource="http://www.opengis.net/def/ont/modspec/RequirementClass"/>
    <skos:definition>A GeoTIFF file is a valid TIFF 6.0 file.</skos:definition>
    <skos:prefLabel>Requirements Class TIFF</skos:prefLabel>
  </rdf:Description>
  <rdf:Description rdf:about="http://www.opengis.net/spec/GeoTIFF/1.1/req/ProjectedCRSGeoKey.private">
    <skos:definition>ProjectedCRSGeoKey values in the range 32768-65535 SHALL be private</skos:definition>
    <rdf:type rdf:resource="http://www.w3.org/2004/02/skos/core#Concept"/>
    <rdf:type rdf:resource="http://www.opengis.net/def/ont/modspec/Requirement"/>
    <skos:broader rdf:resource="http://www.opengis.net/spec/GeoTIFF/1.1/req/ProjectedCRSGeoKey"/>
    <skos:prefLabel>Requirement 12.6</skos:prefLabel>
    <dct:description>ProjectedCRSGeoKey values in the range 32768-65535 SHALL be private</dct:description>
  </rdf:Description>
  <rdf:Description rdf:about="http://www.opengis.net/spec/GeoTIFF/1.1/req/GeoKeyDirectoryTag.keyRevision">
    <skos:broader rdf:resource="http://www.opengis.net/spec/GeoTIFF/1.1/conf/GeoKeyDirectory"/>
    <skos:broader rdf:resource="http://www.opengis.net/spec/GeoTIFF/1.1/req/GeoKeyDirectoryTag"/>
    <rdf:type rdf:resource="http://www.w3.org/2004/02/skos/core#Concept"/>
    <rdf:type rdf:resource="http://www.opengis.net/def/ont/modspec/Requirement"/>
    <dct:description>The second unsigned short integer in the GeoKeyDirectoryTag SHALL hold the
KeyRevision.</dct:description>
    <skos:definition>The second unsigned short integer in the GeoKeyDirectoryTag SHALL hold the
KeyRevision.</skos:definition>
    <skos:prefLabel>Requirement 2.6</skos:prefLabel>
  </rdf:Description>
  <rdf:Description rdf:about="http://www.opengis.net/spec/GeoTIFF/1.1/conf/Core">
    <skos:broader rdf:resource="http://www.opengis.net/spec/GeoTIFF/1.1/csuite"/>
    <spec:conformanceTest rdf:resource="http://www.opengis.net/spec/GeoTIFF/1.1/conf/Core/test"/>
    <spec:conformanceTest rdf:resource="http://www.opengis.net/spec/GeoTIFF/1.1/conf/DoubleParameters"/>
    <spec:conformanceTest rdf:resource="http://www.opengis.net/spec/GeoTIFF/1.1/conf/AsciiParameters"/>
    <spec:conformanceTest rdf:resource="http://www.opengis.net/spec/GeoTIFF/1.1/conf/ShortParameters"/>
    <spec:conformanceTest rdf:resource="http://www.opengis.net/spec/GeoTIFF/1.1/conf/TIFF.Tags"/>
    <spec:conformanceTest rdf:resource="http://www.opengis.net/spec/GeoTIFF/1.1/conf/GeoKeyDirectory"/>
    <skos:narrower rdf:resource="http://www.opengis.net/spec/GeoTIFF/1.1/conf/DoubleParameters"/>
    <skos:narrower rdf:resource="http://www.opengis.net/spec/GeoTIFF/1.1/conf/AsciiParameters"/>
    <skos:narrower rdf:resource="http://www.opengis.net/spec/GeoTIFF/1.1/conf/ShortParameters"/>
    <skos:narrower rdf:resource="http://www.opengis.net/spec/GeoTIFF/1.1/conf/TIFF.Tags"/>
    <skos:narrower rdf:resource="http://www.opengis.net/spec/GeoTIFF/1.1/conf/GeoKeyDirectory"/>
    <skos:narrower rdf:resource="http://www.opengis.net/spec/GeoTIFF/1.1/conf/Core/test"/>
    <skos:definition>Conformance Class TIFF</skos:definition>
    <skos:prefLabel>Conformance Class TIFF</skos:prefLabel>
    <rdf:type rdf:resource="http://www.w3.org/2004/02/skos/core#Concept"/>
    <rdf:type rdf:resource="http://www.opengis.net/def/ont/modspec/ConformanceClass"/>
  </rdf:Description>
  <rdf:Description rdf:about="http://www.opengis.net/spec/GeoTIFF/1.1/req/ProjMethodGeoKey">
    <skos:prefLabel>Requirements Class ProjMethodGeoKey (coordinate operation method)</skos:prefLabel>
    <spec:normativeStatement rdf:resource="http://www.opengis.net/spec/GeoTIFF/1.1/req/ProjMethodGeoKey.reserved"/>
    <spec:normativeStatement rdf:resource="http://www.opengis.net/spec/GeoTIFF/1.1/req/ProjMethodGeoKey.private"/>
    <spec:normativeStatement rdf:resource="http://www.opengis.net/spec/GeoTIFF/1.1/req/ProjMethodGeoKey.ID"/>
    <spec:normativeStatement rdf:resource="http://www.opengis.net/spec/GeoTIFF/1.1/req/ProjMethodGeoKey.type"/>
    <spec:normativeStatement rdf:resource="http://www.opengis.net/spec/GeoTIFF/1.1/req/ProjMethodGeoKey.userdefined"/>
    <spec:normativeStatement rdf:resource="http://www.opengis.net/spec/GeoTIFF/1.1/req/ProjMethodGeoKey.transform"/>
    <skos:narrower rdf:resource="http://www.opengis.net/spec/GeoTIFF/1.1/req/ProjMethodGeoKey.private"/>
    <skos:narrower rdf:resource="http://www.opengis.net/spec/GeoTIFF/1.1/req/ProjMethodGeoKey.ID"/>
    <skos:narrower rdf:resource="http://www.opengis.net/spec/GeoTIFF/1.1/req/ProjMethodGeoKey.type"/>
    <skos:narrower rdf:resource="http://www.opengis.net/spec/GeoTIFF/1.1/req/ProjMethodGeoKey.reserved"/>
    <skos:narrower rdf:resource="http://www.opengis.net/spec/GeoTIFF/1.1/req/ProjMethodGeoKey.transform"/>
    <skos:narrower rdf:resource="http://www.opengis.net/spec/GeoTIFF/1.1/req/ProjMethodGeoKey.userdefined"/>
    <skos:definition>The ProjMethodGeoKey key is used to specify a map projection method from the GeoTIFF v1.0 coordinate transformation code list (Annex C) or to indicate that the map projection method is user-defined.




Note


In GeoTIFF 1.0 this key was called ProjCoordTransGeoKey.







Note


GeoTIFF v1.0 did not make reference to the EPSG coordinate operation methods (a future version of GeoTIFF might do this).</skos:definition>
    <skos:broader rdf:resource="http://www.opengis.net/spec/GeoTIFF/1.1/conf/ShortParameters"/>
    <skos:broader rdf:resource="http://www.opengis.net/def/docs/19-008r4"/>
    <rdf:type rdf:resource="http://www.opengis.net/def/ont/modspec/RequirementClass"/>
    <rdf:type rdf:resource="http://www.w3.org/2004/02/skos/core#Concept"/>
  </rdf:Description>
  <rdf:Description rdf:about="http://www.opengis.net/spec/GeoTIFF/1.1/req/GeoKeyDirectoryTag.numberOfKeys">
    <rdf:type rdf:resource="http://www.opengis.net/def/ont/modspec/Requirement"/>
    <rdf:type rdf:resource="http://www.w3.org/2004/02/skos/core#Concept"/>
    <dct:description>The fourth unsigned short integer in the GeoKeyDirectoryTag SHALL hold the
NumberOfKeys defined in the rest of the GeoKeyDirectoryTag.</dct:description>
    <skos:prefLabel>Requirement 2.10</skos:prefLabel>
    <skos:definition>The fourth unsigned short integer in the GeoKeyDirectoryTag SHALL hold the
NumberOfKeys defined in the rest of the GeoKeyDirectoryTag.</skos:definition>
    <skos:broader rdf:resource="http://www.opengis.net/spec/GeoTIFF/1.1/conf/GeoKeyDirectory"/>
    <skos:broader rdf:resource="http://www.opengis.net/spec/GeoTIFF/1.1/req/GeoKeyDirectoryTag"/>
  </rdf:Description>
  <rdf:Description rdf:about="http://www.opengis.net/spec/GeoTIFF/1.1/req/GeoKeyDirectoryTag">
    <spec:normativeStatement rdf:resource="http://www.opengis.net/spec/GeoTIFF/1.1/req/GeoKeyDirectoryTag.keyEntryKeyID"/>
    <spec:normativeStatement rdf:resource="http://www.opengis.net/spec/GeoTIFF/1.1/req/GeoKeyDirectoryTag.keyRevision"/>
    <spec:normativeStatement rdf:resource="http://www.opengis.net/spec/GeoTIFF/1.1/req/GeoKeyDirectoryTag.numberOfKeys"/>
    <spec:normativeStatement rdf:resource="http://www.opengis.net/spec/GeoTIFF/1.1/req/GeoKeyDirectoryTag.minorRevision"/>
    <spec:normativeStatement rdf:resource="http://www.opengis.net/spec/GeoTIFF/1.1/req/GeoKeyDirectoryTag.keyEntry"/>
    <spec:normativeStatement rdf:resource="http://www.opengis.net/spec/GeoTIFF/1.1/req/GeoKeyDirectoryTag.keyEntryValueOffset"/>
    <spec:normativeStatement rdf:resource="http://www.opengis.net/spec/GeoTIFF/1.1/req/GeoKeyDirectoryTag.keyEntrySetCount"/>
    <spec:normativeStatement rdf:resource="http://www.opengis.net/spec/GeoTIFF/1.1/req/GeoKeyDirectoryTag.keyDirectoryVersion"/>
    <spec:normativeStatement rdf:resource="http://www.opengis.net/spec/GeoTIFF/1.1/req/GeoKeyDirectoryTag.keyRevisionValue"/>
    <spec:normativeStatement rdf:resource="http://www.opengis.net/spec/GeoTIFF/1.1/req/GeoKeyDirectoryTag.count"/>
    <spec:normativeStatement rdf:resource="http://www.opengis.net/spec/GeoTIFF/1.1/req/GeoKeyDirectoryTag.ID"/>
    <spec:normativeStatement rdf:resource="http://www.opengis.net/spec/GeoTIFF/1.1/req/GeoKeyDirectoryTag.type"/>
    <spec:normativeStatement rdf:resource="http://www.opengis.net/spec/GeoTIFF/1.1/req/GeoKeyDirectoryTag.keyEntryTIFFTagLocation"/>
    <spec:normativeStatement rdf:resource="http://www.opengis.net/spec/GeoTIFF/1.1/req/GeoKeyDirectoryTag.keyEntryKeyCount"/>
    <spec:normativeStatement rdf:resource="http://www.opengis.net/spec/GeoTIFF/1.1/req/GeoKeyDirectoryTag.keyDirectoryVersionValue"/>
    <spec:normativeStatement rdf:resource="http://www.opengis.net/spec/GeoTIFF/1.1/req/GeoKeyDirectoryTag.minorRevisionValue"/>
    <skos:narrower rdf:resource="http://www.opengis.net/spec/GeoTIFF/1.1/req/GeoKeyDirectoryTag.minorRevision"/>
    <skos:narrower rdf:resource="http://www.opengis.net/spec/GeoTIFF/1.1/req/GeoKeyDirectoryTag.keyEntryKeyID"/>
    <skos:narrower rdf:resource="http://www.opengis.net/spec/GeoTIFF/1.1/req/GeoKeyDirectoryTag.keyEntry"/>
    <skos:narrower rdf:resource="http://www.opengis.net/spec/GeoTIFF/1.1/req/GeoKeyDirectoryTag.keyEntryValueOffset"/>
    <skos:narrower rdf:resource="http://www.opengis.net/spec/GeoTIFF/1.1/req/GeoKeyDirectoryTag.keyDirectoryVersion"/>
    <skos:narrower rdf:resource="http://www.opengis.net/spec/GeoTIFF/1.1/req/GeoKeyDirectoryTag.keyRevisionValue"/>
    <skos:narrower rdf:resource="http://www.opengis.net/spec/GeoTIFF/1.1/req/GeoKeyDirectoryTag.count"/>
    <skos:narrower rdf:resource="http://www.opengis.net/spec/GeoTIFF/1.1/req/GeoKeyDirectoryTag.keyEntrySetCount"/>
    <skos:narrower rdf:resource="http://www.opengis.net/spec/GeoTIFF/1.1/req/GeoKeyDirectoryTag.ID"/>
    <skos:narrower rdf:resource="http://www.opengis.net/spec/GeoTIFF/1.1/req/GeoKeyDirectoryTag.type"/>
    <skos:narrower rdf:resource="http://www.opengis.net/spec/GeoTIFF/1.1/req/GeoKeyDirectoryTag.keyEntryTIFFTagLocation"/>
    <skos:narrower rdf:resource="http://www.opengis.net/spec/GeoTIFF/1.1/req/GeoKeyDirectoryTag.keyEntryKeyCount"/>
    <skos:narrower rdf:resource="http://www.opengis.net/spec/GeoTIFF/1.1/req/GeoKeyDirectoryTag.keyDirectoryVersionValue"/>
    <skos:narrower rdf:resource="http://www.opengis.net/spec/GeoTIFF/1.1/req/GeoKeyDirectoryTag.keyRevision"/>
    <skos:narrower rdf:resource="http://www.opengis.net/spec/GeoTIFF/1.1/req/GeoKeyDirectoryTag.minorRevisionValue"/>
    <skos:narrower rdf:resource="http://www.opengis.net/spec/GeoTIFF/1.1/req/GeoKeyDirectoryTag.numberOfKeys"/>
    <rdf:type rdf:resource="http://www.w3.org/2004/02/skos/core#Concept"/>
    <rdf:type rdf:resource="http://www.opengis.net/def/ont/modspec/RequirementClass"/>
    <skos:prefLabel>Requirements Class GeoKeyDirectoryTag</skos:prefLabel>
    <skos:definition>The GeoKeyDirectoryTag Requirements Class specifies the requirements for implementing the reserved GeoKeyDirectoryTag TIFF tag.

A GeoTIFF file stores projection parameters in a set of Keys which are virtually identical in function to a TIFF tag, but have one more level of abstraction above TIFF. Like a tag, a Key has an ID number ranging from 0 to 65535, but unlike TIFF tags, all key ID’s are available for use in GeoTIFF parameter definitions.

The Keys in GeoTIFF (also called GeoKeys) are all referenced from the GeoKeyDirectoryTag tag. The first four keys form the GeoKey Directory Header. The keys which make up this header are: KeyDirectoryVersion, KeyRevision, MinorRevision, and NumberOfKeys.

The GeoKey Directory Header is followed by &lt;NumberOfKeys&gt; Key Entries. Each Key Entry consists of four values.



KeyID gives the key-ID value of the Key (identical in function to TIFF tag ID, but completely independent of TIFF tag-space).


TIFFTagLocation indicates which TIFF tag contains the value(s) of the Key: if TIFFTagLocation is 0, then the value is SHORT, and is contained in the ValueOffset entry. Otherwise, the type (format) of the value is implied by the TIFF-Type of the tag containing the value.


Count indicates the number of values in this key.


ValueOffset ValueOffset indicates the index- offset into the TagArray indicated by TIFFTagLocation, if it is nonzero. If TIFFTagLocation=0, then ValueOffset contains the actual (SHORT) value of the Key, and Count=1 is implied. Note that the offset is not a byte-offset, but rather an index based on the natural data type of the specified tag array.</skos:definition>
    <skos:broader rdf:resource="http://www.opengis.net/def/docs/19-008r4"/>
  </rdf:Description>
  <rdf:Description rdf:about="http://www.opengis.net/spec/GeoTIFF/1.1/req/EllipsoidGeoKey.reserved">
    <skos:definition>EllipsoidGeoKey values in the range 1-1023 SHALL be reserved</skos:definition>
    <rdf:type rdf:resource="http://www.opengis.net/def/ont/modspec/Requirement"/>
    <rdf:type rdf:resource="http://www.w3.org/2004/02/skos/core#Concept"/>
    <skos:prefLabel>Requirement 21.3</skos:prefLabel>
    <skos:broader rdf:resource="http://www.opengis.net/spec/GeoTIFF/1.1/req/EllipsoidGeoKey"/>
    <dct:description>EllipsoidGeoKey values in the range 1-1023 SHALL be reserved</dct:description>
  </rdf:Description>
  <rdf:Description rdf:about="http://www.opengis.net/spec/GeoTIFF/1.1/conf/Core/test">
    <skos:broader rdf:resource="http://www.opengis.net/spec/GeoTIFF/1.1/conf/Core"/>
    <spec:requirement rdf:resource="http://www.opengis.net/spec/GeoTIFF/1.1/req/TIFF"/>
    <spec:requirement rdf:resource="http://www.opengis.net/spec/GeoTIFF/1.1/req/ByteOrder"/>
    <spec:requirement rdf:resource="http://www.opengis.net/spec/GeoTIFF/1.1/req/DataTypes"/>
    <skos:narrower rdf:resource="http://www.opengis.net/spec/GeoTIFF/1.1/req/TIFF"/>
    <skos:narrower rdf:resource="http://www.opengis.net/spec/GeoTIFF/1.1/req/DataTypes"/>
    <skos:narrower rdf:resource="http://www.opengis.net/spec/GeoTIFF/1.1/req/ByteOrder"/>
    <skos:prefLabel>TIFF Core Test</skos:prefLabel>
    <rdf:type rdf:resource="http://www.opengis.net/def/ont/modspec/ConformanceTest"/>
    <rdf:type rdf:resource="http://www.w3.org/2004/02/skos/core#Concept"/>
    <spec:method>There is no authoritative conformance test for TIFF 6.0. 2 basic tests may be
done on TIFF header (4 first bytes), called TIFF magic: • Bytes 0-1 (byte
order within the file) = 0X4949 (II = little endian) or 0X4D4D (MM = big
endian). • Bytes 2-3 = the short integer value 42 interpreted using the byte
order specified in bytes 0-1.

The best that can be achieved is to use a TIFF reference implementation to
successfully read a GeoTIFF file. The OGC recommends the use of tiffdump based
on the open source LibTIFF library (&lt;https://gitlab.com/libtiff/libtiff&gt;) for
dumping the content of TIFF tags (displaying error messages if any), or
opensource TIFF file validator (such as the JHOVE tool, opensource developed
in Java - cf. &lt;http://jhove.openpreservation.org/&gt;).

Once TIFF 6.0 conformance has been validated, execute test
&lt;http://www.opengis.net/spec/GeoTIFF/1.1/conf/TIFF.Tags&gt;.</spec:method>
    <spec:method rdf:datatype="http://www.w3.org/1999/02/22-rdf-syntax-ns#HTML">%3Cdiv%20class%3D%22paragraph%22%3E%0A%3Cp%3EThere%20is%20no%20authoritative%20conformance%20test%20for%20TIFF%206.0.%0A2%20basic%20tests%20may%20be%20done%20on%20TIFF%20header%20%284%20first%20bytes%29%2C%20called%20TIFF%20magic%3A%0A%E2%80%A2%20Bytes%200-1%20%28byte%20order%20within%20the%20file%29%20%3D%200X4949%20%28%22II%22%20%3D%20little%20endian%29%20or%200X4D4D%20%28%22MM%22%20%3D%20big%20endian%29.%0A%E2%80%A2%20Bytes%202-3%20%3D%20the%20short%20integer%20value%2042%20interpreted%20using%20the%20byte%20order%20specified%20in%20bytes%200-1.%3C/p%3E%0A%3C/div%3E%3Cdiv%20class%3D%22paragraph%22%3E%0A%3Cp%3EThe%20best%20that%20can%20be%20achieved%20is%20to%20use%20a%20TIFF%20reference%20implementation%20to%20successfully%20read%20a%20GeoTIFF%20file.%20The%20OGC%20recommends%20the%20use%20of%20tiffdump%20based%20on%20the%20open%20source%20LibTIFF%20library%20%28%3Ca%20href%3D%22https%3A//gitlab.com/libtiff/libtiff%22%20class%3D%22bare%22%3Ehttps%3A//gitlab.com/libtiff/libtiff%3C/a%3E%29%20for%20dumping%20the%20content%20of%20TIFF%20tags%20%28displaying%20error%20messages%20if%20any%29%2C%20or%20opensource%20TIFF%20file%20validator%20%28such%20as%20the%20JHOVE%20tool%2C%20opensource%20developed%20in%20Java%20-%20cf.%20%3Ca%20href%3D%22http%3A//jhove.openpreservation.org/%22%20class%3D%22bare%22%3Ehttp%3A//jhove.openpreservation.org/%3C/a%3E%29.%3C/p%3E%0A%3C/div%3E%3Cdiv%20class%3D%22paragraph%22%3E%0A%3Cp%3EOnce%20TIFF%206.0%20conformance%20has%20been%20validated%2C%20execute%20test%20%3Ca%20href%3D%22http%3A//www.opengis.net/spec/GeoTIFF/1.1/conf/TIFF.Tags%22%20class%3D%22bare%22%3Ehttp%3A//www.opengis.net/spec/GeoTIFF/1.1/conf/TIFF.Tags%3C/a%3E.%3C/p%3E%0A%3C/div%3E</spec:method>
    <spec:purpose>Verify that the GeoTIFF file conforms to the TIFF specification.</spec:purpose>
    <spec:testType rdf:resource="http://www.opengis.net/def/ont/modspec/Basic"/>
    <skos:definition>TIFF Core Test</skos:definition>
  </rdf:Description>
  <rdf:Description rdf:about="http://www.opengis.net/spec/GeoTIFF/1.1/req/ProjectionGeoKey">
    <skos:prefLabel>Requirements Class ProjectionGeoKey</skos:prefLabel>
    <rdf:type rdf:resource="http://www.opengis.net/def/ont/modspec/RequirementClass"/>
    <rdf:type rdf:resource="http://www.w3.org/2004/02/skos/core#Concept"/>
    <skos:broader rdf:resource="http://www.opengis.net/spec/GeoTIFF/1.1/conf/ShortParameters"/>
    <skos:broader rdf:resource="http://www.opengis.net/def/docs/19-008r4"/>
    <skos:narrower rdf:resource="http://www.opengis.net/spec/GeoTIFF/1.1/req/ProjectionGeoKey.EPSG"/>
    <skos:narrower rdf:resource="http://www.opengis.net/spec/GeoTIFF/1.1/req/ProjectionGeoKey.type"/>
    <skos:narrower rdf:resource="http://www.opengis.net/spec/GeoTIFF/1.1/req/ProjectionGeoKey.private"/>
    <skos:narrower rdf:resource="http://www.opengis.net/spec/GeoTIFF/1.1/req/ProjectionGeoKey.ID"/>
    <skos:narrower rdf:resource="http://www.opengis.net/spec/GeoTIFF/1.1/req/ProjectionGeoKey.reserved"/>
    <skos:narrower rdf:resource="http://www.opengis.net/spec/GeoTIFF/1.1/req/ProjectionGeoKey.userdefined"/>
    <spec:normativeStatement rdf:resource="http://www.opengis.net/spec/GeoTIFF/1.1/req/ProjectionGeoKey.type"/>
    <spec:normativeStatement rdf:resource="http://www.opengis.net/spec/GeoTIFF/1.1/req/ProjectionGeoKey.private"/>
    <spec:normativeStatement rdf:resource="http://www.opengis.net/spec/GeoTIFF/1.1/req/ProjectionGeoKey.EPSG"/>
    <spec:normativeStatement rdf:resource="http://www.opengis.net/spec/GeoTIFF/1.1/req/ProjectionGeoKey.ID"/>
    <spec:normativeStatement rdf:resource="http://www.opengis.net/spec/GeoTIFF/1.1/req/ProjectionGeoKey.userdefined"/>
    <spec:normativeStatement rdf:resource="http://www.opengis.net/spec/GeoTIFF/1.1/req/ProjectionGeoKey.reserved"/>
    <skos:definition>The ProjectionGeoKey key is used to specify a map projection from the GeoTIFF CRS register or to indicate that the map projection is user-defined. In the EPSG Dataset a map projection is a coordinate conversion, a subtype of coordinate operation.</skos:definition>
  </rdf:Description>
  <rdf:Description rdf:about="http://www.opengis.net/spec/GeoTIFF/1.1/req/UnitsGeoKey.angular">
    <skos:definition>GeogAngularUnitsGeoKey and GeogAzimuthUnitsGeoKey values in the range
1024-32766 SHALL be EPSG Unit Of Measure (UOM) codes with type = angle.NOTE:
In GeoTIFF v1.0 the range was 9100-9199</skos:definition>
    <rdf:type rdf:resource="http://www.opengis.net/def/ont/modspec/Requirement"/>
    <rdf:type rdf:resource="http://www.w3.org/2004/02/skos/core#Concept"/>
    <skos:prefLabel>Requirement 16.4</skos:prefLabel>
    <dct:description>GeogAngularUnitsGeoKey and GeogAzimuthUnitsGeoKey values in the range
1024-32766 SHALL be EPSG Unit Of Measure (UOM) codes with type = angle.NOTE:
In GeoTIFF v1.0 the range was 9100-9199</dct:description>
    <skos:broader rdf:resource="http://www.opengis.net/spec/GeoTIFF/1.1/req/UnitsGeoKey"/>
  </rdf:Description>
  <rdf:Description rdf:about="http://www.opengis.net/spec/GeoTIFF/1.1/conf/GeoKeyDirectory">
    <skos:broader rdf:resource="http://www.opengis.net/spec/GeoTIFF/1.1/conf/Core"/>
    <spec:requirement rdf:resource="http://www.opengis.net/spec/GeoTIFF/1.1/req/GeoKeyDirectoryTag.keyEntryTIFFTagLocation"/>
    <spec:requirement rdf:resource="http://www.opengis.net/spec/GeoTIFF/1.1/req/GeoKeyDirectoryTag.minorRevisionValue"/>
    <spec:requirement rdf:resource="http://www.opengis.net/spec/GeoTIFF/1.1/req/GeoKeySort"/>
    <spec:requirement rdf:resource="http://www.opengis.net/spec/GeoTIFF/1.1/req/GeoKeyDirectoryTag.keyDirectoryVersionValue"/>
    <spec:requirement rdf:resource="http://www.opengis.net/spec/GeoTIFF/1.1/req/GeoKeyDirectoryTag.keyRevision"/>
    <spec:requirement rdf:resource="http://www.opengis.net/spec/GeoTIFF/1.1/req/GeoKeyDirectoryTag.numberOfKeys"/>
    <spec:requirement rdf:resource="http://www.opengis.net/spec/GeoTIFF/1.1/req/GeoKeyDirectoryTag.minorRevision"/>
    <spec:requirement rdf:resource="http://www.opengis.net/spec/GeoTIFF/1.1/req/GeoKeyDirectoryTag.keyEntryKeyID"/>
    <spec:requirement rdf:resource="http://www.opengis.net/spec/GeoTIFF/1.1/req/GeoKeyDirectoryTag.keyEntry"/>
    <spec:requirement rdf:resource="http://www.opengis.net/spec/GeoTIFF/1.1/req/GeoKeyDirectoryTag.keyEntrySetCount"/>
    <spec:requirement rdf:resource="http://www.opengis.net/spec/GeoTIFF/1.1/req/GeoKeyDirectoryTag.keyDirectoryVersion"/>
    <spec:requirement rdf:resource="http://www.opengis.net/spec/GeoTIFF/1.1/req/GeoKeyDirectoryTag.keyRevisionValue"/>
    <rdf:type rdf:resource="http://www.opengis.net/def/ont/modspec/ConformanceTest"/>
    <rdf:type rdf:resource="http://www.w3.org/2004/02/skos/core#Concept"/>
    <spec:method rdf:datatype="http://www.w3.org/1999/02/22-rdf-syntax-ns#HTML">%3Cdiv%3E%3Cdiv%3EPre-conditions%3Cdiv%3E%3Cdiv%3EA%20GeoKey%20Directory%20has%20been%20located%3C/div%3E%3C/div%3E%3Cdiv%20class%3D%22olist%20arabic%22%3E%0A%3Col%20class%3D%22arabic%22%3E%0A%3Cli%3E%0A%3Cp%3EValidate%20and%20process%20the%20GeoKey%20Directory%20Header%3C/p%3E%0A%3Cdiv%20class%3D%22ulist%22%3E%0A%3Cul%3E%0A%3Cli%3E%0A%3Cp%3EVerify%20that%20Bytes%200-1%20%3D%201%20%28Key%20Directory%20Version%29.%3C/p%3E%0A%3C/li%3E%0A%3Cli%3E%0A%3Cp%3EVerify%20that%20Bytes%202-3%20%3D%201%20%28Key%20Revision%29%3C/p%3E%0A%3C/li%3E%0A%3Cli%3E%0A%3Cp%3EVerify%20that%20Bytes%204-5%20%3D%200%20or%201%20%28Key%20Minor%20Revision%29%3C/p%3E%0A%3C/li%3E%0A%3Cli%3E%0A%3Cp%3EBytes%206-7%20contain%20the%20number%20of%20Key%20Entry%20Sets%20in%20this%20directory.%20Set%20KeySetCount%20to%20this%20value.%3C/p%3E%0A%3C/li%3E%0A%3C/ul%3E%0A%3C/div%3E%0A%3C/li%3E%0A%3Cli%3E%0A%3Cp%3EProcess%20each%20Key%20Entry%20Set%20using%20the%20following%20pseudocode%3A%3C/p%3E%0A%3Cdiv%20class%3D%22literalblock%22%3E%0A%3Cdiv%20class%3D%22content%22%3E%0A%3Cpre%3ESET%20GeoKeyOffset%20%3D%208%0AWHILE%20KeySetCount%20is%20not%200%0A%20%20%20%7B%0A%20%20%20Verify%20that%20the%20GeoKey%20%28first%20Short%20integer%29%20is%20greater%20than%20the%20previous%20GeoKey.%0A%20%20%20Process%20the%20second%20Short%20integer%20in%20the%20Key%20Entry%20Set%0A%20%20%20%20%20%20%20%7B%0A%20%20%20%20%20%20%20IF%20value%20%3D%200%20THEN%20Execute%20test%20http%3A//www.opengis.net/spec/GeoTIFF/1.1/conf/Short_Param%20passing%20GeoKeyOffset%20as%20a%20parameter%0A%20%20%20%20%20%20%20IF%20value%20%3D%2034735%20THEN%20Execute%20test%20http%3A//www.opengis.net/spec/GeoTIFF/1.1/conf/Short_Param%20passing%20GeoKeyOffset%20as%20a%20parameter%0A%20%20%20%20%20%20%20IF%20value%20%3D%2034736%20THEN%20Execute%20test%20http%3A//www.opengis.net/spec/GeoTIFF/1.1/conf/Double_Param%20passing%20GeoKeyOffset%20as%20a%20parameter%0A%20%20%20%20%20%20%20IF%20value%20%3D%2034737%20THEN%20%20Execute%20test%20http%3A//www.opengis.net/spec/GeoTIFF/1.1/conf/ASCII_Param%20passing%20GeoKeyOffset%20as%20a%20parameter%0A%20%20%20%20%20%20%20%7D%0A%20%20%20SET%20GeoKeyOffset%20%3D%20GeoKeyOffset%20%2B%208%0A%20%20%20KeySetCount%20%3D%20KeySetCount%20-%201%0A%20%20%20%7D%3C/pre%3E%0A%3C/div%3E%0A%3C/div%3E%0A%3C/li%3E%0A%3Cli%3E%0A%3Cp%3EValidate%20that%20the%20number%20of%20Key%20Sets%20processed%20equal%20the%20number%20specified%20in%20the%20header.%3C/p%3E%0A%3C/li%3E%0A%3C/ol%3E%0A%3C/div%3E</spec:method>
    <spec:method>Pre-conditions

A GeoKey Directory has been located

Text Variables

**Variable**

|

**Scope**

|

**Description**

---|---|---

IFD_Offset

|

Local

|

Location within the TIFF file of an IFD

GeoKeyDirectory

|

Global

|

Location of the GeoTIFF GeoKey directory

ASCIIValues

|

Global

|

Location of the ASCII values for GeoTIFF ASCII GeoKeys

DoubleValues

|

Global

|

Location of the Double values for GeoTIFF Double GeoKeys

GeoKeyOffset

|

Parameter

|

Location of this GeoKey in the GeoKey directory

KeySetCount

|

Local

|

The number of entries in the GeoKey directory

  1. Validate and process the GeoKey Directory Header

    * Verify that Bytes 0-1 = 1 (Key Directory Version).

    * Verify that Bytes 2-3 = 1 (Key Revision)

    * Verify that Bytes 4-5 = 0 or 1 (Key Minor Revision)

    * Bytes 6-7 contain the number of Key Entry Sets in this directory. Set KeySetCount to this value.

  2. Process each Key Entry Set using the following pseudocode:

        SET GeoKeyOffset = 8
    WHILE KeySetCount is not 0
       {
       Verify that the GeoKey (first Short integer) is greater than the previous GeoKey.
       Process the second Short integer in the Key Entry Set
           {
           IF value = 0 THEN Execute test http://www.opengis.net/spec/GeoTIFF/1.1/conf/Short_Param passing GeoKeyOffset as a parameter
           IF value = 34735 THEN Execute test http://www.opengis.net/spec/GeoTIFF/1.1/conf/Short_Param passing GeoKeyOffset as a parameter
           IF value = 34736 THEN Execute test http://www.opengis.net/spec/GeoTIFF/1.1/conf/Double_Param passing GeoKeyOffset as a parameter
           IF value = 34737 THEN  Execute test http://www.opengis.net/spec/GeoTIFF/1.1/conf/ASCII_Param passing GeoKeyOffset as a parameter
           }
       SET GeoKeyOffset = GeoKeyOffset + 8
       KeySetCount = KeySetCount - 1
       }

  3. Validate that the number of Key Sets processed equal the number specified in the header.</spec:method>
    <skos:narrower rdf:resource="http://www.opengis.net/spec/GeoTIFF/1.1/req/GeoKeyDirectoryTag.keyEntryTIFFTagLocation"/>
    <skos:narrower rdf:resource="http://www.opengis.net/spec/GeoTIFF/1.1/req/GeoKeyDirectoryTag.keyDirectoryVersionValue"/>
    <skos:narrower rdf:resource="http://www.opengis.net/spec/GeoTIFF/1.1/req/GeoKeyDirectoryTag.minorRevisionValue"/>
    <skos:narrower rdf:resource="http://www.opengis.net/spec/GeoTIFF/1.1/req/GeoKeySort"/>
    <skos:narrower rdf:resource="http://www.opengis.net/spec/GeoTIFF/1.1/req/GeoKeyDirectoryTag.keyRevision"/>
    <skos:narrower rdf:resource="http://www.opengis.net/spec/GeoTIFF/1.1/req/GeoKeyDirectoryTag.numberOfKeys"/>
    <skos:narrower rdf:resource="http://www.opengis.net/spec/GeoTIFF/1.1/req/GeoKeyDirectoryTag.minorRevision"/>
    <skos:narrower rdf:resource="http://www.opengis.net/spec/GeoTIFF/1.1/req/GeoKeyDirectoryTag.keyEntryKeyID"/>
    <skos:narrower rdf:resource="http://www.opengis.net/spec/GeoTIFF/1.1/req/GeoKeyDirectoryTag.keyEntry"/>
    <skos:narrower rdf:resource="http://www.opengis.net/spec/GeoTIFF/1.1/req/GeoKeyDirectoryTag.keyEntrySetCount"/>
    <skos:narrower rdf:resource="http://www.opengis.net/spec/GeoTIFF/1.1/req/GeoKeyDirectoryTag.keyDirectoryVersion"/>
    <skos:narrower rdf:resource="http://www.opengis.net/spec/GeoTIFF/1.1/req/GeoKeyDirectoryTag.keyRevisionValue"/>
    <spec:purpose>Verify the GeoKey Directory</spec:purpose>
    <skos:definition>GeoKey Directory Test</skos:definition>
    <spec:testType rdf:resource="http://www.opengis.net/def/ont/modspec/Basic"/>
    <skos:prefLabel>GeoKey Directory Test</skos:prefLabel>
  </rdf:Description>
  <rdf:Description rdf:about="http://www.opengis.net/spec/GeoTIFF/1.1/req/PrimeMeridianGeoKey.private">
    <skos:definition>PrimeMeridianGeoKey values in the range 32768-65535 SHALL be private</skos:definition>
    <skos:prefLabel>Requirement 19.6</skos:prefLabel>
    <rdf:type rdf:resource="http://www.opengis.net/def/ont/modspec/Requirement"/>
    <rdf:type rdf:resource="http://www.w3.org/2004/02/skos/core#Concept"/>
    <skos:broader rdf:resource="http://www.opengis.net/spec/GeoTIFF/1.1/req/PrimeMeridianGeoKey"/>
    <dct:description>PrimeMeridianGeoKey values in the range 32768-65535 SHALL be private</dct:description>
  </rdf:Description>
  <rdf:Description rdf:about="http://www.opengis.net/spec/GeoTIFF/1.1/req/GeoKeyDirectoryTag.keyEntryValueOffset">
    <dct:description>The fourth unsigned short integer in the Key Entry SHALL hold either the key
value (if TIFF Tag location = 0) or the index into the tag indicated by the
TIFF Tag Location value.</dct:description>
    <skos:broader rdf:resource="http://www.opengis.net/spec/GeoTIFF/1.1/conf/ShortParameters"/>
    <skos:broader rdf:resource="http://www.opengis.net/spec/GeoTIFF/1.1/req/GeoKeyDirectoryTag"/>
    <skos:broader rdf:resource="http://www.opengis.net/spec/GeoTIFF/1.1/conf/DoubleParameters"/>
    <skos:broader rdf:resource="http://www.opengis.net/spec/GeoTIFF/1.1/conf/AsciiParameters"/>
    <rdf:type rdf:resource="http://www.opengis.net/def/ont/modspec/Requirement"/>
    <rdf:type rdf:resource="http://www.w3.org/2004/02/skos/core#Concept"/>
    <skos:definition>The fourth unsigned short integer in the Key Entry SHALL hold either the key
value (if TIFF Tag location = 0) or the index into the tag indicated by the
TIFF Tag Location value.</skos:definition>
    <skos:prefLabel>Requirement 2.16</skos:prefLabel>
  </rdf:Description>
  <rdf:Description rdf:about="http://www.opengis.net/spec/GeoTIFF/1.1/req/EllipsoidSemiMinorAxisGeoKey.units">
    <rdf:type rdf:resource="http://www.opengis.net/def/ont/modspec/Requirement"/>
    <rdf:type rdf:resource="http://www.w3.org/2004/02/skos/core#Concept"/>
    <skos:broader rdf:resource="http://www.opengis.net/spec/GeoTIFF/1.1/req/EllipsoidSemiMajorAxisGeoKey"/>
    <skos:prefLabel>Requirement 23.3</skos:prefLabel>
    <skos:definition>The units of the EllipsoidSemiMinorAxisGeoKey SHALL be defined by the value of
GeogLinearUnitsGeoKey</skos:definition>
    <dct:description>The units of the EllipsoidSemiMinorAxisGeoKey SHALL be defined by the value of
GeogLinearUnitsGeoKey</dct:description>
  </rdf:Description>
  <rdf:Description rdf:about="http://www.opengis.net/spec/GeoTIFF/1.1/conf/ShortParameters">
    <skos:narrower rdf:resource="http://www.opengis.net/spec/GeoTIFF/1.1/req/ProjMethodGeoKey"/>
    <skos:narrower rdf:resource="http://www.opengis.net/spec/GeoTIFF/1.1/req/GTRasterTypeGeoKey"/>
    <skos:narrower rdf:resource="http://www.opengis.net/spec/GeoTIFF/1.1/req/GeoKeyDirectoryTag.keyEntryValueOffset"/>
    <skos:narrower rdf:resource="http://www.opengis.net/spec/GeoTIFF/1.1/req/ProjectionGeoKey"/>
    <skos:narrower rdf:resource="http://www.opengis.net/spec/GeoTIFF/1.1/req/ProjectedCRSGeoKey"/>
    <skos:narrower rdf:resource="http://www.opengis.net/spec/GeoTIFF/1.1/req/VerticalDatumGeoKey"/>
    <skos:narrower rdf:resource="http://www.opengis.net/spec/GeoTIFF/1.1/req/GTModelTypeGeoKey"/>
    <skos:narrower rdf:resource="http://www.opengis.net/spec/GeoTIFF/1.1/req/GeodeticDatumGeoKey"/>
    <skos:narrower rdf:resource="http://www.opengis.net/spec/GeoTIFF/1.1/req/UnitsGeoKey"/>
    <skos:narrower rdf:resource="http://www.opengis.net/spec/GeoTIFF/1.1/req/EllipsoidGeoKey"/>
    <skos:narrower rdf:resource="http://www.opengis.net/spec/GeoTIFF/1.1/req/GeoShortParams.Location"/>
    <skos:narrower rdf:resource="http://www.opengis.net/spec/GeoTIFF/1.1/req/GeoShortParams.Criteria"/>
    <skos:narrower rdf:resource="http://www.opengis.net/spec/GeoTIFF/1.1/req/GeoKeyDirectoryTag.KeyEntry.ID"/>
    <skos:narrower rdf:resource="http://www.opengis.net/spec/GeoTIFF/1.1/req/GeodeticCRSGeoKey"/>
    <skos:narrower rdf:resource="http://www.opengis.net/spec/GeoTIFF/1.1/req/PrimeMeridianGeoKey"/>
    <skos:narrower rdf:resource="http://www.opengis.net/spec/GeoTIFF/1.1/req/GeoKeyDirectoryTag.keyEntryTIFFTagLocation"/>
    <skos:narrower rdf:resource="http://www.opengis.net/spec/GeoTIFF/1.1/req/VerticalGeoKey"/>
    <skos:narrower rdf:resource="http://www.opengis.net/spec/GeoTIFF/1.1/req/GeoKeyDirectoryTag.keyEntryKeyCount"/>
    <spec:requirement rdf:resource="http://www.opengis.net/spec/GeoTIFF/1.1/req/GeoKeyDirectoryTag.keyEntryValueOffset"/>
    <spec:requirement rdf:resource="http://www.opengis.net/spec/GeoTIFF/1.1/req/ProjectionGeoKey"/>
    <spec:requirement rdf:resource="http://www.opengis.net/spec/GeoTIFF/1.1/req/ProjectedCRSGeoKey"/>
    <spec:requirement rdf:resource="http://www.opengis.net/spec/GeoTIFF/1.1/req/VerticalDatumGeoKey"/>
    <spec:requirement rdf:resource="http://www.opengis.net/spec/GeoTIFF/1.1/req/GeodeticDatumGeoKey"/>
    <spec:requirement rdf:resource="http://www.opengis.net/spec/GeoTIFF/1.1/req/UnitsGeoKey"/>
    <spec:requirement rdf:resource="http://www.opengis.net/spec/GeoTIFF/1.1/req/EllipsoidGeoKey"/>
    <spec:requirement rdf:resource="http://www.opengis.net/spec/GeoTIFF/1.1/req/GeoShortParams.Location"/>
    <spec:requirement rdf:resource="http://www.opengis.net/spec/GeoTIFF/1.1/req/GeoShortParams.Criteria"/>
    <spec:requirement rdf:resource="http://www.opengis.net/spec/GeoTIFF/1.1/req/GeoKeyDirectoryTag.KeyEntry.ID"/>
    <spec:requirement rdf:resource="http://www.opengis.net/spec/GeoTIFF/1.1/req/GeodeticCRSGeoKey"/>
    <spec:requirement rdf:resource="http://www.opengis.net/spec/GeoTIFF/1.1/req/PrimeMeridianGeoKey"/>
    <spec:requirement rdf:resource="http://www.opengis.net/spec/GeoTIFF/1.1/req/GeoKeyDirectoryTag.keyEntryTIFFTagLocation"/>
    <spec:requirement rdf:resource="http://www.opengis.net/spec/GeoTIFF/1.1/req/VerticalGeoKey"/>
    <spec:requirement rdf:resource="http://www.opengis.net/spec/GeoTIFF/1.1/req/GeoKeyDirectoryTag.keyEntryKeyCount"/>
    <spec:requirement rdf:resource="http://www.opengis.net/spec/GeoTIFF/1.1/req/GTModelTypeGeoKey"/>
    <spec:requirement rdf:resource="http://www.opengis.net/spec/GeoTIFF/1.1/req/ProjMethodGeoKey"/>
    <spec:requirement rdf:resource="http://www.opengis.net/spec/GeoTIFF/1.1/req/GTRasterTypeGeoKey"/>
    <spec:method rdf:datatype="http://www.w3.org/1999/02/22-rdf-syntax-ns#HTML">%3Cdiv%3E%3Cdiv%3EPre-conditions%3Cdiv%3E%3Cdiv%3EThe%20GeoKeyDirectory%20and%20GeoKeyOffset%20values%20have%20been%20set%3C/div%3E%3C/div%3E%3Cdiv%20class%3D%22literalblock%22%3E%0A%3Cdiv%20class%3D%22content%22%3E%0A%3Cpre%3ELocate%20the%20Key%20Entry%20Set%20using%20the%20GeoKeyDirectory%20and%20GeoKeyOffset%20values.%3C/pre%3E%0A%3C/div%3E%0A%3C/div%3E%3Cdiv%20class%3D%22literalblock%22%3E%0A%3Cdiv%20class%3D%22content%22%3E%0A%3Cpre%3EProcess%20the%20second%20Short%20integer%20in%20the%20Key%20Entry%20Set%0A%20%20%20%20%7B%0A%20%20%20%20IF%20value%20%21%3D%200%20OR%2034735%20THEN%20error%20out%0A%20%20%20%20%7D%0AProcess%20the%20first%20Short%20integer%20in%20the%20Key%20Entry%20Set%0A%20%20%20%20%7B%0A%20%20%20%20SET%20GeoKey%20to%20the%20value%0A%20%20%20%20%7D%0AProcess%20the%20third%20Short%20integer%20in%20the%20Key%20Entry%20Set%0A%20%20%20%20%7B%0A%20%20%20%20SET%20KeyLength%20to%20the%20value%0A%20%20%20%20%7D%0AIF%20KeyLength%20%3D%201%20THEN%0A%20%20%20%20SET%20KeyValueOffset%20%3D%20GeoKeyDirectory%20%2B%20GeoKeyOffset%20%2B%206%0AELSE%0A%20%20%20%20%7B%0A%20%20%20%20Process%20the%20fourth%20Short%20integer%20in%20the%20Key%20Entry%20Set%0A%20%20%20%20%20%20%20%20%7B%0A%20%20%20%20%20%20%20%20SET%20KeyValueOffset%20to%20the%20value%0A%20%20%20%20%20%20%20%20%7D%0A%20%20%20%20SET%20KeyValueOffset%20%3D%20GeoKeyDirectory%20%2B%20%28KeyValueOffset%20%2A%202%29%0A%20%20%20%20%7D%3C/pre%3E%0A%3C/div%3E%0A%3C/div%3E%3Cdiv%20class%3D%22literalblock%22%3E%0A%3Cdiv%20class%3D%22content%22%3E%0A%3Cpre%3ERead%20a%20KeyLength%20Short%20values%20from%20the%20GeoTIFF%20file%20starting%20at%20KeyValueOffset.%0AValidate%20the%20value%0A%20%20%20%20Locate%20the%20GeoKey%20in%20the%20following%20table%0A%20%20%20%20Verify%20that%20the%20values%20read%20satisfy%20the%20constraints%20defined%20in%20the%20associated%20Requirements%20Class.%0A%20%20%20%20Verify%20that%20any%20GeoKeys%20required%20by%20the%20associated%20Requirements%20Class%20are%20present%20in%20the%20GeoKey%20Directory.%3C/pre%3E%0A%3C/div%3E%0A%3C/div%3E</spec:method>
    <spec:method>Pre-conditions

The GeoKeyDirectory and GeoKeyOffset values have been set

Text Variables

**Variable**

|

**Scope**

|

**Description**

---|---|---

GeoKeyDirectory

|

Global

|

Location of the GeoTIFF GeoKey directory

GeoKeyOffset

|

Parameter

|

Location of this Key Entry Set in the GeoKey directory

GeoKey

|

Local

|

Temporary value of the GeoKey

KeyLength

|

Local

|

Temporary value for the length of the value for the GeoKey

KeyValueOffset

|

Local

|

The location of the GeoKey value in the file


    Locate the Key Entry Set using the GeoKeyDirectory and GeoKeyOffset values.


    Process the second Short integer in the Key Entry Set
        {
        IF value != 0 OR 34735 THEN error out
        }
    Process the first Short integer in the Key Entry Set
        {
        SET GeoKey to the value
        }
    Process the third Short integer in the Key Entry Set
        {
        SET KeyLength to the value
        }
    IF KeyLength = 1 THEN
        SET KeyValueOffset = GeoKeyDirectory + GeoKeyOffset + 6
    ELSE
        {
        Process the fourth Short integer in the Key Entry Set
            {
            SET KeyValueOffset to the value
            }
        SET KeyValueOffset = GeoKeyDirectory + (KeyValueOffset * 2)
        }


    Read a KeyLength Short values from the GeoTIFF file starting at KeyValueOffset.
    Validate the value
        Locate the GeoKey in the following table
        Verify that the values read satisfy the constraints defined in the associated Requirements Class.
        Verify that any GeoKeys required by the associated Requirements Class are present in the GeoKey Directory.</spec:method>
    <skos:definition>Short Parameters Test</skos:definition>
    <rdf:type rdf:resource="http://www.w3.org/2004/02/skos/core#Concept"/>
    <rdf:type rdf:resource="http://www.opengis.net/def/ont/modspec/ConformanceTest"/>
    <spec:testType rdf:resource="http://www.opengis.net/def/ont/modspec/Basic"/>
    <spec:purpose>Verify Short parameters</spec:purpose>
    <skos:broader rdf:resource="http://www.opengis.net/spec/GeoTIFF/1.1/conf/Core"/>
    <skos:prefLabel>Short Parameters Test</skos:prefLabel>
  </rdf:Description>
  <rdf:Description rdf:about="http://www.opengis.net/spec/GeoTIFF/1.1/req/ProjectionGeoKey.reserved">
    <rdf:type rdf:resource="http://www.opengis.net/def/ont/modspec/Requirement"/>
    <rdf:type rdf:resource="http://www.w3.org/2004/02/skos/core#Concept"/>
    <dct:description>ProjectionGeoKey values in the range 1-1023 SHALL be reserved</dct:description>
    <skos:broader rdf:resource="http://www.opengis.net/spec/GeoTIFF/1.1/req/ProjectionGeoKey"/>
    <skos:definition>ProjectionGeoKey values in the range 1-1023 SHALL be reserved</skos:definition>
    <skos:prefLabel>Requirement 26.3</skos:prefLabel>
  </rdf:Description>
  <rdf:Description rdf:about="http://www.opengis.net/spec/GeoTIFF/1.1/req/GeoKeyCode">
    <skos:prefLabel>Requirements Class GeoKeyCode</skos:prefLabel>
    <rdf:type rdf:resource="http://www.w3.org/2004/02/skos/core#Concept"/>
    <rdf:type rdf:resource="http://www.opengis.net/def/ont/modspec/RequirementClass"/>
    <skos:narrower rdf:resource="http://www.opengis.net/spec/GeoTIFF/1.1/req/GeoKeyCode.undefined"/>
    <skos:narrower rdf:resource="http://www.opengis.net/spec/GeoTIFF/1.1/req/GeoKeyCode.userDefined"/>
    <skos:broader rdf:resource="http://www.opengis.net/def/docs/19-008r4"/>
    <spec:normativeStatement rdf:resource="http://www.opengis.net/spec/GeoTIFF/1.1/req/GeoKeyCode.undefined"/>
    <spec:normativeStatement rdf:resource="http://www.opengis.net/spec/GeoTIFF/1.1/req/GeoKeyCode.userDefined"/>
    <skos:definition>For consistency, several key codes have the same meaning in all implemented GeoKeys

The undefined code means that this parameter is intentionally omitted or unknown.

In some cases, additional GeoKeys are required when the User-Defined value is used. Those requirements are included within a Requirements Class, where appropriate.</skos:definition>
  </rdf:Description>
  <rdf:Description rdf:about="http://www.opengis.net/spec/GeoTIFF/1.1/req/GeodeticDatumGeoKey.type">
    <skos:broader rdf:resource="http://www.opengis.net/spec/GeoTIFF/1.1/req/GeodeticDatumGeoKey"/>
    <dct:description>The GeodeticDatumGeoKey SHALL have type = SHORT</dct:description>
    <rdf:type rdf:resource="http://www.opengis.net/def/ont/modspec/Requirement"/>
    <rdf:type rdf:resource="http://www.w3.org/2004/02/skos/core#Concept"/>
    <skos:prefLabel>Requirement 18.2</skos:prefLabel>
    <skos:definition>The GeodeticDatumGeoKey SHALL have type = SHORT</skos:definition>
  </rdf:Description>
  <rdf:Description rdf:about="http://www.opengis.net/spec/GeoTIFF/1.1/req/VerticalDatumGeoKey">
    <rdf:type rdf:resource="http://www.w3.org/2004/02/skos/core#Concept"/>
    <rdf:type rdf:resource="http://www.opengis.net/def/ont/modspec/RequirementClass"/>
    <skos:narrower rdf:resource="http://www.opengis.net/spec/GeoTIFF/1.1/req/VerticalDatumGeoKey.EPSG"/>
    <skos:narrower rdf:resource="http://www.opengis.net/spec/GeoTIFF/1.1/req/VerticalDatumGeoKey.reserved"/>
    <skos:narrower rdf:resource="http://www.opengis.net/spec/GeoTIFF/1.1/req/VerticalDatumGeoKey.type"/>
    <skos:narrower rdf:resource="http://www.opengis.net/spec/GeoTIFF/1.1/req/VerticalDatumGeoKey.private"/>
    <skos:narrower rdf:resource="http://www.opengis.net/spec/GeoTIFF/1.1/req/VerticalDatumGeoKey.userdefined"/>
    <skos:narrower rdf:resource="http://www.opengis.net/spec/GeoTIFF/1.1/req/VerticalDatumGeoKey.ID"/>
    <spec:normativeStatement rdf:resource="http://www.opengis.net/spec/GeoTIFF/1.1/req/VerticalDatumGeoKey.ID"/>
    <spec:normativeStatement rdf:resource="http://www.opengis.net/spec/GeoTIFF/1.1/req/VerticalDatumGeoKey.EPSG"/>
    <spec:normativeStatement rdf:resource="http://www.opengis.net/spec/GeoTIFF/1.1/req/VerticalDatumGeoKey.type"/>
    <spec:normativeStatement rdf:resource="http://www.opengis.net/spec/GeoTIFF/1.1/req/VerticalDatumGeoKey.private"/>
    <spec:normativeStatement rdf:resource="http://www.opengis.net/spec/GeoTIFF/1.1/req/VerticalDatumGeoKey.userdefined"/>
    <spec:normativeStatement rdf:resource="http://www.opengis.net/spec/GeoTIFF/1.1/req/VerticalDatumGeoKey.reserved"/>
    <skos:broader rdf:resource="http://www.opengis.net/spec/GeoTIFF/1.1/conf/ShortParameters"/>
    <skos:broader rdf:resource="http://www.opengis.net/def/docs/19-008r4"/>
    <skos:definition>This key may be used to specify the vertical datum for a user-defined vertical coordinate reference system.</skos:definition>
    <skos:prefLabel>Requirements Class Vertical Datum</skos:prefLabel>
  </rdf:Description>
  <rdf:Description rdf:about="http://www.opengis.net/spec/GeoTIFF/1.1/req/GeodeticCRSGeoKey.reserved">
    <rdf:type rdf:resource="http://www.opengis.net/def/ont/modspec/Requirement"/>
    <rdf:type rdf:resource="http://www.w3.org/2004/02/skos/core#Concept"/>
    <skos:broader rdf:resource="http://www.opengis.net/spec/GeoTIFF/1.1/req/GeodeticCRSGeoKey"/>
    <skos:definition>GeodeticCRSGeoKey values in the range 1-1023 SHALL be reserved.NOTE: In
GeoTIFF v1.0 the reserved ranges were 1001-3999 and 5000-32766.</skos:definition>
    <dct:description>GeodeticCRSGeoKey values in the range 1-1023 SHALL be reserved.NOTE: In
GeoTIFF v1.0 the reserved ranges were 1001-3999 and 5000-32766.</dct:description>
    <skos:prefLabel>Requirement 13.3</skos:prefLabel>
  </rdf:Description>
  <rdf:Description rdf:about="http://www.opengis.net/spec/GeoTIFF/1.1/req/EllipsoidSemiMajorAxisGeoKey.ID">
    <skos:definition>The EllipsoidSemiMajorAxisGeoKey SHALL have ID = 2057</skos:definition>
    <rdf:type rdf:resource="http://www.opengis.net/def/ont/modspec/Requirement"/>
    <rdf:type rdf:resource="http://www.w3.org/2004/02/skos/core#Concept"/>
    <skos:broader rdf:resource="http://www.opengis.net/spec/GeoTIFF/1.1/req/EllipsoidSemiMajorAxisGeoKey"/>
    <dct:description>The EllipsoidSemiMajorAxisGeoKey SHALL have ID = 2057</dct:description>
    <skos:prefLabel>Requirement 22.1</skos:prefLabel>
  </rdf:Description>
  <rdf:Description rdf:about="http://www.opengis.net/spec/GeoTIFF/1.1/req/CitationGeoKeys.ID">
    <skos:broader rdf:resource="http://www.opengis.net/spec/GeoTIFF/1.1/req/CitationGeoKeys"/>
    <skos:prefLabel>Requirement 15.1</skos:prefLabel>
    <skos:definition>The GTCitationGeoKey SHALL have ID = 1026The GeodeticCitationGeoKey SHALL have
ID = 2049The ProjectedCitationGeoKey SHALL have ID = 3073The
VerticalCitationGeoKey SHALL have ID = 4097</skos:definition>
    <dct:description>The GTCitationGeoKey SHALL have ID = 1026The GeodeticCitationGeoKey SHALL have
ID = 2049The ProjectedCitationGeoKey SHALL have ID = 3073The
VerticalCitationGeoKey SHALL have ID = 4097</dct:description>
    <rdf:type rdf:resource="http://www.opengis.net/def/ont/modspec/Requirement"/>
    <rdf:type rdf:resource="http://www.w3.org/2004/02/skos/core#Concept"/>
  </rdf:Description>
  <rdf:Description rdf:about="http://www.opengis.net/spec/GeoTIFF/1.1/req/ModelTransformationTag">
    <rdf:type rdf:resource="http://www.opengis.net/def/ont/modspec/RequirementClass"/>
    <rdf:type rdf:resource="http://www.w3.org/2004/02/skos/core#Concept"/>
    <skos:definition></skos:definition>
    <skos:narrower rdf:resource="http://www.opengis.net/spec/GeoTIFF/1.1/req/ModelTransformationTag.count"/>
    <skos:narrower rdf:resource="http://www.opengis.net/spec/GeoTIFF/1.1/req/ModelTransformationTag.ID"/>
    <skos:narrower rdf:resource="http://www.opengis.net/spec/GeoTIFF/1.1/req/ModelTransformationTag.type"/>
    <spec:normativeStatement rdf:resource="http://www.opengis.net/spec/GeoTIFF/1.1/req/ModelTransformationTag.ID"/>
    <spec:normativeStatement rdf:resource="http://www.opengis.net/spec/GeoTIFF/1.1/req/ModelTransformationTag.count"/>
    <spec:normativeStatement rdf:resource="http://www.opengis.net/spec/GeoTIFF/1.1/req/ModelTransformationTag.type"/>
    <skos:broader rdf:resource="http://www.opengis.net/def/docs/19-008r4"/>
    <skos:prefLabel>Requirements Class ModelTransformationTag</skos:prefLabel>
  </rdf:Description>
  <rdf:Description rdf:about="http://www.opengis.net/spec/GeoTIFF/1.1/req/ProjectedCRSGeoKey.EPSG">
    <skos:definition>ProjectedCRSGeoKey values in the range 1024-32766 SHALL be EPSG Projected CRS
CodesNOTE: In GeoTIFF v1.0 the range was 20000-32760. Several values in this
range have been deprecated or deleted from the EPSG Dataset and should no
longer be used. See</skos:definition>
    <rdf:type rdf:resource="http://www.opengis.net/def/ont/modspec/Requirement"/>
    <rdf:type rdf:resource="http://www.w3.org/2004/02/skos/core#Concept"/>
    <skos:broader rdf:resource="http://www.opengis.net/spec/GeoTIFF/1.1/req/ProjectedCRSGeoKey"/>
    <dct:description>ProjectedCRSGeoKey values in the range 1024-32766 SHALL be EPSG Projected CRS
CodesNOTE: In GeoTIFF v1.0 the range was 20000-32760. Several values in this
range have been deprecated or deleted from the EPSG Dataset and should no
longer be used. See</dct:description>
    <skos:prefLabel>Requirement 12.4</skos:prefLabel>
  </rdf:Description>
  <rdf:Description rdf:about="http://www.opengis.net/spec/GeoTIFF/1.1/conf/Raster2Model_CoordinateTransformation_GeoKey/ModelPixelScaleTag">
    <skos:prefLabel>ModelPixelScaleTag Test</skos:prefLabel>
    <spec:requirement rdf:resource="http://www.opengis.net/spec/GeoTIFF/1.1/req/ModelPixelScaleTag.axisReversal"/>
    <spec:requirement rdf:resource="http://www.opengis.net/spec/GeoTIFF/1.1/req/ModelPixelScaleTag.standardConvention"/>
    <skos:narrower rdf:resource="http://www.opengis.net/spec/GeoTIFF/1.1/req/ModelPixelScaleTag.axisReversal"/>
    <skos:narrower rdf:resource="http://www.opengis.net/spec/GeoTIFF/1.1/req/ModelPixelScaleTag.standardConvention"/>
    <skos:broader rdf:resource="http://www.opengis.net/spec/GeoTIFF/1.1/conf/Raster2Model_CoordinateTransformation_GeoKey"/>
    <spec:method>Pre-conditions

The TagLength and TagValue values have been set.

Text Variables

**Variable**

|

**Scope**

|

**Description**

---|---|---

TagLength

|

Parameter

|

Length of the value of a TIFF Tag

TagValue

|

Parameter

|

Location of the value of a TIFF tag in the GeoTIFF file


    Verify that the TagLength is three (3)


    Read three double values from the GeoTIFF file starting at TagValue.</spec:method>
    <spec:method rdf:datatype="http://www.w3.org/1999/02/22-rdf-syntax-ns#HTML">%3Cdiv%3E%3Cdiv%3EPre-conditions%3Cdiv%3E%3Cdiv%3EThe%20TagLength%20and%20TagValue%20values%20have%20been%20set.%3C/div%3E%3C/div%3E%3Cdiv%20class%3D%22literalblock%22%3E%0A%3Cdiv%20class%3D%22content%22%3E%0A%3Cpre%3EVerify%20that%20the%20TagLength%20is%20three%20%283%29%3C/pre%3E%0A%3C/div%3E%0A%3C/div%3E%3Cdiv%20class%3D%22literalblock%22%3E%0A%3Cdiv%20class%3D%22content%22%3E%0A%3Cpre%3ERead%20three%20double%20values%20from%20the%20GeoTIFF%20file%20starting%20at%20TagValue.%3C/pre%3E%0A%3C/div%3E%0A%3C/div%3E</spec:method>
    <rdf:type rdf:resource="http://www.opengis.net/def/ont/modspec/ConformanceTest"/>
    <rdf:type rdf:resource="http://www.w3.org/2004/02/skos/core#Concept"/>
    <spec:purpose>Verify the contents of the ModelPixelScaleTag parameter</spec:purpose>
    <spec:testType rdf:resource="http://www.opengis.net/def/ont/modspec/Basic"/>
    <skos:definition>ModelPixelScaleTag Test</skos:definition>
  </rdf:Description>
  <rdf:Description rdf:about="http://www.opengis.net/spec/GeoTIFF/1.1/conf/AsciiParameters">
    <skos:definition>ASCII Parameters Test</skos:definition>
    <skos:narrower rdf:resource="http://www.opengis.net/spec/GeoTIFF/1.1/req/GeoKeyDirectoryTag.keyEntryKeyCount"/>
    <skos:narrower rdf:resource="http://www.opengis.net/spec/GeoTIFF/1.1/req/GeoKeyDirectoryTag.KeyEntryKeyID"/>
    <skos:narrower rdf:resource="http://www.opengis.net/spec/GeoTIFF/1.1/req/GeoKeyDirectoryTag.keyEntryValueOffset"/>
    <skos:narrower rdf:resource="http://www.opengis.net/spec/GeoTIFF/1.1/req/GeoKeyDirectoryTag.keyEntryTIFFTagLocation"/>
    <skos:narrower rdf:resource="http://www.opengis.net/spec/GeoTIFF/1.1/req/CitationGeoKeys"/>
    <skos:narrower rdf:resource="http://www.opengis.net/spec/GeoTIFF/1.1/req/GeoAsciiParamsTag.count"/>
    <skos:narrower rdf:resource="http://www.opengis.net/spec/GeoTIFF/1.1/req/GeoAsciiParamsTag.ID"/>
    <skos:broader rdf:resource="http://www.opengis.net/spec/GeoTIFF/1.1/conf/Core"/>
    <spec:requirement rdf:resource="http://www.opengis.net/spec/GeoTIFF/1.1/req/GeoKeyDirectoryTag.keyEntryTIFFTagLocation"/>
    <spec:requirement rdf:resource="http://www.opengis.net/spec/GeoTIFF/1.1/req/CitationGeoKeys"/>
    <spec:requirement rdf:resource="http://www.opengis.net/spec/GeoTIFF/1.1/req/GeoAsciiParamsTag.ID"/>
    <spec:requirement rdf:resource="http://www.opengis.net/spec/GeoTIFF/1.1/req/GeoKeyDirectoryTag.keyEntryKeyCount"/>
    <spec:requirement rdf:resource="http://www.opengis.net/spec/GeoTIFF/1.1/req/GeoKeyDirectoryTag.KeyEntryKeyID"/>
    <spec:requirement rdf:resource="http://www.opengis.net/spec/GeoTIFF/1.1/req/GeoKeyDirectoryTag.keyEntryValueOffset"/>
    <spec:requirement rdf:resource="http://www.opengis.net/spec/GeoTIFF/1.1/req/GeoAsciiParamsTag.count"/>
    <rdf:type rdf:resource="http://www.opengis.net/def/ont/modspec/ConformanceTest"/>
    <rdf:type rdf:resource="http://www.w3.org/2004/02/skos/core#Concept"/>
    <skos:prefLabel>ASCII Parameters Test</skos:prefLabel>
    <spec:method>Pre-conditions

The GeoKeyDirectory, ASCIIValues and GeoKeyOffset values have been set.

Text Variables

**Variable**

|

**Scope**

|

**Description**

---|---|---

GeoKeyDirectory

|

Global

|

Location of the GeoTIFF GeoKey directory

ASCIIValues

|

Global

|

Location of the ASCII values for GeoTIFF ASCII GeoKeys

GeoKeyOffset

|

Parameter

|

Location of this Key Entry Set in the GeoKey directory

GeoKey

|

Local

|

Temporary value of the GeoKey

KeyLength

|

Local

|

Temporary value for the length of the value for the GeoKey

KeyValueOffset

|

Local

|

The location of the GeoKey value in the file


    Locate the Key Entry Set using the GeoKeyDirectory and GeoKeyOffset values.


    Process the second Short integer in the Key Entry Set
        {
        IF value != 34737 THEN error out
        }
    Process the first Short integer in the Key Entry Set
        {
        Set GeoKey to the value
        }
    Process the third Short integer in the Key Entry Set
        {
        Set KeyLength to the value
        }
    Process the fourth Short integer in the Key Entry Set
        {
        SET KeyValueOffset to the value
        }
    SET KeyValueOffset = AsciiValues + KeyValueOffset


    Read a KeyLength ASCII string values from the GeoTIFF file starting at KeyValueOffset.
        - The individual strings are delimited by the | character.
        - The set of ASCII strings is null terminated.
    Validate the value
        Locate the GeoKey in the following table
        Verify that the values read satisfy the constraints defined in the associated Requirements Class.
        Verify that any GeoKeys required by the associated Requirements Class are present in the GeoKey Directory.</spec:method>
    <spec:method rdf:datatype="http://www.w3.org/1999/02/22-rdf-syntax-ns#HTML">%3Cdiv%3E%3Cdiv%3EPre-conditions%3Cdiv%3E%3Cdiv%3EThe%20GeoKeyDirectory%2C%20ASCIIValues%20and%20GeoKeyOffset%20values%20have%20been%20set.%3C/div%3E%3C/div%3E%3Cdiv%20class%3D%22literalblock%22%3E%0A%3Cdiv%20class%3D%22content%22%3E%0A%3Cpre%3ELocate%20the%20Key%20Entry%20Set%20using%20the%20GeoKeyDirectory%20and%20GeoKeyOffset%20values.%3C/pre%3E%0A%3C/div%3E%0A%3C/div%3E%3Cdiv%20class%3D%22literalblock%22%3E%0A%3Cdiv%20class%3D%22content%22%3E%0A%3Cpre%3EProcess%20the%20second%20Short%20integer%20in%20the%20Key%20Entry%20Set%0A%20%20%20%20%7B%0A%20%20%20%20IF%20value%20%21%3D%2034737%20THEN%20error%20out%0A%20%20%20%20%7D%0AProcess%20the%20first%20Short%20integer%20in%20the%20Key%20Entry%20Set%0A%20%20%20%20%7B%0A%20%20%20%20Set%20GeoKey%20to%20the%20value%0A%20%20%20%20%7D%0AProcess%20the%20third%20Short%20integer%20in%20the%20Key%20Entry%20Set%0A%20%20%20%20%7B%0A%20%20%20%20Set%20KeyLength%20to%20the%20value%0A%20%20%20%20%7D%0AProcess%20the%20fourth%20Short%20integer%20in%20the%20Key%20Entry%20Set%0A%20%20%20%20%7B%0A%20%20%20%20SET%20KeyValueOffset%20to%20the%20value%0A%20%20%20%20%7D%0ASET%20KeyValueOffset%20%3D%20AsciiValues%20%2B%20KeyValueOffset%3C/pre%3E%0A%3C/div%3E%0A%3C/div%3E%3Cdiv%20class%3D%22literalblock%22%3E%0A%3Cdiv%20class%3D%22content%22%3E%0A%3Cpre%3ERead%20a%20KeyLength%20ASCII%20string%20values%20from%20the%20GeoTIFF%20file%20starting%20at%20KeyValueOffset.%0A%20%20%20%20-%20The%20individual%20strings%20are%20delimited%20by%20the%20%22%7C%22%20character.%0A%20%20%20%20-%20The%20set%20of%20ASCII%20strings%20is%20null%20terminated.%0AValidate%20the%20value%0A%20%20%20%20Locate%20the%20GeoKey%20in%20the%20following%20table%0A%20%20%20%20Verify%20that%20the%20values%20read%20satisfy%20the%20constraints%20defined%20in%20the%20associated%20Requirements%20Class.%0A%20%20%20%20Verify%20that%20any%20GeoKeys%20required%20by%20the%20associated%20Requirements%20Class%20are%20present%20in%20the%20GeoKey%20Directory.%3C/pre%3E%0A%3C/div%3E%0A%3C/div%3E</spec:method>
    <spec:purpose>Verify ASCII parameters</spec:purpose>
    <spec:testType rdf:resource="http://www.opengis.net/def/ont/modspec/Basic"/>
  </rdf:Description>
  <rdf:Description rdf:about="http://www.opengis.net/spec/GeoTIFF/1.1/req/GTModelTypeGeoKey">
    <spec:normativeStatement rdf:resource="http://www.opengis.net/spec/GeoTIFF/1.1/req/GTModelTypeGeoKey.projCRS"/>
    <spec:normativeStatement rdf:resource="http://www.opengis.net/spec/GeoTIFF/1.1/req/GTModelTypeGeoKey.reserved"/>
    <spec:normativeStatement rdf:resource="http://www.opengis.net/spec/GeoTIFF/1.1/req/GTModelTypeGeoKey.private"/>
    <spec:normativeStatement rdf:resource="http://www.opengis.net/spec/GeoTIFF/1.1/req/GTModelTypeGeoKey.geocenCRS"/>
    <spec:normativeStatement rdf:resource="http://www.opengis.net/spec/GeoTIFF/1.1/req/GTModelTypeGeoKey.ID"/>
    <spec:normativeStatement rdf:resource="http://www.opengis.net/spec/GeoTIFF/1.1/req/GTModelTypeGeoKey.value"/>
    <spec:normativeStatement rdf:resource="http://www.opengis.net/spec/GeoTIFF/1.1/req/GTModelTypeGeoKey.userdefined"/>
    <spec:normativeStatement rdf:resource="http://www.opengis.net/spec/GeoTIFF/1.1/req/GTModelTypeGeoKey.type"/>
    <spec:normativeStatement rdf:resource="http://www.opengis.net/spec/GeoTIFF/1.1/req/GTModelTypeGeoKey.geogCRS"/>
    <spec:normativeStatement rdf:resource="http://www.opengis.net/spec/GeoTIFF/1.1/req/GTModelTypeGeoKey.required"/>
    <skos:narrower rdf:resource="http://www.opengis.net/spec/GeoTIFF/1.1/req/GTModelTypeGeoKey.geocenCRS"/>
    <skos:narrower rdf:resource="http://www.opengis.net/spec/GeoTIFF/1.1/req/GTModelTypeGeoKey.value"/>
    <skos:narrower rdf:resource="http://www.opengis.net/spec/GeoTIFF/1.1/req/GTModelTypeGeoKey.reserved"/>
    <skos:narrower rdf:resource="http://www.opengis.net/spec/GeoTIFF/1.1/req/GTModelTypeGeoKey.private"/>
    <skos:narrower rdf:resource="http://www.opengis.net/spec/GeoTIFF/1.1/req/GTModelTypeGeoKey.ID"/>
    <skos:narrower rdf:resource="http://www.opengis.net/spec/GeoTIFF/1.1/req/GTModelTypeGeoKey.userdefined"/>
    <skos:narrower rdf:resource="http://www.opengis.net/spec/GeoTIFF/1.1/req/GTModelTypeGeoKey.required"/>
    <skos:narrower rdf:resource="http://www.opengis.net/spec/GeoTIFF/1.1/req/GTModelTypeGeoKey.projCRS"/>
    <skos:narrower rdf:resource="http://www.opengis.net/spec/GeoTIFF/1.1/req/GTModelTypeGeoKey.type"/>
    <skos:narrower rdf:resource="http://www.opengis.net/spec/GeoTIFF/1.1/req/GTModelTypeGeoKey.geogCRS"/>
    <skos:prefLabel>Requirements Class GTModelTypeGeoKey</skos:prefLabel>
    <skos:definition>This GeoKey defines the type of Model coordinate reference system used, to which the transformation from the raster space is made:



Model CRS is unknown or unspecified;


Model CRS is a Geographic 2D CRS;


Model CRS is a Geocentric CRS;


Model CRS is a Projected CRS; and


Model CRS is user-defined.



If the Model coordinate reference system is from the GeoTIFF standard CRS register (i.e., EPSG register), then only the registered CRS code need be specified. See Requirements for definition of Model CRS (when Model is from GeoTIFF CRS register).

If the Model coordinate reference system is not from the GeoTIFF standard CRS register, then it requires the specification of some or all CRS elements. See Requirements for definition of user-defined Model CRS.

The GeoTIFF v1.0 format has also been used to describe pseudo-3D compound CRSs consisting of a projected CRS and a vertical CRS or a geographic 2D CRS and a vertical CRS, as well as a geographic 3D CRS. In this document, this usage is permitted but not explicitly described through the GTModelTypeGeoKey. Recommendations are given in Annex D.




Note


The GTCitationGeoKey is also provided to give an ASCII reference to published documentation on the overall configuration of the GeoTIFF file (see Requirements Class Citation GeoKeys).</skos:definition>
    <skos:broader rdf:resource="http://www.opengis.net/def/docs/19-008r4"/>
    <skos:broader rdf:resource="http://www.opengis.net/spec/GeoTIFF/1.1/conf/ShortParameters"/>
    <rdf:type rdf:resource="http://www.w3.org/2004/02/skos/core#Concept"/>
    <rdf:type rdf:resource="http://www.opengis.net/def/ont/modspec/RequirementClass"/>
  </rdf:Description>
  <rdf:Description rdf:about="http://www.opengis.net/spec/GeoTIFF/1.1/req/GeoKeyDirectoryTag.count">
    <dct:description>The GeoKeyDirectoryTag SHALL include at least 4 keys (short integers) as
header information</dct:description>
    <rdf:type rdf:resource="http://www.opengis.net/def/ont/modspec/Requirement"/>
    <rdf:type rdf:resource="http://www.w3.org/2004/02/skos/core#Concept"/>
    <skos:broader rdf:resource="http://www.opengis.net/spec/GeoTIFF/1.1/conf/TIFF.Tags"/>
    <skos:broader rdf:resource="http://www.opengis.net/spec/GeoTIFF/1.1/req/GeoKeyDirectoryTag"/>
    <skos:prefLabel>Requirement 2.3</skos:prefLabel>
    <skos:definition>The GeoKeyDirectoryTag SHALL include at least 4 keys (short integers) as
header information</skos:definition>
  </rdf:Description>
  <rdf:Description rdf:about="http://www.opengis.net/spec/GeoTIFF/1.1/csuite">
    <skos:narrower rdf:resource="http://www.opengis.net/spec/GeoTIFF/1.1/conf/Core"/>
    <skos:narrower rdf:resource="http://www.opengis.net/spec/GeoTIFF/1.1/conf/Raster2Model_CoordinateTransformation_GeoKey"/>
    <rdf:type rdf:resource="http://www.opengis.net/def/ont/modspec/ConformanceSuite"/>
    <rdf:type rdf:resource="http://www.w3.org/2004/02/skos/core#Concept"/>
    <spec:class rdf:resource="http://www.opengis.net/spec/GeoTIFF/1.1/conf/Core"/>
    <spec:class rdf:resource="http://www.opengis.net/spec/GeoTIFF/1.1/conf/Raster2Model_CoordinateTransformation_GeoKey"/>
  </rdf:Description>
  <rdf:Description rdf:about="http://www.opengis.net/spec/GeoTIFF/1.1/req/PrimeMeridianLongitudeGeoKey.type">
    <rdf:type rdf:resource="http://www.opengis.net/def/ont/modspec/Requirement"/>
    <rdf:type rdf:resource="http://www.w3.org/2004/02/skos/core#Concept"/>
    <skos:prefLabel>Requirement 20.2</skos:prefLabel>
    <skos:broader rdf:resource="http://www.opengis.net/spec/GeoTIFF/1.1/req/PrimeMeridianLongitudeGeoKey"/>
    <dct:description>The PrimeMeridianLongitudeGeoKey SHALL have type = DOUBLE</dct:description>
    <skos:definition>The PrimeMeridianLongitudeGeoKey SHALL have type = DOUBLE</skos:definition>
  </rdf:Description>
  <rdf:Description rdf:about="http://www.opengis.net/spec/GeoTIFF/1.1/req/GeoAsciiParamsTag.type">
    <skos:definition>The GeoAsciiParamsTag SHALL have type = ASCII</skos:definition>
    <rdf:type rdf:resource="http://www.opengis.net/def/ont/modspec/Requirement"/>
    <rdf:type rdf:resource="http://www.w3.org/2004/02/skos/core#Concept"/>
    <skos:broader rdf:resource="http://www.opengis.net/spec/GeoTIFF/1.1/conf/TIFF.Tags"/>
    <skos:broader rdf:resource="http://www.opengis.net/spec/GeoTIFF/1.1/req/GeoAsciiParamsTag"/>
    <skos:prefLabel>Requirement 6.5</skos:prefLabel>
    <dct:description>The GeoAsciiParamsTag SHALL have type = ASCII</dct:description>
  </rdf:Description>
  <rdf:Description rdf:about="http://www.opengis.net/spec/GeoTIFF/1.1/conf/Raster2Model_CoordinateTransformation_GeoKey/ModelTiepointTag">
    <skos:definition>ModelTiepointTag Test</skos:definition>
    <rdf:type rdf:resource="http://www.opengis.net/def/ont/modspec/ConformanceTest"/>
    <rdf:type rdf:resource="http://www.w3.org/2004/02/skos/core#Concept"/>
    <skos:broader rdf:resource="http://www.opengis.net/spec/GeoTIFF/1.1/conf/Raster2Model_CoordinateTransformation_GeoKey"/>
    <skos:prefLabel>ModelTiepointTag Test</skos:prefLabel>
    <spec:method>Pre-conditions

The TagLength and TagValue values have been set.

Text Variables

**Variable**

|

**Scope**

|

**Description**

---|---|---

TagLength

|

Parameter

|

Length of the value of a TIFF Tag

TagValue

|

Parameter

|

Location of the value of a TIFF tag in the GeoTIFF file


    Verify that the TagLength is six (6)


    Read six double values from the GeoTIFF file starting at TagValue.</spec:method>
    <spec:method rdf:datatype="http://www.w3.org/1999/02/22-rdf-syntax-ns#HTML">%3Cdiv%3E%3Cdiv%3EPre-conditions%3Cdiv%3E%3Cdiv%3EThe%20TagLength%20and%20TagValue%20values%20have%20been%20set.%3C/div%3E%3C/div%3E%3Cdiv%20class%3D%22literalblock%22%3E%0A%3Cdiv%20class%3D%22content%22%3E%0A%3Cpre%3EVerify%20that%20the%20TagLength%20is%20six%20%286%29%3C/pre%3E%0A%3C/div%3E%0A%3C/div%3E%3Cdiv%20class%3D%22literalblock%22%3E%0A%3Cdiv%20class%3D%22content%22%3E%0A%3Cpre%3ERead%20six%20double%20values%20from%20the%20GeoTIFF%20file%20starting%20at%20TagValue.%3C/pre%3E%0A%3C/div%3E%0A%3C/div%3E</spec:method>
    <spec:requirement rdf:resource="http://www.opengis.net/spec/GeoTIFF/1.1/req/ModelTiepointTag.count"/>
    <skos:narrower rdf:resource="http://www.opengis.net/spec/GeoTIFF/1.1/req/ModelTiepointTag.count"/>
    <spec:purpose>Verify the contents of the ModelTiepointTag parameter</spec:purpose>
    <spec:testType rdf:resource="http://www.opengis.net/def/ont/modspec/Basic"/>
  </rdf:Description>
  <rdf:Description rdf:about="http://www.opengis.net/spec/GeoTIFF/1.1/req/ProjMethodGeoKey.userdefined">
    <rdf:type rdf:resource="http://www.opengis.net/def/ont/modspec/Requirement"/>
    <rdf:type rdf:resource="http://www.w3.org/2004/02/skos/core#Concept"/>
    <skos:broader rdf:resource="http://www.opengis.net/spec/GeoTIFF/1.1/req/ProjMethodGeoKey"/>
    <skos:prefLabel>Requirement 27.5</skos:prefLabel>
    <skos:definition>If the ProjectionMethodGeoKey value is 32767 (User-Defined) then the
ProjectedCitationGeoKey and keys for each map projection parameter (coordinate
operation parameter) appropriate to that method SHALL be populated.</skos:definition>
    <dct:description>If the ProjectionMethodGeoKey value is 32767 (User-Defined) then the
ProjectedCitationGeoKey and keys for each map projection parameter (coordinate
operation parameter) appropriate to that method SHALL be populated.</dct:description>
  </rdf:Description>
  <rdf:Description rdf:about="http://www.opengis.net/spec/GeoTIFF/1.1/req/GeoKeyCode.undefined">
    <rdf:type rdf:resource="http://www.w3.org/2004/02/skos/core#Concept"/>
    <rdf:type rdf:resource="http://www.opengis.net/def/ont/modspec/Requirement"/>
    <skos:broader rdf:resource="http://www.opengis.net/spec/GeoTIFF/1.1/req/GeoKeyCode"/>
    <skos:definition>GeoKeys with a value of 0 SHALL indicate intentionally omitted parameters</skos:definition>
    <skos:prefLabel>Requirement 3.1</skos:prefLabel>
    <dct:description>GeoKeys with a value of 0 SHALL indicate intentionally omitted parameters</dct:description>
  </rdf:Description>
  <rdf:Description rdf:about="http://www.opengis.net/spec/GeoTIFF/1.1/req/GeoKeyDirectoryTag.keyEntry">
    <skos:broader rdf:resource="http://www.opengis.net/spec/GeoTIFF/1.1/conf/GeoKeyDirectory"/>
    <skos:broader rdf:resource="http://www.opengis.net/spec/GeoTIFF/1.1/req/GeoKeyDirectoryTag"/>
    <rdf:type rdf:resource="http://www.w3.org/2004/02/skos/core#Concept"/>
    <rdf:type rdf:resource="http://www.opengis.net/def/ont/modspec/Requirement"/>
    <skos:prefLabel>Requirement 2.12</skos:prefLabel>
    <dct:description>Each Key Entry in the Key Entry Set SHALL include 4 unsigned short integer
values</dct:description>
    <skos:definition>Each Key Entry in the Key Entry Set SHALL include 4 unsigned short integer
values</skos:definition>
  </rdf:Description>
  <rdf:Description rdf:about="http://www.opengis.net/spec/GeoTIFF/1.1/req/ByteOrder">
    <skos:broader rdf:resource="http://www.opengis.net/spec/GeoTIFF/1.1/conf/Core/test"/>
    <skos:broader rdf:resource="http://www.opengis.net/spec/GeoTIFF/1.1/req/Core"/>
    <skos:broader rdf:resource="http://www.opengis.net/spec/GeoTIFF/1.1/conf/TIFF.Tags"/>
    <rdf:type rdf:resource="http://www.w3.org/2004/02/skos/core#Concept"/>
    <rdf:type rdf:resource="http://www.opengis.net/def/ont/modspec/Requirement"/>
    <skos:prefLabel>Requirement 1.4</skos:prefLabel>
    <dct:description>GeoTIFF implementation software SHALL honor the 'byte-order' indicator by
performing byte swaps as necessary to provide an accurate in-memory
representation of the values encoded in the GeoTIFF file</dct:description>
    <skos:definition>GeoTIFF implementation software SHALL honor the 'byte-order' indicator by
performing byte swaps as necessary to provide an accurate in-memory
representation of the values encoded in the GeoTIFF file</skos:definition>
  </rdf:Description>
  <rdf:Description rdf:about="http://www.opengis.net/spec/GeoTIFF/1.1/req/CitationGeoKeys">
    <skos:broader rdf:resource="http://www.opengis.net/spec/GeoTIFF/1.1/conf/AsciiParameters"/>
    <skos:broader rdf:resource="http://www.opengis.net/def/docs/19-008r4"/>
    <spec:normativeStatement rdf:resource="http://www.opengis.net/spec/GeoTIFF/1.1/req/CitationGeoKeys.type"/>
    <spec:normativeStatement rdf:resource="http://www.opengis.net/spec/GeoTIFF/1.1/req/CitationGeoKeys.ID"/>
    <skos:narrower rdf:resource="http://www.opengis.net/spec/GeoTIFF/1.1/req/CitationGeoKeys.type"/>
    <skos:narrower rdf:resource="http://www.opengis.net/spec/GeoTIFF/1.1/req/CitationGeoKeys.ID"/>
    <rdf:type rdf:resource="http://www.opengis.net/def/ont/modspec/RequirementClass"/>
    <rdf:type rdf:resource="http://www.w3.org/2004/02/skos/core#Concept"/>
    <skos:definition>The GTCitationGeoKey is provided to give an ASCII reference to published documentation on the overall configuration of the GeoTIFF file.
The GeodeticCitationGeoKey, ProjectedCitationGeoKey and VerticalCitationGeoKey are used to describe Model CRS elements through ASCII free text. A citation may be included with a CRS identified through the GeoTIFF CRS register ([Requirements for definition of Model CRS (when Model CRS is from GeoTIFF CRS register)]). A citation is mandatory for a user-defined CRSs and CRS objects (Requirements for definition of user-defined Model CRS). The GeodeticCitationGeoKey, ProjectedCitationGeoKey and VerticalCitationGeoKey are used with CRSs and CRS components.




Note


In GeoTIFF 1.0 the GeodeticCitationGeoKey key was called GeogCitationGeoKey and the ProjectedCitationGeoKey key was called PCSCitationGeoKey.</skos:definition>
    <skos:prefLabel>Requirements Class Citation GeoKeys</skos:prefLabel>
  </rdf:Description>
  <rdf:Description rdf:about="http://www.opengis.net/spec/GeoTIFF/1.1/req/ModelPixelScaleTag.count">
    <skos:broader rdf:resource="http://www.opengis.net/spec/GeoTIFF/1.1/req/ModelPixelScaleTag"/>
    <skos:definition>The ModelPixelScaleTag SHALL have 3 values representing the scale factor in
the X, Y, and Z directions</skos:definition>
    <rdf:type rdf:resource="http://www.opengis.net/def/ont/modspec/Requirement"/>
    <rdf:type rdf:resource="http://www.w3.org/2004/02/skos/core#Concept"/>
    <dct:description>The ModelPixelScaleTag SHALL have 3 values representing the scale factor in
the X, Y, and Z directions</dct:description>
    <skos:prefLabel>Requirement 10.3</skos:prefLabel>
  </rdf:Description>
  <rdf:Description rdf:about="http://www.opengis.net/spec/GeoTIFF/1.1/req/GTRasterTypeGeoKey.value">
    <skos:prefLabel>Requirement 7.3</skos:prefLabel>
    <skos:definition>The GTRasterTypeGeoKey value SHALL be:* 0 to indicate that the Raster type is
undefined or unknown; or* 1 to indicate that the Raster type is PixelIsArea;
or* 2 to indicate that the Raster type is PixelIsPoint; or* 32767 to indicate
that the Raster type is user-defined.Recommendation: the use of 0 (undefined)
or 32767 (user-defined) is not recommended</skos:definition>
    <rdf:type rdf:resource="http://www.w3.org/2004/02/skos/core#Concept"/>
    <rdf:type rdf:resource="http://www.opengis.net/def/ont/modspec/Requirement"/>
    <skos:broader rdf:resource="http://www.opengis.net/spec/GeoTIFF/1.1/req/GTRasterTypeGeoKey"/>
    <dct:description>The GTRasterTypeGeoKey value SHALL be:* 0 to indicate that the Raster type is
undefined or unknown; or* 1 to indicate that the Raster type is PixelIsArea;
or* 2 to indicate that the Raster type is PixelIsPoint; or* 32767 to indicate
that the Raster type is user-defined.Recommendation: the use of 0 (undefined)
or 32767 (user-defined) is not recommended</dct:description>
  </rdf:Description>
  <rdf:Description rdf:about="http://www.opengis.net/spec/GeoTIFF/1.1/req/GTModelTypeGeoKey.reserved">
    <rdf:type rdf:resource="http://www.w3.org/2004/02/skos/core#Concept"/>
    <rdf:type rdf:resource="http://www.opengis.net/def/ont/modspec/Requirement"/>
    <skos:prefLabel>Requirement 8.5</skos:prefLabel>
    <skos:broader rdf:resource="http://www.opengis.net/spec/GeoTIFF/1.1/req/GTModelTypeGeoKey"/>
    <dct:description>GTModelTypeGeoKey values in the range 4-32766 SHALL be reserved</dct:description>
    <skos:definition>GTModelTypeGeoKey values in the range 4-32766 SHALL be reserved</skos:definition>
  </rdf:Description>
  <rdf:Description rdf:about="http://www.opengis.net/spec/GeoTIFF/1.1/req/UnitsGeoKey.userdefinedGeogLinear">
    <rdf:type rdf:resource="http://www.w3.org/2004/02/skos/core#Concept"/>
    <rdf:type rdf:resource="http://www.opengis.net/def/ont/modspec/Requirement"/>
    <skos:definition>A GeogLinearUnitsGeoKey value of 32767 SHALL be a user-defined linear unit. If
the value is 32767 (User-Defined) then the GeodeticCitationGeoKey and the
GeogLinearUnitSizeGeoKey SHALL be populated</skos:definition>
    <dct:description>A GeogLinearUnitsGeoKey value of 32767 SHALL be a user-defined linear unit. If
the value is 32767 (User-Defined) then the GeodeticCitationGeoKey and the
GeogLinearUnitSizeGeoKey SHALL be populated</dct:description>
    <skos:broader rdf:resource="http://www.opengis.net/spec/GeoTIFF/1.1/req/UnitsGeoKey"/>
    <skos:prefLabel>Requirement 16.7</skos:prefLabel>
  </rdf:Description>
  <rdf:Description rdf:about="http://www.opengis.net/spec/GeoTIFF/1.1/req/DataGeoTags">
    <dct:description>GeoTIFF files SHALL encode all GeoTIFF specific information using the
following specified reserved TIFF tags \- 34735 GeoKeyDirectoryTag (mandatory)
\- 34736 GeoDoubleParamsTag (optional) \- 34737 GeoAsciiParamsTag (optional)
\- 33550 ModelPixelScaleTag (optional) \- 33922 ModelTiepointTag (conditional)
\- 34264 ModelTransformationTag (conditional) The conditional tags shall
follow the following rules: \- One of ModelTiepointTag or
ModelTransformationTag SHALL be included in an Image File Directory (IFD) \-
If the ModelTransformationTag is included in an IFD, then a ModelPixelScaleTag
SHALL NOT be included \- If the ModelPixelScaleTag is included in an IFD, then
a ModelTiepointTag SHALL also be included.</dct:description>
    <skos:prefLabel>Requirement 1.2</skos:prefLabel>
    <rdf:type rdf:resource="http://www.opengis.net/def/ont/modspec/Requirement"/>
    <rdf:type rdf:resource="http://www.w3.org/2004/02/skos/core#Concept"/>
    <skos:broader rdf:resource="http://www.opengis.net/spec/GeoTIFF/1.1/conf/TIFF.Tags"/>
    <skos:broader rdf:resource="http://www.opengis.net/spec/GeoTIFF/1.1/req/Core"/>
    <skos:definition>GeoTIFF files SHALL encode all GeoTIFF specific information using the
following specified reserved TIFF tags \- 34735 GeoKeyDirectoryTag (mandatory)
\- 34736 GeoDoubleParamsTag (optional) \- 34737 GeoAsciiParamsTag (optional)
\- 33550 ModelPixelScaleTag (optional) \- 33922 ModelTiepointTag (conditional)
\- 34264 ModelTransformationTag (conditional) The conditional tags shall
follow the following rules: \- One of ModelTiepointTag or
ModelTransformationTag SHALL be included in an Image File Directory (IFD) \-
If the ModelTransformationTag is included in an IFD, then a ModelPixelScaleTag
SHALL NOT be included \- If the ModelPixelScaleTag is included in an IFD, then
a ModelTiepointTag SHALL also be included.</skos:definition>
  </rdf:Description>
  <rdf:Description rdf:about="http://www.opengis.net/spec/GeoTIFF/1.1/req/ProjectedCRSGeoKey.ID">
    <skos:prefLabel>Requirement 12.1</skos:prefLabel>
    <rdf:type rdf:resource="http://www.w3.org/2004/02/skos/core#Concept"/>
    <rdf:type rdf:resource="http://www.opengis.net/def/ont/modspec/Requirement"/>
    <skos:definition>The ProjectedCRSGeoKey SHALL have ID = 3072</skos:definition>
    <skos:broader rdf:resource="http://www.opengis.net/spec/GeoTIFF/1.1/req/ProjectedCRSGeoKey"/>
    <dct:description>The ProjectedCRSGeoKey SHALL have ID = 3072</dct:description>
  </rdf:Description>
  <rdf:Description rdf:about="http://www.opengis.net/spec/GeoTIFF/1.1/req/GeoKeyDirectoryTag.keyDirectoryVersion">
    <skos:definition>The first unsigned short integer in the GeoKeyDirectoryTag SHALL hold the
KeyDirectoryVersion.</skos:definition>
    <rdf:type rdf:resource="http://www.opengis.net/def/ont/modspec/Requirement"/>
    <rdf:type rdf:resource="http://www.w3.org/2004/02/skos/core#Concept"/>
    <skos:broader rdf:resource="http://www.opengis.net/spec/GeoTIFF/1.1/conf/GeoKeyDirectory"/>
    <skos:broader rdf:resource="http://www.opengis.net/spec/GeoTIFF/1.1/req/GeoKeyDirectoryTag"/>
    <dct:description>The first unsigned short integer in the GeoKeyDirectoryTag SHALL hold the
KeyDirectoryVersion.</dct:description>
    <skos:prefLabel>Requirement 2.4</skos:prefLabel>
  </rdf:Description>
  <rdf:Description rdf:about="http://www.opengis.net/spec/GeoTIFF/1.1/req/UnitsGeoKey.userdefinedProjLinear">
    <skos:broader rdf:resource="http://www.opengis.net/spec/GeoTIFF/1.1/req/UnitsGeoKey"/>
    <skos:definition>A ProjLinearUnitsGeoKey value of 32767 SHALL be a user-defined linear unit. If
the value is 32767 (User-Defined) then the ProjectedCitationGeoKey and the
ProjLinearUnitSizeGeoKey SHALL be populated.</skos:definition>
    <skos:prefLabel>Requirement 16.8</skos:prefLabel>
    <rdf:type rdf:resource="http://www.opengis.net/def/ont/modspec/Requirement"/>
    <rdf:type rdf:resource="http://www.w3.org/2004/02/skos/core#Concept"/>
    <dct:description>A ProjLinearUnitsGeoKey value of 32767 SHALL be a user-defined linear unit. If
the value is 32767 (User-Defined) then the ProjectedCitationGeoKey and the
ProjLinearUnitSizeGeoKey SHALL be populated.</dct:description>
  </rdf:Description>
  <rdf:Description rdf:about="http://www.opengis.net/spec/GeoTIFF/1.1/req/GTRasterTypeGeoKey.reserved">
    <skos:prefLabel>Requirement 7.4</skos:prefLabel>
    <rdf:type rdf:resource="http://www.opengis.net/def/ont/modspec/Requirement"/>
    <rdf:type rdf:resource="http://www.w3.org/2004/02/skos/core#Concept"/>
    <skos:broader rdf:resource="http://www.opengis.net/spec/GeoTIFF/1.1/req/GTRasterTypeGeoKey"/>
    <dct:description>GTRasterTypeGeoKey values in the range 3-32766 SHALL be reserved</dct:description>
    <skos:definition>GTRasterTypeGeoKey values in the range 3-32766 SHALL be reserved</skos:definition>
  </rdf:Description>
  <rdf:Description rdf:about="http://www.opengis.net/spec/GeoTIFF/1.1/reqVerticalGeoKey.private">
    <dct:description>VerticalGeoKey values in the range 32768-65535 SHALL be private</dct:description>
    <skos:broader rdf:resource="http://www.opengis.net/spec/GeoTIFF/1.1/req/VerticalGeoKey"/>
    <rdf:type rdf:resource="http://www.w3.org/2004/02/skos/core#Concept"/>
    <rdf:type rdf:resource="http://www.opengis.net/def/ont/modspec/Requirement"/>
    <skos:definition>VerticalGeoKey values in the range 32768-65535 SHALL be private</skos:definition>
    <skos:prefLabel>Requirement 14.6</skos:prefLabel>
  </rdf:Description>
  <rdf:Description rdf:about="http://www.opengis.net/spec/GeoTIFF/1.1/req/UnitsGeoKey.private">
    <rdf:type rdf:resource="http://www.opengis.net/def/ont/modspec/Requirement"/>
    <rdf:type rdf:resource="http://www.w3.org/2004/02/skos/core#Concept"/>
    <skos:definition>GeogAngularUnitsGeoKey, GeogAzimuthUnitsGeoKey, GeogLinearUnitsGeoKey,
ProjLinearUnitsGeoKey and VerticalUnitsGeoKey values in the range 32768-65535
SHALL be private.</skos:definition>
    <skos:prefLabel>Requirement 16.10</skos:prefLabel>
    <skos:broader rdf:resource="http://www.opengis.net/spec/GeoTIFF/1.1/req/UnitsGeoKey"/>
    <dct:description>GeogAngularUnitsGeoKey, GeogAzimuthUnitsGeoKey, GeogLinearUnitsGeoKey,
ProjLinearUnitsGeoKey and VerticalUnitsGeoKey values in the range 32768-65535
SHALL be private.</dct:description>
  </rdf:Description>
  <rdf:Description rdf:about="http://www.opengis.net/spec/GeoTIFF/1.1/req/VerticalGeoKey.reserved">
    <rdf:type rdf:resource="http://www.w3.org/2004/02/skos/core#Concept"/>
    <rdf:type rdf:resource="http://www.opengis.net/def/ont/modspec/Requirement"/>
    <skos:prefLabel>Requirement 14.3</skos:prefLabel>
    <dct:description>VerticalGeoKey values in the range 1-1023 SHALL be reservedNOTE: In GeoTIFF
v1.0 the reserved ranges were 0001-4999 and 6000-32766.</dct:description>
    <skos:definition>VerticalGeoKey values in the range 1-1023 SHALL be reservedNOTE: In GeoTIFF
v1.0 the reserved ranges were 0001-4999 and 6000-32766.</skos:definition>
    <skos:broader rdf:resource="http://www.opengis.net/spec/GeoTIFF/1.1/req/VerticalGeoKey"/>
  </rdf:Description>
  <rdf:Description rdf:about="http://www.opengis.net/spec/GeoTIFF/1.1/req/ModelTiepointTag">
    <spec:normativeStatement rdf:resource="http://www.opengis.net/spec/GeoTIFF/1.1/req/ModelTiepointTag.count"/>
    <spec:normativeStatement rdf:resource="http://www.opengis.net/spec/GeoTIFF/1.1/req/ModelTiepointTag.ID"/>
    <spec:normativeStatement rdf:resource="http://www.opengis.net/spec/GeoTIFF/1.1/req/ModelTiepointTag.type"/>
    <skos:narrower rdf:resource="http://www.opengis.net/spec/GeoTIFF/1.1/req/ModelTiepointTag.count"/>
    <skos:narrower rdf:resource="http://www.opengis.net/spec/GeoTIFF/1.1/req/ModelTiepointTag.type"/>
    <skos:narrower rdf:resource="http://www.opengis.net/spec/GeoTIFF/1.1/req/ModelTiepointTag.ID"/>
    <rdf:type rdf:resource="http://www.w3.org/2004/02/skos/core#Concept"/>
    <rdf:type rdf:resource="http://www.opengis.net/def/ont/modspec/RequirementClass"/>
    <skos:definition></skos:definition>
    <skos:broader rdf:resource="http://www.opengis.net/def/docs/19-008r4"/>
    <skos:prefLabel>Requirements Class ModelTiepointTag</skos:prefLabel>
  </rdf:Description>
  <rdf:Description rdf:about="http://www.opengis.net/spec/GeoTIFF/1.1/req/GeoAsciiParamsTag">
    <skos:definition>The following requirements govern the storage of parameter values when the values are of type ASCII. All text values in a TIFF file must be null-terminated ASCII.

Example of a GeoAscii tag containing only one string: NAD27 / UTM zone 11N|{NULL} (where {NULL} is the ASCII character of code 0)

Example of a GeoAscii tag containing two strings: NAD27 / UTM zone 11N|NAD27|{NULL}</skos:definition>
    <spec:normativeStatement rdf:resource="http://www.opengis.net/spec/GeoTIFF/1.1/req/GeoAsciiParamsTag.NULLWrite"/>
    <spec:normativeStatement rdf:resource="http://www.opengis.net/spec/GeoTIFF/1.1/req/GeoAsciiParamsTag.count"/>
    <spec:normativeStatement rdf:resource="http://www.opengis.net/spec/GeoTIFF/1.1/req/GeoAsciiParamsTag.terminator"/>
    <spec:normativeStatement rdf:resource="http://www.opengis.net/spec/GeoTIFF/1.1/req/GeoAsciiParamsTag.type"/>
    <spec:normativeStatement rdf:resource="http://www.opengis.net/spec/GeoTIFF/1.1/req/GeoAsciiParamsTag.ID"/>
    <rdf:type rdf:resource="http://www.opengis.net/def/ont/modspec/RequirementClass"/>
    <rdf:type rdf:resource="http://www.w3.org/2004/02/skos/core#Concept"/>
    <skos:broader rdf:resource="http://www.opengis.net/def/docs/19-008r4"/>
    <skos:narrower rdf:resource="http://www.opengis.net/spec/GeoTIFF/1.1/req/GeoAsciiParamsTag.NULLWrite"/>
    <skos:narrower rdf:resource="http://www.opengis.net/spec/GeoTIFF/1.1/req/GeoAsciiParamsTag.terminator"/>
    <skos:narrower rdf:resource="http://www.opengis.net/spec/GeoTIFF/1.1/req/GeoAsciiParamsTag.type"/>
    <skos:narrower rdf:resource="http://www.opengis.net/spec/GeoTIFF/1.1/req/GeoAsciiParamsTag.count"/>
    <skos:narrower rdf:resource="http://www.opengis.net/spec/GeoTIFF/1.1/req/GeoAsciiParamsTag.ID"/>
    <skos:prefLabel>Requirements Class GeoAsciiParamsTag</skos:prefLabel>
  </rdf:Description>
  <rdf:Description rdf:about="http://www.opengis.net/spec/GeoTIFF/1.1/req/GeoKeyDirectoryTag.keyEntryTIFFTagLocation">
    <dct:description>The second unsigned short integer in the Key Entry SHALL hold the TIFF Tag
Location. The value of this entry shall be a valid GeoTIFF tag identifier or a
zero (0)</dct:description>
    <skos:broader rdf:resource="http://www.opengis.net/spec/GeoTIFF/1.1/conf/AsciiParameters"/>
    <skos:broader rdf:resource="http://www.opengis.net/spec/GeoTIFF/1.1/conf/ShortParameters"/>
    <skos:broader rdf:resource="http://www.opengis.net/spec/GeoTIFF/1.1/conf/GeoKeyDirectory"/>
    <skos:broader rdf:resource="http://www.opengis.net/spec/GeoTIFF/1.1/req/GeoKeyDirectoryTag"/>
    <skos:broader rdf:resource="http://www.opengis.net/spec/GeoTIFF/1.1/conf/DoubleParameters"/>
    <rdf:type rdf:resource="http://www.opengis.net/def/ont/modspec/Requirement"/>
    <rdf:type rdf:resource="http://www.w3.org/2004/02/skos/core#Concept"/>
    <skos:definition>The second unsigned short integer in the Key Entry SHALL hold the TIFF Tag
Location. The value of this entry shall be a valid GeoTIFF tag identifier or a
zero (0)</skos:definition>
    <skos:prefLabel>Requirement 2.14</skos:prefLabel>
  </rdf:Description>
  <rdf:Description rdf:about="http://www.opengis.net/spec/GeoTIFF/1.1/req/UnitsGeoKey.userdefinedAngular">
    <rdf:type rdf:resource="http://www.opengis.net/def/ont/modspec/Requirement"/>
    <rdf:type rdf:resource="http://www.w3.org/2004/02/skos/core#Concept"/>
    <dct:description>A GeogAngularUnitsGeoKey or a GeogAzimuthUnitsGeoKey value of 32767 SHALL be a
user-defined angular unit. If the value is 32767 (User-Defined) then the
GeodeticCitationGeoKey and the GeogAngularUnitSizeGeoKey SHALL be populated</dct:description>
    <skos:definition>A GeogAngularUnitsGeoKey or a GeogAzimuthUnitsGeoKey value of 32767 SHALL be a
user-defined angular unit. If the value is 32767 (User-Defined) then the
GeodeticCitationGeoKey and the GeogAngularUnitSizeGeoKey SHALL be populated</skos:definition>
    <skos:broader rdf:resource="http://www.opengis.net/spec/GeoTIFF/1.1/req/UnitsGeoKey"/>
    <skos:prefLabel>Requirement 16.6</skos:prefLabel>
  </rdf:Description>
  <rdf:Description rdf:about="http://www.opengis.net/spec/GeoTIFF/1.1/req/GeoShortParamsTag.Criteria">
    <skos:prefLabel>Requirement 4.1</skos:prefLabel>
    <rdf:type rdf:resource="http://www.w3.org/2004/02/skos/core#Concept"/>
    <rdf:type rdf:resource="http://www.opengis.net/def/ont/modspec/Requirement"/>
    <skos:definition>In the case where a Parameter of type Short has more than one value, those
values SHALL be stored in the GeoKeysDirectory</skos:definition>
    <dct:description>In the case where a Parameter of type Short has more than one value, those
values SHALL be stored in the GeoKeysDirectory</dct:description>
    <skos:broader rdf:resource="http://www.opengis.net/spec/GeoTIFF/1.1/req/GeoShortParamsTag"/>
  </rdf:Description>
  <rdf:Description rdf:about="http://www.opengis.net/spec/GeoTIFF/1.1/req/PrimeMeridianGeoKey">
    <skos:narrower rdf:resource="http://www.opengis.net/spec/GeoTIFF/1.1/req/PrimeMeridianGeoKey.EPSG"/>
    <skos:narrower rdf:resource="http://www.opengis.net/spec/GeoTIFF/1.1/req/PrimeMeridianGeoKey.type"/>
    <skos:narrower rdf:resource="http://www.opengis.net/spec/GeoTIFF/1.1/req/PrimeMeridianGeoKey.userdefined"/>
    <skos:narrower rdf:resource="http://www.opengis.net/spec/GeoTIFF/1.1/req/PrimeMeridianGeoKey.reserved"/>
    <skos:narrower rdf:resource="http://www.opengis.net/spec/GeoTIFF/1.1/req/PrimeMeridianGeoKey.private"/>
    <skos:narrower rdf:resource="http://www.opengis.net/spec/GeoTIFF/1.1/req/PrimeMeridianGeoKey.ID"/>
    <skos:broader rdf:resource="http://www.opengis.net/def/docs/19-008r4"/>
    <skos:broader rdf:resource="http://www.opengis.net/spec/GeoTIFF/1.1/conf/ShortParameters"/>
    <skos:definition>This key is used to specify a Prime Meridian from the GeoTIFF CRS register or to indicate that the Prime Meridian is user-defined. The default is Greenwich, England.




Note


In GeoTIFF 1.0 this key was called GeogPrimeMeridianGeoKey.</skos:definition>
    <spec:normativeStatement rdf:resource="http://www.opengis.net/spec/GeoTIFF/1.1/req/PrimeMeridianGeoKey.EPSG"/>
    <spec:normativeStatement rdf:resource="http://www.opengis.net/spec/GeoTIFF/1.1/req/PrimeMeridianGeoKey.type"/>
    <spec:normativeStatement rdf:resource="http://www.opengis.net/spec/GeoTIFF/1.1/req/PrimeMeridianGeoKey.userdefined"/>
    <spec:normativeStatement rdf:resource="http://www.opengis.net/spec/GeoTIFF/1.1/req/PrimeMeridianGeoKey.private"/>
    <spec:normativeStatement rdf:resource="http://www.opengis.net/spec/GeoTIFF/1.1/req/PrimeMeridianGeoKey.reserved"/>
    <spec:normativeStatement rdf:resource="http://www.opengis.net/spec/GeoTIFF/1.1/req/PrimeMeridianGeoKey.ID"/>
    <rdf:type rdf:resource="http://www.opengis.net/def/ont/modspec/RequirementClass"/>
    <rdf:type rdf:resource="http://www.w3.org/2004/02/skos/core#Concept"/>
    <skos:prefLabel>Requirements Class PrimeMeridianGeoKey</skos:prefLabel>
  </rdf:Description>
  <rdf:Description rdf:about="http://www.opengis.net/spec/GeoTIFF/1.1/req/ProjMethodGeoKey.transform">
    <rdf:type rdf:resource="http://www.w3.org/2004/02/skos/core#Concept"/>
    <rdf:type rdf:resource="http://www.opengis.net/def/ont/modspec/Requirement"/>
    <skos:definition>ProjMethodGeoKey values in the range 1-27 SHALL be GeoTIFF map projection
method codesNOTE: See Annex C</skos:definition>
    <dct:description>ProjMethodGeoKey values in the range 1-27 SHALL be GeoTIFF map projection
method codesNOTE: See Annex C</dct:description>
    <skos:broader rdf:resource="http://www.opengis.net/spec/GeoTIFF/1.1/req/ProjMethodGeoKey"/>
    <skos:prefLabel>Requirement 27.3</skos:prefLabel>
  </rdf:Description>
  <rdf:Description rdf:about="http://www.opengis.net/spec/GeoTIFF/1.1/req/GeoKeyDirectoryTag.keyRevisionValue">
    <skos:definition>The value of KeyRevision SHALL be 1.</skos:definition>
    <skos:prefLabel>Requirement 2.7</skos:prefLabel>
    <skos:broader rdf:resource="http://www.opengis.net/spec/GeoTIFF/1.1/req/GeoKeyDirectoryTag"/>
    <skos:broader rdf:resource="http://www.opengis.net/spec/GeoTIFF/1.1/conf/GeoKeyDirectory"/>
    <rdf:type rdf:resource="http://www.w3.org/2004/02/skos/core#Concept"/>
    <rdf:type rdf:resource="http://www.opengis.net/def/ont/modspec/Requirement"/>
    <dct:description>The value of KeyRevision SHALL be 1.</dct:description>
  </rdf:Description>
  <rdf:Description rdf:about="http://www.opengis.net/spec/GeoTIFF/1.1/req/ModelPixelScaleTag.type">
    <skos:definition>The ModelPixelScaleTag SHALL have type = DOUBLE</skos:definition>
    <skos:prefLabel>Requirement 10.2</skos:prefLabel>
    <rdf:type rdf:resource="http://www.opengis.net/def/ont/modspec/Requirement"/>
    <rdf:type rdf:resource="http://www.w3.org/2004/02/skos/core#Concept"/>
    <skos:broader rdf:resource="http://www.opengis.net/spec/GeoTIFF/1.1/conf/TIFF.Tags"/>
    <skos:broader rdf:resource="http://www.opengis.net/spec/GeoTIFF/1.1/req/ModelPixelScaleTag"/>
    <dct:description>The ModelPixelScaleTag SHALL have type = DOUBLE</dct:description>
  </rdf:Description>
  <rdf:Description rdf:about="http://www.opengis.net/spec/GeoTIFF/1.1/req/GeodeticDatumGeoKey">
    <spec:normativeStatement rdf:resource="http://www.opengis.net/spec/GeoTIFF/1.1/req/GeodeticDatumGeoKey.EPSG"/>
    <spec:normativeStatement rdf:resource="http://www.opengis.net/spec/GeoTIFF/1.1/req/GeodeticDatumGeoKey.private"/>
    <spec:normativeStatement rdf:resource="http://www.opengis.net/spec/GeoTIFF/1.1/req/GeodeticDatumGeoKey.reserved"/>
    <spec:normativeStatement rdf:resource="http://www.opengis.net/spec/GeoTIFF/1.1/req/GeodeticDatumGeoKey.userdefined"/>
    <spec:normativeStatement rdf:resource="http://www.opengis.net/spec/GeoTIFF/1.1/req/GeodeticDatumGeoKey.ID"/>
    <spec:normativeStatement rdf:resource="http://www.opengis.net/spec/GeoTIFF/1.1/req/GeodeticDatumGeoKey.type"/>
    <skos:broader rdf:resource="http://www.opengis.net/def/docs/19-008r4"/>
    <skos:broader rdf:resource="http://www.opengis.net/spec/GeoTIFF/1.1/conf/ShortParameters"/>
    <rdf:type rdf:resource="http://www.w3.org/2004/02/skos/core#Concept"/>
    <rdf:type rdf:resource="http://www.opengis.net/def/ont/modspec/RequirementClass"/>
    <skos:narrower rdf:resource="http://www.opengis.net/spec/GeoTIFF/1.1/req/GeodeticDatumGeoKey.userdefined"/>
    <skos:narrower rdf:resource="http://www.opengis.net/spec/GeoTIFF/1.1/req/GeodeticDatumGeoKey.private"/>
    <skos:narrower rdf:resource="http://www.opengis.net/spec/GeoTIFF/1.1/req/GeodeticDatumGeoKey.reserved"/>
    <skos:narrower rdf:resource="http://www.opengis.net/spec/GeoTIFF/1.1/req/GeodeticDatumGeoKey.ID"/>
    <skos:narrower rdf:resource="http://www.opengis.net/spec/GeoTIFF/1.1/req/GeodeticDatumGeoKey.EPSG"/>
    <skos:narrower rdf:resource="http://www.opengis.net/spec/GeoTIFF/1.1/req/GeodeticDatumGeoKey.type"/>
    <skos:definition>This key is used to specify a geodetic datum from the GeoTIFF CRS register, or to indicate that the geodetic datum or one or both of its component ellipsoid or prime meridian is user-defined.




Note


In GeoTIFF 1.0 this key was called GeogGeodeticDatumGeoKey.</skos:definition>
    <skos:prefLabel>Requirements Class GeodeticDatumGeoKey</skos:prefLabel>
  </rdf:Description>
  <rdf:Description rdf:about="http://www.opengis.net/spec/GeoTIFF/1.1/req/GeoShortParamsTag.Location">
    <skos:prefLabel>Requirement 4.2</skos:prefLabel>
    <rdf:type rdf:resource="http://www.opengis.net/def/ont/modspec/Requirement"/>
    <rdf:type rdf:resource="http://www.w3.org/2004/02/skos/core#Concept"/>
    <skos:broader rdf:resource="http://www.opengis.net/spec/GeoTIFF/1.1/req/GeoShortParamsTag"/>
    <dct:description>Parameter values stored in the GeoKeysDirectory SHALL appear after the last
Key Entry</dct:description>
    <skos:definition>Parameter values stored in the GeoKeysDirectory SHALL appear after the last
Key Entry</skos:definition>
  </rdf:Description>
  <rdf:Description rdf:about="http://www.opengis.net/spec/GeoTIFF/1.1/req/ModelPixelScaleTag.axisReversal">
    <skos:broader rdf:resource="http://www.opengis.net/spec/GeoTIFF/1.1/req/ModelPixelScaleTag"/>
    <skos:broader rdf:resource="http://www.opengis.net/spec/GeoTIFF/1.1/conf/Raster2Model_CoordinateTransformation_GeoKey/ModelPixelScaleTag"/>
    <skos:prefLabel>Requirement 10.5</skos:prefLabel>
    <dct:description>Simple reversals of orientation from the standard relationship between raster
and model space (e.g., horizontal or vertical flips) SHALL be indicated by
reversal of sign in the corresponding component of the ModelPixelScaleTag.
GeoTIFF compliant readers shall honor this sign-reversal convention.</dct:description>
    <rdf:type rdf:resource="http://www.opengis.net/def/ont/modspec/Requirement"/>
    <rdf:type rdf:resource="http://www.w3.org/2004/02/skos/core#Concept"/>
    <skos:definition>Simple reversals of orientation from the standard relationship between raster
and model space (e.g., horizontal or vertical flips) SHALL be indicated by
reversal of sign in the corresponding component of the ModelPixelScaleTag.
GeoTIFF compliant readers shall honor this sign-reversal convention.</skos:definition>
  </rdf:Description>
  <rdf:Description rdf:about="http://www.opengis.net/spec/GeoTIFF/1.1/req/ProjectedCRSGeoKey.type">
    <rdf:type rdf:resource="http://www.w3.org/2004/02/skos/core#Concept"/>
    <rdf:type rdf:resource="http://www.opengis.net/def/ont/modspec/Requirement"/>
    <skos:broader rdf:resource="http://www.opengis.net/spec/GeoTIFF/1.1/req/ProjectedCRSGeoKey"/>
    <dct:description>The ProjectedCRSGeoKey SHALL have type = SHORT</dct:description>
    <skos:prefLabel>Requirement 12.2</skos:prefLabel>
    <skos:definition>The ProjectedCRSGeoKey SHALL have type = SHORT</skos:definition>
  </rdf:Description>
  <rdf:Description rdf:about="http://www.opengis.net/spec/GeoTIFF/1.1/conf/Raster2Model_CoordinateTransformation_GeoKey">
    <skos:narrower rdf:resource="http://www.opengis.net/spec/GeoTIFF/1.1/conf/Raster2Model_CoordinateTransformation_GeoKey/ModelTiepointTag"/>
    <skos:narrower rdf:resource="http://www.opengis.net/spec/GeoTIFF/1.1/conf/Raster2Model_CoordinateTransformation_GeoKey/ModelPixelScaleTag"/>
    <skos:narrower rdf:resource="http://www.opengis.net/spec/GeoTIFF/1.1/conf/Raster2Model_CoordinateTransformation_GeoKey/ModelTransformationTag"/>
    <skos:broader rdf:resource="http://www.opengis.net/spec/GeoTIFF/1.1/csuite"/>
    <skos:definition>Conformance Class Raster2Model_CoordinateTransformation_GeoKey</skos:definition>
    <rdf:type rdf:resource="http://www.opengis.net/def/ont/modspec/ConformanceClass"/>
    <rdf:type rdf:resource="http://www.w3.org/2004/02/skos/core#Concept"/>
    <spec:conformanceTest rdf:resource="http://www.opengis.net/spec/GeoTIFF/1.1/conf/Raster2Model_CoordinateTransformation_GeoKey/ModelTiepointTag"/>
    <spec:conformanceTest rdf:resource="http://www.opengis.net/spec/GeoTIFF/1.1/conf/Raster2Model_CoordinateTransformation_GeoKey/ModelPixelScaleTag"/>
    <spec:conformanceTest rdf:resource="http://www.opengis.net/spec/GeoTIFF/1.1/conf/Raster2Model_CoordinateTransformation_GeoKey/ModelTransformationTag"/>
    <skos:prefLabel>Conformance Class Raster2Model_CoordinateTransformation_GeoKey</skos:prefLabel>
  </rdf:Description>
  <rdf:Description rdf:about="http://www.opengis.net/spec/GeoTIFF/1.1/req/GeodeticDatumGeoKey.reserved">
    <skos:definition>GeodeticDatumGeoKey values in the range 1-1023 SHALL be reserved.NOTE: In
GeoTIFF v1.0 the reserved ranges were 1001-5999 and 7000-32766.</skos:definition>
    <rdf:type rdf:resource="http://www.w3.org/2004/02/skos/core#Concept"/>
    <rdf:type rdf:resource="http://www.opengis.net/def/ont/modspec/Requirement"/>
    <skos:prefLabel>Requirement 18.3</skos:prefLabel>
    <skos:broader rdf:resource="http://www.opengis.net/spec/GeoTIFF/1.1/req/GeodeticDatumGeoKey"/>
    <dct:description>GeodeticDatumGeoKey values in the range 1-1023 SHALL be reserved.NOTE: In
GeoTIFF v1.0 the reserved ranges were 1001-5999 and 7000-32766.</dct:description>
  </rdf:Description>
  <rdf:Description rdf:about="http://www.opengis.net/spec/GeoTIFF/1.1/req/GTModelTypeGeoKey.ID">
    <rdf:type rdf:resource="http://www.opengis.net/def/ont/modspec/Requirement"/>
    <rdf:type rdf:resource="http://www.w3.org/2004/02/skos/core#Concept"/>
    <dct:description>The GTModelTypeGeoKey SHALL have ID = 1024</dct:description>
    <skos:broader rdf:resource="http://www.opengis.net/spec/GeoTIFF/1.1/req/GTModelTypeGeoKey"/>
    <skos:definition>The GTModelTypeGeoKey SHALL have ID = 1024</skos:definition>
    <skos:prefLabel>Requirement 8.2</skos:prefLabel>
  </rdf:Description>
  <rdf:Description rdf:about="http://www.opengis.net/spec/GeoTIFF/1.1/req/GTModelTypeGeoKey.projCRS">
    <rdf:type rdf:resource="http://www.opengis.net/def/ont/modspec/Requirement"/>
    <rdf:type rdf:resource="http://www.w3.org/2004/02/skos/core#Concept"/>
    <skos:broader rdf:resource="http://www.opengis.net/spec/GeoTIFF/1.1/req/GTModelTypeGeoKey"/>
    <dct:description>If the GTModelTypeGeoKey value is 1 (Model CRS is a projected 2D CRS) then the
GeoTIFF file SHALL include a ProjectedCRSGeoKey.</dct:description>
    <skos:definition>If the GTModelTypeGeoKey value is 1 (Model CRS is a projected 2D CRS) then the
GeoTIFF file SHALL include a ProjectedCRSGeoKey.</skos:definition>
    <skos:prefLabel>Requirement 8.7</skos:prefLabel>
  </rdf:Description>
  <rdf:Description rdf:about="http://www.opengis.net/spec/GeoTIFF/1.1/req/ProjectedCRSGeoKey.reserved">
    <rdf:type rdf:resource="http://www.opengis.net/def/ont/modspec/Requirement"/>
    <rdf:type rdf:resource="http://www.w3.org/2004/02/skos/core#Concept"/>
    <skos:definition>ProjectedCRSGeoKey values in the range 1-1023 SHALL be reserved.</skos:definition>
    <skos:broader rdf:resource="http://www.opengis.net/spec/GeoTIFF/1.1/req/ProjectedCRSGeoKey"/>
    <dct:description>ProjectedCRSGeoKey values in the range 1-1023 SHALL be reserved.</dct:description>
    <skos:prefLabel>Requirement 12.3</skos:prefLabel>
  </rdf:Description>
  <rdf:Description rdf:about="http://www.opengis.net/spec/GeoTIFF/1.1/req/DataTypes">
    <dct:description>GeoTIFF implementation software SHALL support all documented TIFF 6.0 tag
data-types, and in particular ASCII, SHORT and the IEEE double-precision
floating point DOUBLE types</dct:description>
    <skos:broader rdf:resource="http://www.opengis.net/spec/GeoTIFF/1.1/req/Core"/>
    <skos:broader rdf:resource="http://www.opengis.net/spec/GeoTIFF/1.1/conf/Core/test"/>
    <rdf:type rdf:resource="http://www.w3.org/2004/02/skos/core#Concept"/>
    <rdf:type rdf:resource="http://www.opengis.net/def/ont/modspec/Requirement"/>
    <skos:definition>GeoTIFF implementation software SHALL support all documented TIFF 6.0 tag
data-types, and in particular ASCII, SHORT and the IEEE double-precision
floating point DOUBLE types</skos:definition>
    <skos:prefLabel>Requirement 1.3</skos:prefLabel>
  </rdf:Description>
  <rdf:Description rdf:about="http://www.opengis.net/spec/GeoTIFF/1.1/req/ProjectionGeoKey.private">
    <skos:broader rdf:resource="http://www.opengis.net/spec/GeoTIFF/1.1/req/ProjectionGeoKey"/>
    <dct:description>ProjectionGeoKey values in the range 32768-65535 SHALL be private</dct:description>
    <rdf:type rdf:resource="http://www.opengis.net/def/ont/modspec/Requirement"/>
    <rdf:type rdf:resource="http://www.w3.org/2004/02/skos/core#Concept"/>
    <skos:prefLabel>Requirement 26.6</skos:prefLabel>
    <skos:definition>ProjectionGeoKey values in the range 32768-65535 SHALL be private</skos:definition>
  </rdf:Description>
  <rdf:Description rdf:about="http://www.opengis.net/spec/GeoTIFF/1.1/req/ProjectionGeoKey.EPSG">
    <skos:definition>ProjectionGeoKey values in the range 1024-32766 SHALL be valid EPSG map
projection (coordinate operation) codesNOTE: In GeoTIFF v1.0 the range was
10000-19999. Several values in this range have been deprecated or deleted from
the EPSG Dataset. See</skos:definition>
    <skos:broader rdf:resource="http://www.opengis.net/spec/GeoTIFF/1.1/req/ProjectionGeoKey"/>
    <skos:prefLabel>Requirement 26.4</skos:prefLabel>
    <rdf:type rdf:resource="http://www.opengis.net/def/ont/modspec/Requirement"/>
    <rdf:type rdf:resource="http://www.w3.org/2004/02/skos/core#Concept"/>
    <dct:description>ProjectionGeoKey values in the range 1024-32766 SHALL be valid EPSG map
projection (coordinate operation) codesNOTE: In GeoTIFF v1.0 the range was
10000-19999. Several values in this range have been deprecated or deleted from
the EPSG Dataset. See</dct:description>
  </rdf:Description>
  <rdf:Description rdf:about="http://www.opengis.net/spec/GeoTIFF/1.1/conf/Raster2Model_CoordinateTransformation_GeoKey/ModelTransformationTag">
    <spec:testType rdf:resource="http://www.opengis.net/def/ont/modspec/Basic"/>
    <skos:prefLabel>ModelTransformationTag Test</skos:prefLabel>
    <skos:broader rdf:resource="http://www.opengis.net/spec/GeoTIFF/1.1/conf/Raster2Model_CoordinateTransformation_GeoKey"/>
    <rdf:type rdf:resource="http://www.opengis.net/def/ont/modspec/ConformanceTest"/>
    <rdf:type rdf:resource="http://www.w3.org/2004/02/skos/core#Concept"/>
    <spec:method rdf:datatype="http://www.w3.org/1999/02/22-rdf-syntax-ns#HTML">%3Cdiv%3E%3Cdiv%3EPre-conditions%3Cdiv%3E%3Cdiv%3EThe%20TagLength%20and%20TagValue%20values%20have%20been%20set.%3C/div%3E%3C/div%3E%3Cdiv%20class%3D%22literalblock%22%3E%0A%3Cdiv%20class%3D%22content%22%3E%0A%3Cpre%3EVerify%20that%20the%20TagLength%20is%20sixteen%20%2816%29%3C/pre%3E%0A%3C/div%3E%0A%3C/div%3E%3Cdiv%20class%3D%22literalblock%22%3E%0A%3Cdiv%20class%3D%22content%22%3E%0A%3Cpre%3ERead%20sixteen%20double%20values%20from%20the%20GeoTIFF%20file%20starting%20at%20TagValue.%3C/pre%3E%0A%3C/div%3E%0A%3C/div%3E</spec:method>
    <spec:method>Pre-conditions

The TagLength and TagValue values have been set.

Text Variables

**Variable**

|

**Scope**

|

**Description**

---|---|---

TagLength

|

Parameter

|

Length of the value of a TIFF Tag

TagValue

|

Parameter

|

Location of the value of a TIFF tag in the GeoTIFF file


    Verify that the TagLength is sixteen (16)


    Read sixteen double values from the GeoTIFF file starting at TagValue.</spec:method>
    <spec:purpose>Verify the contents of the ModelTransformationTag parameter</spec:purpose>
    <spec:requirement rdf:resource="http://www.opengis.net/spec/GeoTIFF/1.1/req/ModelTransformationTag.count"/>
    <skos:narrower rdf:resource="http://www.opengis.net/spec/GeoTIFF/1.1/req/ModelTransformationTag.count"/>
    <skos:definition>ModelTransformationTag Test</skos:definition>
  </rdf:Description>
  <rdf:Description rdf:about="http://www.opengis.net/spec/GeoTIFF/1.1/req/ModelTiepointTag.count">
    <skos:prefLabel>Requirement 9.3</skos:prefLabel>
    <skos:definition>The ModelTiepointTag SHALL have 6 values for each of the tiepoints</skos:definition>
    <skos:broader rdf:resource="http://www.opengis.net/spec/GeoTIFF/1.1/conf/Raster2Model_CoordinateTransformation_GeoKey/ModelTiepointTag"/>
    <skos:broader rdf:resource="http://www.opengis.net/spec/GeoTIFF/1.1/req/ModelTiepointTag"/>
    <rdf:type rdf:resource="http://www.opengis.net/def/ont/modspec/Requirement"/>
    <rdf:type rdf:resource="http://www.w3.org/2004/02/skos/core#Concept"/>
    <dct:description>The ModelTiepointTag SHALL have 6 values for each of the tiepoints</dct:description>
  </rdf:Description>
  <rdf:Description rdf:about="http://www.opengis.net/spec/GeoTIFF/1.1/req/GeodeticCRSGeoKey.type">
    <skos:broader rdf:resource="http://www.opengis.net/spec/GeoTIFF/1.1/req/GeodeticCRSGeoKey"/>
    <rdf:type rdf:resource="http://www.opengis.net/def/ont/modspec/Requirement"/>
    <rdf:type rdf:resource="http://www.w3.org/2004/02/skos/core#Concept"/>
    <skos:definition>The GeodeticCRSGeoKey SHALL have type = SHORT</skos:definition>
    <dct:description>The GeodeticCRSGeoKey SHALL have type = SHORT</dct:description>
    <skos:prefLabel>Requirement 13.2</skos:prefLabel>
  </rdf:Description>
  <rdf:Description rdf:about="http://www.opengis.net/spec/GeoTIFF/1.1/req/GeoAsciiParamsTag.ID">
    <skos:broader rdf:resource="http://www.opengis.net/spec/GeoTIFF/1.1/conf/AsciiParameters"/>
    <skos:broader rdf:resource="http://www.opengis.net/spec/GeoTIFF/1.1/conf/TIFF.Tags"/>
    <skos:broader rdf:resource="http://www.opengis.net/spec/GeoTIFF/1.1/req/GeoAsciiParamsTag"/>
    <skos:prefLabel>Requirement 6.1</skos:prefLabel>
    <skos:definition>The GeoAsciiParamsTag SHALL have ID = 34737</skos:definition>
    <rdf:type rdf:resource="http://www.opengis.net/def/ont/modspec/Requirement"/>
    <rdf:type rdf:resource="http://www.w3.org/2004/02/skos/core#Concept"/>
    <dct:description>The GeoAsciiParamsTag SHALL have ID = 34737</dct:description>
  </rdf:Description>
  <rdf:Description rdf:about="http://www.opengis.net/spec/GeoTIFF/1.1/req/GeodeticCRSGeoKey.private">
    <skos:definition>GeodeticCRSGeoKey values in the range 32768-65535 SHALL be private</skos:definition>
    <skos:broader rdf:resource="http://www.opengis.net/spec/GeoTIFF/1.1/req/GeodeticCRSGeoKey"/>
    <rdf:type rdf:resource="http://www.opengis.net/def/ont/modspec/Requirement"/>
    <rdf:type rdf:resource="http://www.w3.org/2004/02/skos/core#Concept"/>
    <skos:prefLabel>Requirement 13.6</skos:prefLabel>
    <dct:description>GeodeticCRSGeoKey values in the range 32768-65535 SHALL be private</dct:description>
  </rdf:Description>
  <rdf:Description rdf:about="http://www.opengis.net/spec/GeoTIFF/1.1/req/GeoShortParamsTag">
    <rdf:type rdf:resource="http://www.opengis.net/def/ont/modspec/RequirementClass"/>
    <rdf:type rdf:resource="http://www.w3.org/2004/02/skos/core#Concept"/>
    <skos:narrower rdf:resource="http://www.opengis.net/spec/GeoTIFF/1.1/req/GeoShortParamsTag.Location"/>
    <skos:narrower rdf:resource="http://www.opengis.net/spec/GeoTIFF/1.1/req/GeoShortParamsTag.Criteria"/>
    <skos:broader rdf:resource="http://www.opengis.net/def/docs/19-008r4"/>
    <spec:normativeStatement rdf:resource="http://www.opengis.net/spec/GeoTIFF/1.1/req/GeoShortParamsTag.Location"/>
    <spec:normativeStatement rdf:resource="http://www.opengis.net/spec/GeoTIFF/1.1/req/GeoShortParamsTag.Criteria"/>
    <skos:prefLabel>Requirements Class GeoShortParamsTag</skos:prefLabel>
    <skos:definition>The following requirements govern the storage of parameter values when there are two or more values of type Short.</skos:definition>
  </rdf:Description>
  <rdf:Description rdf:about="http://www.opengis.net/spec/GeoTIFF/1.1/req/GeoKeyDirectoryTag.keyDirectoryVersionValue">
    <skos:prefLabel>Requirement 2.5</skos:prefLabel>
    <rdf:type rdf:resource="http://www.opengis.net/def/ont/modspec/Requirement"/>
    <rdf:type rdf:resource="http://www.w3.org/2004/02/skos/core#Concept"/>
    <skos:broader rdf:resource="http://www.opengis.net/spec/GeoTIFF/1.1/req/GeoKeyDirectoryTag"/>
    <skos:broader rdf:resource="http://www.opengis.net/spec/GeoTIFF/1.1/conf/GeoKeyDirectory"/>
    <skos:definition>The value of KeyDirectoryVersion SHALL be 1.</skos:definition>
    <dct:description>The value of KeyDirectoryVersion SHALL be 1.</dct:description>
  </rdf:Description>
  <rdf:Description rdf:about="http://www.opengis.net/spec/GeoTIFF/1.1/req/ProjMethodGeoKey.private">
    <dct:description>ProjMethodGeoKey values in the range 32768-65535 SHALL be private</dct:description>
    <skos:prefLabel>Requirement 27.6</skos:prefLabel>
    <skos:definition>ProjMethodGeoKey values in the range 32768-65535 SHALL be private</skos:definition>
    <rdf:type rdf:resource="http://www.opengis.net/def/ont/modspec/Requirement"/>
    <rdf:type rdf:resource="http://www.w3.org/2004/02/skos/core#Concept"/>
    <skos:broader rdf:resource="http://www.opengis.net/spec/GeoTIFF/1.1/req/ProjMethodGeoKey"/>
  </rdf:Description>
  <rdf:Description rdf:about="http://www.opengis.net/spec/GeoTIFF/1.1/req/GTModelTypeGeoKey.geocenCRS">
    <dct:description>If the GTModelTypeGeoKey value is 3 (Model CRS is a geocentric CRS) then the
GeoTIFF file SHALL include a GeodeticCRSGeoKey.</dct:description>
    <rdf:type rdf:resource="http://www.opengis.net/def/ont/modspec/Requirement"/>
    <rdf:type rdf:resource="http://www.w3.org/2004/02/skos/core#Concept"/>
    <skos:definition>If the GTModelTypeGeoKey value is 3 (Model CRS is a geocentric CRS) then the
GeoTIFF file SHALL include a GeodeticCRSGeoKey.</skos:definition>
    <skos:prefLabel>Requirement 8.9</skos:prefLabel>
    <skos:broader rdf:resource="http://www.opengis.net/spec/GeoTIFF/1.1/req/GTModelTypeGeoKey"/>
  </rdf:Description>
  <rdf:Description rdf:about="http://www.opengis.net/spec/GeoTIFF/1.1/req/ProjMethodGeoKey.type">
    <skos:definition>The ProjMethodGeoKey SHALL have type = SHORT</skos:definition>
    <rdf:type rdf:resource="http://www.opengis.net/def/ont/modspec/Requirement"/>
    <rdf:type rdf:resource="http://www.w3.org/2004/02/skos/core#Concept"/>
    <skos:broader rdf:resource="http://www.opengis.net/spec/GeoTIFF/1.1/req/ProjMethodGeoKey"/>
    <dct:description>The ProjMethodGeoKey SHALL have type = SHORT</dct:description>
    <skos:prefLabel>Requirement 27.2</skos:prefLabel>
  </rdf:Description>
  <rdf:Description rdf:about="http://www.opengis.net/spec/GeoTIFF/1.1/req/EllipsoidGeoKey.private">
    <skos:prefLabel>Requirement 21.6</skos:prefLabel>
    <dct:description>EllipsoidGeoKey values in the range 32768-65535 SHALL be private</dct:description>
    <rdf:type rdf:resource="http://www.opengis.net/def/ont/modspec/Requirement"/>
    <rdf:type rdf:resource="http://www.w3.org/2004/02/skos/core#Concept"/>
    <skos:definition>EllipsoidGeoKey values in the range 32768-65535 SHALL be private</skos:definition>
    <skos:broader rdf:resource="http://www.opengis.net/spec/GeoTIFF/1.1/req/EllipsoidGeoKey"/>
  </rdf:Description>
  <rdf:Description rdf:about="http://www.opengis.net/spec/GeoTIFF/1.1/req/GTRasterTypeGeoKey.type">
    <rdf:type rdf:resource="http://www.opengis.net/def/ont/modspec/Requirement"/>
    <rdf:type rdf:resource="http://www.w3.org/2004/02/skos/core#Concept"/>
    <dct:description>The GTRasterTypeGeoKey SHALL have type = SHORT</dct:description>
    <skos:definition>The GTRasterTypeGeoKey SHALL have type = SHORT</skos:definition>
    <skos:broader rdf:resource="http://www.opengis.net/spec/GeoTIFF/1.1/req/GTRasterTypeGeoKey"/>
    <skos:prefLabel>Requirement 7.2</skos:prefLabel>
  </rdf:Description>
  <rdf:Description rdf:about="http://www.opengis.net/spec/GeoTIFF/1.1/req/ProjectionGeoKey.type">
    <dct:description>The ProjectionGeoKey SHALL have type = SHORT</dct:description>
    <rdf:type rdf:resource="http://www.w3.org/2004/02/skos/core#Concept"/>
    <rdf:type rdf:resource="http://www.opengis.net/def/ont/modspec/Requirement"/>
    <skos:broader rdf:resource="http://www.opengis.net/spec/GeoTIFF/1.1/req/ProjectionGeoKey"/>
    <skos:definition>The ProjectionGeoKey SHALL have type = SHORT</skos:definition>
    <skos:prefLabel>Requirement 26.2</skos:prefLabel>
  </rdf:Description>
  <rdf:Description rdf:about="http://www.opengis.net/spec/GeoTIFF/1.1/req/ProjectedCRSGeoKey">
    <skos:narrower rdf:resource="http://www.opengis.net/spec/GeoTIFF/1.1/req/ProjectedCRSGeoKey.private"/>
    <skos:narrower rdf:resource="http://www.opengis.net/spec/GeoTIFF/1.1/req/ProjectedCRSGeoKey.userdefined"/>
    <skos:narrower rdf:resource="http://www.opengis.net/spec/GeoTIFF/1.1/req/ProjectedCRSGeoKey.ID"/>
    <skos:narrower rdf:resource="http://www.opengis.net/spec/GeoTIFF/1.1/req/ProjectedCRSGeoKey.EPSG"/>
    <skos:narrower rdf:resource="http://www.opengis.net/spec/GeoTIFF/1.1/req/ProjectedCRSGeoKey.reserved"/>
    <skos:narrower rdf:resource="http://www.opengis.net/spec/GeoTIFF/1.1/req/ProjectedCRSGeoKey.type"/>
    <spec:normativeStatement rdf:resource="http://www.opengis.net/spec/GeoTIFF/1.1/req/ProjectedCRSGeoKey.userdefined"/>
    <spec:normativeStatement rdf:resource="http://www.opengis.net/spec/GeoTIFF/1.1/req/ProjectedCRSGeoKey.private"/>
    <spec:normativeStatement rdf:resource="http://www.opengis.net/spec/GeoTIFF/1.1/req/ProjectedCRSGeoKey.EPSG"/>
    <spec:normativeStatement rdf:resource="http://www.opengis.net/spec/GeoTIFF/1.1/req/ProjectedCRSGeoKey.type"/>
    <spec:normativeStatement rdf:resource="http://www.opengis.net/spec/GeoTIFF/1.1/req/ProjectedCRSGeoKey.ID"/>
    <spec:normativeStatement rdf:resource="http://www.opengis.net/spec/GeoTIFF/1.1/req/ProjectedCRSGeoKey.reserved"/>
    <skos:broader rdf:resource="http://www.opengis.net/spec/GeoTIFF/1.1/conf/ShortParameters"/>
    <skos:broader rdf:resource="http://www.opengis.net/def/docs/19-008r4"/>
    <rdf:type rdf:resource="http://www.opengis.net/def/ont/modspec/RequirementClass"/>
    <rdf:type rdf:resource="http://www.w3.org/2004/02/skos/core#Concept"/>
    <skos:definition>This key is used to specify the projected coordinate reference system from the GeoTIFF CRS register or to indicate that the Model CRS is a user-defined projected coordinate reference system.




Note


In GeoTIFF 1.0 this key was called ProjectedCSTypeGeoKey.</skos:definition>
    <skos:prefLabel>Requirements Class ProjectedCRSGeoKey</skos:prefLabel>
  </rdf:Description>
  <rdf:Description rdf:about="http://www.opengis.net/spec/GeoTIFF/1.1/req/EllipsoidSemiMajorAxisGeoKey.type">
    <skos:definition>The EllipsoidSemiMajorAxisGeoKey SHALL have type = DOUBLE</skos:definition>
    <dct:description>The EllipsoidSemiMajorAxisGeoKey SHALL have type = DOUBLE</dct:description>
    <rdf:type rdf:resource="http://www.opengis.net/def/ont/modspec/Requirement"/>
    <rdf:type rdf:resource="http://www.w3.org/2004/02/skos/core#Concept"/>
    <skos:prefLabel>Requirement 22.2</skos:prefLabel>
    <skos:broader rdf:resource="http://www.opengis.net/spec/GeoTIFF/1.1/req/EllipsoidSemiMajorAxisGeoKey"/>
  </rdf:Description>
  <rdf:Description rdf:about="http://www.opengis.net/spec/GeoTIFF/1.1/req/GeoKeyDirectoryTag.minorRevisionValue">
    <skos:definition>The MinorRevision for this standard SHALL be 0 or 1.0 = GeoTIFF 1.0 version.
Accepted for existing files (GeoTIFF 1.0) that do not use values / codes that
are suppressed in this version1 = this version 1.1. Recommended for production
/ writing a GeoTIFF file according to this standard (and developing software).
Shall be used for files keys and codes not covered by GeoTIFF 1.0 (e.g.
VerticalGeoKey).</skos:definition>
    <skos:prefLabel>Requirement 2.9</skos:prefLabel>
    <skos:broader rdf:resource="http://www.opengis.net/spec/GeoTIFF/1.1/conf/GeoKeyDirectory"/>
    <skos:broader rdf:resource="http://www.opengis.net/spec/GeoTIFF/1.1/req/GeoKeyDirectoryTag"/>
    <rdf:type rdf:resource="http://www.opengis.net/def/ont/modspec/Requirement"/>
    <rdf:type rdf:resource="http://www.w3.org/2004/02/skos/core#Concept"/>
    <dct:description>The MinorRevision for this standard SHALL be 0 or 1.0 = GeoTIFF 1.0 version.
Accepted for existing files (GeoTIFF 1.0) that do not use values / codes that
are suppressed in this version1 = this version 1.1. Recommended for production
/ writing a GeoTIFF file according to this standard (and developing software).
Shall be used for files keys and codes not covered by GeoTIFF 1.0 (e.g.
VerticalGeoKey).</dct:description>
  </rdf:Description>
  <rdf:Description rdf:about="http://www.opengis.net/spec/GeoTIFF/1.1/req/GeodeticCRSGeoKey.user-defined">
    <dct:description>If the GeodeticCRSGeoKey value is 32767 (User-Defined) then the
GeodeticCitationGeoKey, GeodeticDatumGeoKey and at least one of
GeogAngularUnitsGeoKey or GeogLinearUnitsGeoKey SHALL be populated.NOTE: if
the user-defined CRS is geographic 2D, GeogAngularUnitsGeoKey should be
populated ; if the user-defined CRS is geocentric, GeogLinearUnitsGeoKey
should be populated.</dct:description>
    <skos:broader rdf:resource="http://www.opengis.net/spec/GeoTIFF/1.1/req/GeodeticCRSGeoKey"/>
    <skos:definition>If the GeodeticCRSGeoKey value is 32767 (User-Defined) then the
GeodeticCitationGeoKey, GeodeticDatumGeoKey and at least one of
GeogAngularUnitsGeoKey or GeogLinearUnitsGeoKey SHALL be populated.NOTE: if
the user-defined CRS is geographic 2D, GeogAngularUnitsGeoKey should be
populated ; if the user-defined CRS is geocentric, GeogLinearUnitsGeoKey
should be populated.</skos:definition>
    <skos:prefLabel>Requirement 13.5</skos:prefLabel>
    <rdf:type rdf:resource="http://www.opengis.net/def/ont/modspec/Requirement"/>
    <rdf:type rdf:resource="http://www.w3.org/2004/02/skos/core#Concept"/>
  </rdf:Description>
  <rdf:Description rdf:about="http://www.opengis.net/spec/GeoTIFF/1.1/req/EllipsoidGeoKey.EPSG">
    <rdf:type rdf:resource="http://www.opengis.net/def/ont/modspec/Requirement"/>
    <rdf:type rdf:resource="http://www.w3.org/2004/02/skos/core#Concept"/>
    <skos:broader rdf:resource="http://www.opengis.net/spec/GeoTIFF/1.1/req/EllipsoidGeoKey"/>
    <skos:prefLabel>Requirement 21.4</skos:prefLabel>
    <skos:definition>EllipsoidGeoKey values in the range 1024-32766 SHALL be EPSG ellipsoid
CodesNOTE: In GeoTIFF v1.0 the range was 7000-7999. Several values in this
range have been deprecated or deleted from the EPSG Dataset and should no
longer be used. See</skos:definition>
    <dct:description>EllipsoidGeoKey values in the range 1024-32766 SHALL be EPSG ellipsoid
CodesNOTE: In GeoTIFF v1.0 the range was 7000-7999. Several values in this
range have been deprecated or deleted from the EPSG Dataset and should no
longer be used. See</dct:description>
  </rdf:Description>
  <rdf:Description rdf:about="http://www.opengis.net/spec/GeoTIFF/1.1/req/ModelTiepointTag.ID">
    <skos:broader rdf:resource="http://www.opengis.net/spec/GeoTIFF/1.1/conf/TIFF.Tags"/>
    <skos:broader rdf:resource="http://www.opengis.net/spec/GeoTIFF/1.1/req/ModelTiepointTag"/>
    <dct:description>The ModelTiepointTag SHALL have ID = 33922</dct:description>
    <skos:definition>The ModelTiepointTag SHALL have ID = 33922</skos:definition>
    <rdf:type rdf:resource="http://www.w3.org/2004/02/skos/core#Concept"/>
    <rdf:type rdf:resource="http://www.opengis.net/def/ont/modspec/Requirement"/>
    <skos:prefLabel>Requirement 9.1</skos:prefLabel>
  </rdf:Description>
  <rdf:Description rdf:about="http://www.opengis.net/spec/GeoTIFF/1.1/req/PrimeMeridianGeoKey.EPSG">
    <skos:prefLabel>Requirement 19.4</skos:prefLabel>
    <dct:description>PrimeMeridianGeoKey values in the range 1024-32766 SHALL be EPSG Prime
Meridian CodesNOTE: In GeoTIFF v1.0 the range was 8000-8999</dct:description>
    <skos:definition>PrimeMeridianGeoKey values in the range 1024-32766 SHALL be EPSG Prime
Meridian CodesNOTE: In GeoTIFF v1.0 the range was 8000-8999</skos:definition>
    <rdf:type rdf:resource="http://www.opengis.net/def/ont/modspec/Requirement"/>
    <rdf:type rdf:resource="http://www.w3.org/2004/02/skos/core#Concept"/>
    <skos:broader rdf:resource="http://www.opengis.net/spec/GeoTIFF/1.1/req/PrimeMeridianGeoKey"/>
  </rdf:Description>
  <rdf:Description rdf:about="http://www.opengis.net/spec/GeoTIFF/1.1/req/GTModelTypeGeoKey.required">
    <rdf:type rdf:resource="http://www.opengis.net/def/ont/modspec/Requirement"/>
    <rdf:type rdf:resource="http://www.w3.org/2004/02/skos/core#Concept"/>
    <skos:definition>A GeoTIFF file SHALL include a GTModelTypeGeoKey</skos:definition>
    <dct:description>A GeoTIFF file SHALL include a GTModelTypeGeoKey</dct:description>
    <skos:broader rdf:resource="http://www.opengis.net/spec/GeoTIFF/1.1/req/GTModelTypeGeoKey"/>
    <skos:prefLabel>Requirement 8.1</skos:prefLabel>
  </rdf:Description>
  <rdf:Description rdf:about="http://www.opengis.net/spec/GeoTIFF/1.1/req/VerticalGeoKey.ID">
    <skos:prefLabel>Requirement 14.1</skos:prefLabel>
    <dct:description>The VerticalGeoKey SHALL have ID = 4096</dct:description>
    <skos:definition>The VerticalGeoKey SHALL have ID = 4096</skos:definition>
    <rdf:type rdf:resource="http://www.opengis.net/def/ont/modspec/Requirement"/>
    <rdf:type rdf:resource="http://www.w3.org/2004/02/skos/core#Concept"/>
    <skos:broader rdf:resource="http://www.opengis.net/spec/GeoTIFF/1.1/req/VerticalGeoKey"/>
  </rdf:Description>
  <rdf:Description rdf:about="http://www.opengis.net/spec/GeoTIFF/1.1/req/ModelTiepointTag.type">
    <rdf:type rdf:resource="http://www.w3.org/2004/02/skos/core#Concept"/>
    <rdf:type rdf:resource="http://www.opengis.net/def/ont/modspec/Requirement"/>
    <skos:prefLabel>Requirement 9.2</skos:prefLabel>
    <skos:definition>The ModelTiepointTag SHALL have type = DOUBLE</skos:definition>
    <skos:broader rdf:resource="http://www.opengis.net/spec/GeoTIFF/1.1/req/ModelTiepointTag"/>
    <skos:broader rdf:resource="http://www.opengis.net/spec/GeoTIFF/1.1/conf/TIFF.Tags"/>
    <dct:description>The ModelTiepointTag SHALL have type = DOUBLE</dct:description>
  </rdf:Description>
  <rdf:Description rdf:about="http://www.opengis.net/spec/GeoTIFF/1.1/req/GeoShortParams.Criteria">
    <skos:broader rdf:resource="http://www.opengis.net/spec/GeoTIFF/1.1/conf/ShortParameters"/>
  </rdf:Description>
  <rdf:Description rdf:about="http://www.opengis.net/spec/GeoTIFF/1.1/req/VerticalGeoKey.EPSG">
    <skos:broader rdf:resource="http://www.opengis.net/spec/GeoTIFF/1.1/req/VerticalGeoKey"/>
    <skos:definition>VerticalGeoKey values in the range 1024-32766 SHALL be either EPSG Vertical
CRS Codes or EPSG geographic 3D CRS codesNOTE: In GeoTIFF v1.0 the ranges were
5000-5099 and 5200-5999. As at 2018-05-29 no EPSG vertical CRSs have been or
are in this range. Values in this range have been and are used as EPSG
vertical datum codes; in this document their use as codes for vertical CRSs is
deprecated.</skos:definition>
    <rdf:type rdf:resource="http://www.w3.org/2004/02/skos/core#Concept"/>
    <rdf:type rdf:resource="http://www.opengis.net/def/ont/modspec/Requirement"/>
    <skos:prefLabel>Requirement 14.4</skos:prefLabel>
    <dct:description>VerticalGeoKey values in the range 1024-32766 SHALL be either EPSG Vertical
CRS Codes or EPSG geographic 3D CRS codesNOTE: In GeoTIFF v1.0 the ranges were
5000-5099 and 5200-5999. As at 2018-05-29 no EPSG vertical CRSs have been or
are in this range. Values in this range have been and are used as EPSG
vertical datum codes; in this document their use as codes for vertical CRSs is
deprecated.</dct:description>
  </rdf:Description>
  <rdf:Description rdf:about="http://www.opengis.net/spec/GeoTIFF/1.1/req/UnitSizeGeoKey">
    <skos:narrower rdf:resource="http://www.opengis.net/spec/GeoTIFF/1.1/req/UnitSizeGeoKey.units"/>
    <skos:narrower rdf:resource="http://www.opengis.net/spec/GeoTIFF/1.1/req/UnitSizeGeoKey.ID"/>
    <skos:narrower rdf:resource="http://www.opengis.net/spec/GeoTIFF/1.1/req/UnitSizeGeoKey.type"/>
    <skos:definition>These keys allow the definition of size of user-defined angular and linear units, given in the SI base unit for that unit type (meters for length, radians for angle).

Note: this specification does not support user-defined units for vertical coordinate reference systems.</skos:definition>
    <skos:prefLabel>Requirements Class Unit Size GeoKeys</skos:prefLabel>
    <spec:normativeStatement rdf:resource="http://www.opengis.net/spec/GeoTIFF/1.1/req/UnitSizeGeoKey.units"/>
    <spec:normativeStatement rdf:resource="http://www.opengis.net/spec/GeoTIFF/1.1/req/UnitSizeGeoKey.ID"/>
    <spec:normativeStatement rdf:resource="http://www.opengis.net/spec/GeoTIFF/1.1/req/UnitSizeGeoKey.type"/>
    <rdf:type rdf:resource="http://www.opengis.net/def/ont/modspec/RequirementClass"/>
    <rdf:type rdf:resource="http://www.w3.org/2004/02/skos/core#Concept"/>
    <skos:broader rdf:resource="http://www.opengis.net/def/docs/19-008r4"/>
    <skos:broader rdf:resource="http://www.opengis.net/spec/GeoTIFF/1.1/conf/DoubleParameters"/>
  </rdf:Description>
  <rdf:Description rdf:about="http://www.opengis.net/spec/GeoTIFF/1.1/req/ModelPixelScaleTag.standardConvention">
    <dct:description>A positive ScaleX in the ModelPixelScaleTag SHALL indicate that model space X
coordinates increase as raster space I indices increase. This is the standard
horizontal relationship between raster space and model space. A positive
ScaleY in the ModelPixelScaleTag SHALL indicate that model space Y coordinates
decrease as raster space J indices increase. This is the standard vertical
relationship between raster space and model space. The ScaleZ is primarily
used to map the pixel value of a digital elevation model into the correct
Z-scale (in other words a Z-Scaling factor).</dct:description>
    <skos:prefLabel>Requirement 10.4</skos:prefLabel>
    <skos:broader rdf:resource="http://www.opengis.net/spec/GeoTIFF/1.1/req/ModelPixelScaleTag"/>
    <skos:broader rdf:resource="http://www.opengis.net/spec/GeoTIFF/1.1/conf/Raster2Model_CoordinateTransformation_GeoKey/ModelPixelScaleTag"/>
    <skos:definition>A positive ScaleX in the ModelPixelScaleTag SHALL indicate that model space X
coordinates increase as raster space I indices increase. This is the standard
horizontal relationship between raster space and model space. A positive
ScaleY in the ModelPixelScaleTag SHALL indicate that model space Y coordinates
decrease as raster space J indices increase. This is the standard vertical
relationship between raster space and model space. The ScaleZ is primarily
used to map the pixel value of a digital elevation model into the correct
Z-scale (in other words a Z-Scaling factor).</skos:definition>
    <rdf:type rdf:resource="http://www.opengis.net/def/ont/modspec/Requirement"/>
    <rdf:type rdf:resource="http://www.w3.org/2004/02/skos/core#Concept"/>
  </rdf:Description>
  <rdf:Description rdf:about="http://www.opengis.net/spec/GeoTIFF/1.1/req/UnitsGeoKey.type">
    <skos:broader rdf:resource="http://www.opengis.net/spec/GeoTIFF/1.1/req/UnitsGeoKey"/>
    <rdf:type rdf:resource="http://www.opengis.net/def/ont/modspec/Requirement"/>
    <rdf:type rdf:resource="http://www.w3.org/2004/02/skos/core#Concept"/>
    <skos:prefLabel>Requirement 16.2</skos:prefLabel>
    <dct:description>The GeogAngularUnitsGeoKey, the GeogAzimuthUnitsGeoKey, the
GeogLinearUnitsGeoKey, the ProjLinearUnitsGeoKey and the VerticalUnitsGeoKey
SHALL each have type = SHORT</dct:description>
    <skos:definition>The GeogAngularUnitsGeoKey, the GeogAzimuthUnitsGeoKey, the
GeogLinearUnitsGeoKey, the ProjLinearUnitsGeoKey and the VerticalUnitsGeoKey
SHALL each have type = SHORT</skos:definition>
  </rdf:Description>
  <rdf:Description rdf:about="http://www.opengis.net/spec/GeoTIFF/1.1/req/GeoKeyDirectoryTag.keyEntrySetCount">
    <dct:description>The GeoKeyDirectoryTag SHALL hold NumberOfKeys KeyEntry Sets in addition to
the header information</dct:description>
    <skos:broader rdf:resource="http://www.opengis.net/spec/GeoTIFF/1.1/conf/GeoKeyDirectory"/>
    <skos:broader rdf:resource="http://www.opengis.net/spec/GeoTIFF/1.1/req/GeoKeyDirectoryTag"/>
    <skos:prefLabel>Requirement 2.11</skos:prefLabel>
    <rdf:type rdf:resource="http://www.w3.org/2004/02/skos/core#Concept"/>
    <rdf:type rdf:resource="http://www.opengis.net/def/ont/modspec/Requirement"/>
    <skos:definition>The GeoKeyDirectoryTag SHALL hold NumberOfKeys KeyEntry Sets in addition to
the header information</skos:definition>
  </rdf:Description>
  <rdf:Description rdf:about="http://www.opengis.net/spec/GeoTIFF/1.1/req/EllipsoidGeoKey.type">
    <rdf:type rdf:resource="http://www.w3.org/2004/02/skos/core#Concept"/>
    <rdf:type rdf:resource="http://www.opengis.net/def/ont/modspec/Requirement"/>
    <skos:broader rdf:resource="http://www.opengis.net/spec/GeoTIFF/1.1/req/EllipsoidGeoKey"/>
    <dct:description>The EllipsoidGeoKey SHALL have type = SHORT</dct:description>
    <skos:prefLabel>Requirement 21.2</skos:prefLabel>
    <skos:definition>The EllipsoidGeoKey SHALL have type = SHORT</skos:definition>
  </rdf:Description>
  <rdf:Description rdf:about="http://www.opengis.net/spec/GeoTIFF/1.1/req/TIFF">
    <dct:description>A GeoTIFF file SHALL be compliant with the TIFF 6.0 specification</dct:description>
    <rdf:type rdf:resource="http://www.opengis.net/def/ont/modspec/Requirement"/>
    <rdf:type rdf:resource="http://www.w3.org/2004/02/skos/core#Concept"/>
    <skos:broader rdf:resource="http://www.opengis.net/spec/GeoTIFF/1.1/conf/TIFF.Tags"/>
    <skos:broader rdf:resource="http://www.opengis.net/spec/GeoTIFF/1.1/conf/Core/test"/>
    <skos:broader rdf:resource="http://www.opengis.net/spec/GeoTIFF/1.1/req/Core"/>
    <skos:prefLabel>Requirement 1.1</skos:prefLabel>
    <skos:definition>A GeoTIFF file SHALL be compliant with the TIFF 6.0 specification</skos:definition>
  </rdf:Description>
  <rdf:Description rdf:about="http://www.opengis.net/spec/GeoTIFF/1.1/req/GeoShortParams.Location">
    <skos:broader rdf:resource="http://www.opengis.net/spec/GeoTIFF/1.1/conf/ShortParameters"/>
  </rdf:Description>
  <rdf:Description rdf:about="http://www.opengis.net/spec/GeoTIFF/1.1/req/ModelTransformationTag.ID">
    <rdf:type rdf:resource="http://www.opengis.net/def/ont/modspec/Requirement"/>
    <rdf:type rdf:resource="http://www.w3.org/2004/02/skos/core#Concept"/>
    <skos:broader rdf:resource="http://www.opengis.net/spec/GeoTIFF/1.1/conf/TIFF.Tags"/>
    <skos:broader rdf:resource="http://www.opengis.net/spec/GeoTIFF/1.1/req/ModelTransformationTag"/>
    <skos:prefLabel>Requirement 11.1</skos:prefLabel>
    <dct:description>The ModelTransformationTag SHALL have ID = 34264</dct:description>
    <skos:definition>The ModelTransformationTag SHALL have ID = 34264</skos:definition>
  </rdf:Description>
  <rdf:Description rdf:about="http://www.opengis.net/spec/GeoTIFF/1.1/req/VerticalDatumGeoKey.userdefined">
    <rdf:type rdf:resource="http://www.opengis.net/def/ont/modspec/Requirement"/>
    <rdf:type rdf:resource="http://www.w3.org/2004/02/skos/core#Concept"/>
    <skos:definition>If the VerticalDatumGeoKey value is 32767 (User-Defined) then the
VerticalCitationGeoKey SHALL be populated.</skos:definition>
    <skos:prefLabel>Requirement 25.5</skos:prefLabel>
    <dct:description>If the VerticalDatumGeoKey value is 32767 (User-Defined) then the
VerticalCitationGeoKey SHALL be populated.</dct:description>
    <skos:broader rdf:resource="http://www.opengis.net/spec/GeoTIFF/1.1/req/VerticalDatumGeoKey"/>
  </rdf:Description>
  <rdf:Description rdf:about="http://www.opengis.net/spec/GeoTIFF/1.1/req/GeoKeySort">
    <rdf:type rdf:resource="http://www.opengis.net/def/ont/modspec/Requirement"/>
    <rdf:type rdf:resource="http://www.w3.org/2004/02/skos/core#Concept"/>
    <skos:broader rdf:resource="http://www.opengis.net/spec/GeoTIFF/1.1/conf/GeoKeyDirectory"/>
    <skos:broader rdf:resource="http://www.opengis.net/spec/GeoTIFF/1.1/req/Core"/>
    <skos:definition>The GeoKey entries in a GeoTIFF file SHALL be written out to the file with the
key-IDs sorted in ascending order</skos:definition>
    <skos:prefLabel>Requirement 1.6</skos:prefLabel>
    <dct:description>The GeoKey entries in a GeoTIFF file SHALL be written out to the file with the
key-IDs sorted in ascending order</dct:description>
  </rdf:Description>
  <rdf:Description rdf:about="http://www.opengis.net/spec/GeoTIFF/1.1/req/UnitsGeoKey.userdefinedVertical">
    <rdf:type rdf:resource="http://www.opengis.net/def/ont/modspec/Requirement"/>
    <rdf:type rdf:resource="http://www.w3.org/2004/02/skos/core#Concept"/>
    <skos:definition>A VerticalUnitsGeoKey value of 32767 (user defined) SHALL not be usedNOTE: The
rationale for this is that it would require a VerticalUnitSizeGeoKey, which
does not exist in GeoTIFF 1.0. For vertical units, this document supports only
EPSG linear units.</skos:definition>
    <skos:prefLabel>Requirement 16.9</skos:prefLabel>
    <skos:broader rdf:resource="http://www.opengis.net/spec/GeoTIFF/1.1/req/UnitsGeoKey"/>
    <dct:description>A VerticalUnitsGeoKey value of 32767 (user defined) SHALL not be usedNOTE: The
rationale for this is that it would require a VerticalUnitSizeGeoKey, which
does not exist in GeoTIFF 1.0. For vertical units, this document supports only
EPSG linear units.</dct:description>
  </rdf:Description>
  <rdf:Description rdf:about="http://www.opengis.net/spec/GeoTIFF/1.1/req/GeoDoubleParamsTag.count">
    <rdf:type rdf:resource="http://www.opengis.net/def/ont/modspec/Requirement"/>
    <rdf:type rdf:resource="http://www.w3.org/2004/02/skos/core#Concept"/>
    <skos:broader rdf:resource="http://www.opengis.net/spec/GeoTIFF/1.1/conf/TIFF.Tags"/>
    <skos:broader rdf:resource="http://www.opengis.net/spec/GeoTIFF/1.1/req/GeoDoubleParamsTag"/>
    <skos:broader rdf:resource="http://www.opengis.net/spec/GeoTIFF/1.1/conf/DoubleParameters"/>
    <dct:description>The GeoDoubleParamsTag MAY hold any number of key parameters with type =
Double.</dct:description>
    <skos:definition>The GeoDoubleParamsTag MAY hold any number of key parameters with type =
Double.</skos:definition>
    <skos:prefLabel>Requirement 5.2</skos:prefLabel>
  </rdf:Description>
  <rdf:Description rdf:about="http://www.opengis.net/spec/GeoTIFF/1.1/req/EllipsoidSemiMinorAxisGeoKey.type">
    <skos:prefLabel>Requirement 23.2</skos:prefLabel>
    <skos:definition>The EllipsoidSemiMinorAxisGeoKey SHALL have type = DOUBLE</skos:definition>
    <rdf:type rdf:resource="http://www.opengis.net/def/ont/modspec/Requirement"/>
    <rdf:type rdf:resource="http://www.w3.org/2004/02/skos/core#Concept"/>
    <skos:broader rdf:resource="http://www.opengis.net/spec/GeoTIFF/1.1/req/EllipsoidSemiMajorAxisGeoKey"/>
    <dct:description>The EllipsoidSemiMinorAxisGeoKey SHALL have type = DOUBLE</dct:description>
  </rdf:Description>
  <rdf:Description rdf:about="http://www.opengis.net/spec/GeoTIFF/1.1/req/GTModelTypeGeoKey.geogCRS">
    <skos:broader rdf:resource="http://www.opengis.net/spec/GeoTIFF/1.1/req/GTModelTypeGeoKey"/>
    <rdf:type rdf:resource="http://www.w3.org/2004/02/skos/core#Concept"/>
    <rdf:type rdf:resource="http://www.opengis.net/def/ont/modspec/Requirement"/>
    <skos:definition>If the GTModelTypeGeoKey value is 2 (Model CRS is a geographic 2D CRS) then
the GeoTIFF file SHALL include a GeodeticCRSGeoKey.</skos:definition>
    <skos:prefLabel>Requirement 8.8</skos:prefLabel>
    <dct:description>If the GTModelTypeGeoKey value is 2 (Model CRS is a geographic 2D CRS) then
the GeoTIFF file SHALL include a GeodeticCRSGeoKey.</dct:description>
  </rdf:Description>
  <rdf:Description rdf:about="http://www.opengis.net/spec/GeoTIFF/1.1/req/EllipsoidInvFlatteningGeoKey.ID">
    <rdf:type rdf:resource="http://www.opengis.net/def/ont/modspec/Requirement"/>
    <rdf:type rdf:resource="http://www.w3.org/2004/02/skos/core#Concept"/>
    <skos:prefLabel>Requirement 24.1</skos:prefLabel>
    <skos:broader rdf:resource="http://www.opengis.net/spec/GeoTIFF/1.1/req/EllipsoidSemiMajorAxisGeoKey"/>
    <skos:definition>The EllipsoidInvFlatteningGeoKey SHALL have ID = 2059</skos:definition>
    <dct:description>The EllipsoidInvFlatteningGeoKey SHALL have ID = 2059</dct:description>
  </rdf:Description>
  <rdf:Description rdf:about="http://www.opengis.net/spec/GeoTIFF/1.1/req/PrimeMeridianLongitudeGeoKey.units">
    <dct:description>The unit for the PrimeMeridianLongitudeGeoKey value SHALL be GeogAngularUnits</dct:description>
    <rdf:type rdf:resource="http://www.w3.org/2004/02/skos/core#Concept"/>
    <rdf:type rdf:resource="http://www.opengis.net/def/ont/modspec/Requirement"/>
    <skos:broader rdf:resource="http://www.opengis.net/spec/GeoTIFF/1.1/req/PrimeMeridianLongitudeGeoKey"/>
    <skos:definition>The unit for the PrimeMeridianLongitudeGeoKey value SHALL be GeogAngularUnits</skos:definition>
    <skos:prefLabel>Requirement 20.3</skos:prefLabel>
  </rdf:Description>
  <rdf:Description rdf:about="http://www.opengis.net/spec/GeoTIFF/1.1/req/VerticalDatumGeoKey.ID">
    <skos:prefLabel>Requirement 25.1</skos:prefLabel>
    <rdf:type rdf:resource="http://www.w3.org/2004/02/skos/core#Concept"/>
    <rdf:type rdf:resource="http://www.opengis.net/def/ont/modspec/Requirement"/>
    <skos:broader rdf:resource="http://www.opengis.net/spec/GeoTIFF/1.1/req/VerticalDatumGeoKey"/>
    <dct:description>The VerticalDatumGeoKey SHALL have ID = 4098</dct:description>
    <skos:definition>The VerticalDatumGeoKey SHALL have ID = 4098</skos:definition>
  </rdf:Description>
  <rdf:Description rdf:about="http://www.opengis.net/spec/GeoTIFF/1.1/req/VerticalDatumGeoKey.private">
    <dct:description>VerticalDatumGeoKey values in the range 32768-65535 SHALL be private</dct:description>
    <rdf:type rdf:resource="http://www.w3.org/2004/02/skos/core#Concept"/>
    <rdf:type rdf:resource="http://www.opengis.net/def/ont/modspec/Requirement"/>
    <skos:prefLabel>Requirement 25.6</skos:prefLabel>
    <skos:broader rdf:resource="http://www.opengis.net/spec/GeoTIFF/1.1/req/VerticalDatumGeoKey"/>
    <skos:definition>VerticalDatumGeoKey values in the range 32768-65535 SHALL be private</skos:definition>
  </rdf:Description>
  <rdf:Description rdf:about="http://www.opengis.net/spec/GeoTIFF/1.1/req/GeoAsciiParamsTag.count">
    <rdf:type rdf:resource="http://www.w3.org/2004/02/skos/core#Concept"/>
    <rdf:type rdf:resource="http://www.opengis.net/def/ont/modspec/Requirement"/>
    <skos:prefLabel>Requirement 6.2</skos:prefLabel>
    <skos:broader rdf:resource="http://www.opengis.net/spec/GeoTIFF/1.1/req/GeoAsciiParamsTag"/>
    <skos:broader rdf:resource="http://www.opengis.net/spec/GeoTIFF/1.1/conf/AsciiParameters"/>
    <dct:description>The GeoAsciiParamsTag SHALL contain the values of the key parameters of type =
ASCII referenced by the GeoKeyDirectoryTag. If there is no key parameters of
type = ASCII, it SHALL not be present</dct:description>
    <skos:definition>The GeoAsciiParamsTag SHALL contain the values of the key parameters of type =
ASCII referenced by the GeoKeyDirectoryTag. If there is no key parameters of
type = ASCII, it SHALL not be present</skos:definition>
  </rdf:Description>
  <rdf:Description rdf:about="http://www.opengis.net/spec/GeoTIFF/1.1/req/UnitSizeGeoKey.ID">
    <skos:broader rdf:resource="http://www.opengis.net/spec/GeoTIFF/1.1/req/UnitSizeGeoKey"/>
    <skos:prefLabel>Requirement 17.1</skos:prefLabel>
    <rdf:type rdf:resource="http://www.opengis.net/def/ont/modspec/Requirement"/>
    <rdf:type rdf:resource="http://www.w3.org/2004/02/skos/core#Concept"/>
    <skos:definition>The GeogAngularUnitSizeGeoKey SHALL have ID = 2055The GeogLinearUnitSizeGeoKey
SHALL have ID = 2053The ProjLinearUnitSizeGeoKey SHALL have ID = 3077</skos:definition>
    <dct:description>The GeogAngularUnitSizeGeoKey SHALL have ID = 2055The GeogLinearUnitSizeGeoKey
SHALL have ID = 2053The ProjLinearUnitSizeGeoKey SHALL have ID = 3077</dct:description>
  </rdf:Description>
  <rdf:Description rdf:about="http://www.opengis.net/spec/GeoTIFF/1.1/req/CitationGeoKeys.type">
    <skos:definition>The CitationGeoKeys SHALL have type = ASCII</skos:definition>
    <skos:broader rdf:resource="http://www.opengis.net/spec/GeoTIFF/1.1/req/CitationGeoKeys"/>
    <dct:description>The CitationGeoKeys SHALL have type = ASCII</dct:description>
    <rdf:type rdf:resource="http://www.opengis.net/def/ont/modspec/Requirement"/>
    <rdf:type rdf:resource="http://www.w3.org/2004/02/skos/core#Concept"/>
    <skos:prefLabel>Requirement 15.2</skos:prefLabel>
  </rdf:Description>
  <rdf:Description rdf:about="http://www.opengis.net/spec/GeoTIFF/1.1/req/GeodeticDatumGeoKey.EPSG">
    <rdf:type rdf:resource="http://www.opengis.net/def/ont/modspec/Requirement"/>
    <rdf:type rdf:resource="http://www.w3.org/2004/02/skos/core#Concept"/>
    <skos:definition>GeodeticDatumGeoKey values in the range 1024-32766 SHALL be EPSG geodetic
datum codes.NOTE: In GeoTIFF v1.0 the range was 6000-6999. Several values in
this range have been deprecated or deleted from the EPSG Dataset and should no
longer be used. See</skos:definition>
    <dct:description>GeodeticDatumGeoKey values in the range 1024-32766 SHALL be EPSG geodetic
datum codes.NOTE: In GeoTIFF v1.0 the range was 6000-6999. Several values in
this range have been deprecated or deleted from the EPSG Dataset and should no
longer be used. See</dct:description>
    <skos:prefLabel>Requirement 18.4</skos:prefLabel>
    <skos:broader rdf:resource="http://www.opengis.net/spec/GeoTIFF/1.1/req/GeodeticDatumGeoKey"/>
  </rdf:Description>
  <rdf:Description rdf:about="http://www.opengis.net/spec/GeoTIFF/1.1/req/GTModelTypeGeoKey.type">
    <skos:broader rdf:resource="http://www.opengis.net/spec/GeoTIFF/1.1/req/GTModelTypeGeoKey"/>
    <skos:definition>The GTModelTypeGeoKey SHALL have type = SHORT</skos:definition>
    <skos:prefLabel>Requirement 8.3</skos:prefLabel>
    <rdf:type rdf:resource="http://www.opengis.net/def/ont/modspec/Requirement"/>
    <rdf:type rdf:resource="http://www.w3.org/2004/02/skos/core#Concept"/>
    <dct:description>The GTModelTypeGeoKey SHALL have type = SHORT</dct:description>
  </rdf:Description>
  <rdf:Description rdf:about="http://www.opengis.net/spec/GeoTIFF/1.1/req/EllipsoidGeoKey.ID">
    <skos:definition>The EllipsoidGeoKey SHALL have ID = 2056</skos:definition>
    <rdf:type rdf:resource="http://www.w3.org/2004/02/skos/core#Concept"/>
    <rdf:type rdf:resource="http://www.opengis.net/def/ont/modspec/Requirement"/>
    <skos:broader rdf:resource="http://www.opengis.net/spec/GeoTIFF/1.1/req/EllipsoidGeoKey"/>
    <skos:prefLabel>Requirement 21.1</skos:prefLabel>
    <dct:description>The EllipsoidGeoKey SHALL have ID = 2056</dct:description>
  </rdf:Description>
  <rdf:Description rdf:about="http://www.opengis.net/spec/GeoTIFF/1.1/req/ProjectionGeoKey.ID">
    <rdf:type rdf:resource="http://www.w3.org/2004/02/skos/core#Concept"/>
    <rdf:type rdf:resource="http://www.opengis.net/def/ont/modspec/Requirement"/>
    <dct:description>The ProjectionGeoKey SHALL have ID = 3074</dct:description>
    <skos:broader rdf:resource="http://www.opengis.net/spec/GeoTIFF/1.1/req/ProjectionGeoKey"/>
    <skos:definition>The ProjectionGeoKey SHALL have ID = 3074</skos:definition>
    <skos:prefLabel>Requirement 26.1</skos:prefLabel>
  </rdf:Description>
  <rdf:Description rdf:about="http://www.opengis.net/spec/docs/19-008r4-anno">
    <rdf:type rdf:resource="http://www.w3.org/2002/07/owl#Ontology"/>
  </rdf:Description>
  <rdf:Description rdf:about="http://www.opengis.net/spec/GeoTIFF/1.1/req/GTModelTypeGeoKey.private">
    <skos:prefLabel>Requirement 8.6</skos:prefLabel>
    <skos:definition>GTModelTypeGeoKey values in the range 32768-65535 SHALL be private</skos:definition>
    <skos:broader rdf:resource="http://www.opengis.net/spec/GeoTIFF/1.1/req/GTModelTypeGeoKey"/>
    <rdf:type rdf:resource="http://www.w3.org/2004/02/skos/core#Concept"/>
    <rdf:type rdf:resource="http://www.opengis.net/def/ont/modspec/Requirement"/>
    <dct:description>GTModelTypeGeoKey values in the range 32768-65535 SHALL be private</dct:description>
  </rdf:Description>
  <rdf:Description rdf:about="http://www.opengis.net/spec/GeoTIFF/1.1/req/GeoAsciiParamsTag.terminator">
    <skos:broader rdf:resource="http://www.opengis.net/spec/GeoTIFF/1.1/req/GeoAsciiParamsTag"/>
    <rdf:type rdf:resource="http://www.w3.org/2004/02/skos/core#Concept"/>
    <rdf:type rdf:resource="http://www.opengis.net/def/ont/modspec/Requirement"/>
    <skos:prefLabel>Requirement 6.3</skos:prefLabel>
    <skos:definition>The pipe character | in the GeoAsciiParamsTag SHALL be used as the character
to terminate a string written in as ASCII tagNOTE: If multiple strings are
written in the same tag, this terminator character also serves as a
separator.NOTE: This requirement only applies for the content of the tag. The
TIFF specification requires that the last byte of a TIFF tag of type ASCII is
NULL.</skos:definition>
    <dct:description>The pipe character | in the GeoAsciiParamsTag SHALL be used as the character
to terminate a string written in as ASCII tagNOTE: If multiple strings are
written in the same tag, this terminator character also serves as a
separator.NOTE: This requirement only applies for the content of the tag. The
TIFF specification requires that the last byte of a TIFF tag of type ASCII is
NULL.</dct:description>
  </rdf:Description>
  <rdf:Description rdf:about="http://www.opengis.net/spec/GeoTIFF/1.1/req/EllipsoidGeoKey.user-defined">
    <skos:definition>If the EllipsoidGeoKey value is 32767 (User-Defined) then the GTCitationGeoKey
and the EllipsoidSemiMajorAxisGeoKey SHALL be populated together with the one
of either the EllipsoidSemiMinorAxisGeoKey or the
EllipsoidInvFlatteningGeoKey.</skos:definition>
    <rdf:type rdf:resource="http://www.w3.org/2004/02/skos/core#Concept"/>
    <rdf:type rdf:resource="http://www.opengis.net/def/ont/modspec/Requirement"/>
    <skos:prefLabel>Requirement 21.5</skos:prefLabel>
    <skos:broader rdf:resource="http://www.opengis.net/spec/GeoTIFF/1.1/req/EllipsoidGeoKey"/>
    <dct:description>If the EllipsoidGeoKey value is 32767 (User-Defined) then the GTCitationGeoKey
and the EllipsoidSemiMajorAxisGeoKey SHALL be populated together with the one
of either the EllipsoidSemiMinorAxisGeoKey or the
EllipsoidInvFlatteningGeoKey.</dct:description>
  </rdf:Description>
  <rdf:Description rdf:about="http://www.opengis.net/spec/GeoTIFF/1.1/req/PrimeMeridianLongitudeGeoKey.ID">
    <rdf:type rdf:resource="http://www.opengis.net/def/ont/modspec/Requirement"/>
    <rdf:type rdf:resource="http://www.w3.org/2004/02/skos/core#Concept"/>
    <skos:prefLabel>Requirement 20.1</skos:prefLabel>
    <dct:description>The PrimeMeridianLongitudeGeoKey SHALL have ID = 2061</dct:description>
    <skos:broader rdf:resource="http://www.opengis.net/spec/GeoTIFF/1.1/req/PrimeMeridianLongitudeGeoKey"/>
    <skos:definition>The PrimeMeridianLongitudeGeoKey SHALL have ID = 2061</skos:definition>
  </rdf:Description>
  <rdf:Description rdf:about="http://www.opengis.net/spec/GeoTIFF/1.1/req/EllipsoidSemiMajorAxisGeoKey.units">
    <rdf:type rdf:resource="http://www.w3.org/2004/02/skos/core#Concept"/>
    <rdf:type rdf:resource="http://www.opengis.net/def/ont/modspec/Requirement"/>
    <skos:definition>The units of the EllipsoidSemiMajorAxisGeoKey SHALL be defined by the value of
GeogLinearUnitsGeoKey</skos:definition>
    <dct:description>The units of the EllipsoidSemiMajorAxisGeoKey SHALL be defined by the value of
GeogLinearUnitsGeoKey</dct:description>
    <skos:prefLabel>Requirement 22.3</skos:prefLabel>
    <skos:broader rdf:resource="http://www.opengis.net/spec/GeoTIFF/1.1/req/EllipsoidSemiMajorAxisGeoKey"/>
  </rdf:Description>
  <rdf:Description rdf:about="http://www.opengis.net/spec/GeoTIFF/1.1/req/ModelPixelScaleTag.ID">
    <rdf:type rdf:resource="http://www.opengis.net/def/ont/modspec/Requirement"/>
    <rdf:type rdf:resource="http://www.w3.org/2004/02/skos/core#Concept"/>
    <skos:broader rdf:resource="http://www.opengis.net/spec/GeoTIFF/1.1/conf/TIFF.Tags"/>
    <skos:broader rdf:resource="http://www.opengis.net/spec/GeoTIFF/1.1/req/ModelPixelScaleTag"/>
    <skos:prefLabel>Requirement 10.1</skos:prefLabel>
    <dct:description>The ModelPixelScaleTag SHALL have ID = 33550</dct:description>
    <skos:definition>The ModelPixelScaleTag SHALL have ID = 33550</skos:definition>
  </rdf:Description>
  <rdf:Description rdf:about="http://www.opengis.net/spec/GeoTIFF/1.1/req/ModelTransformationTag.count">
    <rdf:type rdf:resource="http://www.opengis.net/def/ont/modspec/Requirement"/>
    <rdf:type rdf:resource="http://www.w3.org/2004/02/skos/core#Concept"/>
    <skos:broader rdf:resource="http://www.opengis.net/spec/GeoTIFF/1.1/req/ModelTransformationTag"/>
    <skos:broader rdf:resource="http://www.opengis.net/spec/GeoTIFF/1.1/conf/Raster2Model_CoordinateTransformation_GeoKey/ModelTransformationTag"/>
    <skos:prefLabel>Requirement 11.3</skos:prefLabel>
    <skos:definition>The ModelTransformationTag SHALL have 16 values representing the terms of the
4 by 4 transformation matrix. The terms SHALL be in row-major order</skos:definition>
    <dct:description>The ModelTransformationTag SHALL have 16 values representing the terms of the
4 by 4 transformation matrix. The terms SHALL be in row-major order</dct:description>
  </rdf:Description>
  <rdf:Description rdf:about="http://www.opengis.net/spec/GeoTIFF/1.1/req/VerticalDatumGeoKey.reserved">
    <skos:definition>VerticalDatumGeoKey values in the range 1-1023 SHALL be reservedNOTE: In
GeoTIFF v1.0 the reserved range was 16384-32766.</skos:definition>
    <skos:broader rdf:resource="http://www.opengis.net/spec/GeoTIFF/1.1/req/VerticalDatumGeoKey"/>
    <skos:prefLabel>Requirement 25.3</skos:prefLabel>
    <dct:description>VerticalDatumGeoKey values in the range 1-1023 SHALL be reservedNOTE: In
GeoTIFF v1.0 the reserved range was 16384-32766.</dct:description>
    <rdf:type rdf:resource="http://www.opengis.net/def/ont/modspec/Requirement"/>
    <rdf:type rdf:resource="http://www.w3.org/2004/02/skos/core#Concept"/>
  </rdf:Description>
  <rdf:Description rdf:about="http://www.opengis.net/spec/GeoTIFF/1.1/req/GeodeticCRSGeoKey.ID">
    <rdf:type rdf:resource="http://www.w3.org/2004/02/skos/core#Concept"/>
    <rdf:type rdf:resource="http://www.opengis.net/def/ont/modspec/Requirement"/>
    <skos:definition>The GeodeticCRSGeoKey SHALL have ID = 2048</skos:definition>
    <dct:description>The GeodeticCRSGeoKey SHALL have ID = 2048</dct:description>
    <skos:prefLabel>Requirement 13.1</skos:prefLabel>
    <skos:broader rdf:resource="http://www.opengis.net/spec/GeoTIFF/1.1/req/GeodeticCRSGeoKey"/>
  </rdf:Description>
  <rdf:Description rdf:about="http://www.opengis.net/spec/GeoTIFF/1.1/req/ProjectionGeoKey.userdefined">
    <rdf:type rdf:resource="http://www.w3.org/2004/02/skos/core#Concept"/>
    <rdf:type rdf:resource="http://www.opengis.net/def/ont/modspec/Requirement"/>
    <skos:broader rdf:resource="http://www.opengis.net/spec/GeoTIFF/1.1/req/ProjectionGeoKey"/>
    <dct:description>If the ProjectionGeoKey value is 32767 (User-Defined) then the
ProjectedCitationGeoKey, ProjectionMethodGeoKey, and ProjLinearUnitsGeoKey
SHALL be populated</dct:description>
    <skos:prefLabel>Requirement 26.5</skos:prefLabel>
    <skos:definition>If the ProjectionGeoKey value is 32767 (User-Defined) then the
ProjectedCitationGeoKey, ProjectionMethodGeoKey, and ProjLinearUnitsGeoKey
SHALL be populated</skos:definition>
  </rdf:Description>
  <rdf:Description rdf:about="http://www.opengis.net/spec/GeoTIFF/1.1/req/ProjScalarParameterGeoKey">
    <skos:broader rdf:resource="http://www.opengis.net/spec/GeoTIFF/1.1/conf/DoubleParameters"/>
  </rdf:Description>
  <rdf:Description rdf:about="http://www.opengis.net/spec/GeoTIFF/1.1/req/UnitsGeoKey.ID">
    <rdf:type rdf:resource="http://www.opengis.net/def/ont/modspec/Requirement"/>
    <rdf:type rdf:resource="http://www.w3.org/2004/02/skos/core#Concept"/>
    <skos:broader rdf:resource="http://www.opengis.net/spec/GeoTIFF/1.1/req/UnitsGeoKey"/>
    <dct:description>The GeogAngularUnitsGeoKey SHALL have ID = 2054The GeogAzimuthUnitsGeoKey
SHALL have ID = 2060The GeogLinearUnitsGeoKey SHALL have ID = 2052The
ProjLinearUnitsGeoKey SHALL have ID = 3076The VerticalUnitsGeoKey SHALL have
ID = 4099</dct:description>
    <skos:definition>The GeogAngularUnitsGeoKey SHALL have ID = 2054The GeogAzimuthUnitsGeoKey
SHALL have ID = 2060The GeogLinearUnitsGeoKey SHALL have ID = 2052The
ProjLinearUnitsGeoKey SHALL have ID = 3076The VerticalUnitsGeoKey SHALL have
ID = 4099</skos:definition>
    <skos:prefLabel>Requirement 16.1</skos:prefLabel>
  </rdf:Description>
  <rdf:Description rdf:about="http://www.opengis.net/spec/GeoTIFF/1.1/req/GeoKeyDirectoryTag.keyEntryKeyCount">
    <skos:definition>The Third unsigned short integer in the Key Entry SHALL indicate the number of
values associated with this key.</skos:definition>
    <skos:prefLabel>Requirement 2.15</skos:prefLabel>
    <rdf:type rdf:resource="http://www.w3.org/2004/02/skos/core#Concept"/>
    <rdf:type rdf:resource="http://www.opengis.net/def/ont/modspec/Requirement"/>
    <skos:broader rdf:resource="http://www.opengis.net/spec/GeoTIFF/1.1/req/GeoKeyDirectoryTag"/>
    <skos:broader rdf:resource="http://www.opengis.net/spec/GeoTIFF/1.1/conf/DoubleParameters"/>
    <skos:broader rdf:resource="http://www.opengis.net/spec/GeoTIFF/1.1/conf/AsciiParameters"/>
    <skos:broader rdf:resource="http://www.opengis.net/spec/GeoTIFF/1.1/conf/ShortParameters"/>
    <dct:description>The Third unsigned short integer in the Key Entry SHALL indicate the number of
values associated with this key.</dct:description>
  </rdf:Description>
  <rdf:Description rdf:about="http://www.opengis.net/spec/GeoTIFF/1.1/req/GeoKeyCode.userDefined">
    <rdf:type rdf:resource="http://www.w3.org/2004/02/skos/core#Concept"/>
    <rdf:type rdf:resource="http://www.opengis.net/def/ont/modspec/Requirement"/>
    <skos:broader rdf:resource="http://www.opengis.net/spec/GeoTIFF/1.1/req/GeoKeyCode"/>
    <skos:prefLabel>Requirement 3.2</skos:prefLabel>
    <dct:description>GeoKeys with a value of 32767 SHALL indicate user-defined parameters</dct:description>
    <skos:definition>GeoKeys with a value of 32767 SHALL indicate user-defined parameters</skos:definition>
  </rdf:Description>
  <rdf:Description rdf:about="http://www.opengis.net/spec/GeoTIFF/1.1/req/GeodeticDatumGeoKey.private">
    <rdf:type rdf:resource="http://www.w3.org/2004/02/skos/core#Concept"/>
    <rdf:type rdf:resource="http://www.opengis.net/def/ont/modspec/Requirement"/>
    <dct:description>GeodeticDatumGeoKey values in the range 32768-65535 SHALL be private</dct:description>
    <skos:definition>GeodeticDatumGeoKey values in the range 32768-65535 SHALL be private</skos:definition>
    <skos:broader rdf:resource="http://www.opengis.net/spec/GeoTIFF/1.1/req/GeodeticDatumGeoKey"/>
    <skos:prefLabel>Requirement 18.6</skos:prefLabel>
  </rdf:Description>
  <rdf:Description rdf:about="http://www.opengis.net/spec/GeoTIFF/1.1/req/VerticalDatumGeoKey.EPSG">
    <rdf:type rdf:resource="http://www.w3.org/2004/02/skos/core#Concept"/>
    <rdf:type rdf:resource="http://www.opengis.net/def/ont/modspec/Requirement"/>
    <dct:description>VerticalDatumGeoKey values in the range 1024-32766 SHALL be EPSG vertical
datum codesNOTE: In GeoTIFF v1.0 the range was given as 1-16383 but without
reference to EPSG.</dct:description>
    <skos:broader rdf:resource="http://www.opengis.net/spec/GeoTIFF/1.1/req/VerticalDatumGeoKey"/>
    <skos:definition>VerticalDatumGeoKey values in the range 1024-32766 SHALL be EPSG vertical
datum codesNOTE: In GeoTIFF v1.0 the range was given as 1-16383 but without
reference to EPSG.</skos:definition>
    <skos:prefLabel>Requirement 25.4</skos:prefLabel>
  </rdf:Description>
  <rdf:Description rdf:about="http://www.opengis.net/spec/GeoTIFF/1.1/req/PrimeMeridianGeoKey.ID">
    <skos:definition>The PrimeMeridianGeoKey SHALL have ID = 2051</skos:definition>
    <skos:broader rdf:resource="http://www.opengis.net/spec/GeoTIFF/1.1/req/PrimeMeridianGeoKey"/>
    <rdf:type rdf:resource="http://www.opengis.net/def/ont/modspec/Requirement"/>
    <rdf:type rdf:resource="http://www.w3.org/2004/02/skos/core#Concept"/>
    <skos:prefLabel>Requirement 19.1</skos:prefLabel>
    <dct:description>The PrimeMeridianGeoKey SHALL have ID = 2051</dct:description>
  </rdf:Description>
  <rdf:Description rdf:about="http://www.opengis.net/spec/GeoTIFF/1.1/req/ProjectedCRSGeoKey.userdefined">
    <rdf:type rdf:resource="http://www.opengis.net/def/ont/modspec/Requirement"/>
    <rdf:type rdf:resource="http://www.w3.org/2004/02/skos/core#Concept"/>
    <skos:definition>A ProjectedCRSGeoKey value of 32767 SHALL be a user-defined projected CRS. If
the ProjectedCRSGeoKey value is 32767 (User-Defined) then the
ProjectedCitationGeoKey, GeodeticCRSGeoKey and ProjectionGeoKey SHALL be
populated.</skos:definition>
    <dct:description>A ProjectedCRSGeoKey value of 32767 SHALL be a user-defined projected CRS. If
the ProjectedCRSGeoKey value is 32767 (User-Defined) then the
ProjectedCitationGeoKey, GeodeticCRSGeoKey and ProjectionGeoKey SHALL be
populated.</dct:description>
    <skos:broader rdf:resource="http://www.opengis.net/spec/GeoTIFF/1.1/req/ProjectedCRSGeoKey"/>
    <skos:prefLabel>Requirement 12.5</skos:prefLabel>
  </rdf:Description>
  <rdf:Description rdf:about="http://www.opengis.net/spec/GeoTIFF/1.1/req/UnitsGeoKey.linear">
    <skos:definition>GeogLinearUnitsGeoKey, ProjLinearUnitsGeoKey and VerticalUnitsGeoKey values in
the range 1024-32766 SHALL be EPSG Unit Of Measure (UOM) codes with type =
length.NOTE: In GeoTIFF v1.0 the range was 9000-9099. Several values in this
range have been deprecated or deleted from the EPSG Dataset and should no
longer be used. See</skos:definition>
    <skos:prefLabel>Requirement 16.5</skos:prefLabel>
    <rdf:type rdf:resource="http://www.w3.org/2004/02/skos/core#Concept"/>
    <rdf:type rdf:resource="http://www.opengis.net/def/ont/modspec/Requirement"/>
    <skos:broader rdf:resource="http://www.opengis.net/spec/GeoTIFF/1.1/req/UnitsGeoKey"/>
    <dct:description>GeogLinearUnitsGeoKey, ProjLinearUnitsGeoKey and VerticalUnitsGeoKey values in
the range 1024-32766 SHALL be EPSG Unit Of Measure (UOM) codes with type =
length.NOTE: In GeoTIFF v1.0 the range was 9000-9099. Several values in this
range have been deprecated or deleted from the EPSG Dataset and should no
longer be used. See</dct:description>
  </rdf:Description>
  <rdf:Description rdf:about="http://www.opengis.net/spec/GeoTIFF/1.1/req/VerticalDatumGeoKey.type">
    <dct:description>The VerticalDatumGeoKey SHALL have type = SHORT</dct:description>
    <rdf:type rdf:resource="http://www.w3.org/2004/02/skos/core#Concept"/>
    <rdf:type rdf:resource="http://www.opengis.net/def/ont/modspec/Requirement"/>
    <skos:broader rdf:resource="http://www.opengis.net/spec/GeoTIFF/1.1/req/VerticalDatumGeoKey"/>
    <skos:definition>The VerticalDatumGeoKey SHALL have type = SHORT</skos:definition>
    <skos:prefLabel>Requirement 25.2</skos:prefLabel>
  </rdf:Description>
  <rdf:Description rdf:about="http://www.opengis.net/spec/GeoTIFF/1.1/req/TagSort">
    <skos:prefLabel>Requirement 1.5</skos:prefLabel>
    <rdf:type rdf:resource="http://www.opengis.net/def/ont/modspec/Requirement"/>
    <rdf:type rdf:resource="http://www.w3.org/2004/02/skos/core#Concept"/>
    <skos:broader rdf:resource="http://www.opengis.net/spec/GeoTIFF/1.1/conf/TIFF.Tags"/>
    <skos:broader rdf:resource="http://www.opengis.net/spec/GeoTIFF/1.1/req/Core"/>
    <skos:definition>The TIFF tags in a GeoTIFF file SHALL be written out to the file with the tag-
IDs sorted in ascending order</skos:definition>
    <dct:description>The TIFF tags in a GeoTIFF file SHALL be written out to the file with the tag-
IDs sorted in ascending order</dct:description>
  </rdf:Description>
  <rdf:Description rdf:about="http://www.opengis.net/spec/GeoTIFF/1.1/req/GeoKeyDirectoryTag.minorRevision">
    <skos:prefLabel>Requirement 2.8</skos:prefLabel>
    <skos:broader rdf:resource="http://www.opengis.net/spec/GeoTIFF/1.1/req/GeoKeyDirectoryTag"/>
    <skos:broader rdf:resource="http://www.opengis.net/spec/GeoTIFF/1.1/conf/GeoKeyDirectory"/>
    <dct:description>The third unsigned short integer in the GeoKeyDirectoryTag SHALL hold the
MinorRevision.</dct:description>
    <rdf:type rdf:resource="http://www.opengis.net/def/ont/modspec/Requirement"/>
    <rdf:type rdf:resource="http://www.w3.org/2004/02/skos/core#Concept"/>
    <skos:definition>The third unsigned short integer in the GeoKeyDirectoryTag SHALL hold the
MinorRevision.</skos:definition>
  </rdf:Description>
  <rdf:Description rdf:about="http://www.opengis.net/spec/GeoTIFF/1.1/req/UnitSizeGeoKey.type">
    <skos:broader rdf:resource="http://www.opengis.net/spec/GeoTIFF/1.1/req/UnitSizeGeoKey"/>
    <skos:definition>The GeogAngularUnitSizeGeoKey, GeogLinearUnitSizeGeoKey and
ProjLinearUnitSizeGeoKey SHALL each have type = DOUBLE</skos:definition>
    <rdf:type rdf:resource="http://www.w3.org/2004/02/skos/core#Concept"/>
    <rdf:type rdf:resource="http://www.opengis.net/def/ont/modspec/Requirement"/>
    <skos:prefLabel>Requirement 17.2</skos:prefLabel>
    <dct:description>The GeogAngularUnitSizeGeoKey, GeogLinearUnitSizeGeoKey and
ProjLinearUnitSizeGeoKey SHALL each have type = DOUBLE</dct:description>
  </rdf:Description>
  <rdf:Description rdf:about="http://www.opengis.net/spec/GeoTIFF/1.1/req/PrimeMeridianGeoKey.type">
    <rdf:type rdf:resource="http://www.opengis.net/def/ont/modspec/Requirement"/>
    <rdf:type rdf:resource="http://www.w3.org/2004/02/skos/core#Concept"/>
    <skos:broader rdf:resource="http://www.opengis.net/spec/GeoTIFF/1.1/req/PrimeMeridianGeoKey"/>
    <dct:description>The PrimeMeridianGeoKey SHALL have type = SHORT</dct:description>
    <skos:definition>The PrimeMeridianGeoKey SHALL have type = SHORT</skos:definition>
    <skos:prefLabel>Requirement 19.2</skos:prefLabel>
  </rdf:Description>
  <rdf:Description rdf:about="http://www.opengis.net/spec/GeoTIFF/1.1/req/GeoKeyDirectoryTag.ID">
    <skos:definition>The GeoKeyDirectoryTag SHALL have ID = 34735</skos:definition>
    <dct:description>The GeoKeyDirectoryTag SHALL have ID = 34735</dct:description>
    <rdf:type rdf:resource="http://www.w3.org/2004/02/skos/core#Concept"/>
    <rdf:type rdf:resource="http://www.opengis.net/def/ont/modspec/Requirement"/>
    <skos:prefLabel>Requirement 2.1</skos:prefLabel>
    <skos:broader rdf:resource="http://www.opengis.net/spec/GeoTIFF/1.1/conf/TIFF.Tags"/>
    <skos:broader rdf:resource="http://www.opengis.net/spec/GeoTIFF/1.1/req/GeoKeyDirectoryTag"/>
  </rdf:Description>
  <rdf:Description rdf:about="http://www.opengis.net/spec/GeoTIFF/1.1/req/GTRasterTypeGeoKey.private">
    <skos:prefLabel>Requirement 7.5</skos:prefLabel>
    <rdf:type rdf:resource="http://www.opengis.net/def/ont/modspec/Requirement"/>
    <rdf:type rdf:resource="http://www.w3.org/2004/02/skos/core#Concept"/>
    <dct:description>GTRasterTypeGeoKey values in the range 32768-65535 SHALL be private</dct:description>
    <skos:definition>GTRasterTypeGeoKey values in the range 32768-65535 SHALL be private</skos:definition>
    <skos:broader rdf:resource="http://www.opengis.net/spec/GeoTIFF/1.1/req/GTRasterTypeGeoKey"/>
  </rdf:Description>
  <rdf:Description rdf:about="http://www.opengis.net/spec/GeoTIFF/1.1/req/EllipsoidSemiMinorAxisGeoKey.ID">
    <skos:prefLabel>Requirement 23.1</skos:prefLabel>
    <rdf:type rdf:resource="http://www.w3.org/2004/02/skos/core#Concept"/>
    <rdf:type rdf:resource="http://www.opengis.net/def/ont/modspec/Requirement"/>
    <skos:broader rdf:resource="http://www.opengis.net/spec/GeoTIFF/1.1/req/EllipsoidSemiMajorAxisGeoKey"/>
    <skos:definition>The EllipsoidSemiMinorAxisGeoKey SHALL have ID = 2058</skos:definition>
    <dct:description>The EllipsoidSemiMinorAxisGeoKey SHALL have ID = 2058</dct:description>
  </rdf:Description>
  <rdf:Description rdf:about="http://www.opengis.net/spec/GeoTIFF/1.1/req/GeoKeyDirectoryTag.type">
    <rdf:type rdf:resource="http://www.w3.org/2004/02/skos/core#Concept"/>
    <rdf:type rdf:resource="http://www.opengis.net/def/ont/modspec/Requirement"/>
    <dct:description>The GeoKeyDirectoryTag SHALL have type = SHORT (2-byte unsigned integer)</dct:description>
    <skos:broader rdf:resource="http://www.opengis.net/spec/GeoTIFF/1.1/conf/TIFF.Tags"/>
    <skos:broader rdf:resource="http://www.opengis.net/spec/GeoTIFF/1.1/req/GeoKeyDirectoryTag"/>
    <skos:definition>The GeoKeyDirectoryTag SHALL have type = SHORT (2-byte unsigned integer)</skos:definition>
    <skos:prefLabel>Requirement 2.2</skos:prefLabel>
  </rdf:Description>
  <rdf:Description rdf:about="http://www.opengis.net/spec/GeoTIFF/1.1/req/GTRasterTypeGeoKey.ID">
    <dct:description>The GTRasterTypeGeoKey SHALL have ID = 1025</dct:description>
    <rdf:type rdf:resource="http://www.opengis.net/def/ont/modspec/Requirement"/>
    <rdf:type rdf:resource="http://www.w3.org/2004/02/skos/core#Concept"/>
    <skos:prefLabel>Requirement 7.1</skos:prefLabel>
    <skos:definition>The GTRasterTypeGeoKey SHALL have ID = 1025</skos:definition>
    <skos:broader rdf:resource="http://www.opengis.net/spec/GeoTIFF/1.1/req/GTRasterTypeGeoKey"/>
  </rdf:Description>
  <rdf:Description rdf:about="http://www.opengis.net/spec/GeoTIFF/1.1/req/ProjLinearParameterGeoKey">
    <skos:broader rdf:resource="http://www.opengis.net/spec/GeoTIFF/1.1/conf/DoubleParameters"/>
  </rdf:Description>
  <rdf:Description rdf:about="http://www.opengis.net/spec/GeoTIFF/1.1/req/GeoAsciiParamsTag.NULLWrite">
    <rdf:type rdf:resource="http://www.opengis.net/def/ont/modspec/Requirement"/>
    <rdf:type rdf:resource="http://www.w3.org/2004/02/skos/core#Concept"/>
    <skos:prefLabel>Requirement 6.4</skos:prefLabel>
    <dct:description>NULL (ASCII code = 0) characters SHALL not be present in the string content
written in the GeoAsciiParamsTagNOTE: this requirement only applies for the
content of the tag. The TIFF specification requires that the last byte of a
TIFF tag of type ASCII is NULL.</dct:description>
    <skos:definition>NULL (ASCII code = 0) characters SHALL not be present in the string content
written in the GeoAsciiParamsTagNOTE: this requirement only applies for the
content of the tag. The TIFF specification requires that the last byte of a
TIFF tag of type ASCII is NULL.</skos:definition>
    <skos:broader rdf:resource="http://www.opengis.net/spec/GeoTIFF/1.1/req/GeoAsciiParamsTag"/>
  </rdf:Description>
  <rdf:Description rdf:about="http://www.opengis.net/spec/GeoTIFF/1.1/req/GeodeticCRSGeoKey.EPSG">
    <skos:definition>GeodeticCRSGeoKey values in the range 1024-32766 SHALL be EPSG geographic 2D
or geocentric CRS codesNOTE: In GeoTIFF v1.0 the range was 4000-4999. Several
values in this range have been deprecated or deleted from the EPSG Dataset and
should no longer be used. See</skos:definition>
    <skos:broader rdf:resource="http://www.opengis.net/spec/GeoTIFF/1.1/req/GeodeticCRSGeoKey"/>
    <rdf:type rdf:resource="http://www.opengis.net/def/ont/modspec/Requirement"/>
    <rdf:type rdf:resource="http://www.w3.org/2004/02/skos/core#Concept"/>
    <skos:prefLabel>Requirement 13.4</skos:prefLabel>
    <dct:description>GeodeticCRSGeoKey values in the range 1024-32766 SHALL be EPSG geographic 2D
or geocentric CRS codesNOTE: In GeoTIFF v1.0 the range was 4000-4999. Several
values in this range have been deprecated or deleted from the EPSG Dataset and
should no longer be used. See</dct:description>
  </rdf:Description>
  <rdf:Description rdf:about="http://www.opengis.net/spec/GeoTIFF/1.1/req/GeodeticDatumGeoKey.userdefined">
    <dct:description>If the GeodeticDatumGeoKey value is 32767 (User-Defined) then the
GeodeticCitationGeoKey, PrimeMeridianGeoKey and EllipsoidGeoKey SHALL be
populated.</dct:description>
    <rdf:type rdf:resource="http://www.w3.org/2004/02/skos/core#Concept"/>
    <rdf:type rdf:resource="http://www.opengis.net/def/ont/modspec/Requirement"/>
    <skos:prefLabel>Requirement 18.5</skos:prefLabel>
    <skos:definition>If the GeodeticDatumGeoKey value is 32767 (User-Defined) then the
GeodeticCitationGeoKey, PrimeMeridianGeoKey and EllipsoidGeoKey SHALL be
populated.</skos:definition>
    <skos:broader rdf:resource="http://www.opengis.net/spec/GeoTIFF/1.1/req/GeodeticDatumGeoKey"/>
  </rdf:Description>
  <rdf:Description rdf:about="http://www.opengis.net/spec/GeoTIFF/1.1/req/EllipsoidSemiMinorAxisGeoKey">
    <skos:broader rdf:resource="http://www.opengis.net/spec/GeoTIFF/1.1/conf/DoubleParameters"/>
  </rdf:Description>
  <rdf:Description rdf:about="http://www.opengis.net/spec/GeoTIFF/1.1/req/GTModelTypeGeoKey.value">
    <rdf:type rdf:resource="http://www.w3.org/2004/02/skos/core#Concept"/>
    <rdf:type rdf:resource="http://www.opengis.net/def/ont/modspec/Requirement"/>
    <skos:definition>The GTModelTypeGeoKey value SHALL be:* 0 to indicate that the Model CRS in
undefined or unknown; or* 1 to indicate that the Model CRS is a 2D projected
coordinate reference system, indicated by the value of the ProjectedCRSGeoKey;
or* 2 to indicate that the Model CRS is a geographic 2D coordinate reference
system, indicated by the value of the GeodeticCRSGeoKey; or* 3 to indicate
that the Model CRS is a geocentric Cartesian 3D coordinate reference system,
indicated by the value of the GeodeticCRSGeoKey; or* 32767 to indicate that
the Model CRS type is user-defined.</skos:definition>
    <skos:prefLabel>Requirement 8.4</skos:prefLabel>
    <dct:description>The GTModelTypeGeoKey value SHALL be:* 0 to indicate that the Model CRS in
undefined or unknown; or* 1 to indicate that the Model CRS is a 2D projected
coordinate reference system, indicated by the value of the ProjectedCRSGeoKey;
or* 2 to indicate that the Model CRS is a geographic 2D coordinate reference
system, indicated by the value of the GeodeticCRSGeoKey; or* 3 to indicate
that the Model CRS is a geocentric Cartesian 3D coordinate reference system,
indicated by the value of the GeodeticCRSGeoKey; or* 32767 to indicate that
the Model CRS type is user-defined.</dct:description>
    <skos:broader rdf:resource="http://www.opengis.net/spec/GeoTIFF/1.1/req/GTModelTypeGeoKey"/>
  </rdf:Description>
  <rdf:Description rdf:about="http://www.opengis.net/spec/GeoTIFF/1.1/req/ProjAzimuthAngleGeoKey">
    <skos:broader rdf:resource="http://www.opengis.net/spec/GeoTIFF/1.1/conf/DoubleParameters"/>
  </rdf:Description>
  <rdf:Description rdf:about="http://www.opengis.net/spec/GeoTIFF/1.1/req/GeoKeyDirectoryTag.KeyEntry.ID">
    <skos:broader rdf:resource="http://www.opengis.net/spec/GeoTIFF/1.1/conf/ShortParameters"/>
    <skos:broader rdf:resource="http://www.opengis.net/spec/GeoTIFF/1.1/conf/DoubleParameters"/>
  </rdf:Description>
  <rdf:Description rdf:about="http://www.opengis.net/spec/GeoTIFF/1.1/req/UnitSizeGeoKey.units">
    <dct:description>The units of the GeogAngularUnitSizeGeoKey value SHALL be radians.The units of
the GeogLinearUnitSizeGeoKey value SHALL be meters.The units of the
ProjLinearUnitSizeGeoKey value SHALL be meters.</dct:description>
    <rdf:type rdf:resource="http://www.opengis.net/def/ont/modspec/Requirement"/>
    <rdf:type rdf:resource="http://www.w3.org/2004/02/skos/core#Concept"/>
    <skos:broader rdf:resource="http://www.opengis.net/spec/GeoTIFF/1.1/req/UnitSizeGeoKey"/>
    <skos:prefLabel>Requirement 17.3</skos:prefLabel>
    <skos:definition>The units of the GeogAngularUnitSizeGeoKey value SHALL be radians.The units of
the GeogLinearUnitSizeGeoKey value SHALL be meters.The units of the
ProjLinearUnitSizeGeoKey value SHALL be meters.</skos:definition>
  </rdf:Description>
  <rdf:Description rdf:about="http://www.opengis.net/spec/GeoTIFF/1.1/req/GeoKeyDirectoryTag.KeyEntryKeyID">
    <skos:broader rdf:resource="http://www.opengis.net/spec/GeoTIFF/1.1/conf/AsciiParameters"/>
  </rdf:Description>
  <rdf:Description rdf:about="http://www.opengis.net/spec/GeoTIFF/1.1/req/EllipsoidInvFlatteningGeoKey">
    <skos:broader rdf:resource="http://www.opengis.net/spec/GeoTIFF/1.1/conf/DoubleParameters"/>
  </rdf:Description>
</rdf:RDF>
